<?xml version="1.0" encoding="UTF-8"?>
<rdf:RDF
	xmlns="https://dev-lexic.swissgeol.ch/TectonicUnits/"
	xmlns:grddl="http://www.w3.org/2003/g/data-view#"
	xmlns:dct="http://purl.org/dc/terms/"
	xmlns:rdf="http://www.w3.org/1999/02/22-rdf-syntax-ns#"
	xmlns:owl="http://www.w3.org/2002/07/owl#"
	xmlns:xsd="http://www.w3.org/2001/XMLSchema#"
	xmlns:skos="http://www.w3.org/2004/02/skos/core#"
	xmlns:rdfs="http://www.w3.org/2000/01/rdf-schema#"
	xmlns:dc="http://purl.org/dc/elements/1.1/">

<rdf:Description rdf:about="https://dev-lexic.swissgeol.ch/TectonicUnits/">
	<rdf:type rdf:resource="http://www.w3.org/2002/07/owl#Ontology"/>
</rdf:Description>

<rdf:Description rdf:about="https://dev-lexic.swissgeol.ch/TectonicUnits">
	<rdf:type rdf:resource="http://www.w3.org/2004/02/skos/core#ConceptScheme"/>
	<skos:prefLabel xml:lang="en">TectonicUnits</skos:prefLabel>
</rdf:Description>

<rdf:Description rdf:about="https://dev-lexic.swissgeol.ch/TectonicUnits/AutochthonousNorthAlpineForeland">
	<rdf:type rdf:resource="http://www.w3.org/2004/02/skos/core#Concept"/>
	<rdfs:isDefinedBy xml:lang="en">Gouffon Yves (Editor) (2024): Tectonic Map of Switzerland 1:500000, Explanatory notes. Federal Office of Topography swisstopo, Wabern</rdfs:isDefinedBy>
	<rdfs:comment rdf:datatype="http://www.w3.org/1999/02/22-rdf-syntax-ns#HTML">https://data.geo.admin.ch/ch.swisstopo.geologie-tektonische_karte/pdf/Erl-TK500_2024.pdf</rdfs:comment>
	<skos:definition xml:lang="en">The Autochthonous North Alpine Foreland consists of the European platform with its Cenozoic graben structures of eastern France, southwestern Germany and northern Switzerland. The boundary between the Autochthonous North Alpine Foreland and the Detached North Alpine Foreland marks the northernmost limit of significant Alpine compressional deformation.</skos:definition>
	<skos:inScheme rdf:resource="https://dev-lexic.swissgeol.ch/TectonicUnits"/>
	<skos:topConceptOf rdf:resource="https://dev-lexic.swissgeol.ch/TectonicUnits"/>
	<skos:prefLabel xml:lang="en">Autochthonous North Alpine Foreland</skos:prefLabel>
	<skos:prefLabel xml:lang="de">Autochthones Nordalpines Vorland</skos:prefLabel>
	<skos:prefLabel xml:lang="fr">Avant-pays nord-alpin autochtone</skos:prefLabel>
	<skos:prefLabel xml:lang="it">Avampaese nordalpino autoctono</skos:prefLabel>
	<skos:narrower rdf:resource="https://dev-lexic.swissgeol.ch/TectonicUnits/BresseGraben"/>
	<skos:narrower rdf:resource="https://dev-lexic.swissgeol.ch/TectonicUnits/Haute-SaonePlatform"/>
	<skos:narrower rdf:resource="https://dev-lexic.swissgeol.ch/TectonicUnits/UpperRhineGraben"/>
	<skos:narrower rdf:resource="https://dev-lexic.swissgeol.ch/TectonicUnits/SouthGermanPlatform"/>
	<skos:narrower rdf:resource="https://dev-lexic.swissgeol.ch/TectonicUnits/TransitionZoneBetweenDetachedAndAutochthonousNorthAlpineForeland"/>
	<skos:related rdf:resource="https://dev-lexic.swissgeol.ch/TectonicUnits/DetachedNorthAlpineForeland"/>
	<status xmlns="http://www.w3.org/ns/adms#" rdf:resource="https://dev-lexic.swissgeol.ch/active"/>
</rdf:Description>

<rdf:Description rdf:about="https://dev-lexic.swissgeol.ch/TectonicUnits/BresseGraben">
	<rdf:type rdf:resource="http://www.w3.org/2004/02/skos/core#Concept"/>
	<rdfs:isDefinedBy xml:lang="en">Gouffon Yves (Editor) (2024): Tectonic Map of Switzerland 1:500000, Explanatory notes. Federal Office of Topography swisstopo, Wabern</rdfs:isDefinedBy>
	<skos:definition xml:lang="en">The N–S trending Bresse Graben is a segment of the European Cenozoic Rift System, filled with Paleogene–Neogene sediments which are up to 2 km thick. It is ca. 35–60 km wide and stretches roughly from Lyon to Dijon. It is clearly separated from the Haute-Saône Platform by NNE–SSW to NE–SW oriented normal faults.</skos:definition>
	<skos:inScheme rdf:resource="https://dev-lexic.swissgeol.ch/TectonicUnits"/>
	<skos:prefLabel xml:lang="en">Bresse Graben</skos:prefLabel>
	<skos:prefLabel xml:lang="de">Bresse-Graben</skos:prefLabel>
	<skos:prefLabel xml:lang="fr">Graben de la Bresse</skos:prefLabel>
	<skos:prefLabel xml:lang="it">Graben della Bresse</skos:prefLabel>
	<skos:altLabel xml:lang="fr">fossé bressan</skos:altLabel>
	<skos:broader rdf:resource="https://dev-lexic.swissgeol.ch/TectonicUnits/AutochthonousNorthAlpineForeland"/>
	<status xmlns="http://www.w3.org/ns/adms#" rdf:resource="https://dev-lexic.swissgeol.ch/active"/>
</rdf:Description>

<rdf:Description rdf:about="https://dev-lexic.swissgeol.ch/TectonicUnits/Haute-SaonePlatform">
	<rdf:type rdf:resource="http://www.w3.org/2004/02/skos/core#Concept"/>
	<rdfs:isDefinedBy xml:lang="en">Gouffon Yves (Editor) (2024): Tectonic Map of Switzerland 1:500000, Explanatory notes. Federal Office of Topography swisstopo, Wabern</rdfs:isDefinedBy>
	<skos:definition xml:lang="en">The Haute-Saône Platform forms the southeastern rim of the Paris Basin and is formed predominantly by Mesozoic sediments, with some post-rift Neogene Molasse sediments. It is mostly located in France except for the Ajoie area. At its eastern boundary, the separation from the northern part of the Upper Rhine Graben is clearly defined by NNE–SSW trending normal faults. In the south, however, the situation is more complex. Here, the limestone plateau of Ajoie, regarded as belonging to the Haute-Saône Platform, is separated from the northward-adjacent Upper Rhine Graben by a W–E trending flexure dissected by N–S trending normal faults. To the south, the Haute-Saône Platform is mostly bounded by the Detached North Alpine Foreland, in particluar by the frontal Faisceaux of the External Folded Jura. South of the Ajoie area, where the External Folded Jura is missing, the Internal Folded Jura is thrust directly onto the Haute-Saône Platform.</skos:definition>
	<skos:inScheme rdf:resource="https://dev-lexic.swissgeol.ch/TectonicUnits"/>
	<skos:prefLabel xml:lang="de">Haute-Saône-Tafel</skos:prefLabel>
	<skos:prefLabel xml:lang="it">Altopiano della Haute-Saône</skos:prefLabel>
	<skos:prefLabel xml:lang="fr">Plateau de la Haute-Saône</skos:prefLabel>
	<skos:prefLabel xml:lang="en">Haute-Saône Platform</skos:prefLabel>
	<skos:altLabel xml:lang="de">autochthoner Tafeljura</skos:altLabel>
	<skos:altLabel xml:lang="de">Nordfranzösisches Schichtstufenland</skos:altLabel>
	<skos:broader rdf:resource="https://dev-lexic.swissgeol.ch/TectonicUnits/AutochthonousNorthAlpineForeland"/>
	<status xmlns="http://www.w3.org/ns/adms#" rdf:resource="https://dev-lexic.swissgeol.ch/active"/>
</rdf:Description>

<rdf:Description rdf:about="https://dev-lexic.swissgeol.ch/TectonicUnits/UpperRhineGraben">
	<rdf:type rdf:resource="http://www.w3.org/2004/02/skos/core#Concept"/>
	<rdfs:isDefinedBy xml:lang="en">Gouffon Yves (Editor) (2024): Tectonic Map of Switzerland 1:500000, Explanatory notes. Federal Office of Topography swisstopo, Wabern</rdfs:isDefinedBy>
	<skos:definition xml:lang="en">The NNE–SSW trending Upper Rhine Graben is a segment of the European Cenozoic Rift System located north of Basel, filled with Paleogene–Neogene sediments of 2–3 km thickness. It is up to 40 km wide and separates the Haute-Saône Platform to the west from the South German Platform to the east. The graben shoulders are bounded by steep normal faults and include isolated, lowered blocks of Mesozoic platform sediments along the rift-internal sides (the so-called Vorberg Zone, e.g., Isteiner Klotz north of Basel). The Schwarzwald Fault forms the eastern border of the graben. The southwestern border of the graben with the Haute-Saône Platform forms a flexure. In the southeast, the graben borders the External Folded Jura; the corresponding flexure is accentuated and overprinted by Alpine deformation.</skos:definition>
	<skos:inScheme rdf:resource="https://dev-lexic.swissgeol.ch/TectonicUnits"/>
	<skos:prefLabel xml:lang="en">Upper Rhine Graben</skos:prefLabel>
	<skos:prefLabel xml:lang="de">Oberrhein-Graben</skos:prefLabel>
	<skos:prefLabel xml:lang="fr">Graben du Haut Rhin</skos:prefLabel>
	<skos:prefLabel xml:lang="it">Graben dell'Alto Reno</skos:prefLabel>
	<skos:altLabel xml:lang="fr">fossé rhénan</skos:altLabel>
	<skos:broader rdf:resource="https://dev-lexic.swissgeol.ch/TectonicUnits/AutochthonousNorthAlpineForeland"/>
	<status xmlns="http://www.w3.org/ns/adms#" rdf:resource="https://dev-lexic.swissgeol.ch/active"/>
</rdf:Description>

<rdf:Description rdf:about="https://dev-lexic.swissgeol.ch/TectonicUnits/SouthGermanPlatform">
	<rdf:type rdf:resource="http://www.w3.org/2004/02/skos/core#Concept"/>
	<rdfs:isDefinedBy xml:lang="en">Gouffon Yves (Editor) (2024): Tectonic Map of Switzerland 1:500000, Explanatory notes. Federal Office of Topography swisstopo, Wabern</rdfs:isDefinedBy>
	<skos:definition xml:lang="en">The South German Platform consists of an autochthonous Mesozoic–Cenozoic sedimentary cover and its basement (Schwarzwald Massif). It shows a clear segmentation into tectonically distinct regions, between the eastern shoulder of the Upper Rhine Graben and the Hegau-Bodensee Graben, passing northwards to the Schwäbische Alb.</skos:definition>
	<skos:inScheme rdf:resource="https://dev-lexic.swissgeol.ch/TectonicUnits"/>
	<skos:prefLabel xml:lang="en">South German Platform</skos:prefLabel>
	<skos:prefLabel xml:lang="de">Süddeutsche Tafel</skos:prefLabel>
	<skos:prefLabel xml:lang="fr">Plateau de l'Allemagne méridionale</skos:prefLabel>
	<skos:prefLabel xml:lang="it">Altopiano della Germania meridionale</skos:prefLabel>
	<skos:altLabel xml:lang="de">Südwestdeutsches Schichtstufenland</skos:altLabel>
	<skos:altLabel xml:lang="de">autochthoner Tafeljura</skos:altLabel>
	<skos:broader rdf:resource="https://dev-lexic.swissgeol.ch/TectonicUnits/AutochthonousNorthAlpineForeland"/>
	<skos:narrower rdf:resource="https://dev-lexic.swissgeol.ch/TectonicUnits/Hegau-BodenseeGraben"/>
	<status xmlns="http://www.w3.org/ns/adms#" rdf:resource="https://dev-lexic.swissgeol.ch/active"/>
</rdf:Description>

<rdf:Description rdf:about="https://dev-lexic.swissgeol.ch/TectonicUnits/TransitionZoneBetweenDetachedAndAutochthonousNorthAlpineForeland">
	<rdf:type rdf:resource="http://www.w3.org/2004/02/skos/core#Concept"/>
	<rdfs:isDefinedBy xml:lang="en">Gouffon Yves (Editor) (2024): Tectonic Map of Switzerland 1:500000, Explanatory notes. Federal Office of Topography swisstopo, Wabern</rdfs:isDefinedBy>
	<skos:inScheme rdf:resource="https://dev-lexic.swissgeol.ch/TectonicUnits"/>
	<skos:prefLabel xml:lang="en">Transition zone between Detached and Autochthonous North Alpine Foreland</skos:prefLabel>
	<skos:prefLabel xml:lang="de">Übergangszone Abgeschert-Autochthones Vorlandplateau</skos:prefLabel>
	<skos:prefLabel xml:lang="fr">Zone de transition entre Avant-pays nord-alpin décolé et autochtone</skos:prefLabel>
	<skos:prefLabel xml:lang="it">Zona di transizione tra l'Avampaese nordalpino distaccato e autoctono</skos:prefLabel>
	<skos:broader rdf:resource="https://dev-lexic.swissgeol.ch/TectonicUnits/AutochthonousNorthAlpineForeland"/>
	<skos:broader rdf:resource="https://dev-lexic.swissgeol.ch/TectonicUnits/DetachedNorthAlpineForeland"/>
	<status xmlns="http://www.w3.org/ns/adms#" rdf:resource="https://dev-lexic.swissgeol.ch/active"/>
</rdf:Description>

<rdf:Description rdf:about="https://dev-lexic.swissgeol.ch/TectonicUnits/DetachedNorthAlpineForeland">
	<rdf:type rdf:resource="http://www.w3.org/2004/02/skos/core#Concept"/>
	<rdfs:isDefinedBy xml:lang="en">Gouffon Yves (Editor) (2024): Tectonic Map of Switzerland 1:500000, Explanatory notes. Federal Office of Topography swisstopo, Wabern</rdfs:isDefinedBy>
	<rdfs:comment rdf:datatype="http://www.w3.org/1999/02/22-rdf-syntax-ns#HTML">https://data.geo.admin.ch/ch.swisstopo.geologie-tektonische_karte/pdf/Erl-TK500_2024.pdf</rdfs:comment>
	<skos:definition xml:lang="en">The Detached North Alpine Foreland refers to the displaced sedimentary cover north of the front of the Helvetic units. Decoupling between the thrusted and deformed cover and the underlying basement took place in a décollement zone in the evaporites of Muschelkalk Group east of a line Porrentruy–Biel–Fribourg and of the Keuper Group further west. Deformation includes northwestward and northward displacement, thrusting and folding as well as strike-slip deformation. The northern boundary, which coincides with the front of Alpine deformation, is given by the outermost (distal) significant thrusting and folding. The easternmost clear evidence for décollement-related tectonics is given by the Lägern Anticline east of Baden with some more indications from seismic data found south of Bülach. Further to the east, displacement of the sedimentary cover along the decollement zone is presumed to gradually decrease. Accordingly, no precise eastern boundary can be drawn between the Detached North Alpine Foreland and the autochthonous South German Platform and a conceptual transition zone is defined instead.</skos:definition>
	<skos:inScheme rdf:resource="https://dev-lexic.swissgeol.ch/TectonicUnits"/>
	<skos:topConceptOf rdf:resource="https://dev-lexic.swissgeol.ch/TectonicUnits"/>
	<skos:prefLabel xml:lang="en">Detached North Alpine Foreland</skos:prefLabel>
	<skos:prefLabel xml:lang="de">Abgeschertes Nordalpines Vorland</skos:prefLabel>
	<skos:prefLabel xml:lang="fr">Avant-pays nord-alpin décollé</skos:prefLabel>
	<skos:prefLabel xml:lang="it">Avampaese nordalpino distaccato</skos:prefLabel>
	<skos:narrower rdf:resource="https://dev-lexic.swissgeol.ch/TectonicUnits/TransitionZoneBetweenDetachedAndAutochthonousNorthAlpineForeland"/>
	<skos:narrower rdf:resource="https://dev-lexic.swissgeol.ch/TectonicUnits/ExternalFoldedJura"/>
	<skos:narrower rdf:resource="https://dev-lexic.swissgeol.ch/TectonicUnits/SubalpineMolasse"/>
	<skos:narrower rdf:resource="https://dev-lexic.swissgeol.ch/TectonicUnits/InternalFoldedJuraAndForelandPlateau"/>
	<skos:related rdf:resource="https://dev-lexic.swissgeol.ch/TectonicUnits/AutochthonousNorthAlpineForeland"/>
	<status xmlns="http://www.w3.org/ns/adms#" rdf:resource="https://dev-lexic.swissgeol.ch/active"/>
</rdf:Description>

<rdf:Description rdf:about="https://dev-lexic.swissgeol.ch/TectonicUnits/Hegau-BodenseeGraben">
	<rdf:type rdf:resource="http://www.w3.org/2004/02/skos/core#Concept"/>
	<rdfs:isDefinedBy xml:lang="en">Gouffon Yves (Editor) (2024): Tectonic Map of Switzerland 1:500000, Explanatory notes. Federal Office of Topography swisstopo, Wabern</rdfs:isDefinedBy>
	<skos:definition xml:lang="en">The NW–SE trending extensional Hegau-Bodensee Graben represents the southeastern extension of the Freiburg-Bonndorf-Bodensee Fault Zone and is associated with the Neogene Hegau Volcanic Province.</skos:definition>
	<skos:inScheme rdf:resource="https://dev-lexic.swissgeol.ch/TectonicUnits"/>
	<skos:prefLabel xml:lang="en">Hegau-Bodensee Graben</skos:prefLabel>
	<skos:prefLabel xml:lang="de">Hegau-Bodensee-Graben</skos:prefLabel>
	<skos:prefLabel xml:lang="fr">Graben du Hegau-Bodensee</skos:prefLabel>
	<skos:prefLabel xml:lang="it">Graben del Hegau-Bodensee</skos:prefLabel>
	<skos:broader rdf:resource="https://dev-lexic.swissgeol.ch/TectonicUnits/SouthGermanPlatform"/>
	<skos:related rdf:resource="https://dev-lexic.swissgeol.ch/TectonicUnits/HegauVolcanicSuite"/>
	<status xmlns="http://www.w3.org/ns/adms#" rdf:resource="https://dev-lexic.swissgeol.ch/active"/>
</rdf:Description>

<rdf:Description rdf:about="https://dev-lexic.swissgeol.ch/TectonicUnits/ExternalFoldedJura">
	<rdf:type rdf:resource="http://www.w3.org/2004/02/skos/core#Concept"/>
	<rdfs:isDefinedBy xml:lang="en">Gouffon Yves (Editor) (2024): Tectonic Map of Switzerland 1:500000, Explanatory notes. Federal Office of Topography swisstopo, Wabern</rdfs:isDefinedBy>
	<skos:definition xml:lang="en">The External Folded Jura is the outermost part of the arcuate Jura mountain range (and hence of the Detached Northern Alpine Foreland) consisting of low-relief Plateaux, only slightly faulted, separated from each other by narrow, highly deformed Faisceaux.</skos:definition>
	<skos:inScheme rdf:resource="https://dev-lexic.swissgeol.ch/TectonicUnits"/>
	<skos:prefLabel xml:lang="en">External Folded Jura</skos:prefLabel>
	<skos:prefLabel xml:lang="de">Externer Faltenjura</skos:prefLabel>
	<skos:prefLabel xml:lang="fr">Jura Plissé Externe</skos:prefLabel>
	<skos:prefLabel xml:lang="it">Giura Piegato Esterno</skos:prefLabel>
	<skos:altLabel xml:lang="fr">Jura externe</skos:altLabel>
	<skos:broader rdf:resource="https://dev-lexic.swissgeol.ch/TectonicUnits/DetachedNorthAlpineForeland"/>
	<skos:narrower rdf:resource="https://dev-lexic.swissgeol.ch/TectonicUnits/Faisceaux"/>
	<skos:narrower rdf:resource="https://dev-lexic.swissgeol.ch/TectonicUnits/Plateaux"/>
	<skos:related rdf:resource="https://dev-lexic.swissgeol.ch/TectonicUnits/InternalFoldedJuraAndForelandPlateau"/>
	<status xmlns="http://www.w3.org/ns/adms#" rdf:resource="https://dev-lexic.swissgeol.ch/active"/>
</rdf:Description>

<rdf:Description rdf:about="https://dev-lexic.swissgeol.ch/TectonicUnits/SubalpineMolasse">
	<rdf:type rdf:resource="http://www.w3.org/2004/02/skos/core#Concept"/>
	<rdfs:isDefinedBy xml:lang="en">Gouffon Yves (Editor) (2024): Tectonic Map of Switzerland 1:500000, Explanatory notes. Federal Office of Topography swisstopo, Wabern</rdfs:isDefinedBy>
	<skos:definition xml:lang="en">The Subalpine Molasse constitutes the southernmost subdomain of the Detached North Alpine Foreland, situated between the Foreland Plateau to the north and the first basal thrust of the Alpine nappes to the south. It consists of a stack of imbricated thrust slices where the beds generally dip towards the SE. The Subalpine Molasse mainly includes coarse-grained foreland basin strata that were deposited between about 32 and 20 Ma. They chronicle the change from the underfilled Flysch to the filled/overfilled Molasse stage of foreland basin evolution.</skos:definition>
	<skos:inScheme rdf:resource="https://dev-lexic.swissgeol.ch/TectonicUnits"/>
	<skos:prefLabel xml:lang="en">Subalpine Molasse</skos:prefLabel>
	<skos:prefLabel xml:lang="de">Subalpine Molasse</skos:prefLabel>
	<skos:prefLabel xml:lang="fr">Molasse Subalpine</skos:prefLabel>
	<skos:prefLabel xml:lang="it">Molassa Subalpina</skos:prefLabel>
	<skos:broader rdf:resource="https://dev-lexic.swissgeol.ch/TectonicUnits/DetachedNorthAlpineForeland"/>
	<skos:narrower rdf:resource="https://dev-lexic.swissgeol.ch/TectonicUnits/Marbach-BerneckTriangleZone"/>
	<skos:narrower rdf:resource="https://dev-lexic.swissgeol.ch/TectonicUnits/SubalpineSliceComplex"/>
	<status xmlns="http://www.w3.org/ns/adms#" rdf:resource="https://dev-lexic.swissgeol.ch/active"/>
</rdf:Description>

<rdf:Description rdf:about="https://dev-lexic.swissgeol.ch/TectonicUnits/InternalFoldedJuraAndForelandPlateau">
	<rdf:type rdf:resource="http://www.w3.org/2004/02/skos/core#Concept"/>
	<rdfs:isDefinedBy xml:lang="en">Gouffon Yves (Editor) (2024): Tectonic Map of Switzerland 1:500000, Explanatory notes. Federal Office of Topography swisstopo, Wabern</rdfs:isDefinedBy>
	<skos:definition xml:lang="en">The Internal Folded Jura and the Foreland Plateau are tectonically united as a median sector within the Detached North Alpine Foreland. Its frontal part (Internal Folded Jura) forms an intensely deformed arcuate chain («Haute Chaîne»), whereas its hinter part comprises the «Plateau Molasse» and its Mesozoic basement, only affected by NE–SW trending low amplitude folds. </skos:definition>
	<skos:inScheme rdf:resource="https://dev-lexic.swissgeol.ch/TectonicUnits"/>
	<skos:prefLabel xml:lang="en">Internal Folded Jura and Foreland Plateau</skos:prefLabel>
	<skos:prefLabel xml:lang="de">Interner Faltenjura und Vorlandplateau</skos:prefLabel>
	<skos:prefLabel xml:lang="fr">Jura Plissé Interne et Plateau de l'Avant-pays</skos:prefLabel>
	<skos:prefLabel xml:lang="it">Giura Piegato Interno e Altopiano dell’Avampaese</skos:prefLabel>
	<skos:altLabel xml:lang="fr">Jura interne; Haute-Chaîne; Plateau molassique</skos:altLabel>
	<skos:broader rdf:resource="https://dev-lexic.swissgeol.ch/TectonicUnits/DetachedNorthAlpineForeland"/>
	<skos:related rdf:resource="https://dev-lexic.swissgeol.ch/TectonicUnits/ExternalFoldedJura"/>
	<status xmlns="http://www.w3.org/ns/adms#" rdf:resource="https://dev-lexic.swissgeol.ch/active"/>
</rdf:Description>

<rdf:Description rdf:about="https://dev-lexic.swissgeol.ch/TectonicUnits/HegauVolcanicSuite">
	<rdf:type rdf:resource="http://www.w3.org/2004/02/skos/core#Concept"/>
	<rdfs:isDefinedBy xml:lang="en">Gouffon Yves (Editor) (2024): Tectonic Map of Switzerland 1:500000, Explanatory notes. Federal Office of Topography swisstopo, Wabern</rdfs:isDefinedBy>
	<skos:definition xml:lang="en">The Miocene Hegau Volcanic Suite, situated in the Autochthonous North Alpine Foreland of Germany (area of Singen northwest of the Bodensee), is related to intraplate magmatism of alkaline basaltic composition. The Hegau volcanism seems to be associated with extension within the NW–SE striking Hegau-Bodensee Graben structure and regional uplift of the Schwarzwald area. Volcanic activity is of Middle to Late Miocene age, with various episodes succeeding each other between some 14 and 7 Ma: pyroclastics (“Deckentuffe”), including extensive layers of volcanic ash (up to 100 m thick) as well as chimney and crater fills, came first, followed by olivine nephelinites, hornblende tuffs and finally phonolites.
The Upper Freshwater Molasse of northeastern Switzerland contains several levels of bentonite (fossil weathering products of volcanic ash deposits) radiometrically dated between 15.3 and 14.2 Ma (Gubler 2020 and ref. therein), the ages of which coincide with the onset of Hegau volcanism. A younger bentonite layer near Frauenfeld was dated by Rahn &amp; Selbekk (2007) at around 11.5 Ma.</skos:definition>
	<skos:inScheme rdf:resource="https://dev-lexic.swissgeol.ch/TectonicUnits"/>
	<skos:prefLabel xml:lang="en">Hegau Volcanic Suite</skos:prefLabel>
	<skos:prefLabel xml:lang="de">Vulkanische Serie des Hegaus</skos:prefLabel>
	<skos:prefLabel xml:lang="fr">Série volcanique de l‘Hegau</skos:prefLabel>
	<skos:prefLabel xml:lang="it">Serie vulcanica dell‘Hegau</skos:prefLabel>
	<skos:altLabel xml:lang="de">Hegau-Provinz</skos:altLabel>
	<skos:broader rdf:resource="https://dev-lexic.swissgeol.ch/TectonicUnits/CenozoicMagmaticRocks"/>
	<skos:related rdf:resource="https://dev-lexic.swissgeol.ch/TectonicUnits/Hegau-BodenseeGraben"/>
	<status xmlns="http://www.w3.org/ns/adms#" rdf:resource="https://dev-lexic.swissgeol.ch/active"/>
</rdf:Description>

<rdf:Description rdf:about="https://dev-lexic.swissgeol.ch/TectonicUnits/CenozoicMagmaticRocks">
	<rdf:type rdf:resource="http://www.w3.org/2004/02/skos/core#Concept"/>
	<rdfs:isDefinedBy xml:lang="en">Gouffon Yves (Editor) (2024): Tectonic Map of Switzerland 1:500000, Explanatory notes. Federal Office of Topography swisstopo, Wabern</rdfs:isDefinedBy>
	<rdfs:comment rdf:datatype="http://www.w3.org/1999/02/22-rdf-syntax-ns#HTML">https://data.geo.admin.ch/ch.swisstopo.geologie-tektonische_karte/pdf/Erl-TK500_2024.pdf</rdfs:comment>
	<rdfs:comment rdf:datatype="http://www.w3.org/1999/02/22-rdf-syntax-ns#HTML">https://www.strati.ch/en/tectonic/cenozoic-magmatites</rdfs:comment>
	<skos:definition xml:lang="en">Several magmatic events occurred during the Alpine orogeny. Two groups of magmatic rocks need to be distinguished: the Hegau Volcanic Suite in the Autochthonous North Alpine Foreland and the extensive Periadriatic province in southern parts of the Alps.</skos:definition>
	<skos:inScheme rdf:resource="https://dev-lexic.swissgeol.ch/TectonicUnits"/>
	<skos:topConceptOf rdf:resource="https://dev-lexic.swissgeol.ch/TectonicUnits"/>
	<skos:prefLabel xml:lang="en">Cenozoic magmatic rocks</skos:prefLabel>
	<skos:prefLabel xml:lang="de">Känozoische magmatische Gesteine</skos:prefLabel>
	<skos:prefLabel xml:lang="fr">Roches magmatiques cénozoïques</skos:prefLabel>
	<skos:prefLabel xml:lang="it">Rocce magmatiche cenozoiche</skos:prefLabel>
	<skos:narrower rdf:resource="https://dev-lexic.swissgeol.ch/TectonicUnits/HegauVolcanicSuite"/>
	<skos:narrower rdf:resource="https://dev-lexic.swissgeol.ch/TectonicUnits/PeriadriaticMagmaticProvince"/>
	<status xmlns="http://www.w3.org/ns/adms#" rdf:resource="https://dev-lexic.swissgeol.ch/active"/>
</rdf:Description>

<rdf:Description rdf:about="https://dev-lexic.swissgeol.ch/TectonicUnits/Faisceaux">
	<rdf:type rdf:resource="http://www.w3.org/2004/02/skos/core#Concept"/>
	<rdfs:isDefinedBy xml:lang="en">Gouffon Yves (Editor) (2024): Tectonic Map of Switzerland 1:500000, Explanatory notes. Federal Office of Topography swisstopo, Wabern</rdfs:isDefinedBy>
	<skos:definition xml:lang="en">The Faisceaux are narrow zones of intense deformation of the External Folded Jura. They separate largely undeformed or only slightly deformed tabular areas known as Plateaux.</skos:definition>
	<skos:inScheme rdf:resource="https://dev-lexic.swissgeol.ch/TectonicUnits"/>
	<skos:prefLabel xml:lang="en">Faisceaux</skos:prefLabel>
	<skos:prefLabel xml:lang="de">Faisceaux</skos:prefLabel>
	<skos:prefLabel xml:lang="fr">Faisceaux</skos:prefLabel>
	<skos:prefLabel xml:lang="it">Faisceaux</skos:prefLabel>
	<skos:broader rdf:resource="https://dev-lexic.swissgeol.ch/TectonicUnits/ExternalFoldedJura"/>
	<status xmlns="http://www.w3.org/ns/adms#" rdf:resource="https://dev-lexic.swissgeol.ch/active"/>
</rdf:Description>

<rdf:Description rdf:about="https://dev-lexic.swissgeol.ch/TectonicUnits/Plateaux">
	<rdf:type rdf:resource="http://www.w3.org/2004/02/skos/core#Concept"/>
	<rdfs:isDefinedBy xml:lang="en">Gouffon Yves (Editor) (2024): Tectonic Map of Switzerland 1:500000, Explanatory notes. Federal Office of Topography swisstopo, Wabern</rdfs:isDefinedBy>
	<skos:definition xml:lang="en">The Plateaux are largely undeformed or only slightly deformed tabular areas of the External Folded Jura. They are separated by narrow zones of intense deformation known as Faisceaux.</skos:definition>
	<skos:inScheme rdf:resource="https://dev-lexic.swissgeol.ch/TectonicUnits"/>
	<skos:prefLabel xml:lang="en">Plateaux</skos:prefLabel>
	<skos:prefLabel xml:lang="fr">Plateaux</skos:prefLabel>
	<skos:prefLabel xml:lang="it">Plateaux</skos:prefLabel>
	<skos:prefLabel xml:lang="de">Plateaux</skos:prefLabel>
	<skos:altLabel xml:lang="de">abgescherter Tafeljura</skos:altLabel>
	<skos:altLabel xml:lang="en">Plateaus</skos:altLabel>
	<skos:broader rdf:resource="https://dev-lexic.swissgeol.ch/TectonicUnits/ExternalFoldedJura"/>
	<status xmlns="http://www.w3.org/ns/adms#" rdf:resource="https://dev-lexic.swissgeol.ch/active"/>
</rdf:Description>

<rdf:Description rdf:about="https://dev-lexic.swissgeol.ch/TectonicUnits/Marbach-BerneckTriangleZone">
	<rdf:type rdf:resource="http://www.w3.org/2004/02/skos/core#Concept"/>
	<rdfs:isDefinedBy xml:lang="en">Gouffon Yves (Editor) (2024): Tectonic Map of Switzerland 1:500000, Explanatory notes. Federal Office of Topography swisstopo, Wabern</rdfs:isDefinedBy>
	<skos:definition xml:lang="en">The Marbach–Berneck Triangle Zone refers to a wedge of Molasse units situated between a S-vergent backthrust that delineates the southern boundary of the Foreland Plateau Molasse and a N-vergent thrust, which marks the northern boundary of the Subalpine Molasse. This discontinuous zone occurs in the Entlebuch area (west-southwest of Luzern) and between the Zürichsee and Lustenau in the Alpine Rhine Valley.</skos:definition>
	<skos:inScheme rdf:resource="https://dev-lexic.swissgeol.ch/TectonicUnits"/>
	<skos:prefLabel xml:lang="en">Marbach-Berneck Triangle Zone</skos:prefLabel>
	<skos:prefLabel xml:lang="de">Marbach-Berneck-Dreieckzone</skos:prefLabel>
	<skos:prefLabel xml:lang="fr">Zone triangulaire de Marbach-Berneck</skos:prefLabel>
	<skos:prefLabel xml:lang="it">Zona triangolare di Marbach-Berneck</skos:prefLabel>
	<skos:altLabel xml:lang="de">Triangelzone</skos:altLabel>
	<skos:broader rdf:resource="https://dev-lexic.swissgeol.ch/TectonicUnits/SubalpineMolasse"/>
	<status xmlns="http://www.w3.org/ns/adms#" rdf:resource="https://dev-lexic.swissgeol.ch/active"/>
</rdf:Description>

<rdf:Description rdf:about="https://dev-lexic.swissgeol.ch/TectonicUnits/SubalpineSliceComplex">
	<rdf:type rdf:resource="http://www.w3.org/2004/02/skos/core#Concept"/>
	<rdfs:isDefinedBy xml:lang="en">Gouffon Yves (Editor) (2024): Tectonic Map of Switzerland 1:500000, Explanatory notes. Federal Office of Topography swisstopo, Wabern</rdfs:isDefinedBy>
	<skos:definition xml:lang="en">The Subalpine Slice Complex of the Molasse Basin defines the northwestern limit of the Alpine nappes across Switzerland (from Le Léman to south of the Bodensee).</skos:definition>
	<skos:inScheme rdf:resource="https://dev-lexic.swissgeol.ch/TectonicUnits"/>
	<skos:prefLabel xml:lang="en">Subalpine Slice Complex</skos:prefLabel>
	<skos:prefLabel xml:lang="de">Subalpiner Schuppenkomplex</skos:prefLabel>
	<skos:prefLabel xml:lang="fr">Complexe d'écailles de la Molasse Subalpine</skos:prefLabel>
	<skos:prefLabel xml:lang="it">Complesso di scaglie della Molassa Subalpina</skos:prefLabel>
	<skos:broader rdf:resource="https://dev-lexic.swissgeol.ch/TectonicUnits/SubalpineMolasse"/>
	<skos:narrower rdf:resource="https://dev-lexic.swissgeol.ch/TectonicUnits/BelmontSlice"/>
	<skos:narrower rdf:resource="https://dev-lexic.swissgeol.ch/TectonicUnits/Lutry-ThononSlice"/>
	<skos:narrower rdf:resource="https://dev-lexic.swissgeol.ch/TectonicUnits/Brecorens-LucingesSlice"/>
	<skos:narrower rdf:resource="https://dev-lexic.swissgeol.ch/TectonicUnits/CullySlice"/>
	<skos:narrower rdf:resource="https://dev-lexic.swissgeol.ch/TectonicUnits/LavauxSlice"/>
	<skos:narrower rdf:resource="https://dev-lexic.swissgeol.ch/TectonicUnits/MontPelerinSlice"/>
	<skos:narrower rdf:resource="https://dev-lexic.swissgeol.ch/TectonicUnits/Vevey-EvianSlice"/>
	<skos:narrower rdf:resource="https://dev-lexic.swissgeol.ch/TectonicUnits/Gerignoz-LaRocheSlice"/>
	<skos:narrower rdf:resource="https://dev-lexic.swissgeol.ch/TectonicUnits/VaulruzSlice"/>
	<skos:narrower rdf:resource="https://dev-lexic.swissgeol.ch/TectonicUnits/Champotey-RamseraSlice"/>
	<skos:narrower rdf:resource="https://dev-lexic.swissgeol.ch/TectonicUnits/LaPattaz-LaHolenaSlice"/>
	<skos:narrower rdf:resource="https://dev-lexic.swissgeol.ch/TectonicUnits/VillarvolardSlice"/>
	<skos:narrower rdf:resource="https://dev-lexic.swissgeol.ch/TectonicUnits/SeftigschwandSlice"/>
	<skos:narrower rdf:resource="https://dev-lexic.swissgeol.ch/TectonicUnits/GiebeleggSlice"/>
	<skos:narrower rdf:resource="https://dev-lexic.swissgeol.ch/TectonicUnits/SteffisburgSlice"/>
	<skos:narrower rdf:resource="https://dev-lexic.swissgeol.ch/TectonicUnits/SchangnauSlice"/>
	<skos:narrower rdf:resource="https://dev-lexic.swissgeol.ch/TectonicUnits/HornbueelSliceZone"/>
	<skos:narrower rdf:resource="https://dev-lexic.swissgeol.ch/TectonicUnits/Blueme-BeichleSlice"/>
	<skos:narrower rdf:resource="https://dev-lexic.swissgeol.ch/TectonicUnits/WolfseggSlice"/>
	<skos:narrower rdf:resource="https://dev-lexic.swissgeol.ch/TectonicUnits/RalligenSliceZone"/>
	<skos:narrower rdf:resource="https://dev-lexic.swissgeol.ch/TectonicUnits/HilfernSlice"/>
	<skos:narrower rdf:resource="https://dev-lexic.swissgeol.ch/TectonicUnits/HoehronenSlice"/>
	<skos:narrower rdf:resource="https://dev-lexic.swissgeol.ch/TectonicUnits/StJostSlice"/>
	<skos:narrower rdf:resource="https://dev-lexic.swissgeol.ch/TectonicUnits/Rigi-RossbergSlice"/>
	<skos:narrower rdf:resource="https://dev-lexic.swissgeol.ch/TectonicUnits/GaebrisSlice"/>
	<skos:narrower rdf:resource="https://dev-lexic.swissgeol.ch/TectonicUnits/KronbergSlice"/>
	<skos:narrower rdf:resource="https://dev-lexic.swissgeol.ch/TectonicUnits/KronbergSouthernZone"/>
	<skos:narrower rdf:resource="https://dev-lexic.swissgeol.ch/TectonicUnits/SchorhuettenbergSlice"/>
	<skos:narrower rdf:resource="https://dev-lexic.swissgeol.ch/TectonicUnits/Speer-StockbergSlice"/>
	<skos:narrower rdf:resource="https://dev-lexic.swissgeol.ch/TectonicUnits/ChraezerliSlice"/>
	<skos:narrower rdf:resource="https://dev-lexic.swissgeol.ch/TectonicUnits/HirschbergSlice"/>
	<skos:narrower rdf:resource="https://dev-lexic.swissgeol.ch/TectonicUnits/HoelzlibergSlice"/>
	<skos:narrower rdf:resource="https://dev-lexic.swissgeol.ch/TectonicUnits/EichbergSlice"/>
	<status xmlns="http://www.w3.org/ns/adms#" rdf:resource="https://dev-lexic.swissgeol.ch/active"/>
</rdf:Description>

<rdf:Description rdf:about="https://dev-lexic.swissgeol.ch/TectonicUnits/BelmontSlice">
	<rdf:type rdf:resource="http://www.w3.org/2004/02/skos/core#Concept"/>
	<rdfs:isDefinedBy xml:lang="en">Gouffon Yves (Editor) (2024): Tectonic Map of Switzerland 1:500000, Explanatory notes. Federal Office of Topography swisstopo, Wabern</rdfs:isDefinedBy>
	<skos:definition xml:lang="en">The Belmont Slice, made up of «Molasse Rouge» and «Molasse à Charbon», is bounded at its base (to the NW) by the Paudèze Fault, which forms the front of the Subalpine Molasse. At its summit (towards the SE), it is separated from the Lutry-Thonon Slice by the Lutrive Fault.</skos:definition>
	<skos:definition xml:lang="fr">L'Écaille de Belmont, constituée de Molasse Rouge et de Molasse à Charbon, est délimitée à sa base (au NW) par l'accident de la Paudèze qui constitue le front de la Molasse subalpine. A son sommet (vers le SE), elle est séparée de l'Écaille de Lutry-Thonon par la faille de la Lutrive.</skos:definition>
	<skos:inScheme rdf:resource="https://dev-lexic.swissgeol.ch/TectonicUnits"/>
	<skos:prefLabel xml:lang="en">Belmont Slice</skos:prefLabel>
	<skos:prefLabel xml:lang="de">Belmont-Schuppe</skos:prefLabel>
	<skos:prefLabel xml:lang="fr">Écaille de Belmont</skos:prefLabel>
	<skos:prefLabel xml:lang="it">Scaglia di Belmont</skos:prefLabel>
	<skos:altLabel xml:lang="fr">écaille de la Paudèze</skos:altLabel>
	<skos:broader rdf:resource="https://dev-lexic.swissgeol.ch/TectonicUnits/SubalpineSliceComplex"/>
	<status xmlns="http://www.w3.org/ns/adms#" rdf:resource="https://dev-lexic.swissgeol.ch/active"/>
</rdf:Description>

<rdf:Description rdf:about="https://dev-lexic.swissgeol.ch/TectonicUnits/Lutry-ThononSlice">
	<rdf:type rdf:resource="http://www.w3.org/2004/02/skos/core#Concept"/>
	<rdfs:isDefinedBy xml:lang="en">Gouffon Yves (Editor) (2024): Tectonic Map of Switzerland 1:500000, Explanatory notes. Federal Office of Topography swisstopo, Wabern</rdfs:isDefinedBy>
	<skos:definition xml:lang="en">In its Swiss part, the Lutry-Thonon Slice consists solely of Molasse Rouge. It is separated from the Belmont Slice by the Lutrive Fault at its base (to the NW), while the Grandvaux Fault separates it from the Cully Slice at its summit (to the SE). In its French part, it includes, in addition to the «Molasse Rouge», the «Grès et Marnes Gris à Gypse» and the «Molasse Grise de Lausanne».</skos:definition>
	<skos:inScheme rdf:resource="https://dev-lexic.swissgeol.ch/TectonicUnits"/>
	<skos:prefLabel xml:lang="en">Lutry-Thonon Slice</skos:prefLabel>
	<skos:prefLabel xml:lang="de">Lutry-Thonon-Schuppe</skos:prefLabel>
	<skos:prefLabel xml:lang="fr">Écaille de Lutry-Thonon</skos:prefLabel>
	<skos:prefLabel xml:lang="it">Scaglia di Lutry-Thonon</skos:prefLabel>
	<skos:broader rdf:resource="https://dev-lexic.swissgeol.ch/TectonicUnits/SubalpineSliceComplex"/>
	<status xmlns="http://www.w3.org/ns/adms#" rdf:resource="https://dev-lexic.swissgeol.ch/active"/>
</rdf:Description>

<rdf:Description rdf:about="https://dev-lexic.swissgeol.ch/TectonicUnits/Brecorens-LucingesSlice">
	<rdf:type rdf:resource="http://www.w3.org/2004/02/skos/core#Concept"/>
	<rdfs:isDefinedBy xml:lang="en">Gouffon Yves (Editor) (2024): Tectonic Map of Switzerland 1:500000, Explanatory notes. Federal Office of Topography swisstopo, Wabern</rdfs:isDefinedBy>
	<skos:definition xml:lang="en">The Brécorens-Lucinges Slice is situated in the inner zone of the Subalpine Molasse of Haute-Savoie, between the Lutry-Evian Slice (below) and the Voirons Nappe (above, with intercalated Infraprealpine Mélange).</skos:definition>
	<skos:inScheme rdf:resource="https://dev-lexic.swissgeol.ch/TectonicUnits"/>
	<skos:prefLabel xml:lang="en">Brécorens-Lucinges Slice</skos:prefLabel>
	<skos:prefLabel xml:lang="de">Brécorens-Lucinges-Schuppe</skos:prefLabel>
	<skos:prefLabel xml:lang="fr">Écaille de Brécorens-Lucinges</skos:prefLabel>
	<skos:prefLabel xml:lang="it">Scaglia di Brécorens-Lucinges</skos:prefLabel>
	<skos:altLabel xml:lang="fr">écaille de Bellevue</skos:altLabel>
	<skos:broader rdf:resource="https://dev-lexic.swissgeol.ch/TectonicUnits/SubalpineSliceComplex"/>
	<status xmlns="http://www.w3.org/ns/adms#" rdf:resource="https://dev-lexic.swissgeol.ch/active"/>
</rdf:Description>

<rdf:Description rdf:about="https://dev-lexic.swissgeol.ch/TectonicUnits/CullySlice">
	<rdf:type rdf:resource="http://www.w3.org/2004/02/skos/core#Concept"/>
	<rdfs:isDefinedBy xml:lang="en">Gouffon Yves (Editor) (2024): Tectonic Map of Switzerland 1:500000, Explanatory notes. Federal Office of Topography swisstopo, Wabern</rdfs:isDefinedBy>
	<skos:definition xml:lang="en">The Cully Slice, composed of Cornalle Sandstone, is overthrust (to the NW) onto the Molasse Rouge of the Lutry-Thonon Slice along the Grandvaux Fault. The Riex-Bahyse Fault separates it upwards (to the SE) from the Lavaux Slice (made up of Cornalle Sandstone as well).</skos:definition>
	<skos:inScheme rdf:resource="https://dev-lexic.swissgeol.ch/TectonicUnits"/>
	<skos:prefLabel xml:lang="en">Cully Slice</skos:prefLabel>
	<skos:prefLabel xml:lang="de">Cully-Schuppe</skos:prefLabel>
	<skos:prefLabel xml:lang="fr">Écaille de Cully</skos:prefLabel>
	<skos:prefLabel xml:lang="it">Scaglia di Cully</skos:prefLabel>
	<skos:broader rdf:resource="https://dev-lexic.swissgeol.ch/TectonicUnits/SubalpineSliceComplex"/>
	<status xmlns="http://www.w3.org/ns/adms#" rdf:resource="https://dev-lexic.swissgeol.ch/active"/>
</rdf:Description>

<rdf:Description rdf:about="https://dev-lexic.swissgeol.ch/TectonicUnits/LavauxSlice">
	<rdf:type rdf:resource="http://www.w3.org/2004/02/skos/core#Concept"/>
	<rdfs:isDefinedBy xml:lang="en">Gouffon Yves (Editor) (2024): Tectonic Map of Switzerland 1:500000, Explanatory notes. Federal Office of Topography swisstopo, Wabern</rdfs:isDefinedBy>
	<skos:definition xml:lang="en">The Lavaux Slice, made up of Cornalle Sandstone, is separated from the Cully Slice by the Riex-Bahyse Fault at its base, while the Bois du Tey Fault separates it from the Mont Pèlerin Slice at its summit.</skos:definition>
	<skos:inScheme rdf:resource="https://dev-lexic.swissgeol.ch/TectonicUnits"/>
	<skos:prefLabel xml:lang="en">Lavaux Slice</skos:prefLabel>
	<skos:prefLabel xml:lang="de">Lavaux-Schuppe</skos:prefLabel>
	<skos:prefLabel xml:lang="fr">Écaille de Lavaux</skos:prefLabel>
	<skos:prefLabel xml:lang="it">Scaglia di Lavaux</skos:prefLabel>
	<skos:broader rdf:resource="https://dev-lexic.swissgeol.ch/TectonicUnits/SubalpineSliceComplex"/>
	<status xmlns="http://www.w3.org/ns/adms#" rdf:resource="https://dev-lexic.swissgeol.ch/active"/>
</rdf:Description>

<rdf:Description rdf:about="https://dev-lexic.swissgeol.ch/TectonicUnits/MontPelerinSlice">
	<rdf:type rdf:resource="http://www.w3.org/2004/02/skos/core#Concept"/>
	<rdfs:isDefinedBy xml:lang="en">Gouffon Yves (Editor) (2024): Tectonic Map of Switzerland 1:500000, Explanatory notes. Federal Office of Topography swisstopo, Wabern</rdfs:isDefinedBy>
	<skos:definition xml:lang="en">The Mont Pèlerin Slice is made up of «Molasse Rouge» and Mont Pèlerin Conglomerate. It is separated from the Lavaux Slcie by the Bois du Tey Fault at its base (to the NW), while the Veveyse Fault separates it from the Vevey-Evian Slice at its summit (to the SE).</skos:definition>
	<skos:inScheme rdf:resource="https://dev-lexic.swissgeol.ch/TectonicUnits"/>
	<skos:prefLabel xml:lang="en">Mont Pèlerin Slice</skos:prefLabel>
	<skos:prefLabel xml:lang="de">Mont-Pèlerin-Schuppe</skos:prefLabel>
	<skos:prefLabel xml:lang="fr">Écaille du Mont Pèlerin</skos:prefLabel>
	<skos:prefLabel xml:lang="it">Scaglia del Mont Pèlerin</skos:prefLabel>
	<skos:broader rdf:resource="https://dev-lexic.swissgeol.ch/TectonicUnits/SubalpineSliceComplex"/>
	<status xmlns="http://www.w3.org/ns/adms#" rdf:resource="https://dev-lexic.swissgeol.ch/active"/>
</rdf:Description>

<rdf:Description rdf:about="https://dev-lexic.swissgeol.ch/TectonicUnits/Vevey-EvianSlice">
	<rdf:type rdf:resource="http://www.w3.org/2004/02/skos/core#Concept"/>
	<rdfs:isDefinedBy xml:lang="en">Gouffon Yves (Editor) (2024): Tectonic Map of Switzerland 1:500000, Explanatory notes. Federal Office of Topography swisstopo, Wabern</rdfs:isDefinedBy>
	<skos:definition xml:lang="en">The Vevey–Evian Slice consists exclusively of «Molasse Rouge» (Vevey-type, proximal facies). Its front, the Veveyse Fault, successively intersects the Mont Pèlerin, Lavaux and Cully slices. It is separated from the front of the preapine units by two narrow UMM slices.</skos:definition>
	<skos:inScheme rdf:resource="https://dev-lexic.swissgeol.ch/TectonicUnits"/>
	<skos:prefLabel xml:lang="en">Vevey-Evian Slice</skos:prefLabel>
	<skos:prefLabel xml:lang="de">Vevey-Evian-Schuppe</skos:prefLabel>
	<skos:prefLabel xml:lang="fr">Écaille de Vevey-Evian</skos:prefLabel>
	<skos:prefLabel xml:lang="it">Scaglia di Vevey-Evian</skos:prefLabel>
	<skos:broader rdf:resource="https://dev-lexic.swissgeol.ch/TectonicUnits/SubalpineSliceComplex"/>
	<status xmlns="http://www.w3.org/ns/adms#" rdf:resource="https://dev-lexic.swissgeol.ch/active"/>
</rdf:Description>

<rdf:Description rdf:about="https://dev-lexic.swissgeol.ch/TectonicUnits/Gerignoz-LaRocheSlice">
	<rdf:type rdf:resource="http://www.w3.org/2004/02/skos/core#Concept"/>
	<rdfs:isDefinedBy xml:lang="en">Gouffon Yves (Editor) (2024): Tectonic Map of Switzerland 1:500000, Explanatory notes. Federal Office of Topography swisstopo, Wabern</rdfs:isDefinedBy>
	<skos:definition xml:lang="en">The Gérignoz–La Roche Slice is the frontal slice of the Subalpine Molasse in the Fribourg region. It is composed of a tectonised series («Couches du Gérignoz») more or less equivalent to (or transitional between) «Molasse Rouge» and «Molasse à Charbon».</skos:definition>
	<skos:inScheme rdf:resource="https://dev-lexic.swissgeol.ch/TectonicUnits"/>
	<skos:prefLabel xml:lang="en">Gérignoz - La Roche Slice</skos:prefLabel>
	<skos:prefLabel xml:lang="de">Gérignoz-La-Roche-Schuppe</skos:prefLabel>
	<skos:prefLabel xml:lang="fr">Écaille du Gérignoz - La Roche</skos:prefLabel>
	<skos:prefLabel xml:lang="it">Scaglia del Gérignoz - La Roche</skos:prefLabel>
	<skos:broader rdf:resource="https://dev-lexic.swissgeol.ch/TectonicUnits/SubalpineSliceComplex"/>
	<status xmlns="http://www.w3.org/ns/adms#" rdf:resource="https://dev-lexic.swissgeol.ch/active"/>
</rdf:Description>

<rdf:Description rdf:about="https://dev-lexic.swissgeol.ch/TectonicUnits/VaulruzSlice">
	<rdf:type rdf:resource="http://www.w3.org/2004/02/skos/core#Concept"/>
	<rdfs:isDefinedBy xml:lang="en">Gouffon Yves (Editor) (2024): Tectonic Map of Switzerland 1:500000, Explanatory notes. Federal Office of Topography swisstopo, Wabern</rdfs:isDefinedBy>
	<skos:definition xml:lang="en">The Vaulruz Slice is a tectonic unit of the Subalpine Molasse of Western Switzerland (between Châtel-St-Denis and Bulle/Gruyère region). It is composed of Lower Marine Molasse (UMM) and basal parts of the Lower Freshwater Molasse (USM, «Molasse Rouge»).</skos:definition>
	<skos:inScheme rdf:resource="https://dev-lexic.swissgeol.ch/TectonicUnits"/>
	<skos:prefLabel xml:lang="en">Vaulruz Slice</skos:prefLabel>
	<skos:prefLabel xml:lang="de">Vaulruz-Schuppe</skos:prefLabel>
	<skos:prefLabel xml:lang="fr">Écaille de Vaulruz</skos:prefLabel>
	<skos:prefLabel xml:lang="it">Scaglia di Vaulruz</skos:prefLabel>
	<skos:altLabel xml:lang="fr">écaille de Prévondavau</skos:altLabel>
	<skos:broader rdf:resource="https://dev-lexic.swissgeol.ch/TectonicUnits/SubalpineSliceComplex"/>
	<status xmlns="http://www.w3.org/ns/adms#" rdf:resource="https://dev-lexic.swissgeol.ch/active"/>
</rdf:Description>

<rdf:Description rdf:about="https://dev-lexic.swissgeol.ch/TectonicUnits/Champotey-RamseraSlice">
	<rdf:type rdf:resource="http://www.w3.org/2004/02/skos/core#Concept"/>
	<rdfs:isDefinedBy xml:lang="en">Gouffon Yves (Editor) (2024): Tectonic Map of Switzerland 1:500000, Explanatory notes. Federal Office of Topography swisstopo, Wabern</rdfs:isDefinedBy>
	<skos:definition xml:lang="en">The Champotey–Ramsera Slice is a tectonic unit of the Subalpine Molasse in the Bulle/Gruyère region, comprised between the Vaulruz Slice (below) and the La Pattaz - La Holena Slice (above). It is composed of Lower Marine Molasse (UMM).</skos:definition>
	<skos:inScheme rdf:resource="https://dev-lexic.swissgeol.ch/TectonicUnits"/>
	<skos:prefLabel xml:lang="en">Champotey-Ramsera Slice</skos:prefLabel>
	<skos:prefLabel xml:lang="de">Champotey-Ramsera-Schuppe</skos:prefLabel>
	<skos:prefLabel xml:lang="fr">Écaille de Champotey-Ramsera</skos:prefLabel>
	<skos:prefLabel xml:lang="it">Scaglia di Champotey-Ramsera</skos:prefLabel>
	<skos:broader rdf:resource="https://dev-lexic.swissgeol.ch/TectonicUnits/SubalpineSliceComplex"/>
	<status xmlns="http://www.w3.org/ns/adms#" rdf:resource="https://dev-lexic.swissgeol.ch/active"/>
</rdf:Description>

<rdf:Description rdf:about="https://dev-lexic.swissgeol.ch/TectonicUnits/LaPattaz-LaHolenaSlice">
	<rdf:type rdf:resource="http://www.w3.org/2004/02/skos/core#Concept"/>
	<rdfs:isDefinedBy xml:lang="en">Gouffon Yves (Editor) (2024): Tectonic Map of Switzerland 1:500000, Explanatory notes. Federal Office of Topography swisstopo, Wabern</rdfs:isDefinedBy>
	<skos:definition xml:lang="en">The La Pattaz–La Holena Slice is a tectonic unit of the Subalpine Molasse in the Bulle/Gruyère region, comprised between the Champotey–Ramsera Slice (below, to the north) and the Villarvolard Slice (above, to the south). It is composed of Lower Marine Molasse (UMM).</skos:definition>
	<skos:inScheme rdf:resource="https://dev-lexic.swissgeol.ch/TectonicUnits"/>
	<skos:prefLabel xml:lang="en">La Pattaz - La Holena Slice</skos:prefLabel>
	<skos:prefLabel xml:lang="de">La-Pattaz-La-Holena-Schuppe</skos:prefLabel>
	<skos:prefLabel xml:lang="fr">Écaille de La Pattaz - La Holena</skos:prefLabel>
	<skos:prefLabel xml:lang="it">Scaglia di La Pattaz - La Holena</skos:prefLabel>
	<skos:broader rdf:resource="https://dev-lexic.swissgeol.ch/TectonicUnits/SubalpineSliceComplex"/>
	<status xmlns="http://www.w3.org/ns/adms#" rdf:resource="https://dev-lexic.swissgeol.ch/active"/>
</rdf:Description>

<rdf:Description rdf:about="https://dev-lexic.swissgeol.ch/TectonicUnits/VillarvolardSlice">
	<rdf:type rdf:resource="http://www.w3.org/2004/02/skos/core#Concept"/>
	<rdfs:isDefinedBy xml:lang="en">Gouffon Yves (Editor) (2024): Tectonic Map of Switzerland 1:500000, Explanatory notes. Federal Office of Topography swisstopo, Wabern</rdfs:isDefinedBy>
	<skos:definition xml:lang="en">The Villarvolard Slice is the southernmost (most internal) tectonic unit of the Subalpine Molasse of Western Switzerland (between the Léman and the Berra regions). It is composed of basal Lower Marine Molasse (UMM, transitional from the – originally underlying – flysch facies).</skos:definition>
	<skos:inScheme rdf:resource="https://dev-lexic.swissgeol.ch/TectonicUnits"/>
	<skos:prefLabel xml:lang="en">Villarvolard Slice</skos:prefLabel>
	<skos:prefLabel xml:lang="de">Villarvolard-Schuppe</skos:prefLabel>
	<skos:prefLabel xml:lang="fr">Écaille de Villarvolard</skos:prefLabel>
	<skos:prefLabel xml:lang="it">Scaglia di Villarvolard</skos:prefLabel>
	<skos:broader rdf:resource="https://dev-lexic.swissgeol.ch/TectonicUnits/SubalpineSliceComplex"/>
	<status xmlns="http://www.w3.org/ns/adms#" rdf:resource="https://dev-lexic.swissgeol.ch/active"/>
</rdf:Description>

<rdf:Description rdf:about="https://dev-lexic.swissgeol.ch/TectonicUnits/SeftigschwandSlice">
	<rdf:type rdf:resource="http://www.w3.org/2004/02/skos/core#Concept"/>
	<rdfs:isDefinedBy xml:lang="en">Gouffon Yves (Editor) (2024): Tectonic Map of Switzerland 1:500000, Explanatory notes. Federal Office of Topography swisstopo, Wabern</rdfs:isDefinedBy>
	<skos:definition xml:lang="en">The Seftigschwand Slice is a tectonic unit of the Subalpine Molasse in the Gurnigel region. It is composed of Lower Freshwater Molasse (USM, «Blättermolasse»).</skos:definition>
	<skos:inScheme rdf:resource="https://dev-lexic.swissgeol.ch/TectonicUnits"/>
	<skos:prefLabel xml:lang="en">Seftigschwand Slice</skos:prefLabel>
	<skos:prefLabel xml:lang="de">Seftigschwand-Schuppe</skos:prefLabel>
	<skos:prefLabel xml:lang="fr">Écaille du Seftigschwand</skos:prefLabel>
	<skos:prefLabel xml:lang="it">Scaglia del Seftigschwand</skos:prefLabel>
	<skos:broader rdf:resource="https://dev-lexic.swissgeol.ch/TectonicUnits/SubalpineSliceComplex"/>
	<status xmlns="http://www.w3.org/ns/adms#" rdf:resource="https://dev-lexic.swissgeol.ch/active"/>
</rdf:Description>

<rdf:Description rdf:about="https://dev-lexic.swissgeol.ch/TectonicUnits/GiebeleggSlice">
	<rdf:type rdf:resource="http://www.w3.org/2004/02/skos/core#Concept"/>
	<rdfs:isDefinedBy xml:lang="en">Gouffon Yves (Editor) (2024): Tectonic Map of Switzerland 1:500000, Explanatory notes. Federal Office of Topography swisstopo, Wabern</rdfs:isDefinedBy>
	<skos:definition xml:lang="en">The Giebelegg Slice is the northernmost (most external) and youngest imbricated zone of the Subalpine Molasse in the Gurnigel area. The strata mostly dip between 60° and 80° (steeper in the east than in the west). It is composed of proximal deposits of the Upper Marine Molasse (OMM) with sediment supply from the Napf (older part) and Guggisberg (younger part) alluvial fans.</skos:definition>
	<skos:inScheme rdf:resource="https://dev-lexic.swissgeol.ch/TectonicUnits"/>
	<skos:prefLabel xml:lang="en">Giebelegg Slice</skos:prefLabel>
	<skos:prefLabel xml:lang="de">Giebelegg-Schuppe</skos:prefLabel>
	<skos:prefLabel xml:lang="fr">Écaille de la Giebelegg</skos:prefLabel>
	<skos:prefLabel xml:lang="it">Scaglia della Giebelegg</skos:prefLabel>
	<skos:broader rdf:resource="https://dev-lexic.swissgeol.ch/TectonicUnits/SubalpineSliceComplex"/>
	<status xmlns="http://www.w3.org/ns/adms#" rdf:resource="https://dev-lexic.swissgeol.ch/active"/>
</rdf:Description>

<rdf:Description rdf:about="https://dev-lexic.swissgeol.ch/TectonicUnits/SteffisburgSlice">
	<rdf:type rdf:resource="http://www.w3.org/2004/02/skos/core#Concept"/>
	<rdfs:isDefinedBy xml:lang="en">Gouffon Yves (Editor) (2024): Tectonic Map of Switzerland 1:500000, Explanatory notes. Federal Office of Topography swisstopo, Wabern</rdfs:isDefinedBy>
	<skos:definition xml:lang="en">The Steffisburg Slice is the frontal tectonic unit of the Subalpine Molasse in the region directly north of the Thunersee (lower part of the Zulg valley).</skos:definition>
	<skos:inScheme rdf:resource="https://dev-lexic.swissgeol.ch/TectonicUnits"/>
	<skos:prefLabel xml:lang="en">Steffisburg Slice</skos:prefLabel>
	<skos:prefLabel xml:lang="de">Steffisburg-Schuppe</skos:prefLabel>
	<skos:prefLabel xml:lang="fr">Écaille de Steffisburg</skos:prefLabel>
	<skos:prefLabel xml:lang="it">Scaglia di Steffisburg</skos:prefLabel>
	<skos:broader rdf:resource="https://dev-lexic.swissgeol.ch/TectonicUnits/SubalpineSliceComplex"/>
	<status xmlns="http://www.w3.org/ns/adms#" rdf:resource="https://dev-lexic.swissgeol.ch/active"/>
</rdf:Description>

<rdf:Description rdf:about="https://dev-lexic.swissgeol.ch/TectonicUnits/SchangnauSlice">
	<rdf:type rdf:resource="http://www.w3.org/2004/02/skos/core#Concept"/>
	<rdfs:isDefinedBy xml:lang="en">Gouffon Yves (Editor) (2024): Tectonic Map of Switzerland 1:500000, Explanatory notes. Federal Office of Topography swisstopo, Wabern</rdfs:isDefinedBy>
	<skos:definition xml:lang="en">The Schangnau Slice is the second outermost tectonic unit of the Subalpine Molasse, situated between Steffisburg Slice, resp. the Marbach-Berneck Triangle Zone (below, to the north) and the Blueme-Beichle Slice (above, to the south). It consists exclusively of Lower Freshwater Molasse (USM) with characteristic «granitic sandstone».</skos:definition>
	<skos:inScheme rdf:resource="https://dev-lexic.swissgeol.ch/TectonicUnits"/>
	<skos:prefLabel xml:lang="en">Schangnau Slice</skos:prefLabel>
	<skos:prefLabel xml:lang="de">Schangnau-Schuppe</skos:prefLabel>
	<skos:prefLabel xml:lang="fr">Écaille de Schangnau</skos:prefLabel>
	<skos:prefLabel xml:lang="it">Scaglia di Schangnau</skos:prefLabel>
	<skos:altLabel xml:lang="de">Zulg-Hombach-Zone</skos:altLabel>
	<skos:broader rdf:resource="https://dev-lexic.swissgeol.ch/TectonicUnits/SubalpineSliceComplex"/>
	<status xmlns="http://www.w3.org/ns/adms#" rdf:resource="https://dev-lexic.swissgeol.ch/active"/>
</rdf:Description>

<rdf:Description rdf:about="https://dev-lexic.swissgeol.ch/TectonicUnits/HornbueelSliceZone">
	<rdf:type rdf:resource="http://www.w3.org/2004/02/skos/core#Concept"/>
	<rdfs:isDefinedBy xml:lang="en">Gouffon Yves (Editor) (2024): Tectonic Map of Switzerland 1:500000, Explanatory notes. Federal Office of Topography swisstopo, Wabern</rdfs:isDefinedBy>
	<skos:definition xml:lang="en">The Hornbüel Slice Zone is considered as a tectonic melange. It is situated between the Schangnau Slice (below, to the north) and the Blueme-Beichle Slice (above, to the south) and comprises mainly Horw Sandstone, as well as marl, sandstone and conglomerate of the Lower Freshwater Molasse (USM).</skos:definition>
	<skos:inScheme rdf:resource="https://dev-lexic.swissgeol.ch/TectonicUnits"/>
	<skos:prefLabel xml:lang="en">Hornbüel Slice Zone</skos:prefLabel>
	<skos:prefLabel xml:lang="de">Hornbüel-Schuppenzone</skos:prefLabel>
	<skos:prefLabel xml:lang="fr">Zone d'écailles du Hornbüel</skos:prefLabel>
	<skos:prefLabel xml:lang="it">Zona di scaglie del Hornbüel</skos:prefLabel>
	<skos:broader rdf:resource="https://dev-lexic.swissgeol.ch/TectonicUnits/SubalpineSliceComplex"/>
	<status xmlns="http://www.w3.org/ns/adms#" rdf:resource="https://dev-lexic.swissgeol.ch/active"/>
</rdf:Description>

<rdf:Description rdf:about="https://dev-lexic.swissgeol.ch/TectonicUnits/Blueme-BeichleSlice">
	<rdf:type rdf:resource="http://www.w3.org/2004/02/skos/core#Concept"/>
	<rdfs:isDefinedBy xml:lang="en">Gouffon Yves (Editor) (2024): Tectonic Map of Switzerland 1:500000, Explanatory notes. Federal Office of Topography swisstopo, Wabern</rdfs:isDefinedBy>
	<skos:definition xml:lang="en">The Blueme-Beichle Slice is situated in the inner zone of the Subalpine Molasse, between the Schangnau-Slice (below) and the Hilferen-Slice (above). It is composed of rocks of the Lower Marine Molasse (UMM) and of the Lower Freshwater Molasse (USM).</skos:definition>
	<skos:inScheme rdf:resource="https://dev-lexic.swissgeol.ch/TectonicUnits"/>
	<skos:prefLabel xml:lang="en">Blueme-Beichle Slice</skos:prefLabel>
	<skos:prefLabel xml:lang="de">Blueme-Beichle-Schuppe</skos:prefLabel>
	<skos:prefLabel xml:lang="fr">Écaille de la Blueme-Beichle</skos:prefLabel>
	<skos:prefLabel xml:lang="it">Scaglia della Blueme-Beichle</skos:prefLabel>
	<skos:altLabel xml:lang="de">Bäuchlen-Honegg-Schuppe; Beichlen-Farneren-Schuppe</skos:altLabel>
	<skos:broader rdf:resource="https://dev-lexic.swissgeol.ch/TectonicUnits/SubalpineSliceComplex"/>
	<status xmlns="http://www.w3.org/ns/adms#" rdf:resource="https://dev-lexic.swissgeol.ch/active"/>
</rdf:Description>

<rdf:Description rdf:about="https://dev-lexic.swissgeol.ch/TectonicUnits/WolfseggSlice">
	<rdf:type rdf:resource="http://www.w3.org/2004/02/skos/core#Concept"/>
	<rdfs:isDefinedBy xml:lang="en">Gouffon Yves (Editor) (2024): Tectonic Map of Switzerland 1:500000, Explanatory notes. Federal Office of Topography swisstopo, Wabern</rdfs:isDefinedBy>
	<skos:definition xml:lang="en">The Wolfsegg Slice is a small tectonic unit forming the most internal part of the Subalpine Molasse east of the Gurnigel region. It is composed of basal formations of the Lower Marine Molasse (UMM, Jordisboden Marl and Goldegg Sandstone).</skos:definition>
	<skos:inScheme rdf:resource="https://dev-lexic.swissgeol.ch/TectonicUnits"/>
	<skos:prefLabel xml:lang="en">Wolfsegg Slice</skos:prefLabel>
	<skos:prefLabel xml:lang="de">Wolfsegg-Schuppe</skos:prefLabel>
	<skos:prefLabel xml:lang="fr">Écaille de la Wolfsegg</skos:prefLabel>
	<skos:prefLabel xml:lang="it">Scaglia della Wolfsegg</skos:prefLabel>
	<skos:broader rdf:resource="https://dev-lexic.swissgeol.ch/TectonicUnits/SubalpineSliceComplex"/>
	<status xmlns="http://www.w3.org/ns/adms#" rdf:resource="https://dev-lexic.swissgeol.ch/active"/>
</rdf:Description>

<rdf:Description rdf:about="https://dev-lexic.swissgeol.ch/TectonicUnits/RalligenSliceZone">
	<rdf:type rdf:resource="http://www.w3.org/2004/02/skos/core#Concept"/>
	<rdfs:isDefinedBy xml:lang="en">Gouffon Yves (Editor) (2024): Tectonic Map of Switzerland 1:500000, Explanatory notes. Federal Office of Topography swisstopo, Wabern</rdfs:isDefinedBy>
	<skos:definition xml:lang="en">The Ralligen Slice Zone is a lateral equivalent of the Hilfern Slice in the Thunersee region. It is composed of Lower Marine Molasse (UMM, encompassing the Jordisboden Marl and the Goldegg Sandstone) and takes locally a tectonic mélange character.</skos:definition>
	<skos:inScheme rdf:resource="https://dev-lexic.swissgeol.ch/TectonicUnits"/>
	<skos:prefLabel xml:lang="en">Ralligen Slice Zone</skos:prefLabel>
	<skos:prefLabel xml:lang="de">Ralligen-Schuppenzone</skos:prefLabel>
	<skos:prefLabel xml:lang="fr">Zone d'écailles de Ralligen</skos:prefLabel>
	<skos:prefLabel xml:lang="it">Zona di scaglie di Ralligen</skos:prefLabel>
	<skos:broader rdf:resource="https://dev-lexic.swissgeol.ch/TectonicUnits/SubalpineSliceComplex"/>
	<status xmlns="http://www.w3.org/ns/adms#" rdf:resource="https://dev-lexic.swissgeol.ch/active"/>
</rdf:Description>

<rdf:Description rdf:about="https://dev-lexic.swissgeol.ch/TectonicUnits/HilfernSlice">
	<rdf:type rdf:resource="http://www.w3.org/2004/02/skos/core#Concept"/>
	<rdfs:isDefinedBy xml:lang="en">Gouffon Yves (Editor) (2024): Tectonic Map of Switzerland 1:500000, Explanatory notes. Federal Office of Topography swisstopo, Wabern</rdfs:isDefinedBy>
	<skos:definition xml:lang="en">The Hilfern Slice is the southernmost (most intern) tectonic unit of the Subalpine Molasse between Thunersee and Vierwaldstättersee. It is situated between the Blueme-Beichle Slice (below, to the north) and the Subalpine Flysch Zone (above, to the south). It is mainly composed of rocks of the Lower Marine Molasse (UMM) with subordinated Lower Freshwater Molasse (USM).</skos:definition>
	<skos:inScheme rdf:resource="https://dev-lexic.swissgeol.ch/TectonicUnits"/>
	<skos:prefLabel xml:lang="en">Hilfern Slice</skos:prefLabel>
	<skos:prefLabel xml:lang="de">Hilfern-Schuppe</skos:prefLabel>
	<skos:prefLabel xml:lang="fr">Écaille de la Hilfern</skos:prefLabel>
	<skos:prefLabel xml:lang="it">Scaglia della Hilfern</skos:prefLabel>
	<skos:broader rdf:resource="https://dev-lexic.swissgeol.ch/TectonicUnits/SubalpineSliceComplex"/>
	<status xmlns="http://www.w3.org/ns/adms#" rdf:resource="https://dev-lexic.swissgeol.ch/active"/>
</rdf:Description>

<rdf:Description rdf:about="https://dev-lexic.swissgeol.ch/TectonicUnits/HoehronenSlice">
	<rdf:type rdf:resource="http://www.w3.org/2004/02/skos/core#Concept"/>
	<rdfs:isDefinedBy xml:lang="en">Gouffon Yves (Editor) (2024): Tectonic Map of Switzerland 1:500000, Explanatory notes. Federal Office of Topography swisstopo, Wabern</rdfs:isDefinedBy>
	<skos:definition xml:lang="en">The Höhronen Slice is the frontal slice of the Subalpine Molasse in the Lucerne - Zug region. It is composed of coarse deposits of the Lower Freshwater Molasse (USM).</skos:definition>
	<skos:inScheme rdf:resource="https://dev-lexic.swissgeol.ch/TectonicUnits"/>
	<skos:prefLabel xml:lang="en">Höhronen Slice</skos:prefLabel>
	<skos:prefLabel xml:lang="de">Höhronen-Schuppe</skos:prefLabel>
	<skos:prefLabel xml:lang="fr">Écaille du Höhronen</skos:prefLabel>
	<skos:prefLabel xml:lang="it">Scaglia del Höhronen</skos:prefLabel>
	<skos:broader rdf:resource="https://dev-lexic.swissgeol.ch/TectonicUnits/SubalpineSliceComplex"/>
	<status xmlns="http://www.w3.org/ns/adms#" rdf:resource="https://dev-lexic.swissgeol.ch/active"/>
</rdf:Description>

<rdf:Description rdf:about="https://dev-lexic.swissgeol.ch/TectonicUnits/StJostSlice">
	<rdf:type rdf:resource="http://www.w3.org/2004/02/skos/core#Concept"/>
	<rdfs:isDefinedBy xml:lang="en">Gouffon Yves (Editor) (2024): Tectonic Map of Switzerland 1:500000, Explanatory notes. Federal Office of Topography swisstopo, Wabern</rdfs:isDefinedBy>
	<skos:definition xml:lang="en">The St. Jost Slice is a small tectonic unit of the Subalpine Molasse between the Zugersee and the Linth valley. It is situated between the Höhronen Slice, resp. the Marbach-Berneck Triangle Zone (below, to the north) and the Rigi-Rossberg Slice (above, to the south).</skos:definition>
	<skos:inScheme rdf:resource="https://dev-lexic.swissgeol.ch/TectonicUnits"/>
	<skos:prefLabel xml:lang="en">St. Jost Slice</skos:prefLabel>
	<skos:prefLabel xml:lang="de">St.-Jost-Schuppe</skos:prefLabel>
	<skos:prefLabel xml:lang="fr">Écaille de St-Jost</skos:prefLabel>
	<skos:prefLabel xml:lang="it">Scaglia di St. Jost</skos:prefLabel>
	<skos:altLabel xml:lang="de">Grindelegg-Schuppe</skos:altLabel>
	<skos:broader rdf:resource="https://dev-lexic.swissgeol.ch/TectonicUnits/SubalpineSliceComplex"/>
	<status xmlns="http://www.w3.org/ns/adms#" rdf:resource="https://dev-lexic.swissgeol.ch/active"/>
</rdf:Description>

<rdf:Description rdf:about="https://dev-lexic.swissgeol.ch/TectonicUnits/Rigi-RossbergSlice">
	<rdf:type rdf:resource="http://www.w3.org/2004/02/skos/core#Concept"/>
	<rdfs:isDefinedBy xml:lang="en">Gouffon Yves (Editor) (2024): Tectonic Map of Switzerland 1:500000, Explanatory notes. Federal Office of Topography swisstopo, Wabern</rdfs:isDefinedBy>
	<skos:definition xml:lang="en">The Rigi-Rossberg Slice is the southernmost and highest tectonic unit of the Subalpine Molasse between the Vierwaldstättersee and the Linth valley. It is situated between the Höhronen Slice (below, to the north; regionally with the intercalated St. Jost Slice) and the Alpine front s.s. (above, to the south).</skos:definition>
	<skos:inScheme rdf:resource="https://dev-lexic.swissgeol.ch/TectonicUnits"/>
	<skos:prefLabel xml:lang="en">Rigi-Rossberg Slice</skos:prefLabel>
	<skos:prefLabel xml:lang="de">Rigi-Rossberg-Schuppe</skos:prefLabel>
	<skos:prefLabel xml:lang="fr">Écaille du Rigi-Rossberg</skos:prefLabel>
	<skos:prefLabel xml:lang="it">Scaglia del Rigi-Rossberg</skos:prefLabel>
	<skos:altLabel xml:lang="de">Morgarten-Schuppe</skos:altLabel>
	<skos:broader rdf:resource="https://dev-lexic.swissgeol.ch/TectonicUnits/SubalpineSliceComplex"/>
	<status xmlns="http://www.w3.org/ns/adms#" rdf:resource="https://dev-lexic.swissgeol.ch/active"/>
</rdf:Description>

<rdf:Description rdf:about="https://dev-lexic.swissgeol.ch/TectonicUnits/GaebrisSlice">
	<rdf:type rdf:resource="http://www.w3.org/2004/02/skos/core#Concept"/>
	<rdfs:isDefinedBy xml:lang="en">Gouffon Yves (Editor) (2024): Tectonic Map of Switzerland 1:500000, Explanatory notes. Federal Office of Topography swisstopo, Wabern</rdfs:isDefinedBy>
	<skos:definition xml:lang="en">The Gäbris Slice is a tectonic unit situated in the external zone of the Subalpine Molasse of Eastern Switzerland, bewteen the Marbach-Berneck Triangle Zone (below) and the Kronberg Slice (above).</skos:definition>
	<skos:inScheme rdf:resource="https://dev-lexic.swissgeol.ch/TectonicUnits"/>
	<skos:prefLabel xml:lang="en">Gäbris Slice</skos:prefLabel>
	<skos:prefLabel xml:lang="de">Gäbris-Schuppe</skos:prefLabel>
	<skos:prefLabel xml:lang="fr">Écaille du Gäbris</skos:prefLabel>
	<skos:prefLabel xml:lang="it">Scaglia del Gäbris</skos:prefLabel>
	<skos:broader rdf:resource="https://dev-lexic.swissgeol.ch/TectonicUnits/SubalpineSliceComplex"/>
	<status xmlns="http://www.w3.org/ns/adms#" rdf:resource="https://dev-lexic.swissgeol.ch/active"/>
</rdf:Description>

<rdf:Description rdf:about="https://dev-lexic.swissgeol.ch/TectonicUnits/KronbergSlice">
	<rdf:type rdf:resource="http://www.w3.org/2004/02/skos/core#Concept"/>
	<rdfs:isDefinedBy xml:lang="en">Gouffon Yves (Editor) (2024): Tectonic Map of Switzerland 1:500000, Explanatory notes. Federal Office of Topography swisstopo, Wabern</rdfs:isDefinedBy>
	<skos:definition xml:lang="en">The Kronberg Slice is a large tectonic unit in the median part of the Subalpine Molasse between the Linth and the Rhine valleys. It is composed of a thick sequence of Lower Freshwater Molasse (USM).</skos:definition>
	<skos:inScheme rdf:resource="https://dev-lexic.swissgeol.ch/TectonicUnits"/>
	<skos:prefLabel xml:lang="en">Kronberg Slice</skos:prefLabel>
	<skos:prefLabel xml:lang="de">Kronberg-Schuppe</skos:prefLabel>
	<skos:prefLabel xml:lang="fr">Écaille du Kronberg</skos:prefLabel>
	<skos:prefLabel xml:lang="it">Scaglia del Kronberg</skos:prefLabel>
	<skos:broader rdf:resource="https://dev-lexic.swissgeol.ch/TectonicUnits/SubalpineSliceComplex"/>
	<status xmlns="http://www.w3.org/ns/adms#" rdf:resource="https://dev-lexic.swissgeol.ch/active"/>
</rdf:Description>

<rdf:Description rdf:about="https://dev-lexic.swissgeol.ch/TectonicUnits/KronbergSouthernZone">
	<rdf:type rdf:resource="http://www.w3.org/2004/02/skos/core#Concept"/>
	<rdfs:isDefinedBy xml:lang="en">Gouffon Yves (Editor) (2024): Tectonic Map of Switzerland 1:500000, Explanatory notes. Federal Office of Topography swisstopo, Wabern</rdfs:isDefinedBy>
	<skos:definition xml:lang="en">The «Kronberg Southern Zone» is a strongly deformed zone situated at the southern edge of the Kronberg Slice.</skos:definition>
	<skos:inScheme rdf:resource="https://dev-lexic.swissgeol.ch/TectonicUnits"/>
	<skos:prefLabel xml:lang="en">«Kronberg Southern Zone»</skos:prefLabel>
	<skos:prefLabel xml:lang="de">«Zone Kronberg-Süd»</skos:prefLabel>
	<skos:prefLabel xml:lang="fr">«Zone sud de Kronberg»</skos:prefLabel>
	<skos:prefLabel xml:lang="it">«Zona sud del Kronberg»</skos:prefLabel>
	<skos:broader rdf:resource="https://dev-lexic.swissgeol.ch/TectonicUnits/SubalpineSliceComplex"/>
	<status xmlns="http://www.w3.org/ns/adms#" rdf:resource="https://dev-lexic.swissgeol.ch/active"/>
</rdf:Description>

<rdf:Description rdf:about="https://dev-lexic.swissgeol.ch/TectonicUnits/SchorhuettenbergSlice">
	<rdf:type rdf:resource="http://www.w3.org/2004/02/skos/core#Concept"/>
	<rdfs:isDefinedBy xml:lang="en">Gouffon Yves (Editor) (2024): Tectonic Map of Switzerland 1:500000, Explanatory notes. Federal Office of Topography swisstopo, Wabern</rdfs:isDefinedBy>
	<skos:definition xml:lang="en">The Schorhüttenberg Slice is a tectonic unit situated to the north of the Speer-Stockberg Slice between the Linth and Thur valleys. It is characterised by cross-bedded, calcareous sandstones («Ebnat Sandstone»).</skos:definition>
	<skos:inScheme rdf:resource="https://dev-lexic.swissgeol.ch/TectonicUnits"/>
	<skos:prefLabel xml:lang="en">Schorhüttenberg Slice</skos:prefLabel>
	<skos:prefLabel xml:lang="de">Schorhüttenberg-Schuppe</skos:prefLabel>
	<skos:prefLabel xml:lang="fr">Écaille du Schorhüttenberg</skos:prefLabel>
	<skos:prefLabel xml:lang="it">Scaglia dello Schorhüttenberg</skos:prefLabel>
	<skos:broader rdf:resource="https://dev-lexic.swissgeol.ch/TectonicUnits/SubalpineSliceComplex"/>
	<status xmlns="http://www.w3.org/ns/adms#" rdf:resource="https://dev-lexic.swissgeol.ch/active"/>
</rdf:Description>

<rdf:Description rdf:about="https://dev-lexic.swissgeol.ch/TectonicUnits/Speer-StockbergSlice">
	<rdf:type rdf:resource="http://www.w3.org/2004/02/skos/core#Concept"/>
	<rdfs:isDefinedBy xml:lang="en">Gouffon Yves (Editor) (2024): Tectonic Map of Switzerland 1:500000, Explanatory notes. Federal Office of Topography swisstopo, Wabern</rdfs:isDefinedBy>
	<skos:definition xml:lang="en">The Speer–Stockberg Slice is the southermost (most intern) tectonic unit of the Subalpine Molasse between the Linth and Necker valleys. It is composed of Lower Marine Molasse (UMM) and Lower Freshwater Molasse (USM).</skos:definition>
	<skos:inScheme rdf:resource="https://dev-lexic.swissgeol.ch/TectonicUnits"/>
	<skos:prefLabel xml:lang="en">Speer-Stockberg Slice</skos:prefLabel>
	<skos:prefLabel xml:lang="de">Speer-Stockberg-Schuppe</skos:prefLabel>
	<skos:prefLabel xml:lang="fr">Écaille du Speer-Stockberg</skos:prefLabel>
	<skos:prefLabel xml:lang="it">Scaglia dello Speer-Stockberg</skos:prefLabel>
	<skos:broader rdf:resource="https://dev-lexic.swissgeol.ch/TectonicUnits/SubalpineSliceComplex"/>
	<status xmlns="http://www.w3.org/ns/adms#" rdf:resource="https://dev-lexic.swissgeol.ch/active"/>
</rdf:Description>

<rdf:Description rdf:about="https://dev-lexic.swissgeol.ch/TectonicUnits/ChraezerliSlice">
	<rdf:type rdf:resource="http://www.w3.org/2004/02/skos/core#Concept"/>
	<rdfs:isDefinedBy xml:lang="en">Gouffon Yves (Editor) (2024): Tectonic Map of Switzerland 1:500000, Explanatory notes. Federal Office of Topography swisstopo, Wabern</rdfs:isDefinedBy>
	<skos:definition xml:lang="en">The Chräzerli Slice is a tectonic unit situated to the north of the Speer-Stockberg-Slice (resp. in direct contact with the Säntis Nappe) and thrust onto the kronberg Slice. It is characterized by coarse-grained, poorly sorted, very dolomite-rich calcareous sandstones.</skos:definition>
	<skos:inScheme rdf:resource="https://dev-lexic.swissgeol.ch/TectonicUnits"/>
	<skos:prefLabel xml:lang="en">Chräzerli Slice</skos:prefLabel>
	<skos:prefLabel xml:lang="de">Chräzerli-Schuppe</skos:prefLabel>
	<skos:prefLabel xml:lang="fr">Écaille de Chräzerli</skos:prefLabel>
	<skos:prefLabel xml:lang="it">Scaglia di Chräzerli</skos:prefLabel>
	<skos:altLabel xml:lang="de">Kräzerli-Schuppe</skos:altLabel>
	<skos:broader rdf:resource="https://dev-lexic.swissgeol.ch/TectonicUnits/SubalpineSliceComplex"/>
	<status xmlns="http://www.w3.org/ns/adms#" rdf:resource="https://dev-lexic.swissgeol.ch/active"/>
</rdf:Description>

<rdf:Description rdf:about="https://dev-lexic.swissgeol.ch/TectonicUnits/HirschbergSlice">
	<rdf:type rdf:resource="http://www.w3.org/2004/02/skos/core#Concept"/>
	<rdfs:isDefinedBy xml:lang="en">Gouffon Yves (Editor) (2024): Tectonic Map of Switzerland 1:500000, Explanatory notes. Federal Office of Topography swisstopo, Wabern</rdfs:isDefinedBy>
	<skos:definition xml:lang="en">The Hirschberg Slice is a tectonic unit situated in the inner zone of the Subalpine Molasse of Eastern Switzerland, between the Kronberg Slice (below, to the north) and the Hölzliberg Slice (above, to the south).</skos:definition>
	<skos:inScheme rdf:resource="https://dev-lexic.swissgeol.ch/TectonicUnits"/>
	<skos:prefLabel xml:lang="en">Hirschberg Slice</skos:prefLabel>
	<skos:prefLabel xml:lang="de">Hirschberg-Schuppe</skos:prefLabel>
	<skos:prefLabel xml:lang="fr">Écaille du Hirschberg</skos:prefLabel>
	<skos:prefLabel xml:lang="it">Scaglia del Hirschberg</skos:prefLabel>
	<skos:broader rdf:resource="https://dev-lexic.swissgeol.ch/TectonicUnits/SubalpineSliceComplex"/>
	<status xmlns="http://www.w3.org/ns/adms#" rdf:resource="https://dev-lexic.swissgeol.ch/active"/>
</rdf:Description>

<rdf:Description rdf:about="https://dev-lexic.swissgeol.ch/TectonicUnits/HoelzlibergSlice">
	<rdf:type rdf:resource="http://www.w3.org/2004/02/skos/core#Concept"/>
	<rdfs:isDefinedBy xml:lang="en">Gouffon Yves (Editor) (2024): Tectonic Map of Switzerland 1:500000, Explanatory notes. Federal Office of Topography swisstopo, Wabern</rdfs:isDefinedBy>
	<skos:definition xml:lang="en">The Hölzliberg Slice is a tectonic unit situated in the inner zone of the Subalpine Molasse of Eastern Switzerland, between the Hirschberg Slice (below, to the north) and the Eichberg Slice, resp. the Wildhaus Mélange (above, to the south).</skos:definition>
	<skos:inScheme rdf:resource="https://dev-lexic.swissgeol.ch/TectonicUnits"/>
	<skos:prefLabel xml:lang="en">Hölzliberg Slice</skos:prefLabel>
	<skos:prefLabel xml:lang="de">Hölzliberg-Schuppe</skos:prefLabel>
	<skos:prefLabel xml:lang="fr">Écaille du Hölzliberg</skos:prefLabel>
	<skos:prefLabel xml:lang="it">Scaglia del Hölzliberg</skos:prefLabel>
	<skos:broader rdf:resource="https://dev-lexic.swissgeol.ch/TectonicUnits/SubalpineSliceComplex"/>
	<status xmlns="http://www.w3.org/ns/adms#" rdf:resource="https://dev-lexic.swissgeol.ch/active"/>
</rdf:Description>

<rdf:Description rdf:about="https://dev-lexic.swissgeol.ch/TectonicUnits/EichbergSlice">
	<rdf:type rdf:resource="http://www.w3.org/2004/02/skos/core#Concept"/>
	<rdfs:isDefinedBy xml:lang="en">Gouffon Yves (Editor) (2024): Tectonic Map of Switzerland 1:500000, Explanatory notes. Federal Office of Topography swisstopo, Wabern</rdfs:isDefinedBy>
	<skos:definition xml:lang="en">The Eichberg Slice is a strongly deformed tectonic unit situated in the inner zone of the Subalpine Molasse of Eastern Switzerland, between the Hölzliberg Slice (below) and the Wildhaus Mélange (above, mainly comprising Amden Marl).</skos:definition>
	<skos:inScheme rdf:resource="https://dev-lexic.swissgeol.ch/TectonicUnits"/>
	<skos:prefLabel xml:lang="en">Eichberg Slice</skos:prefLabel>
	<skos:prefLabel xml:lang="de">Eichberg-Schuppe</skos:prefLabel>
	<skos:prefLabel xml:lang="fr">Écaille de Eichberg</skos:prefLabel>
	<skos:prefLabel xml:lang="it">Scaglia di Eichberg</skos:prefLabel>
	<skos:broader rdf:resource="https://dev-lexic.swissgeol.ch/TectonicUnits/SubalpineSliceComplex"/>
	<status xmlns="http://www.w3.org/ns/adms#" rdf:resource="https://dev-lexic.swissgeol.ch/active"/>
</rdf:Description>

<rdf:Description rdf:about="https://dev-lexic.swissgeol.ch/TectonicUnits/Helvetic">
	<rdf:type rdf:resource="http://www.w3.org/2004/02/skos/core#Concept"/>
	<rdfs:isDefinedBy xml:lang="en">Gouffon Yves (Editor) (2024): Tectonic Map of Switzerland 1:500000, Explanatory notes. Federal Office of Topography swisstopo, Wabern</rdfs:isDefinedBy>
	<rdfs:comment rdf:datatype="http://www.w3.org/1999/02/22-rdf-syntax-ns#HTML">https://data.geo.admin.ch/ch.swisstopo.geologie-tektonische_karte/pdf/Erl-TK500_2024.pdf</rdfs:comment>
	<rdfs:comment rdf:datatype="http://www.w3.org/1999/02/22-rdf-syntax-ns#HTML">https://www.strati.ch/en/tectonic/helvetic</rdfs:comment>
	<skos:definition xml:lang="en">The Helvetic tectonic domain comprises the sedimentary series (Late Carboniferous to Early Oligocene) initially deposited on the ante-alpine South European continental margin, as well as the underlying crystalline basement.</skos:definition>
	<skos:inScheme rdf:resource="https://dev-lexic.swissgeol.ch/TectonicUnits"/>
	<skos:topConceptOf rdf:resource="https://dev-lexic.swissgeol.ch/TectonicUnits"/>
	<skos:prefLabel xml:lang="en">Helvetic</skos:prefLabel>
	<skos:prefLabel xml:lang="de">Helvetikum</skos:prefLabel>
	<skos:prefLabel xml:lang="fr">Helvétique</skos:prefLabel>
	<skos:prefLabel xml:lang="it">Elvetico</skos:prefLabel>
	<skos:narrower rdf:resource="https://dev-lexic.swissgeol.ch/TectonicUnits/LowerHelvetic"/>
	<skos:narrower rdf:resource="https://dev-lexic.swissgeol.ch/TectonicUnits/UpperHelvetic"/>
	<status xmlns="http://www.w3.org/ns/adms#" rdf:resource="https://dev-lexic.swissgeol.ch/active"/>
</rdf:Description>

<rdf:Description rdf:about="https://dev-lexic.swissgeol.ch/TectonicUnits/LowerHelvetic">
	<rdf:type rdf:resource="http://www.w3.org/2004/02/skos/core#Concept"/>
	<rdfs:isDefinedBy xml:lang="en">Gouffon Yves (Editor) (2024): Tectonic Map of Switzerland 1:500000, Explanatory notes. Federal Office of Topography swisstopo, Wabern</rdfs:isDefinedBy>
	<skos:definition xml:lang="en">The Lower Helvetic tectonic subdomain comprises all the sedimentary and crystalline units below the Glarus (eastern Switzerland), Axen (central Switzerland), Diablerets and Wildhorn major thrusts (western Switzerland). It corresponds to the External Crystalline Massifs and what was formerly called the “Infrahelvetic complex” that includes imbricates with North Helvetic facies as well as sedimentary nappes with South Helvetic to Ultrahelvetic facies.</skos:definition>
	<skos:inScheme rdf:resource="https://dev-lexic.swissgeol.ch/TectonicUnits"/>
	<skos:prefLabel xml:lang="en">Lower Helvetic</skos:prefLabel>
	<skos:prefLabel xml:lang="de">Unterhelvetikum</skos:prefLabel>
	<skos:prefLabel xml:lang="fr">Helvétique inférieur</skos:prefLabel>
	<skos:prefLabel xml:lang="it">Elvetico inferiore</skos:prefLabel>
	<skos:broader rdf:resource="https://dev-lexic.swissgeol.ch/TectonicUnits/Helvetic"/>
	<skos:narrower rdf:resource="https://dev-lexic.swissgeol.ch/TectonicUnits/SubalpineFlyschZone"/>
	<skos:narrower rdf:resource="https://dev-lexic.swissgeol.ch/TectonicUnits/BelledonneMassif"/>
	<skos:narrower rdf:resource="https://dev-lexic.swissgeol.ch/TectonicUnits/AiguillesRougesMassif"/>
	<skos:narrower rdf:resource="https://dev-lexic.swissgeol.ch/TectonicUnits/MontBlancMassif"/>
	<skos:narrower rdf:resource="https://dev-lexic.swissgeol.ch/TectonicUnits/AarMassif"/>
	<skos:narrower rdf:resource="https://dev-lexic.swissgeol.ch/TectonicUnits/ChainesSubalpinesNappe"/>
	<skos:narrower rdf:resource="https://dev-lexic.swissgeol.ch/TectonicUnits/MorclesNappe"/>
	<skos:narrower rdf:resource="https://dev-lexic.swissgeol.ch/TectonicUnits/ArdonNappe"/>
	<skos:narrower rdf:resource="https://dev-lexic.swissgeol.ch/TectonicUnits/DoldenhornNappe"/>
	<skos:narrower rdf:resource="https://dev-lexic.swissgeol.ch/TectonicUnits/GellihornNappe"/>
	<skos:narrower rdf:resource="https://dev-lexic.swissgeol.ch/TectonicUnits/PlammisNappe"/>
	<skos:narrower rdf:resource="https://dev-lexic.swissgeol.ch/TectonicUnits/JaegerchruezNappe"/>
	<skos:narrower rdf:resource="https://dev-lexic.swissgeol.ch/TectonicUnits/KammlistockNappe"/>
	<skos:narrower rdf:resource="https://dev-lexic.swissgeol.ch/TectonicUnits/GriessstockNappe"/>
	<skos:narrower rdf:resource="https://dev-lexic.swissgeol.ch/TectonicUnits/ClaridenSliceComplex"/>
	<skos:narrower rdf:resource="https://dev-lexic.swissgeol.ch/TectonicUnits/Fiseten-OrthaldenSlices"/>
	<skos:narrower rdf:resource="https://dev-lexic.swissgeol.ch/TectonicUnits/CavistrauNappe"/>
	<skos:narrower rdf:resource="https://dev-lexic.swissgeol.ch/TectonicUnits/Chropfsberg-PizalunSlices"/>
	<skos:narrower rdf:resource="https://dev-lexic.swissgeol.ch/TectonicUnits/MaettentalMelange"/>
	<skos:narrower rdf:resource="https://dev-lexic.swissgeol.ch/TectonicUnits/SchabellMelange"/>
	<skos:narrower rdf:resource="https://dev-lexic.swissgeol.ch/TectonicUnits/TschingelhoernerSlices"/>
	<skos:narrower rdf:resource="https://dev-lexic.swissgeol.ch/TectonicUnits/BlattengratNappe"/>
	<skos:narrower rdf:resource="https://dev-lexic.swissgeol.ch/TectonicUnits/SardonaNappe"/>
	<skos:narrower rdf:resource="https://dev-lexic.swissgeol.ch/TectonicUnits/BadRagazNappe"/>
	<skos:narrower rdf:resource="https://dev-lexic.swissgeol.ch/TectonicUnits/CalandaSlice"/>
	<skos:narrower rdf:resource="https://dev-lexic.swissgeol.ch/TectonicUnits/MarchegghornSlice"/>
	<skos:narrower rdf:resource="https://dev-lexic.swissgeol.ch/TectonicUnits/MiruttaSlice"/>
	<skos:narrower rdf:resource="https://dev-lexic.swissgeol.ch/TectonicUnits/OrglenSlices"/>
	<status xmlns="http://www.w3.org/ns/adms#" rdf:resource="https://dev-lexic.swissgeol.ch/active"/>
</rdf:Description>

<rdf:Description rdf:about="https://dev-lexic.swissgeol.ch/TectonicUnits/UpperHelvetic">
	<rdf:type rdf:resource="http://www.w3.org/2004/02/skos/core#Concept"/>
	<rdfs:isDefinedBy xml:lang="en">Gouffon Yves (Editor) (2024): Tectonic Map of Switzerland 1:500000, Explanatory notes. Federal Office of Topography swisstopo, Wabern</rdfs:isDefinedBy>
	<skos:definition xml:lang="en">The Upper Helvetic is a tectonic subdomain which encompasses the Helvetic Nappes s.s. (ontop of the main Helvetic Thrust, i.e. from west to east, with increasing displacement: Diablerets, Wildhorn, Axen and Glarus thrusts), as well as the overlying units of South Helvetic to Ultrahelvetic paleogeographic origin.</skos:definition>
	<skos:inScheme rdf:resource="https://dev-lexic.swissgeol.ch/TectonicUnits"/>
	<skos:prefLabel xml:lang="en">Upper Helvetic</skos:prefLabel>
	<skos:prefLabel xml:lang="de">Oberhelvetikum</skos:prefLabel>
	<skos:prefLabel xml:lang="fr">Helvétique supérieur</skos:prefLabel>
	<skos:prefLabel xml:lang="it">Elvetico superiore</skos:prefLabel>
	<skos:broader rdf:resource="https://dev-lexic.swissgeol.ch/TectonicUnits/Helvetic"/>
	<skos:narrower rdf:resource="https://dev-lexic.swissgeol.ch/TectonicUnits/MontChetifNappe"/>
	<skos:narrower rdf:resource="https://dev-lexic.swissgeol.ch/TectonicUnits/RoseletteNappe"/>
	<skos:narrower rdf:resource="https://dev-lexic.swissgeol.ch/TectonicUnits/WildhornNappeComplex"/>
	<skos:narrower rdf:resource="https://dev-lexic.swissgeol.ch/TectonicUnits/GlarusNappeComplex"/>
	<skos:narrower rdf:resource="https://dev-lexic.swissgeol.ch/TectonicUnits/AxenNappe"/>
	<skos:narrower rdf:resource="https://dev-lexic.swissgeol.ch/TectonicUnits/DrusbergNappe"/>
	<skos:narrower rdf:resource="https://dev-lexic.swissgeol.ch/TectonicUnits/SaentisNappe"/>
	<skos:narrower rdf:resource="https://dev-lexic.swissgeol.ch/TectonicUnits/HohenemsNappe"/>
	<skos:narrower rdf:resource="https://dev-lexic.swissgeol.ch/TectonicUnits/TavetschNappe"/>
	<skos:narrower rdf:resource="https://dev-lexic.swissgeol.ch/TectonicUnits/IlanzNappe"/>
	<skos:narrower rdf:resource="https://dev-lexic.swissgeol.ch/TectonicUnits/GotthardNappe"/>
	<skos:narrower rdf:resource="https://dev-lexic.swissgeol.ch/TectonicUnits/CamosciNappe"/>
	<skos:narrower rdf:resource="https://dev-lexic.swissgeol.ch/TectonicUnits/ScopiNappe"/>
	<skos:narrower rdf:resource="https://dev-lexic.swissgeol.ch/TectonicUnits/Piora-PeidenSliceComplex"/>
	<skos:narrower rdf:resource="https://dev-lexic.swissgeol.ch/TectonicUnits/HabkernMelangeZone"/>
	<skos:narrower rdf:resource="https://dev-lexic.swissgeol.ch/TectonicUnits/IbergMelange"/>
	<skos:narrower rdf:resource="https://dev-lexic.swissgeol.ch/TectonicUnits/InternalEinsiedelnSlices"/>
	<skos:narrower rdf:resource="https://dev-lexic.swissgeol.ch/TectonicUnits/WildhausMelange"/>
	<skos:narrower rdf:resource="https://dev-lexic.swissgeol.ch/TectonicUnits/LiebensteinNappe"/>
	<skos:narrower rdf:resource="https://dev-lexic.swissgeol.ch/TectonicUnits/FlaescherbergNappe"/>
	<skos:narrower rdf:resource="https://dev-lexic.swissgeol.ch/TectonicUnits/PillonMelangeZone"/>
	<skos:narrower rdf:resource="https://dev-lexic.swissgeol.ch/TectonicUnits/BulleMelangeZone"/>
	<status xmlns="http://www.w3.org/ns/adms#" rdf:resource="https://dev-lexic.swissgeol.ch/active"/>
</rdf:Description>

<rdf:Description rdf:about="https://dev-lexic.swissgeol.ch/TectonicUnits/SubalpineFlyschZone">
	<rdf:type rdf:resource="http://www.w3.org/2004/02/skos/core#Concept"/>
	<rdfs:isDefinedBy xml:lang="en">Gouffon Yves (Editor) (2024): Tectonic Map of Switzerland 1:500000, Explanatory notes. Federal Office of Topography swisstopo, Wabern</rdfs:isDefinedBy>
	<skos:definition xml:lang="en">The Subalpine Flysch Zone is a heterogeneous Lower Helvetic mélange zone, consisting of «wildflysch» and various elements of all sizes of North Helvetic, South Helvetic and Subbriançonnais origin. It extends along the front of the Alps in a narrow, almost continuous band from the Thunersee to the Toggenburg. It lies between the Subalpine Molasse and the Upper Helvetic Drusberg and Säntis nappes.</skos:definition>
	<skos:inScheme rdf:resource="https://dev-lexic.swissgeol.ch/TectonicUnits"/>
	<skos:prefLabel xml:lang="en">Subalpine Flysch Zone</skos:prefLabel>
	<skos:prefLabel xml:lang="de">Subalpine Flysch-Zone</skos:prefLabel>
	<skos:prefLabel xml:lang="fr">Zone du Flysch subalpin</skos:prefLabel>
	<skos:prefLabel xml:lang="it">Zona del Flysch subalpino</skos:prefLabel>
	<skos:broader rdf:resource="https://dev-lexic.swissgeol.ch/TectonicUnits/LowerHelvetic"/>
	<skos:narrower rdf:resource="https://dev-lexic.swissgeol.ch/TectonicUnits/ExternalEinsiedelnSlices"/>
	<status xmlns="http://www.w3.org/ns/adms#" rdf:resource="https://dev-lexic.swissgeol.ch/active"/>
</rdf:Description>

<rdf:Description rdf:about="https://dev-lexic.swissgeol.ch/TectonicUnits/BelledonneMassif">
	<rdf:type rdf:resource="http://www.w3.org/2004/02/skos/core#Concept"/>
	<rdfs:isDefinedBy xml:lang="en">Gouffon Yves (Editor) (2024): Tectonic Map of Switzerland 1:500000, Explanatory notes. Federal Office of Topography swisstopo, Wabern</rdfs:isDefinedBy>
	<skos:definition xml:lang="en">The Belledonne Massif is a Lower Helvetic External Massif of the French Alps. It is constituted of a pre-Variscan polycyclic basement (Precambrian to Early Cretaceous) intruded by Variscan granites and of a Mesozoic sedimentary cover. The Belledonne Massif is separated from the Aiguilles Rouges and Mont Blanc massifs by the axial depression of the Val Montjoie.</skos:definition>
	<skos:inScheme rdf:resource="https://dev-lexic.swissgeol.ch/TectonicUnits"/>
	<skos:prefLabel xml:lang="en">Belledonne Massif</skos:prefLabel>
	<skos:prefLabel xml:lang="de">Belledonne-Massiv</skos:prefLabel>
	<skos:prefLabel xml:lang="fr">Massif de Belledonne</skos:prefLabel>
	<skos:prefLabel xml:lang="it">Massiccio di Belledonne</skos:prefLabel>
	<skos:broader rdf:resource="https://dev-lexic.swissgeol.ch/TectonicUnits/LowerHelvetic"/>
	<skos:narrower rdf:resource="https://dev-lexic.swissgeol.ch/TectonicUnits/ExternalBelledonneMassif"/>
	<skos:narrower rdf:resource="https://dev-lexic.swissgeol.ch/TectonicUnits/MiddleBelledonneMassif"/>
	<skos:narrower rdf:resource="https://dev-lexic.swissgeol.ch/TectonicUnits/InternalBelledonneMassif"/>
	<status xmlns="http://www.w3.org/ns/adms#" rdf:resource="https://dev-lexic.swissgeol.ch/active"/>
</rdf:Description>

<rdf:Description rdf:about="https://dev-lexic.swissgeol.ch/TectonicUnits/AiguillesRougesMassif">
	<rdf:type rdf:resource="http://www.w3.org/2004/02/skos/core#Concept"/>
	<rdfs:isDefinedBy xml:lang="en">Gouffon Yves (Editor) (2024): Tectonic Map of Switzerland 1:500000, Explanatory notes. Federal Office of Topography swisstopo, Wabern</rdfs:isDefinedBy>
	<skos:definition xml:lang="en">The Aiguilles Rouges Massif is a Lower Helvetic External Massif of the French and Western Swiss Alps. It is constituted of a pre-Variscan polycyclic basement (Precambrian to Early Cretaceous) intruded by Variscan granites, of Permo-Carboniferous metasediments and of a Mesozoic–Cenozoic sedimentary cover. The Aiguilles Rouges Massif is separated from the Belledonne Massif by the axial depression of the Val Montjoie and from the Mont Blanc Massif by a thin band of Mesozoic sediments often («Chamonix Syncline»).</skos:definition>
	<skos:inScheme rdf:resource="https://dev-lexic.swissgeol.ch/TectonicUnits"/>
	<skos:prefLabel xml:lang="en">Aiguilles Rouges Massif</skos:prefLabel>
	<skos:prefLabel xml:lang="de">Aiguilles-Rouges-Massiv</skos:prefLabel>
	<skos:prefLabel xml:lang="fr">Massif des Aiguilles Rouges</skos:prefLabel>
	<skos:prefLabel xml:lang="it">Massiccio delle Aiguilles Rouges</skos:prefLabel>
	<skos:broader rdf:resource="https://dev-lexic.swissgeol.ch/TectonicUnits/LowerHelvetic"/>
	<status xmlns="http://www.w3.org/ns/adms#" rdf:resource="https://dev-lexic.swissgeol.ch/active"/>
</rdf:Description>

<rdf:Description rdf:about="https://dev-lexic.swissgeol.ch/TectonicUnits/MontBlancMassif">
	<rdf:type rdf:resource="http://www.w3.org/2004/02/skos/core#Concept"/>
	<rdfs:isDefinedBy xml:lang="en">Gouffon Yves (Editor) (2024): Tectonic Map of Switzerland 1:500000, Explanatory notes. Federal Office of Topography swisstopo, Wabern</rdfs:isDefinedBy>
	<skos:definition xml:lang="en">The Mont Blanc Massif, divided into an external and an internal part by a major fault, is a Lower Helvetic External Massif of the French and Western Swiss Alps. It is constituted of a pre-Variscan polycyclic basement (Precambrian to Early Cretaceous) intruded by Variscan granites and of a Mesozoic–Cenozoic sedimentary cover. The Mont Blanc Massif is separated from the Belledonne Massif by the axial depression of the Val Montjoie and from the Aiguilles Rouges Massif by a thin band of Mesozoic sediments often («Chamonix Syncline»).</skos:definition>
	<skos:inScheme rdf:resource="https://dev-lexic.swissgeol.ch/TectonicUnits"/>
	<skos:prefLabel xml:lang="en">Mont Blanc Massif</skos:prefLabel>
	<skos:prefLabel xml:lang="de">Mont-Blanc-Massiv</skos:prefLabel>
	<skos:prefLabel xml:lang="fr">Massif du Mont Blanc</skos:prefLabel>
	<skos:prefLabel xml:lang="it">Massiccio del Monte Bianco</skos:prefLabel>
	<skos:broader rdf:resource="https://dev-lexic.swissgeol.ch/TectonicUnits/LowerHelvetic"/>
	<skos:narrower rdf:resource="https://dev-lexic.swissgeol.ch/TectonicUnits/ExternalMontBlancMassif"/>
	<skos:narrower rdf:resource="https://dev-lexic.swissgeol.ch/TectonicUnits/InternalMontBlancMassif"/>
	<status xmlns="http://www.w3.org/ns/adms#" rdf:resource="https://dev-lexic.swissgeol.ch/active"/>
</rdf:Description>

<rdf:Description rdf:about="https://dev-lexic.swissgeol.ch/TectonicUnits/AarMassif">
	<rdf:type rdf:resource="http://www.w3.org/2004/02/skos/core#Concept"/>
	<rdfs:isDefinedBy xml:lang="en">Gouffon Yves (Editor) (2024): Tectonic Map of Switzerland 1:500000, Explanatory notes. Federal Office of Topography swisstopo, Wabern</rdfs:isDefinedBy>
	<skos:definition xml:lang="en">The Aar Massif is a Lower Helvetic External Massif of the central part of the Swiss Alps. It is constituted of a pre-Variscan to Variscan polycyclic metamorphic basement with Variscan intrusions, of Permo-Carboniferous grabens filled with volcano-sedimentary rocks and of an autochthonous to parautochthonous Mesozoic–Cenozoic sedimentary cover. It is subdivided by several faults into a large External Aar Massif and a thinner Internal Aar Massif to the south-east.</skos:definition>
	<skos:inScheme rdf:resource="https://dev-lexic.swissgeol.ch/TectonicUnits"/>
	<skos:prefLabel xml:lang="en">Aar Massif</skos:prefLabel>
	<skos:prefLabel xml:lang="de">Aar-Massiv</skos:prefLabel>
	<skos:prefLabel xml:lang="fr">Massif de l'Aar</skos:prefLabel>
	<skos:prefLabel xml:lang="it">Massiccio dell'Aare</skos:prefLabel>
	<skos:broader rdf:resource="https://dev-lexic.swissgeol.ch/TectonicUnits/LowerHelvetic"/>
	<skos:narrower rdf:resource="https://dev-lexic.swissgeol.ch/TectonicUnits/ExternalAarMassif"/>
	<skos:narrower rdf:resource="https://dev-lexic.swissgeol.ch/TectonicUnits/GasternSubmassif"/>
	<skos:narrower rdf:resource="https://dev-lexic.swissgeol.ch/TectonicUnits/KaminspitzSlice"/>
	<skos:narrower rdf:resource="https://dev-lexic.swissgeol.ch/TectonicUnits/StelliSlice"/>
	<skos:narrower rdf:resource="https://dev-lexic.swissgeol.ch/TectonicUnits/TschepSlice"/>
	<skos:narrower rdf:resource="https://dev-lexic.swissgeol.ch/TectonicUnits/HochFulenSlice"/>
	<skos:narrower rdf:resource="https://dev-lexic.swissgeol.ch/TectonicUnits/OrglenSlices_PartAarMassif"/>
	<skos:narrower rdf:resource="https://dev-lexic.swissgeol.ch/TectonicUnits/CalandaSlice_PartAarMassif"/>
	<skos:narrower rdf:resource="https://dev-lexic.swissgeol.ch/TectonicUnits/MiruttaSlice_PartAarMassif"/>
	<skos:narrower rdf:resource="https://dev-lexic.swissgeol.ch/TectonicUnits/PizDartgasSlice"/>
	<status xmlns="http://www.w3.org/ns/adms#" rdf:resource="https://dev-lexic.swissgeol.ch/active"/>
</rdf:Description>

<rdf:Description rdf:about="https://dev-lexic.swissgeol.ch/TectonicUnits/ChainesSubalpinesNappe">
	<rdf:type rdf:resource="http://www.w3.org/2004/02/skos/core#Concept"/>
	<rdfs:isDefinedBy xml:lang="en">Gouffon Yves (Editor) (2024): Tectonic Map of Switzerland 1:500000, Explanatory notes. Federal Office of Topography swisstopo, Wabern</rdfs:isDefinedBy>
	<skos:definition xml:lang="en">The Chaines Subalpines Nappe is a Lower Helvetic tectonic nappe of the French Alps constituted by a succession of large folds with NW vergence to the north of the latitude of Annecy and with W vergence to the south. Its eastern contact is a thrust fault plunging NW over the Aiguilles Rouges and Belledonne massifs. It is overlain to the north by the Pillon Mélange Zone just below the Penninic Prealps, and overlies the southern end of the Subalpine Molasse to the west. The Chaines Subalpines Nappe is subdivided into several units by thrust faults. All these units are composed of Jurassic–Cenozoic sediments of North Helvetic origin, except the most external one, located south of Annecy, whose series is similar to that of the Internal Folded Jura.</skos:definition>
	<skos:inScheme rdf:resource="https://dev-lexic.swissgeol.ch/TectonicUnits"/>
	<skos:prefLabel xml:lang="en">Chaines Subalpines Nappe</skos:prefLabel>
	<skos:prefLabel xml:lang="de">Chaines-Subalpines-Decke</skos:prefLabel>
	<skos:prefLabel xml:lang="fr">Nappe des Chaines Subalpines</skos:prefLabel>
	<skos:prefLabel xml:lang="it">Falda delle Chaines Subalpines</skos:prefLabel>
	<skos:broader rdf:resource="https://dev-lexic.swissgeol.ch/TectonicUnits/LowerHelvetic"/>
	<status xmlns="http://www.w3.org/ns/adms#" rdf:resource="https://dev-lexic.swissgeol.ch/active"/>
</rdf:Description>

<rdf:Description rdf:about="https://dev-lexic.swissgeol.ch/TectonicUnits/MorclesNappe">
	<rdf:type rdf:resource="http://www.w3.org/2004/02/skos/core#Concept"/>
	<rdfs:isDefinedBy xml:lang="en">Gouffon Yves (Editor) (2024): Tectonic Map of Switzerland 1:500000, Explanatory notes. Federal Office of Topography swisstopo, Wabern</rdfs:isDefinedBy>
	<skos:definition xml:lang="en">The Morcles Nappe is a Lower Helvetic tectonic nappe of the French and Western Swiss Alps. It is constituted by a Jurassic–Cenozoic sedimentary series forming a large recumbent fold overlying the northeastern end of the Aiguilles Rouges Massif. This large fold, defined north of the bend that the Rhône forms at Martigny, extends south of the Rhône, in the Dents du Midi area.</skos:definition>
	<skos:inScheme rdf:resource="https://dev-lexic.swissgeol.ch/TectonicUnits"/>
	<skos:prefLabel xml:lang="en">Morcles Nappe</skos:prefLabel>
	<skos:prefLabel xml:lang="de">Morcles-Decke</skos:prefLabel>
	<skos:prefLabel xml:lang="fr">Nappe de Morcles</skos:prefLabel>
	<skos:prefLabel xml:lang="it">Falda di Morcles</skos:prefLabel>
	<skos:broader rdf:resource="https://dev-lexic.swissgeol.ch/TectonicUnits/LowerHelvetic"/>
	<skos:related rdf:resource="https://dev-lexic.swissgeol.ch/TectonicUnits/DoldenhornNappe"/>
	<skos:related rdf:resource="https://dev-lexic.swissgeol.ch/TectonicUnits/ExternalMontBlancMassif"/>
	<status xmlns="http://www.w3.org/ns/adms#" rdf:resource="https://dev-lexic.swissgeol.ch/active"/>
</rdf:Description>

<rdf:Description rdf:about="https://dev-lexic.swissgeol.ch/TectonicUnits/ArdonNappe">
	<rdf:type rdf:resource="http://www.w3.org/2004/02/skos/core#Concept"/>
	<rdfs:isDefinedBy xml:lang="en">Gouffon Yves (Editor) (2024): Tectonic Map of Switzerland 1:500000, Explanatory notes. Federal Office of Topography swisstopo, Wabern</rdfs:isDefinedBy>
	<skos:definition xml:lang="en">The Ardon Nappe is a Lower Helvetic tectonic nappe of the Western Swiss Alps, situated on the north side of the Rhône between Ardon and the Mont Gond, below the Diablerets Thrust. It is rooted on the internal Mont Blanc Massif. This very thin unit is mainly constituted of Early Cretaceous sediments.</skos:definition>
	<skos:inScheme rdf:resource="https://dev-lexic.swissgeol.ch/TectonicUnits"/>
	<skos:prefLabel xml:lang="en">Ardon Nappe</skos:prefLabel>
	<skos:prefLabel xml:lang="de">Ardon-Decke</skos:prefLabel>
	<skos:prefLabel xml:lang="fr">Nappe d'Ardon</skos:prefLabel>
	<skos:prefLabel xml:lang="it">Falda di Ardon</skos:prefLabel>
	<skos:broader rdf:resource="https://dev-lexic.swissgeol.ch/TectonicUnits/LowerHelvetic"/>
	<skos:related rdf:resource="https://dev-lexic.swissgeol.ch/TectonicUnits/InternalMontBlancMassif"/>
	<status xmlns="http://www.w3.org/ns/adms#" rdf:resource="https://dev-lexic.swissgeol.ch/active"/>
</rdf:Description>

<rdf:Description rdf:about="https://dev-lexic.swissgeol.ch/TectonicUnits/DoldenhornNappe">
	<rdf:type rdf:resource="http://www.w3.org/2004/02/skos/core#Concept"/>
	<rdfs:isDefinedBy xml:lang="en">Gouffon Yves (Editor) (2024): Tectonic Map of Switzerland 1:500000, Explanatory notes. Federal Office of Topography swisstopo, Wabern</rdfs:isDefinedBy>
	<skos:definition xml:lang="en">The Doldenhorn Nappe is a Lower Helvetic tectonic nappe situated at the southwestern end of the Aar Massif, where the upper part of the External Aar Massif sedimentary cover is detached and forms a large-scale recumbent fold. Its inverted limb is intensely sheared and characterized by carbonate mylonites («Jungfrau Syncline»). This nappe is stratigraphically and structurally comparable to the Morcles Nappe.</skos:definition>
	<skos:inScheme rdf:resource="https://dev-lexic.swissgeol.ch/TectonicUnits"/>
	<skos:prefLabel xml:lang="en">Doldenhorn Nappe</skos:prefLabel>
	<skos:prefLabel xml:lang="de">Doldenhorn-Decke</skos:prefLabel>
	<skos:prefLabel xml:lang="fr">Nappe du Doldenhorn</skos:prefLabel>
	<skos:prefLabel xml:lang="it">Falda del Doldenhorn</skos:prefLabel>
	<skos:broader rdf:resource="https://dev-lexic.swissgeol.ch/TectonicUnits/LowerHelvetic"/>
	<skos:related rdf:resource="https://dev-lexic.swissgeol.ch/TectonicUnits/MorclesNappe"/>
	<status xmlns="http://www.w3.org/ns/adms#" rdf:resource="https://dev-lexic.swissgeol.ch/active"/>
</rdf:Description>

<rdf:Description rdf:about="https://dev-lexic.swissgeol.ch/TectonicUnits/GellihornNappe">
	<rdf:type rdf:resource="http://www.w3.org/2004/02/skos/core#Concept"/>
	<rdfs:isDefinedBy xml:lang="en">Gouffon Yves (Editor) (2024): Tectonic Map of Switzerland 1:500000, Explanatory notes. Federal Office of Topography swisstopo, Wabern</rdfs:isDefinedBy>
	<skos:definition xml:lang="en">The Gellihorn Nappe is a Lower Helvetic tectonic nappe of the Western Swiss Alps, constituted by a thin series of Late Jurassic to Paleogene limestones. It occupies the same structural position as the Plammis-Jägerchrüz couple, but does not show the same grade of metamorphism.</skos:definition>
	<skos:inScheme rdf:resource="https://dev-lexic.swissgeol.ch/TectonicUnits"/>
	<skos:prefLabel xml:lang="en">Gellihorn Nappe</skos:prefLabel>
	<skos:prefLabel xml:lang="de">Gellihorn-Decke</skos:prefLabel>
	<skos:prefLabel xml:lang="fr">Nappe du Gellihorn</skos:prefLabel>
	<skos:prefLabel xml:lang="it">Falda del Gelihorn</skos:prefLabel>
	<skos:broader rdf:resource="https://dev-lexic.swissgeol.ch/TectonicUnits/LowerHelvetic"/>
	<status xmlns="http://www.w3.org/ns/adms#" rdf:resource="https://dev-lexic.swissgeol.ch/active"/>
</rdf:Description>

<rdf:Description rdf:about="https://dev-lexic.swissgeol.ch/TectonicUnits/PlammisNappe">
	<rdf:type rdf:resource="http://www.w3.org/2004/02/skos/core#Concept"/>
	<rdfs:isDefinedBy xml:lang="en">Gouffon Yves (Editor) (2024): Tectonic Map of Switzerland 1:500000, Explanatory notes. Federal Office of Topography swisstopo, Wabern</rdfs:isDefinedBy>
	<skos:definition xml:lang="en">The Plammis Nappe is a Lower Helvetic tectonic nappe of the Western Swiss Alps, constituted by a Jurassic sedimentary series interpreted as the detached part of the autochthonous cover of the Internal Aar Massif (Baldschieder-Gletsch Submassif). On the slopes between Sierre and Gampel, the Plammis Nappe overlies the autochthonous cover of the External Aar Massif and the Doldenhorn Nappe. It is itself overlain by the Jägerchrüz Nappe.</skos:definition>
	<skos:inScheme rdf:resource="https://dev-lexic.swissgeol.ch/TectonicUnits"/>
	<skos:prefLabel xml:lang="en">Plammis Nappe</skos:prefLabel>
	<skos:prefLabel xml:lang="de">Plammis-Decke</skos:prefLabel>
	<skos:prefLabel xml:lang="fr">Nappe de Plammis</skos:prefLabel>
	<skos:prefLabel xml:lang="it">Falda di Plammis</skos:prefLabel>
	<skos:broader rdf:resource="https://dev-lexic.swissgeol.ch/TectonicUnits/LowerHelvetic"/>
	<status xmlns="http://www.w3.org/ns/adms#" rdf:resource="https://dev-lexic.swissgeol.ch/active"/>
</rdf:Description>

<rdf:Description rdf:about="https://dev-lexic.swissgeol.ch/TectonicUnits/JaegerchruezNappe">
	<rdf:type rdf:resource="http://www.w3.org/2004/02/skos/core#Concept"/>
	<rdfs:isDefinedBy xml:lang="en">Gouffon Yves (Editor) (2024): Tectonic Map of Switzerland 1:500000, Explanatory notes. Federal Office of Topography swisstopo, Wabern</rdfs:isDefinedBy>
	<skos:definition xml:lang="en">The Jägerchrüz Nappe is a Lower Helvetic tectonic nappe of the Western Swiss Alps, constituted by a Triassic–Paleogene sedimentary series overlying the Plammis Nappe and overlain by the Upper Helvetic Wildhorn Nappe Complex.</skos:definition>
	<skos:inScheme rdf:resource="https://dev-lexic.swissgeol.ch/TectonicUnits"/>
	<skos:prefLabel xml:lang="en">Jägerchrüz Nappe</skos:prefLabel>
	<skos:prefLabel xml:lang="de">Jägerchrüz-Decke</skos:prefLabel>
	<skos:prefLabel xml:lang="fr">Nappe du Jägerchrüz</skos:prefLabel>
	<skos:prefLabel xml:lang="it">Falda del Jägerchrüz</skos:prefLabel>
	<skos:broader rdf:resource="https://dev-lexic.swissgeol.ch/TectonicUnits/LowerHelvetic"/>
	<status xmlns="http://www.w3.org/ns/adms#" rdf:resource="https://dev-lexic.swissgeol.ch/active"/>
</rdf:Description>

<rdf:Description rdf:about="https://dev-lexic.swissgeol.ch/TectonicUnits/KammlistockNappe">
	<rdf:type rdf:resource="http://www.w3.org/2004/02/skos/core#Concept"/>
	<rdfs:isDefinedBy xml:lang="en">Gouffon Yves (Editor) (2024): Tectonic Map of Switzerland 1:500000, Explanatory notes. Federal Office of Topography swisstopo, Wabern</rdfs:isDefinedBy>
	<skos:definition xml:lang="en">The Kammlistock Nappe is one of several small Lower Helvetic tectonic units of the Klausenpass region, wedged between the sedimentary series of the Aar massif and the Axen Thrust. It is constituted by Late Jurassic to Paleogene sediments that were deposited further south than the autochthonous-parautochthonous sediments of the Aar Massif, but still in the North Helvetic realm.</skos:definition>
	<skos:inScheme rdf:resource="https://dev-lexic.swissgeol.ch/TectonicUnits"/>
	<skos:prefLabel xml:lang="en">Kammlistock Nappe</skos:prefLabel>
	<skos:prefLabel xml:lang="de">Kammlistock-Decke</skos:prefLabel>
	<skos:prefLabel xml:lang="fr">Nappe du Kammlistock</skos:prefLabel>
	<skos:prefLabel xml:lang="it">Falda del Kammlistock</skos:prefLabel>
	<skos:broader rdf:resource="https://dev-lexic.swissgeol.ch/TectonicUnits/LowerHelvetic"/>
	<status xmlns="http://www.w3.org/ns/adms#" rdf:resource="https://dev-lexic.swissgeol.ch/active"/>
</rdf:Description>

<rdf:Description rdf:about="https://dev-lexic.swissgeol.ch/TectonicUnits/GriessstockNappe">
	<rdf:type rdf:resource="http://www.w3.org/2004/02/skos/core#Concept"/>
	<rdfs:isDefinedBy xml:lang="en">Gouffon Yves (Editor) (2024): Tectonic Map of Switzerland 1:500000, Explanatory notes. Federal Office of Topography swisstopo, Wabern</rdfs:isDefinedBy>
	<skos:definition xml:lang="en">The Griessstock Nappe is one of several small Lower Helvetic tectonic units of the Klausenpass region, wedged between the sedimentary series of the Aar massif and the Axen Thrust. It is constituted by Late Jurassic to Paleogene sediments (Quinten to Taveyannaz formations) that were deposited further south than the autochthonous-parautochthonous sediments of the Aar Massif, but still in the North Helvetic realm.</skos:definition>
	<skos:inScheme rdf:resource="https://dev-lexic.swissgeol.ch/TectonicUnits"/>
	<skos:prefLabel xml:lang="en">Griessstock Nappe</skos:prefLabel>
	<skos:prefLabel xml:lang="de">Griessstock-Decke</skos:prefLabel>
	<skos:prefLabel xml:lang="fr">Nappe du Griessstock</skos:prefLabel>
	<skos:prefLabel xml:lang="it">Falda del Griessstock</skos:prefLabel>
	<skos:broader rdf:resource="https://dev-lexic.swissgeol.ch/TectonicUnits/LowerHelvetic"/>
	<status xmlns="http://www.w3.org/ns/adms#" rdf:resource="https://dev-lexic.swissgeol.ch/active"/>
</rdf:Description>

<rdf:Description rdf:about="https://dev-lexic.swissgeol.ch/TectonicUnits/ClaridenSliceComplex">
	<rdf:type rdf:resource="http://www.w3.org/2004/02/skos/core#Concept"/>
	<rdfs:isDefinedBy xml:lang="en">Gouffon Yves (Editor) (2024): Tectonic Map of Switzerland 1:500000, Explanatory notes. Federal Office of Topography swisstopo, Wabern</rdfs:isDefinedBy>
	<skos:definition xml:lang="en">The Clariden Slice Complex is one of several small Lower Helvetic tectonic units of the Klausenpass region, wedged between the sedimentary series of the Aar massif and the Axen Thrust. It is constituted by Late Jurassic to Paleogene sediments that were deposited further south than the autochthonous-parautochthonous sediments of the Aar Massif, but still in the North Helvetic realm.</skos:definition>
	<skos:inScheme rdf:resource="https://dev-lexic.swissgeol.ch/TectonicUnits"/>
	<skos:prefLabel xml:lang="en">Clariden Slice Complex</skos:prefLabel>
	<skos:prefLabel xml:lang="de">Clariden-Schuppenkomplex</skos:prefLabel>
	<skos:prefLabel xml:lang="fr">Complexe d'écailles du Clariden</skos:prefLabel>
	<skos:prefLabel xml:lang="it">Complesso di scaglie del Clariden</skos:prefLabel>
	<skos:broader rdf:resource="https://dev-lexic.swissgeol.ch/TectonicUnits/LowerHelvetic"/>
	<skos:narrower rdf:resource="https://dev-lexic.swissgeol.ch/TectonicUnits/KlausenpassSlices"/>
	<skos:narrower rdf:resource="https://dev-lexic.swissgeol.ch/TectonicUnits/ChamerstockSlice"/>
	<skos:narrower rdf:resource="https://dev-lexic.swissgeol.ch/TectonicUnits/GeisstrittSlice"/>
	<skos:narrower rdf:resource="https://dev-lexic.swissgeol.ch/TectonicUnits/StichplattenSlice"/>
	<skos:narrower rdf:resource="https://dev-lexic.swissgeol.ch/TectonicUnits/GemsfairenSlice"/>
	<skos:narrower rdf:resource="https://dev-lexic.swissgeol.ch/TectonicUnits/RotstockSlice"/>
	<skos:narrower rdf:resource="https://dev-lexic.swissgeol.ch/TectonicUnits/LangfirnSlice"/>
	<status xmlns="http://www.w3.org/ns/adms#" rdf:resource="https://dev-lexic.swissgeol.ch/active"/>
</rdf:Description>

<rdf:Description rdf:about="https://dev-lexic.swissgeol.ch/TectonicUnits/Fiseten-OrthaldenSlices">
	<rdf:type rdf:resource="http://www.w3.org/2004/02/skos/core#Concept"/>
	<rdfs:isDefinedBy xml:lang="en">Gouffon Yves (Editor) (2024): Tectonic Map of Switzerland 1:500000, Explanatory notes. Federal Office of Topography swisstopo, Wabern</rdfs:isDefinedBy>
	<skos:definition xml:lang="en">The Fiseten-Orthalden Slices are small Lower Helvetic tectonic units of the Klausenpass region, wedged between the sedimentary series of the Aar massif and the Axen Thrust. They are constituted by Late Jurassic to Paleogene sediments that were deposited further south than the autochthonous-parautochthonous sediments of the Aar Massif, but still in the North Helvetic realm.</skos:definition>
	<skos:inScheme rdf:resource="https://dev-lexic.swissgeol.ch/TectonicUnits"/>
	<skos:prefLabel xml:lang="en">Fiseten-Orthalden Slices</skos:prefLabel>
	<skos:prefLabel xml:lang="de">Fiseten-Orthalden-Schuppen</skos:prefLabel>
	<skos:prefLabel xml:lang="fr">Écailles de Fiseten-Orthalden</skos:prefLabel>
	<skos:prefLabel xml:lang="it">Scaglie di Fiseten-Orthalden</skos:prefLabel>
	<skos:broader rdf:resource="https://dev-lexic.swissgeol.ch/TectonicUnits/LowerHelvetic"/>
	<status xmlns="http://www.w3.org/ns/adms#" rdf:resource="https://dev-lexic.swissgeol.ch/active"/>
</rdf:Description>

<rdf:Description rdf:about="https://dev-lexic.swissgeol.ch/TectonicUnits/CavistrauNappe">
	<rdf:type rdf:resource="http://www.w3.org/2004/02/skos/core#Concept"/>
	<rdfs:isDefinedBy xml:lang="en">Gouffon Yves (Editor) (2024): Tectonic Map of Switzerland 1:500000, Explanatory notes. Federal Office of Topography swisstopo, Wabern</rdfs:isDefinedBy>
	<skos:definition xml:lang="en">The Cavistrau Nappe is a Lower Helvetic tectonic nappe on the northern flank of the Surselva. It represents an overturned sequence of Permian to Late Jurassic sediments, which was emplaced onto the Trun-Punteglias Submassif as a W-facing recumbent fold and replaced the autochthonous Jurassic–Paleogene strata that were detached and transported farther nothwestwards.</skos:definition>
	<skos:inScheme rdf:resource="https://dev-lexic.swissgeol.ch/TectonicUnits"/>
	<skos:prefLabel xml:lang="en">Cavistrau Nappe</skos:prefLabel>
	<skos:prefLabel xml:lang="de">Cavistrau-Decke</skos:prefLabel>
	<skos:prefLabel xml:lang="fr">Nappe du Cavistrau</skos:prefLabel>
	<skos:prefLabel xml:lang="it">Falda del Cavistrau</skos:prefLabel>
	<skos:broader rdf:resource="https://dev-lexic.swissgeol.ch/TectonicUnits/LowerHelvetic"/>
	<status xmlns="http://www.w3.org/ns/adms#" rdf:resource="https://dev-lexic.swissgeol.ch/active"/>
</rdf:Description>

<rdf:Description rdf:about="https://dev-lexic.swissgeol.ch/TectonicUnits/Chropfsberg-PizalunSlices">
	<rdf:type rdf:resource="http://www.w3.org/2004/02/skos/core#Concept"/>
	<rdfs:isDefinedBy xml:lang="en">Gouffon Yves (Editor) (2024): Tectonic Map of Switzerland 1:500000, Explanatory notes. Federal Office of Topography swisstopo, Wabern</rdfs:isDefinedBy>
	<skos:definition xml:lang="en">The Chropfsberg-Pizalun Slices are four isolated Lower Helvetic tectonic slices situated south of Sargans on the top of the nappe stack made up of the Blattengrat, Sardona and Bad Ragaz nappes. They include Triassic, Jurassic and Cretaceous strata and occupy the same structural position as the Tschingelhörner Slices, but without direct contact with the Glarus Thrust due to erosion.</skos:definition>
	<skos:inScheme rdf:resource="https://dev-lexic.swissgeol.ch/TectonicUnits"/>
	<skos:prefLabel xml:lang="en">Chropfsberg-Pizalun Slices</skos:prefLabel>
	<skos:prefLabel xml:lang="de">Chropfsberg-Pizalun-Schuppen</skos:prefLabel>
	<skos:prefLabel xml:lang="fr">Écailles de Chropfsberg-Pizalun</skos:prefLabel>
	<skos:prefLabel xml:lang="it">Scaglie di Chropfsberg-Pizalun</skos:prefLabel>
	<skos:broader rdf:resource="https://dev-lexic.swissgeol.ch/TectonicUnits/LowerHelvetic"/>
	<skos:narrower rdf:resource="https://dev-lexic.swissgeol.ch/TectonicUnits/ChropfsbergSlice"/>
	<skos:narrower rdf:resource="https://dev-lexic.swissgeol.ch/TectonicUnits/PizalunSlice"/>
	<skos:narrower rdf:resource="https://dev-lexic.swissgeol.ch/TectonicUnits/GaffiaSlice"/>
	<skos:narrower rdf:resource="https://dev-lexic.swissgeol.ch/TectonicUnits/LogsbachSlice"/>
	<status xmlns="http://www.w3.org/ns/adms#" rdf:resource="https://dev-lexic.swissgeol.ch/active"/>
</rdf:Description>

<rdf:Description rdf:about="https://dev-lexic.swissgeol.ch/TectonicUnits/MaettentalMelange">
	<rdf:type rdf:resource="http://www.w3.org/2004/02/skos/core#Concept"/>
	<rdfs:isDefinedBy xml:lang="en">Gouffon Yves (Editor) (2024): Tectonic Map of Switzerland 1:500000, Explanatory notes. Federal Office of Topography swisstopo, Wabern</rdfs:isDefinedBy>
	<skos:definition xml:lang="en">The Mättental Mélange formed at the footwall of the Upper Helvetic basal thrusts. It lies on top of the Aar Massif sedimentary cover, below the Axen Thrust or the small Lower Helvetic units in the Klausenpass area . This mélange consists of a “wildflysch” with slices of rocks of South Helvetic origin (Cretaceous–Paleogene).</skos:definition>
	<skos:inScheme rdf:resource="https://dev-lexic.swissgeol.ch/TectonicUnits"/>
	<skos:prefLabel xml:lang="en">Mättental Mélange</skos:prefLabel>
	<skos:prefLabel xml:lang="de">Mättental-Melange</skos:prefLabel>
	<skos:prefLabel xml:lang="fr">Mélange du Mättental</skos:prefLabel>
	<skos:prefLabel xml:lang="it">Mélange del Mättental</skos:prefLabel>
	<skos:broader rdf:resource="https://dev-lexic.swissgeol.ch/TectonicUnits/LowerHelvetic"/>
	<skos:related rdf:resource="https://dev-lexic.swissgeol.ch/TectonicUnits/SchabellMelange"/>
	<status xmlns="http://www.w3.org/ns/adms#" rdf:resource="https://dev-lexic.swissgeol.ch/active"/>
</rdf:Description>

<rdf:Description rdf:about="https://dev-lexic.swissgeol.ch/TectonicUnits/SchabellMelange">
	<rdf:type rdf:resource="http://www.w3.org/2004/02/skos/core#Concept"/>
	<rdfs:isDefinedBy xml:lang="en">Gouffon Yves (Editor) (2024): Tectonic Map of Switzerland 1:500000, Explanatory notes. Federal Office of Topography swisstopo, Wabern</rdfs:isDefinedBy>
	<skos:definition xml:lang="en">The Schabell Mélange formed at the footwall of the Upper Helvetic basal thrusts. It lies on top of the parautochthonous flysch of the Aar Massif, Blattengrat and Sardona nappes, below the Glarus Thrust. This mélange consists of a “wildflysch” with many lenses and slices of rock stemming from the immediately underlying units.</skos:definition>
	<skos:inScheme rdf:resource="https://dev-lexic.swissgeol.ch/TectonicUnits"/>
	<skos:prefLabel xml:lang="en">Schabell Mélange</skos:prefLabel>
	<skos:prefLabel xml:lang="de">Schabell-Melange</skos:prefLabel>
	<skos:prefLabel xml:lang="fr">Mélange du Schabell</skos:prefLabel>
	<skos:prefLabel xml:lang="it">Mélange dello Schabell</skos:prefLabel>
	<skos:broader rdf:resource="https://dev-lexic.swissgeol.ch/TectonicUnits/LowerHelvetic"/>
	<skos:related rdf:resource="https://dev-lexic.swissgeol.ch/TectonicUnits/MaettentalMelange"/>
	<status xmlns="http://www.w3.org/ns/adms#" rdf:resource="https://dev-lexic.swissgeol.ch/active"/>
</rdf:Description>

<rdf:Description rdf:about="https://dev-lexic.swissgeol.ch/TectonicUnits/TschingelhoernerSlices">
	<rdf:type rdf:resource="http://www.w3.org/2004/02/skos/core#Concept"/>
	<rdfs:isDefinedBy xml:lang="en">Gouffon Yves (Editor) (2024): Tectonic Map of Switzerland 1:500000, Explanatory notes. Federal Office of Topography swisstopo, Wabern</rdfs:isDefinedBy>
	<skos:definition xml:lang="en">The Tschingelhörner Slices are Lower Helvetic tectonic slices occurring on top of the Schabell Mélange and consisting mainly of Cretaceous limestones. These slices, characteristic of the footwall of the Glarus Thrust, were torn off their substratum during the thrusting of the Glarus Nappe Complex. Further north, under the Glarus Nappe Complex, thin slices of similar but more deformed limestones («Lochsiten-Kalk») occupy the same structural position.</skos:definition>
	<skos:inScheme rdf:resource="https://dev-lexic.swissgeol.ch/TectonicUnits"/>
	<skos:prefLabel xml:lang="en">Tschingelhörner Slices</skos:prefLabel>
	<skos:prefLabel xml:lang="de">Tschingelhörner-Schuppen</skos:prefLabel>
	<skos:prefLabel xml:lang="fr">Écailles des Tschingelhörner</skos:prefLabel>
	<skos:prefLabel xml:lang="it">Scaglie dei Tschingelhörner</skos:prefLabel>
	<skos:broader rdf:resource="https://dev-lexic.swissgeol.ch/TectonicUnits/LowerHelvetic"/>
	<status xmlns="http://www.w3.org/ns/adms#" rdf:resource="https://dev-lexic.swissgeol.ch/active"/>
</rdf:Description>

<rdf:Description rdf:about="https://dev-lexic.swissgeol.ch/TectonicUnits/BlattengratNappe">
	<rdf:type rdf:resource="http://www.w3.org/2004/02/skos/core#Concept"/>
	<rdfs:isDefinedBy xml:lang="en">Gouffon Yves (Editor) (2024): Tectonic Map of Switzerland 1:500000, Explanatory notes. Federal Office of Topography swisstopo, Wabern</rdfs:isDefinedBy>
	<skos:definition xml:lang="en">The Blattengrat Nappe is a Lower Helvetic tectonic nappe emplaced in an early phase onto the future Helvetic domain, subsequently truncated by the Glarus Thrust and simultaneously cut by out-of-sequence thrusts. It is composed mainly of Late Cretaceous to Paleogene sediments of South Helvetic affinity, cropping out in the area between Linthal and Sargans.</skos:definition>
	<skos:inScheme rdf:resource="https://dev-lexic.swissgeol.ch/TectonicUnits"/>
	<skos:prefLabel xml:lang="en">Blattengrat Nappe</skos:prefLabel>
	<skos:prefLabel xml:lang="de">Blattengrat-Decke</skos:prefLabel>
	<skos:prefLabel xml:lang="fr">Nappe du Blattengrat</skos:prefLabel>
	<skos:prefLabel xml:lang="it">Falda del Blattengrat</skos:prefLabel>
	<skos:broader rdf:resource="https://dev-lexic.swissgeol.ch/TectonicUnits/LowerHelvetic"/>
	<skos:narrower rdf:resource="https://dev-lexic.swissgeol.ch/TectonicUnits/MarchegghornSlice_PartBlattengrat"/>
	<skos:narrower rdf:resource="https://dev-lexic.swissgeol.ch/TectonicUnits/CalandaSlice_PartBlattengrat"/>
	<skos:narrower rdf:resource="https://dev-lexic.swissgeol.ch/TectonicUnits/MiruttaSlice_PartBlattengrat"/>
	<status xmlns="http://www.w3.org/ns/adms#" rdf:resource="https://dev-lexic.swissgeol.ch/active"/>
</rdf:Description>

<rdf:Description rdf:about="https://dev-lexic.swissgeol.ch/TectonicUnits/SardonaNappe">
	<rdf:type rdf:resource="http://www.w3.org/2004/02/skos/core#Concept"/>
	<rdfs:isDefinedBy xml:lang="en">Gouffon Yves (Editor) (2024): Tectonic Map of Switzerland 1:500000, Explanatory notes. Federal Office of Topography swisstopo, Wabern</rdfs:isDefinedBy>
	<skos:definition xml:lang="en">The Sardona Nappe is a Lower Helvetic tectonic nappe emplaced in an early phase onto the future Helvetic domain, subsequently truncated by the Glarus Thrust and simultaneously cut by out-of-sequence thrusts. It is composed mainly of Late Cretaceous to Paleogene sediments of Ultrahelvetic affinity, cropping out in the area between Linthal and Sargans.</skos:definition>
	<skos:inScheme rdf:resource="https://dev-lexic.swissgeol.ch/TectonicUnits"/>
	<skos:prefLabel xml:lang="en">Sardona Nappe</skos:prefLabel>
	<skos:prefLabel xml:lang="de">Sardona-Decke</skos:prefLabel>
	<skos:prefLabel xml:lang="fr">Nappe du Sardona</skos:prefLabel>
	<skos:prefLabel xml:lang="it">Falda del Sardona</skos:prefLabel>
	<skos:broader rdf:resource="https://dev-lexic.swissgeol.ch/TectonicUnits/LowerHelvetic"/>
	<skos:narrower rdf:resource="https://dev-lexic.swissgeol.ch/TectonicUnits/MarchegghornSlice_PartSardona"/>
	<skos:narrower rdf:resource="https://dev-lexic.swissgeol.ch/TectonicUnits/OrglenSlices_PartSardona"/>
	<skos:narrower rdf:resource="https://dev-lexic.swissgeol.ch/TectonicUnits/CalandaSlice_PartSardona"/>
	<skos:narrower rdf:resource="https://dev-lexic.swissgeol.ch/TectonicUnits/MiruttaSlice_PartSardona"/>
	<status xmlns="http://www.w3.org/ns/adms#" rdf:resource="https://dev-lexic.swissgeol.ch/active"/>
</rdf:Description>

<rdf:Description rdf:about="https://dev-lexic.swissgeol.ch/TectonicUnits/BadRagazNappe">
	<rdf:type rdf:resource="http://www.w3.org/2004/02/skos/core#Concept"/>
	<rdfs:isDefinedBy xml:lang="en">Gouffon Yves (Editor) (2024): Tectonic Map of Switzerland 1:500000, Explanatory notes. Federal Office of Topography swisstopo, Wabern</rdfs:isDefinedBy>
	<skos:definition xml:lang="en">The Bad Ragaz Nappe is a Lower Helvetic tectonic nappe emplaced in an early phase onto the future Helvetic domain, subsequently truncated by the Glarus Thrust and simultaneously cut by out-of-sequence thrusts. It is composed mainly of Late Cretaceous to Paleogene sediments of South Helvetic affinity, cropping out in the area between Linthal and Sargans.</skos:definition>
	<skos:inScheme rdf:resource="https://dev-lexic.swissgeol.ch/TectonicUnits"/>
	<skos:prefLabel xml:lang="en">Bad Ragaz Nappe</skos:prefLabel>
	<skos:prefLabel xml:lang="de">Bad-Ragaz-Decke</skos:prefLabel>
	<skos:prefLabel xml:lang="fr">Nappe de Bad Ragaz</skos:prefLabel>
	<skos:prefLabel xml:lang="it">Falda di Bad Ragaz</skos:prefLabel>
	<skos:broader rdf:resource="https://dev-lexic.swissgeol.ch/TectonicUnits/LowerHelvetic"/>
	<status xmlns="http://www.w3.org/ns/adms#" rdf:resource="https://dev-lexic.swissgeol.ch/active"/>
</rdf:Description>

<rdf:Description rdf:about="https://dev-lexic.swissgeol.ch/TectonicUnits/CalandaSlice">
	<rdf:type rdf:resource="http://www.w3.org/2004/02/skos/core#Concept"/>
	<rdfs:isDefinedBy xml:lang="en">Gouffon Yves (Editor) (2024): Tectonic Map of Switzerland 1:500000, Explanatory notes. Federal Office of Topography swisstopo, Wabern</rdfs:isDefinedBy>
	<skos:definition xml:lang="en">The Calanda Slice is a post-nappe tectonic slice (due to a late out-of-sequence thrusting) of the parautochthonous cover of the northeastern end of the Aar Massif.</skos:definition>
	<skos:inScheme rdf:resource="https://dev-lexic.swissgeol.ch/TectonicUnits"/>
	<skos:prefLabel xml:lang="en">Calanda Slice</skos:prefLabel>
	<skos:prefLabel xml:lang="de">Calanda-Schuppe</skos:prefLabel>
	<skos:prefLabel xml:lang="fr">Écaille du Calanda</skos:prefLabel>
	<skos:prefLabel xml:lang="it">Scaglia del Calanda</skos:prefLabel>
	<skos:broader rdf:resource="https://dev-lexic.swissgeol.ch/TectonicUnits/LowerHelvetic"/>
	<skos:narrower rdf:resource="https://dev-lexic.swissgeol.ch/TectonicUnits/CalandaSlice_PartAarMassif"/>
	<skos:narrower rdf:resource="https://dev-lexic.swissgeol.ch/TectonicUnits/CalandaSlice_PartBlattengrat"/>
	<skos:narrower rdf:resource="https://dev-lexic.swissgeol.ch/TectonicUnits/CalandaSlice_PartSardona"/>
	<status xmlns="http://www.w3.org/ns/adms#" rdf:resource="https://dev-lexic.swissgeol.ch/active"/>
</rdf:Description>

<rdf:Description rdf:about="https://dev-lexic.swissgeol.ch/TectonicUnits/MarchegghornSlice">
	<rdf:type rdf:resource="http://www.w3.org/2004/02/skos/core#Concept"/>
	<rdfs:isDefinedBy xml:lang="en">Gouffon Yves (Editor) (2024): Tectonic Map of Switzerland 1:500000, Explanatory notes. Federal Office of Topography swisstopo, Wabern</rdfs:isDefinedBy>
	<skos:definition xml:lang="en">The Marchegghorn Slice is a post-nappe tectonic slice (due to a late out-of-sequence thrusting) of the parautochthonous cover of the northeastern end of the Aar Massif.</skos:definition>
	<skos:inScheme rdf:resource="https://dev-lexic.swissgeol.ch/TectonicUnits"/>
	<skos:prefLabel xml:lang="en">Marchegghorn Slice</skos:prefLabel>
	<skos:prefLabel xml:lang="de">Marchegghorn-Schuppe</skos:prefLabel>
	<skos:prefLabel xml:lang="fr">Écaille du Marchegghorn</skos:prefLabel>
	<skos:prefLabel xml:lang="it">Scaglia del Marchegghorn</skos:prefLabel>
	<skos:broader rdf:resource="https://dev-lexic.swissgeol.ch/TectonicUnits/LowerHelvetic"/>
	<skos:narrower rdf:resource="https://dev-lexic.swissgeol.ch/TectonicUnits/MarchegghornSlice_PartBlattengrat"/>
	<skos:narrower rdf:resource="https://dev-lexic.swissgeol.ch/TectonicUnits/MarchegghornSlice_PartSardona"/>
	<status xmlns="http://www.w3.org/ns/adms#" rdf:resource="https://dev-lexic.swissgeol.ch/active"/>
</rdf:Description>

<rdf:Description rdf:about="https://dev-lexic.swissgeol.ch/TectonicUnits/MiruttaSlice">
	<rdf:type rdf:resource="http://www.w3.org/2004/02/skos/core#Concept"/>
	<rdfs:isDefinedBy xml:lang="en">Gouffon Yves (Editor) (2024): Tectonic Map of Switzerland 1:500000, Explanatory notes. Federal Office of Topography swisstopo, Wabern</rdfs:isDefinedBy>
	<skos:definition xml:lang="en">The Mirutta Slice is a post-nappe tectonic slice (due to a late out-of-sequence thrusting) of the parautochthonous cover of the northeastern end of the Aar Massif.</skos:definition>
	<skos:inScheme rdf:resource="https://dev-lexic.swissgeol.ch/TectonicUnits"/>
	<skos:prefLabel xml:lang="en">Mirutta Slice</skos:prefLabel>
	<skos:prefLabel xml:lang="de">Mirutta-Schuppe</skos:prefLabel>
	<skos:prefLabel xml:lang="fr">Écaille du Mirutta</skos:prefLabel>
	<skos:prefLabel xml:lang="it">Scaglia del Mirutta</skos:prefLabel>
	<skos:broader rdf:resource="https://dev-lexic.swissgeol.ch/TectonicUnits/LowerHelvetic"/>
	<skos:narrower rdf:resource="https://dev-lexic.swissgeol.ch/TectonicUnits/MiruttaSlice_PartAarMassif"/>
	<skos:narrower rdf:resource="https://dev-lexic.swissgeol.ch/TectonicUnits/MiruttaSlice_PartBlattengrat"/>
	<skos:narrower rdf:resource="https://dev-lexic.swissgeol.ch/TectonicUnits/MiruttaSlice_PartSardona"/>
	<status xmlns="http://www.w3.org/ns/adms#" rdf:resource="https://dev-lexic.swissgeol.ch/active"/>
</rdf:Description>

<rdf:Description rdf:about="https://dev-lexic.swissgeol.ch/TectonicUnits/OrglenSlices">
	<rdf:type rdf:resource="http://www.w3.org/2004/02/skos/core#Concept"/>
	<rdfs:isDefinedBy xml:lang="en">Gouffon Yves (Editor) (2024): Tectonic Map of Switzerland 1:500000, Explanatory notes. Federal Office of Topography swisstopo, Wabern</rdfs:isDefinedBy>
	<skos:definition xml:lang="en">The Orglen Slices are post-nappe tectonic slices (due to a late out-of-sequence thrusting) of the parautochthonous cover of the northeastern end of the Aar Massif.</skos:definition>
	<skos:inScheme rdf:resource="https://dev-lexic.swissgeol.ch/TectonicUnits"/>
	<skos:prefLabel xml:lang="en">Orglen Slices</skos:prefLabel>
	<skos:prefLabel xml:lang="de">Orglen-Schuppe</skos:prefLabel>
	<skos:prefLabel xml:lang="fr">Écaille de l'Orglen</skos:prefLabel>
	<skos:prefLabel xml:lang="it">Scaglia dell'Orglen</skos:prefLabel>
	<skos:broader rdf:resource="https://dev-lexic.swissgeol.ch/TectonicUnits/LowerHelvetic"/>
	<skos:narrower rdf:resource="https://dev-lexic.swissgeol.ch/TectonicUnits/OrglenSlices_PartAarMassif"/>
	<skos:narrower rdf:resource="https://dev-lexic.swissgeol.ch/TectonicUnits/OrglenSlices_PartSardona"/>
	<status xmlns="http://www.w3.org/ns/adms#" rdf:resource="https://dev-lexic.swissgeol.ch/active"/>
</rdf:Description>

<rdf:Description rdf:about="https://dev-lexic.swissgeol.ch/TectonicUnits/MontChetifNappe">
	<rdf:type rdf:resource="http://www.w3.org/2004/02/skos/core#Concept"/>
	<rdfs:isDefinedBy xml:lang="en">Gouffon Yves (Editor) (2024): Tectonic Map of Switzerland 1:500000, Explanatory notes. Federal Office of Topography swisstopo, Wabern</rdfs:isDefinedBy>
	<skos:definition xml:lang="en">The Mont Chétif Nappe is an Upper Helvetic tectonic nappe of the French and Western Swiss Alps. It forms a band of sedimentary rocks overlying the sedimentary cover of the Internal Mont Blanc Massif from Saxon in the Rhône Valley up to south of the Mont Blanc summit. It seems to be autochthonous above the small Mont Chétif Massif in the Valle d’Aosta. This nappe is assumed to be the root of the Wildhorn Nappe Complex situated north of the Rhône.</skos:definition>
	<skos:inScheme rdf:resource="https://dev-lexic.swissgeol.ch/TectonicUnits"/>
	<skos:prefLabel xml:lang="en">Mont Chétif Nappe</skos:prefLabel>
	<skos:prefLabel xml:lang="de">Mont-Chétif-Decke</skos:prefLabel>
	<skos:prefLabel xml:lang="fr">Nappe du Mont Chétif</skos:prefLabel>
	<skos:prefLabel xml:lang="it">Falda del Mont Chétif</skos:prefLabel>
	<skos:broader rdf:resource="https://dev-lexic.swissgeol.ch/TectonicUnits/UpperHelvetic"/>
	<status xmlns="http://www.w3.org/ns/adms#" rdf:resource="https://dev-lexic.swissgeol.ch/active"/>
</rdf:Description>

<rdf:Description rdf:about="https://dev-lexic.swissgeol.ch/TectonicUnits/RoseletteNappe">
	<rdf:type rdf:resource="http://www.w3.org/2004/02/skos/core#Concept"/>
	<rdfs:isDefinedBy xml:lang="en">Gouffon Yves (Editor) (2024): Tectonic Map of Switzerland 1:500000, Explanatory notes. Federal Office of Topography swisstopo, Wabern</rdfs:isDefinedBy>
	<skos:definition xml:lang="en">The Roselette Nappe is a small Upper Helvetic tectonic nappe situated around the southwestern end of the Mont Blanc Massif. It consists of similar basement and sediment rocks as the Mont Chétif Nappe and occupies a similar structural position above the crystalline basement and sedimentary cover of the Mont Blanc Massif. It is characterized by the presence of several internal thrust faults.</skos:definition>
	<skos:inScheme rdf:resource="https://dev-lexic.swissgeol.ch/TectonicUnits"/>
	<skos:prefLabel xml:lang="en">Roselette Nappe</skos:prefLabel>
	<skos:prefLabel xml:lang="de">Roselette-Decke</skos:prefLabel>
	<skos:prefLabel xml:lang="fr">Nappe de Roselette</skos:prefLabel>
	<skos:prefLabel xml:lang="it">Falda di Roselette</skos:prefLabel>
	<skos:broader rdf:resource="https://dev-lexic.swissgeol.ch/TectonicUnits/UpperHelvetic"/>
	<status xmlns="http://www.w3.org/ns/adms#" rdf:resource="https://dev-lexic.swissgeol.ch/active"/>
</rdf:Description>

<rdf:Description rdf:about="https://dev-lexic.swissgeol.ch/TectonicUnits/WildhornNappeComplex">
	<rdf:type rdf:resource="http://www.w3.org/2004/02/skos/core#Concept"/>
	<rdfs:isDefinedBy xml:lang="en">Gouffon Yves (Editor) (2024): Tectonic Map of Switzerland 1:500000, Explanatory notes. Federal Office of Topography swisstopo, Wabern</rdfs:isDefinedBy>
	<skos:definition xml:lang="en">The Wildhorn Nappe Complex is an Upper Helvetic set of three superposed tectonic nappes in the Western Swiss Alps: the Diablerets Nappe, present only in the southwest, at the base of the complex, is linked by a tight syncline to the Mont Gond Nappe, which is also outcropping mainly in the southwestern part of the complex. The highest Sublage Nappe forms the main body of the complex; it overlies the thin Jägerchrüz Nappe north of Sierre and the Gellihorn Nappe further northeast. The Wildhorn Nappe Complex comprises a complete stratigraphic series ranging from Triassic to Paleogene occupying the Rawil axial depression. It continues to the northeast up to the Kander Valley, where it is replaced by the Axen and Drusberg nappes.</skos:definition>
	<skos:inScheme rdf:resource="https://dev-lexic.swissgeol.ch/TectonicUnits"/>
	<skos:prefLabel xml:lang="en">Wildhorn Nappe Complex</skos:prefLabel>
	<skos:prefLabel xml:lang="de">Wildhorn-Deckenkomplex</skos:prefLabel>
	<skos:prefLabel xml:lang="fr">Complexe de nappes du Wildhorn</skos:prefLabel>
	<skos:prefLabel xml:lang="it">Complesso di falde del Wildhorn</skos:prefLabel>
	<skos:broader rdf:resource="https://dev-lexic.swissgeol.ch/TectonicUnits/UpperHelvetic"/>
	<skos:narrower rdf:resource="https://dev-lexic.swissgeol.ch/TectonicUnits/DiableretsNappe"/>
	<skos:narrower rdf:resource="https://dev-lexic.swissgeol.ch/TectonicUnits/MontGondNappe"/>
	<skos:narrower rdf:resource="https://dev-lexic.swissgeol.ch/TectonicUnits/SublageNappe"/>
	<skos:related rdf:resource="https://dev-lexic.swissgeol.ch/TectonicUnits/DrusbergNappe"/>
	<status xmlns="http://www.w3.org/ns/adms#" rdf:resource="https://dev-lexic.swissgeol.ch/active"/>
</rdf:Description>

<rdf:Description rdf:about="https://dev-lexic.swissgeol.ch/TectonicUnits/GlarusNappeComplex">
	<rdf:type rdf:resource="http://www.w3.org/2004/02/skos/core#Concept"/>
	<rdfs:isDefinedBy xml:lang="en">Gouffon Yves (Editor) (2024): Tectonic Map of Switzerland 1:500000, Explanatory notes. Federal Office of Topography swisstopo, Wabern</rdfs:isDefinedBy>
	<skos:definition xml:lang="en">The Glarus Nappe Complex is an Upper Helvetic tectonic nappe complex extending from the Linth Valley to the Rhine Valley. The stratigraphic series of the Glarus Nappe Complex consists of a thick Verrucano (Permian), Triassic and Jurassic series, as well as Cretaceous and some Paleogene sediments depending on the subunit of the complex.</skos:definition>
	<skos:inScheme rdf:resource="https://dev-lexic.swissgeol.ch/TectonicUnits"/>
	<skos:prefLabel xml:lang="en">Glarus Nappe Complex</skos:prefLabel>
	<skos:prefLabel xml:lang="de">Glarner Deckenkomplex</skos:prefLabel>
	<skos:prefLabel xml:lang="fr">Complexe de nappes de Glaris</skos:prefLabel>
	<skos:prefLabel xml:lang="it">Complesso di falde di Glarona</skos:prefLabel>
	<skos:broader rdf:resource="https://dev-lexic.swissgeol.ch/TectonicUnits/UpperHelvetic"/>
	<skos:narrower rdf:resource="https://dev-lexic.swissgeol.ch/TectonicUnits/WagetenSlice"/>
	<skos:narrower rdf:resource="https://dev-lexic.swissgeol.ch/TectonicUnits/Gonzen-WalenstadtSlices"/>
	<skos:narrower rdf:resource="https://dev-lexic.swissgeol.ch/TectonicUnits/MuertschenNappe"/>
	<status xmlns="http://www.w3.org/ns/adms#" rdf:resource="https://dev-lexic.swissgeol.ch/active"/>
</rdf:Description>

<rdf:Description rdf:about="https://dev-lexic.swissgeol.ch/TectonicUnits/AxenNappe">
	<rdf:type rdf:resource="http://www.w3.org/2004/02/skos/core#Concept"/>
	<rdfs:isDefinedBy xml:lang="en">Gouffon Yves (Editor) (2024): Tectonic Map of Switzerland 1:500000, Explanatory notes. Federal Office of Topography swisstopo, Wabern</rdfs:isDefinedBy>
	<skos:definition xml:lang="en">Within the Upper Helvetic, the Axen Nappe, together with the Drusberg Nappe, represents the continuation of the Wildhorn Nappe Complex east of the Kander Valley. Its internal structure is regionally complicated by additional décollement levels which split the nappe into several slices.</skos:definition>
	<skos:inScheme rdf:resource="https://dev-lexic.swissgeol.ch/TectonicUnits"/>
	<skos:prefLabel xml:lang="en">Axen Nappe</skos:prefLabel>
	<skos:prefLabel xml:lang="de">Axen-Decke</skos:prefLabel>
	<skos:prefLabel xml:lang="fr">Nappe de l'Axen</skos:prefLabel>
	<skos:prefLabel xml:lang="it">Falda dell'Axen</skos:prefLabel>
	<skos:broader rdf:resource="https://dev-lexic.swissgeol.ch/TectonicUnits/UpperHelvetic"/>
	<skos:narrower rdf:resource="https://dev-lexic.swissgeol.ch/TectonicUnits/ToralpSlice"/>
	<skos:narrower rdf:resource="https://dev-lexic.swissgeol.ch/TectonicUnits/SilberenSlices"/>
	<skos:narrower rdf:resource="https://dev-lexic.swissgeol.ch/TectonicUnits/BaechistockSlice"/>
	<skos:narrower rdf:resource="https://dev-lexic.swissgeol.ch/TectonicUnits/WissbergSlice"/>
	<skos:narrower rdf:resource="https://dev-lexic.swissgeol.ch/TectonicUnits/SchaechentalerWindgaellenSlices"/>
	<skos:narrower rdf:resource="https://dev-lexic.swissgeol.ch/TectonicUnits/HoechTurmSlices"/>
	<skos:narrower rdf:resource="https://dev-lexic.swissgeol.ch/TectonicUnits/FriterenSlice"/>
	<skos:narrower rdf:resource="https://dev-lexic.swissgeol.ch/TectonicUnits/AxenNorthSlice"/>
	<skos:narrower rdf:resource="https://dev-lexic.swissgeol.ch/TectonicUnits/AxenSouthSlice"/>
	<status xmlns="http://www.w3.org/ns/adms#" rdf:resource="https://dev-lexic.swissgeol.ch/active"/>
</rdf:Description>

<rdf:Description rdf:about="https://dev-lexic.swissgeol.ch/TectonicUnits/DrusbergNappe">
	<rdf:type rdf:resource="http://www.w3.org/2004/02/skos/core#Concept"/>
	<rdfs:isDefinedBy xml:lang="en">Gouffon Yves (Editor) (2024): Tectonic Map of Switzerland 1:500000, Explanatory notes. Federal Office of Topography swisstopo, Wabern</rdfs:isDefinedBy>
	<skos:definition xml:lang="en">Within the Upper Helvetic, the Drusberg Nappe, together with the Axen Nappe, represents the continuation of the Wildhorn Nappe Complex east of the Kander Valley. The Drusberg Nappe consists only of Cretaceous to Paleogene sediments, locally with slices of Late Jurassic limestone (Quinten Formation) at its base.</skos:definition>
	<skos:inScheme rdf:resource="https://dev-lexic.swissgeol.ch/TectonicUnits"/>
	<skos:prefLabel xml:lang="en">Drusberg Nappe</skos:prefLabel>
	<skos:prefLabel xml:lang="de">Drusberg-Decke</skos:prefLabel>
	<skos:prefLabel xml:lang="fr">Nappe du Drusberg</skos:prefLabel>
	<skos:prefLabel xml:lang="it">Falda del Drusberg</skos:prefLabel>
	<skos:broader rdf:resource="https://dev-lexic.swissgeol.ch/TectonicUnits/UpperHelvetic"/>
	<skos:narrower rdf:resource="https://dev-lexic.swissgeol.ch/TectonicUnits/WissenwandSlice"/>
	<skos:narrower rdf:resource="https://dev-lexic.swissgeol.ch/TectonicUnits/Niederhorn-PilatusSlice"/>
	<skos:narrower rdf:resource="https://dev-lexic.swissgeol.ch/TectonicUnits/Buergenstock-UrmibergSlice"/>
	<skos:narrower rdf:resource="https://dev-lexic.swissgeol.ch/TectonicUnits/HochflueSlice"/>
	<skos:narrower rdf:resource="https://dev-lexic.swissgeol.ch/TectonicUnits/MaisanderSlice"/>
	<skos:narrower rdf:resource="https://dev-lexic.swissgeol.ch/TectonicUnits/AubrigSlice"/>
	<skos:related rdf:resource="https://dev-lexic.swissgeol.ch/TectonicUnits/WildhornNappeComplex"/>
	<status xmlns="http://www.w3.org/ns/adms#" rdf:resource="https://dev-lexic.swissgeol.ch/active"/>
</rdf:Description>

<rdf:Description rdf:about="https://dev-lexic.swissgeol.ch/TectonicUnits/SaentisNappe">
	<rdf:type rdf:resource="http://www.w3.org/2004/02/skos/core#Concept"/>
	<rdfs:isDefinedBy xml:lang="en">Gouffon Yves (Editor) (2024): Tectonic Map of Switzerland 1:500000, Explanatory notes. Federal Office of Topography swisstopo, Wabern</rdfs:isDefinedBy>
	<skos:definition xml:lang="en">The Säntis Nappe is an Upper Helvetic tectonic nappe of the Eastern Swiss Alps, extending from the Linth Valley in the west to the Rhine Valley in the east (including the Fläscher Berg east of Sargans). It overlies the Glarus Nappe Complex north of the Walensee and Seeztal, forming a broad synform, in the core of which are preserved klippen consisting of Upper Helvetic mélanges, as well as Lower and Middle Penninic units.
The Säntis Nappe is composed of Cretaceous and rare Paleogene sediments. Its internal structure is characterized by fold trains and fold-parallel thrust faults, with an important N–S oriented fault between Sax and Appenzell (Sax-Schwende Fault) that can be shown to have been active during the nappe internal deformation.</skos:definition>
	<skos:inScheme rdf:resource="https://dev-lexic.swissgeol.ch/TectonicUnits"/>
	<skos:prefLabel xml:lang="en">Säntis Nappe</skos:prefLabel>
	<skos:prefLabel xml:lang="de">Säntis-Decke</skos:prefLabel>
	<skos:prefLabel xml:lang="fr">Nappe du Säntis</skos:prefLabel>
	<skos:prefLabel xml:lang="it">Falda del Säntis</skos:prefLabel>
	<skos:altLabel xml:lang="de">Churfristen-Decke</skos:altLabel>
	<skos:broader rdf:resource="https://dev-lexic.swissgeol.ch/TectonicUnits/UpperHelvetic"/>
	<status xmlns="http://www.w3.org/ns/adms#" rdf:resource="https://dev-lexic.swissgeol.ch/active"/>
</rdf:Description>

<rdf:Description rdf:about="https://dev-lexic.swissgeol.ch/TectonicUnits/HohenemsNappe">
	<rdf:type rdf:resource="http://www.w3.org/2004/02/skos/core#Concept"/>
	<rdfs:isDefinedBy xml:lang="en">Gouffon Yves (Editor) (2024): Tectonic Map of Switzerland 1:500000, Explanatory notes. Federal Office of Topography swisstopo, Wabern</rdfs:isDefinedBy>
	<skos:definition xml:lang="en">The Hohenems Nappe is an Upper Helvetic tectonic nappe that crops out solely around Hohenems, in the Rhine Valley. It dips southward below the Säntis Nappe, extending in the subsurface as far as Liechtenstein.</skos:definition>
	<skos:inScheme rdf:resource="https://dev-lexic.swissgeol.ch/TectonicUnits"/>
	<skos:prefLabel xml:lang="en">Hohenems Nappe</skos:prefLabel>
	<skos:prefLabel xml:lang="de">Hohenems-Decke</skos:prefLabel>
	<skos:prefLabel xml:lang="fr">Nappe de Hohenems</skos:prefLabel>
	<skos:prefLabel xml:lang="it">Falda di Hohenems</skos:prefLabel>
	<skos:broader rdf:resource="https://dev-lexic.swissgeol.ch/TectonicUnits/UpperHelvetic"/>
	<status xmlns="http://www.w3.org/ns/adms#" rdf:resource="https://dev-lexic.swissgeol.ch/active"/>
</rdf:Description>

<rdf:Description rdf:about="https://dev-lexic.swissgeol.ch/TectonicUnits/TavetschNappe">
	<rdf:type rdf:resource="http://www.w3.org/2004/02/skos/core#Concept"/>
	<rdfs:isDefinedBy xml:lang="en">Gouffon Yves (Editor) (2024): Tectonic Map of Switzerland 1:500000, Explanatory notes. Federal Office of Topography swisstopo, Wabern</rdfs:isDefinedBy>
	<skos:definition xml:lang="en">The Tavetsch Nappe is an Upper Helvetic tectonic unit cropping out in a large part of the upper Surselva (Vorderrhein Valley). It shows two contrasting parts: In the west, a narrow crystalline “massif” (formerly “Tavetsch -Zwischenmassiv”), consisting mainly of paragneisses, lies between the Aar Massif in the north and the Gotthard Nappe in the south. In the east, this crystalline basement thins and terminates towards the east in the core of an anticline, surrounded by Permian Verrucano sediments. The continuation of these sediments is found in the Glarus Nappe Complex.</skos:definition>
	<skos:inScheme rdf:resource="https://dev-lexic.swissgeol.ch/TectonicUnits"/>
	<skos:prefLabel xml:lang="en">Tavetsch Nappe</skos:prefLabel>
	<skos:prefLabel xml:lang="de">Tavetsch-Decke</skos:prefLabel>
	<skos:prefLabel xml:lang="fr">Nappe du Tavetsch</skos:prefLabel>
	<skos:prefLabel xml:lang="it">Falda del Tavetsch</skos:prefLabel>
	<skos:broader rdf:resource="https://dev-lexic.swissgeol.ch/TectonicUnits/UpperHelvetic"/>
	<status xmlns="http://www.w3.org/ns/adms#" rdf:resource="https://dev-lexic.swissgeol.ch/active"/>
</rdf:Description>

<rdf:Description rdf:about="https://dev-lexic.swissgeol.ch/TectonicUnits/IlanzNappe">
	<rdf:type rdf:resource="http://www.w3.org/2004/02/skos/core#Concept"/>
	<rdfs:isDefinedBy xml:lang="en">Gouffon Yves (Editor) (2024): Tectonic Map of Switzerland 1:500000, Explanatory notes. Federal Office of Topography swisstopo, Wabern</rdfs:isDefinedBy>
	<skos:definition xml:lang="en">The Ilanz Nappe is an Upper Helvetic tectonic unit extending south of the eastern part of the Tavetsch Nappe and consisting of Permian Verrucano sediments locally capped by Triassic sediments.</skos:definition>
	<skos:inScheme rdf:resource="https://dev-lexic.swissgeol.ch/TectonicUnits"/>
	<skos:prefLabel xml:lang="en">Ilanz Nappe</skos:prefLabel>
	<skos:prefLabel xml:lang="de">Ilanz-Decke</skos:prefLabel>
	<skos:prefLabel xml:lang="fr">Nappe d'Ilanz</skos:prefLabel>
	<skos:prefLabel xml:lang="it">Falda di Ilanz</skos:prefLabel>
	<skos:broader rdf:resource="https://dev-lexic.swissgeol.ch/TectonicUnits/UpperHelvetic"/>
	<status xmlns="http://www.w3.org/ns/adms#" rdf:resource="https://dev-lexic.swissgeol.ch/active"/>
</rdf:Description>

<rdf:Description rdf:about="https://dev-lexic.swissgeol.ch/TectonicUnits/GotthardNappe">
	<rdf:type rdf:resource="http://www.w3.org/2004/02/skos/core#Concept"/>
	<rdfs:isDefinedBy xml:lang="en">Gouffon Yves (Editor) (2024): Tectonic Map of Switzerland 1:500000, Explanatory notes. Federal Office of Topography swisstopo, Wabern</rdfs:isDefinedBy>
	<skos:definition xml:lang="en">The Gotthard Nappe, extending from Brig in Valais to Ilanz in Graubünden, is an Upper Helvetic tectonic unit with a crystalline core (former “Gotthard Massif”) consisting of pre-Caledonian and pre-Variscan para- and orthogneisses, as well as Late Variscan granitic intrusions. The sedimentary cover of this nappe varies from place to place: “Urseren-Garvera Zone” (including "Goms Massif") at the northern border of the nappe, “Termen Zone” and “Nufenen Zone” at the southern border between Brig and Airolo.</skos:definition>
	<skos:inScheme rdf:resource="https://dev-lexic.swissgeol.ch/TectonicUnits"/>
	<skos:prefLabel xml:lang="en">Gotthard Nappe</skos:prefLabel>
	<skos:prefLabel xml:lang="de">Gotthard-Decke</skos:prefLabel>
	<skos:prefLabel xml:lang="fr">Nappe du Gothard</skos:prefLabel>
	<skos:prefLabel xml:lang="it">Falda del Gottardo</skos:prefLabel>
	<skos:broader rdf:resource="https://dev-lexic.swissgeol.ch/TectonicUnits/UpperHelvetic"/>
	<status xmlns="http://www.w3.org/ns/adms#" rdf:resource="https://dev-lexic.swissgeol.ch/active"/>
</rdf:Description>

<rdf:Description rdf:about="https://dev-lexic.swissgeol.ch/TectonicUnits/CamosciNappe">
	<rdf:type rdf:resource="http://www.w3.org/2004/02/skos/core#Concept"/>
	<rdfs:isDefinedBy xml:lang="en">Gouffon Yves (Editor) (2024): Tectonic Map of Switzerland 1:500000, Explanatory notes. Federal Office of Topography swisstopo, Wabern</rdfs:isDefinedBy>
	<skos:definition xml:lang="en">The Camosci Nappe is a small Upper Helvetic tectonic nappe located south of the Nufenenpass and sandwiched between the Lower Penninic Sion-Courmayeur Nappe to the north and the Lepontic Monte Leone and Lebendun nappes to the south. It is made up of sediments with South Helvetic to Ultrahelvetic affinity.</skos:definition>
	<skos:inScheme rdf:resource="https://dev-lexic.swissgeol.ch/TectonicUnits"/>
	<skos:prefLabel xml:lang="en">Camosci Nappe</skos:prefLabel>
	<skos:prefLabel xml:lang="de">Camosci-Decke</skos:prefLabel>
	<skos:prefLabel xml:lang="fr">Nappe des Camosci</skos:prefLabel>
	<skos:prefLabel xml:lang="it">Falda dei Camosci</skos:prefLabel>
	<skos:broader rdf:resource="https://dev-lexic.swissgeol.ch/TectonicUnits/UpperHelvetic"/>
	<status xmlns="http://www.w3.org/ns/adms#" rdf:resource="https://dev-lexic.swissgeol.ch/active"/>
</rdf:Description>

<rdf:Description rdf:about="https://dev-lexic.swissgeol.ch/TectonicUnits/ScopiNappe">
	<rdf:type rdf:resource="http://www.w3.org/2004/02/skos/core#Concept"/>
	<rdfs:isDefinedBy xml:lang="en">Gouffon Yves (Editor) (2024): Tectonic Map of Switzerland 1:500000, Explanatory notes. Federal Office of Topography swisstopo, Wabern</rdfs:isDefinedBy>
	<skos:definition xml:lang="en">The Scopi Nappe is an Upper Helvetic tectonic nappe extending southeast of the Gotthard Nappe between the Passo del Lucomagno and Ilanz. It consists of an overturned sedimentary sequence of Triassic to Middle Jurassic age and of South Helvetic to Ultrahelvetic origin.</skos:definition>
	<skos:inScheme rdf:resource="https://dev-lexic.swissgeol.ch/TectonicUnits"/>
	<skos:prefLabel xml:lang="en">Scopi Nappe</skos:prefLabel>
	<skos:prefLabel xml:lang="de">Scopi-Decke</skos:prefLabel>
	<skos:prefLabel xml:lang="fr">Nappe du Scopi</skos:prefLabel>
	<skos:prefLabel xml:lang="it">Falda dello Scopi</skos:prefLabel>
	<skos:broader rdf:resource="https://dev-lexic.swissgeol.ch/TectonicUnits/UpperHelvetic"/>
	<status xmlns="http://www.w3.org/ns/adms#" rdf:resource="https://dev-lexic.swissgeol.ch/active"/>
</rdf:Description>

<rdf:Description rdf:about="https://dev-lexic.swissgeol.ch/TectonicUnits/Piora-PeidenSliceComplex">
	<rdf:type rdf:resource="http://www.w3.org/2004/02/skos/core#Concept"/>
	<rdfs:isDefinedBy xml:lang="en">Gouffon Yves (Editor) (2024): Tectonic Map of Switzerland 1:500000, Explanatory notes. Federal Office of Topography swisstopo, Wabern</rdfs:isDefinedBy>
	<skos:definition xml:lang="en">The Piora-Peiden Slice Complex is an Upper Helvetic set of thin tectonic slices that occur continuously from Airolo to Ilanz between the Gotthard or Scopi nappes to the north and the Leventina-Lucomagno or Grava nappes to the south. These slices consist of Triassic to Early Jurassic sediments similar to those of the Scopi Nappe and underwent a first Alpine metamorphic phase of high pressure (similar to Lepontic units).</skos:definition>
	<skos:inScheme rdf:resource="https://dev-lexic.swissgeol.ch/TectonicUnits"/>
	<skos:prefLabel xml:lang="en">Piora-Peiden Slice Complex</skos:prefLabel>
	<skos:prefLabel xml:lang="de">Piora-Peiden-Schuppenkomplex</skos:prefLabel>
	<skos:prefLabel xml:lang="fr">Complexe d'écailles de Piora-Peiden</skos:prefLabel>
	<skos:prefLabel xml:lang="it">Complesso di scaglie di Piora-Peiden</skos:prefLabel>
	<skos:broader rdf:resource="https://dev-lexic.swissgeol.ch/TectonicUnits/UpperHelvetic"/>
	<status xmlns="http://www.w3.org/ns/adms#" rdf:resource="https://dev-lexic.swissgeol.ch/active"/>
</rdf:Description>

<rdf:Description rdf:about="https://dev-lexic.swissgeol.ch/TectonicUnits/HabkernMelangeZone">
	<rdf:type rdf:resource="http://www.w3.org/2004/02/skos/core#Concept"/>
	<rdfs:isDefinedBy xml:lang="en">Gouffon Yves (Editor) (2024): Tectonic Map of Switzerland 1:500000, Explanatory notes. Federal Office of Topography swisstopo, Wabern</rdfs:isDefinedBy>
	<skos:definition xml:lang="en">The Habkern Mélange Zone overlies the Drusberg Nappe between the Thunersee and the Vierwaldstättersee. It is located in a synformal structure and overlain by klippen of the Lower Penninic Schlieren Nappe and Middle Penninic Préalpes Médianes Nappe. Several mélanges are defined in this zone, all containing some “wildflysch” with Late Cretaceous and Paleogene lenses, slices of South Helvetic origin and slices from the overlying Penninic units.</skos:definition>
	<skos:inScheme rdf:resource="https://dev-lexic.swissgeol.ch/TectonicUnits"/>
	<skos:prefLabel xml:lang="en">Habkern Mélange Zone</skos:prefLabel>
	<skos:prefLabel xml:lang="de">Habkern-Melangezone</skos:prefLabel>
	<skos:prefLabel xml:lang="fr">Zone de mélange d'Habkern</skos:prefLabel>
	<skos:prefLabel xml:lang="it">Zona di mélange di Habkern</skos:prefLabel>
	<skos:broader rdf:resource="https://dev-lexic.swissgeol.ch/TectonicUnits/UpperHelvetic"/>
	<status xmlns="http://www.w3.org/ns/adms#" rdf:resource="https://dev-lexic.swissgeol.ch/active"/>
</rdf:Description>

<rdf:Description rdf:about="https://dev-lexic.swissgeol.ch/TectonicUnits/IbergMelange">
	<rdf:type rdf:resource="http://www.w3.org/2004/02/skos/core#Concept"/>
	<rdfs:isDefinedBy xml:lang="en">Gouffon Yves (Editor) (2024): Tectonic Map of Switzerland 1:500000, Explanatory notes. Federal Office of Topography swisstopo, Wabern</rdfs:isDefinedBy>
	<skos:definition xml:lang="en">The Iberg Mélange overlies the Drusberg Nappe in the Iberg Klippen, where it is overlain by Penninic and Austroalpine units. It contains some “wildflysch” with Late Cretaceous and Paleogene lenses, slices of South Helvetic origin and slices from the overlying Penninic units.</skos:definition>
	<skos:inScheme rdf:resource="https://dev-lexic.swissgeol.ch/TectonicUnits"/>
	<skos:prefLabel xml:lang="en">Iberg Mélange</skos:prefLabel>
	<skos:prefLabel xml:lang="de">Iberg-Melange</skos:prefLabel>
	<skos:prefLabel xml:lang="fr">Mélange d'Iberg</skos:prefLabel>
	<skos:prefLabel xml:lang="it">Mélange di Iberg</skos:prefLabel>
	<skos:broader rdf:resource="https://dev-lexic.swissgeol.ch/TectonicUnits/UpperHelvetic"/>
	<status xmlns="http://www.w3.org/ns/adms#" rdf:resource="https://dev-lexic.swissgeol.ch/active"/>
</rdf:Description>

<rdf:Description rdf:about="https://dev-lexic.swissgeol.ch/TectonicUnits/InternalEinsiedelnSlices">
	<rdf:type rdf:resource="http://www.w3.org/2004/02/skos/core#Concept"/>
	<rdfs:isDefinedBy xml:lang="en">Gouffon Yves (Editor) (2024): Tectonic Map of Switzerland 1:500000, Explanatory notes. Federal Office of Topography swisstopo, Wabern</rdfs:isDefinedBy>
	<skos:definition xml:lang="en">The Internal Einsiedeln Slices overlie the Drusberg Nappe and underlie the Wägital Nappe in the region between Schwyz and Wägitalersee. They consist of slices of Late Cretaceous and Paleogene sediments of South Helvetic origin.</skos:definition>
	<skos:inScheme rdf:resource="https://dev-lexic.swissgeol.ch/TectonicUnits"/>
	<skos:prefLabel xml:lang="en">Internal Einsiedeln Slices</skos:prefLabel>
	<skos:prefLabel xml:lang="de">Interne Einsiedeln-Schuppen</skos:prefLabel>
	<skos:prefLabel xml:lang="fr">Écailles internes d'Einsiedeln</skos:prefLabel>
	<skos:prefLabel xml:lang="it">Scaglie interne di Einsiedeln</skos:prefLabel>
	<skos:altLabel xml:lang="de">Innere Einsiedler Schuppenzone</skos:altLabel>
	<skos:broader rdf:resource="https://dev-lexic.swissgeol.ch/TectonicUnits/UpperHelvetic"/>
	<status xmlns="http://www.w3.org/ns/adms#" rdf:resource="https://dev-lexic.swissgeol.ch/active"/>
</rdf:Description>

<rdf:Description rdf:about="https://dev-lexic.swissgeol.ch/TectonicUnits/WildhausMelange">
	<rdf:type rdf:resource="http://www.w3.org/2004/02/skos/core#Concept"/>
	<rdfs:isDefinedBy xml:lang="en">Gouffon Yves (Editor) (2024): Tectonic Map of Switzerland 1:500000, Explanatory notes. Federal Office of Topography swisstopo, Wabern</rdfs:isDefinedBy>
	<skos:definition xml:lang="en">The Wildhaus Mélange overlies the Säntis Nappe in a large-scale synform north of the Walensee and consists of slices of Late Cretaceous and Paleogene strata of South Helvetic to Ultrahelvetic origin packed in a “wildflysch” matrix. Locally it is overlain by klippen of flysch of the Üntschen Nappe (Lower Penninic) or even of the Falknis Nappe (Middle Penninic).</skos:definition>
	<skos:inScheme rdf:resource="https://dev-lexic.swissgeol.ch/TectonicUnits"/>
	<skos:prefLabel xml:lang="en">Wildhaus Mélange</skos:prefLabel>
	<skos:prefLabel xml:lang="de">Wildhaus-Melange</skos:prefLabel>
	<skos:prefLabel xml:lang="fr">Mélange de Wildhaus</skos:prefLabel>
	<skos:prefLabel xml:lang="it">Mélange di Wildhaus</skos:prefLabel>
	<skos:broader rdf:resource="https://dev-lexic.swissgeol.ch/TectonicUnits/UpperHelvetic"/>
	<status xmlns="http://www.w3.org/ns/adms#" rdf:resource="https://dev-lexic.swissgeol.ch/active"/>
</rdf:Description>

<rdf:Description rdf:about="https://dev-lexic.swissgeol.ch/TectonicUnits/LiebensteinNappe">
	<rdf:type rdf:resource="http://www.w3.org/2004/02/skos/core#Concept"/>
	<rdfs:isDefinedBy xml:lang="en">Gouffon Yves (Editor) (2024): Tectonic Map of Switzerland 1:500000, Explanatory notes. Federal Office of Topography swisstopo, Wabern</rdfs:isDefinedBy>
	<skos:definition xml:lang="en">The Liebenstein Nappe represents the continuation of the Wildhaus Mélange in Austria. It consists of a slice complex including a “wildflysch” (“Feuerstätter Nappe”).</skos:definition>
	<skos:inScheme rdf:resource="https://dev-lexic.swissgeol.ch/TectonicUnits"/>
	<skos:prefLabel xml:lang="en">Liebenstein Nappe</skos:prefLabel>
	<skos:prefLabel xml:lang="de">Liebenstein-Decke</skos:prefLabel>
	<skos:prefLabel xml:lang="fr">Nappe de Liebenstein</skos:prefLabel>
	<skos:prefLabel xml:lang="it">Falda di Liebenstein</skos:prefLabel>
	<skos:altLabel xml:lang="en">Feuerstätter Nappe</skos:altLabel>
	<skos:altLabel xml:lang="de">Liebensteiner Decke</skos:altLabel>
	<skos:altLabel xml:lang="de">Liebenstein-Schuppenzone</skos:altLabel>
	<skos:altLabel xml:lang="de">Feuerstätter-Decke</skos:altLabel>
	<skos:broader rdf:resource="https://dev-lexic.swissgeol.ch/TectonicUnits/UpperHelvetic"/>
	<status xmlns="http://www.w3.org/ns/adms#" rdf:resource="https://dev-lexic.swissgeol.ch/active"/>
</rdf:Description>

<rdf:Description rdf:about="https://dev-lexic.swissgeol.ch/TectonicUnits/FlaescherbergNappe">
	<rdf:type rdf:resource="http://www.w3.org/2004/02/skos/core#Concept"/>
	<rdfs:isDefinedBy xml:lang="en">Gouffon Yves (Editor) (2024): Tectonic Map of Switzerland 1:500000, Explanatory notes. Federal Office of Topography swisstopo, Wabern</rdfs:isDefinedBy>
	<skos:definition xml:lang="en">The Fläscherberg Nappe is a small unit that overlies the Säntis Nappe at the southeastern end of the Fläscher Berg, a hill east of Sargans. It is made up of Jurassic sediments of South Helvetic to Ultrahelvetic origin.</skos:definition>
	<skos:inScheme rdf:resource="https://dev-lexic.swissgeol.ch/TectonicUnits"/>
	<skos:prefLabel xml:lang="en">Fläscherberg Nappe</skos:prefLabel>
	<skos:prefLabel xml:lang="de">Fläscherberg-Decke</skos:prefLabel>
	<skos:prefLabel xml:lang="fr">Nappe du Fläscherberg</skos:prefLabel>
	<skos:prefLabel xml:lang="it">Falda del Fläscherberg</skos:prefLabel>
	<skos:altLabel xml:lang="de">Südliche Fläscherberg-Schuppe</skos:altLabel>
	<skos:broader rdf:resource="https://dev-lexic.swissgeol.ch/TectonicUnits/UpperHelvetic"/>
	<status xmlns="http://www.w3.org/ns/adms#" rdf:resource="https://dev-lexic.swissgeol.ch/active"/>
</rdf:Description>

<rdf:Description rdf:about="https://dev-lexic.swissgeol.ch/TectonicUnits/PillonMelangeZone">
	<rdf:type rdf:resource="http://www.w3.org/2004/02/skos/core#Concept"/>
	<rdfs:isDefinedBy xml:lang="en">Gouffon Yves (Editor) (2024): Tectonic Map of Switzerland 1:500000, Explanatory notes. Federal Office of Topography swisstopo, Wabern</rdfs:isDefinedBy>
	<skos:definition xml:lang="en">The Pillon Mélange Zone of the Western Swiss Alps consists of a chaotic system of discontinuous slivers with relatively little "wildflysch" matrix. Some of the slivers are several kilometers long and where formerly considered as “Ultrahelvetic nappes”, whose paleogeographic origin is located south of that of the Wildhorn Nappe Complex, i.e., in the most distal part of the European continental shelf.
The mélange zone can be subdivided into lower mélanges, associated with a specific Helvetic nappe, and upper mélanges, related to the base of the Prealps nappes. It is located on top of the Lower and Upper Helvetic nappes and forms a wide band between the Helvetic units and the Penninic units of the Prealps (formerly called the “Zone des Cols”, “Sattelzone” or “Internal Prealps”).</skos:definition>
	<skos:inScheme rdf:resource="https://dev-lexic.swissgeol.ch/TectonicUnits"/>
	<skos:prefLabel xml:lang="en">Pillon Melange Zone</skos:prefLabel>
	<skos:prefLabel xml:lang="de">Pillon-Melangezone</skos:prefLabel>
	<skos:prefLabel xml:lang="fr">Zone de mélange du Pillon</skos:prefLabel>
	<skos:prefLabel xml:lang="it">Zona di mélange del Pillon</skos:prefLabel>
	<skos:altLabel xml:lang="de">Sattelzone</skos:altLabel>
	<skos:altLabel xml:lang="fr">complexe du Pillon</skos:altLabel>
	<skos:altLabel xml:lang="fr">zone des Cols</skos:altLabel>
	<skos:broader rdf:resource="https://dev-lexic.swissgeol.ch/TectonicUnits/UpperHelvetic"/>
	<status xmlns="http://www.w3.org/ns/adms#" rdf:resource="https://dev-lexic.swissgeol.ch/active"/>
</rdf:Description>

<rdf:Description rdf:about="https://dev-lexic.swissgeol.ch/TectonicUnits/BulleMelangeZone">
	<rdf:type rdf:resource="http://www.w3.org/2004/02/skos/core#Concept"/>
	<rdfs:isDefinedBy xml:lang="en">Gouffon Yves (Editor) (2024): Tectonic Map of Switzerland 1:500000, Explanatory notes. Federal Office of Topography swisstopo, Wabern</rdfs:isDefinedBy>
	<skos:definition xml:lang="en">The Bulle Mélange Zone, at the front of the Western Swiss Alps, lies between the Subalpine Molasse and the Prealps nappes (Gurnigel, Voirons or Préalpes Médianes nappes). It comprises the Infraprealpine Mélange (“wildflysch”) in which slivers are embedded. The four bigger slivers, of kilometer scale, have been defined as slices: Bois de Bouleyres and Montsalvens slices near Bulle, Pléiades Slice north of Montreux and Faucigny Slices north of Bonneville in Savoie. The lithologies of these slivers are of similar types to some of the Pillon Mélange Zone.</skos:definition>
	<skos:inScheme rdf:resource="https://dev-lexic.swissgeol.ch/TectonicUnits"/>
	<skos:prefLabel xml:lang="en">Bulle Mélange Zone</skos:prefLabel>
	<skos:prefLabel xml:lang="de">Bulle-Melangezone</skos:prefLabel>
	<skos:prefLabel xml:lang="fr">Zone de mélange de Bulle</skos:prefLabel>
	<skos:prefLabel xml:lang="it">Zona di mélange di Bulle</skos:prefLabel>
	<skos:broader rdf:resource="https://dev-lexic.swissgeol.ch/TectonicUnits/UpperHelvetic"/>
	<skos:narrower rdf:resource="https://dev-lexic.swissgeol.ch/TectonicUnits/InfraprealpineMelange"/>
	<skos:narrower rdf:resource="https://dev-lexic.swissgeol.ch/TectonicUnits/MontsalvensSlice"/>
	<skos:narrower rdf:resource="https://dev-lexic.swissgeol.ch/TectonicUnits/LesPleiadesSlice"/>
	<skos:narrower rdf:resource="https://dev-lexic.swissgeol.ch/TectonicUnits/FaucignySlices"/>
	<skos:narrower rdf:resource="https://dev-lexic.swissgeol.ch/TectonicUnits/BoisDeBouleyresSlice"/>
	<status xmlns="http://www.w3.org/ns/adms#" rdf:resource="https://dev-lexic.swissgeol.ch/active"/>
</rdf:Description>

<rdf:Description rdf:about="https://dev-lexic.swissgeol.ch/TectonicUnits/ExternalEinsiedelnSlices">
	<rdf:type rdf:resource="http://www.w3.org/2004/02/skos/core#Concept"/>
	<rdfs:isDefinedBy xml:lang="en">Gouffon Yves (Editor) (2024): Tectonic Map of Switzerland 1:500000, Explanatory notes. Federal Office of Topography swisstopo, Wabern</rdfs:isDefinedBy>
	<skos:definition xml:lang="en">The External Einsiedeln Slices are Lower Helvetic tectonic slices of the Subalpine Flysch Zone situated between the Vierwaldstättersee and the Walensee with a characteristic sequence of Cretaceous and Paleogene sediments.</skos:definition>
	<skos:inScheme rdf:resource="https://dev-lexic.swissgeol.ch/TectonicUnits"/>
	<skos:prefLabel xml:lang="en">External Einsiedeln Slices</skos:prefLabel>
	<skos:prefLabel xml:lang="de">Externe Einsiedeln-Schuppen</skos:prefLabel>
	<skos:prefLabel xml:lang="fr">Écailles externes d'Einsiedeln</skos:prefLabel>
	<skos:prefLabel xml:lang="it">Scaglie esterne di Einsiedeln</skos:prefLabel>
	<skos:altLabel xml:lang="de">Äussere Einsiedler Schuppenzone</skos:altLabel>
	<skos:broader rdf:resource="https://dev-lexic.swissgeol.ch/TectonicUnits/SubalpineFlyschZone"/>
	<status xmlns="http://www.w3.org/ns/adms#" rdf:resource="https://dev-lexic.swissgeol.ch/active"/>
</rdf:Description>

<rdf:Description rdf:about="https://dev-lexic.swissgeol.ch/TectonicUnits/ExternalBelledonneMassif">
	<rdf:type rdf:resource="http://www.w3.org/2004/02/skos/core#Concept"/>
	<rdfs:isDefinedBy xml:lang="en">Gouffon Yves (Editor) (2024): Tectonic Map of Switzerland 1:500000, Explanatory notes. Federal Office of Topography swisstopo, Wabern</rdfs:isDefinedBy>
	<skos:inScheme rdf:resource="https://dev-lexic.swissgeol.ch/TectonicUnits"/>
	<skos:prefLabel xml:lang="en">External Belledonne Massif</skos:prefLabel>
	<skos:prefLabel xml:lang="de">Externes Belledonne-Massiv</skos:prefLabel>
	<skos:prefLabel xml:lang="fr">Massif de Belledonne externe</skos:prefLabel>
	<skos:prefLabel xml:lang="it">Massiccio di Belledonne esterno</skos:prefLabel>
	<skos:broader rdf:resource="https://dev-lexic.swissgeol.ch/TectonicUnits/BelledonneMassif"/>
	<status xmlns="http://www.w3.org/ns/adms#" rdf:resource="https://dev-lexic.swissgeol.ch/active"/>
</rdf:Description>

<rdf:Description rdf:about="https://dev-lexic.swissgeol.ch/TectonicUnits/MiddleBelledonneMassif">
	<rdf:type rdf:resource="http://www.w3.org/2004/02/skos/core#Concept"/>
	<rdfs:isDefinedBy xml:lang="en">Gouffon Yves (Editor) (2024): Tectonic Map of Switzerland 1:500000, Explanatory notes. Federal Office of Topography swisstopo, Wabern</rdfs:isDefinedBy>
	<skos:inScheme rdf:resource="https://dev-lexic.swissgeol.ch/TectonicUnits"/>
	<skos:prefLabel xml:lang="en">Middle Belledonne Massif</skos:prefLabel>
	<skos:prefLabel xml:lang="de">Mittleres Belledonne-Massiv</skos:prefLabel>
	<skos:prefLabel xml:lang="fr">Massif de Belledonne médian</skos:prefLabel>
	<skos:prefLabel xml:lang="it">Massiccio di Belledonne mediano</skos:prefLabel>
	<skos:broader rdf:resource="https://dev-lexic.swissgeol.ch/TectonicUnits/BelledonneMassif"/>
	<status xmlns="http://www.w3.org/ns/adms#" rdf:resource="https://dev-lexic.swissgeol.ch/active"/>
</rdf:Description>

<rdf:Description rdf:about="https://dev-lexic.swissgeol.ch/TectonicUnits/InternalBelledonneMassif">
	<rdf:type rdf:resource="http://www.w3.org/2004/02/skos/core#Concept"/>
	<rdfs:isDefinedBy xml:lang="en">Gouffon Yves (Editor) (2024): Tectonic Map of Switzerland 1:500000, Explanatory notes. Federal Office of Topography swisstopo, Wabern</rdfs:isDefinedBy>
	<skos:inScheme rdf:resource="https://dev-lexic.swissgeol.ch/TectonicUnits"/>
	<skos:prefLabel xml:lang="en">Internal Belledonne Massif</skos:prefLabel>
	<skos:prefLabel xml:lang="de">Internes Belledonne-Massiv</skos:prefLabel>
	<skos:prefLabel xml:lang="fr">Massif de Belledonne interne</skos:prefLabel>
	<skos:prefLabel xml:lang="it">Massiccio di Belledonne interno</skos:prefLabel>
	<skos:broader rdf:resource="https://dev-lexic.swissgeol.ch/TectonicUnits/BelledonneMassif"/>
	<status xmlns="http://www.w3.org/ns/adms#" rdf:resource="https://dev-lexic.swissgeol.ch/active"/>
</rdf:Description>

<rdf:Description rdf:about="https://dev-lexic.swissgeol.ch/TectonicUnits/ExternalMontBlancMassif">
	<rdf:type rdf:resource="http://www.w3.org/2004/02/skos/core#Concept"/>
	<rdfs:isDefinedBy xml:lang="en">Gouffon Yves (Editor) (2024): Tectonic Map of Switzerland 1:500000, Explanatory notes. Federal Office of Topography swisstopo, Wabern</rdfs:isDefinedBy>
	<skos:definition xml:lang="en">The External Mont Blanc Massif is made up of gneisses and granites and its sedimentary cover lies in its external, reverse limb and forms the main part of the sediments of the «Chamonix Syncline». It is separated from the Internal Mont Blanc Massif by a major fault and is considered to be the root zone of the Morcles Nappe.</skos:definition>
	<skos:inScheme rdf:resource="https://dev-lexic.swissgeol.ch/TectonicUnits"/>
	<skos:prefLabel xml:lang="en">External Mont Blanc Massif</skos:prefLabel>
	<skos:prefLabel xml:lang="de">Externes Mont-Blanc-Massiv</skos:prefLabel>
	<skos:prefLabel xml:lang="fr">Massif du Mont Blanc externe</skos:prefLabel>
	<skos:prefLabel xml:lang="it">Massiccio del Monte Bianco esterno</skos:prefLabel>
	<skos:broader rdf:resource="https://dev-lexic.swissgeol.ch/TectonicUnits/MontBlancMassif"/>
	<skos:related rdf:resource="https://dev-lexic.swissgeol.ch/TectonicUnits/MorclesNappe"/>
	<status xmlns="http://www.w3.org/ns/adms#" rdf:resource="https://dev-lexic.swissgeol.ch/active"/>
</rdf:Description>

<rdf:Description rdf:about="https://dev-lexic.swissgeol.ch/TectonicUnits/InternalMontBlancMassif">
	<rdf:type rdf:resource="http://www.w3.org/2004/02/skos/core#Concept"/>
	<rdfs:isDefinedBy xml:lang="en">Gouffon Yves (Editor) (2024): Tectonic Map of Switzerland 1:500000, Explanatory notes. Federal Office of Topography swisstopo, Wabern</rdfs:isDefinedBy>
	<skos:definition xml:lang="en">The Internal Mont Blanc Massif is characterized by a large Late Carboniferous intrusion (Mont Blanc Granite) and a thin Mesozoic cover occuring on its normal limb. It is separated from the External Mont Blanc Massif by a major fault and is considered to be the substratum of the Ardon Nappe.</skos:definition>
	<skos:inScheme rdf:resource="https://dev-lexic.swissgeol.ch/TectonicUnits"/>
	<skos:prefLabel xml:lang="de">Internes Mont-Blanc-Massiv</skos:prefLabel>
	<skos:prefLabel xml:lang="fr">Massif du Mont Blanc interne</skos:prefLabel>
	<skos:prefLabel xml:lang="it">Massiccio del Monte Bianco interno</skos:prefLabel>
	<skos:prefLabel xml:lang="en">Internal Mont Blanc Massif</skos:prefLabel>
	<skos:broader rdf:resource="https://dev-lexic.swissgeol.ch/TectonicUnits/MontBlancMassif"/>
	<skos:related rdf:resource="https://dev-lexic.swissgeol.ch/TectonicUnits/ArdonNappe"/>
	<status xmlns="http://www.w3.org/ns/adms#" rdf:resource="https://dev-lexic.swissgeol.ch/active"/>
</rdf:Description>

<rdf:Description rdf:about="https://dev-lexic.swissgeol.ch/TectonicUnits/ExternalAarMassif">
	<rdf:type rdf:resource="http://www.w3.org/2004/02/skos/core#Concept"/>
	<rdfs:isDefinedBy xml:lang="en">Gouffon Yves (Editor) (2024): Tectonic Map of Switzerland 1:500000, Explanatory notes. Federal Office of Topography swisstopo, Wabern</rdfs:isDefinedBy>
	<skos:definition xml:lang="en">The External Aar Massif is situated north of the Rote Kuh-Gampel Shear Zone and makes up almost the entire width of the Aar Massif in its central part. North of the Lötschental, it overthrusts the Gastern Submassif with a contact marked by a thin band of Triassic and Jurassic sediments («Jungfrau Wedge»), which includes overturned sediments of the External Aar Massif. Several large-scale structures follow the general strike of the External Aar Massif. They include longitudinal faults and very tight synclines exposing Late Paleozoic and Mesozoic sediments.</skos:definition>
	<skos:inScheme rdf:resource="https://dev-lexic.swissgeol.ch/TectonicUnits"/>
	<skos:prefLabel xml:lang="en">External Aar Massif</skos:prefLabel>
	<skos:prefLabel xml:lang="de">Externes Aar-Massiv</skos:prefLabel>
	<skos:prefLabel xml:lang="fr">Massif de l'Aar externe</skos:prefLabel>
	<skos:prefLabel xml:lang="it">Massiccio dell'Aare esterno</skos:prefLabel>
	<skos:broader rdf:resource="https://dev-lexic.swissgeol.ch/TectonicUnits/AarMassif"/>
	<status xmlns="http://www.w3.org/ns/adms#" rdf:resource="https://dev-lexic.swissgeol.ch/active"/>
</rdf:Description>

<rdf:Description rdf:about="https://dev-lexic.swissgeol.ch/TectonicUnits/GasternSubmassif">
	<rdf:type rdf:resource="http://www.w3.org/2004/02/skos/core#Concept"/>
	<rdfs:isDefinedBy xml:lang="en">Gouffon Yves (Editor) (2024): Tectonic Map of Switzerland 1:500000, Explanatory notes. Federal Office of Topography swisstopo, Wabern</rdfs:isDefinedBy>
	<skos:definition xml:lang="en">The Gastern Submassif is overthrust by the External Aar Massif north of the Lötschental.</skos:definition>
	<skos:inScheme rdf:resource="https://dev-lexic.swissgeol.ch/TectonicUnits"/>
	<skos:prefLabel xml:lang="en">Gastern Submassif</skos:prefLabel>
	<skos:prefLabel xml:lang="de">Gastern-Teilmassiv</skos:prefLabel>
	<skos:prefLabel xml:lang="fr">Submassif de Gastern</skos:prefLabel>
	<skos:prefLabel xml:lang="it">Submassiccio di Gastern</skos:prefLabel>
	<skos:broader rdf:resource="https://dev-lexic.swissgeol.ch/TectonicUnits/AarMassif"/>
	<status xmlns="http://www.w3.org/ns/adms#" rdf:resource="https://dev-lexic.swissgeol.ch/active"/>
</rdf:Description>

<rdf:Description rdf:about="https://dev-lexic.swissgeol.ch/TectonicUnits/Baldschieder-GletschSubmassif">
	<rdf:type rdf:resource="http://www.w3.org/2004/02/skos/core#Concept"/>
	<rdfs:isDefinedBy xml:lang="en">Gouffon Yves (Editor) (2024): Tectonic Map of Switzerland 1:500000, Explanatory notes. Federal Office of Topography swisstopo, Wabern</rdfs:isDefinedBy>
	<skos:definition xml:lang="en">The Baltschieder-Gletsch Submassif represents the Internal Aar Massif in Valais. It crops out in upper Valais region, south of the Rote Kuh-Gampel Shear Zone – a reactivated paleofault – and its possible continuation between Aletsch and Rhône glaciers. The autochthonous cover of the Baldschieder-Gletsch Submassif is present at its southwestern end the near Raron.</skos:definition>
	<skos:inScheme rdf:resource="https://dev-lexic.swissgeol.ch/TectonicUnits"/>
	<skos:prefLabel xml:lang="en">Baldschieder-Gletsch Submassif</skos:prefLabel>
	<skos:prefLabel xml:lang="de">Baldschieder-Gletsch-Teilmassiv</skos:prefLabel>
	<skos:prefLabel xml:lang="fr">Submassif de Baldschieder-Gletsch</skos:prefLabel>
	<skos:prefLabel xml:lang="it">Submassiccio di Baldschieder-Gletsch</skos:prefLabel>
	<skos:broader rdf:resource="https://dev-lexic.swissgeol.ch/TectonicUnits/InternalAarMassif"/>
	<status xmlns="http://www.w3.org/ns/adms#" rdf:resource="https://dev-lexic.swissgeol.ch/active"/>
</rdf:Description>

<rdf:Description rdf:about="https://dev-lexic.swissgeol.ch/TectonicUnits/Trun-PuntegliasSubmassif">
	<rdf:type rdf:resource="http://www.w3.org/2004/02/skos/core#Concept"/>
	<rdfs:isDefinedBy xml:lang="en">Gouffon Yves (Editor) (2024): Tectonic Map of Switzerland 1:500000, Explanatory notes. Federal Office of Topography swisstopo, Wabern</rdfs:isDefinedBy>
	<skos:definition xml:lang="en">The Trun-Punteglias Submassif represents the Internal Aar Massif in the Surselva (Graubünden), with an autochthonous cover only comprising Triassic sediments.</skos:definition>
	<skos:inScheme rdf:resource="https://dev-lexic.swissgeol.ch/TectonicUnits"/>
	<skos:prefLabel xml:lang="en">Trun-Punteglias Submassif</skos:prefLabel>
	<skos:prefLabel xml:lang="de">Trun-Punteglias-Teilmassiv</skos:prefLabel>
	<skos:prefLabel xml:lang="fr">Submassif de Trun-Punteglias</skos:prefLabel>
	<skos:prefLabel xml:lang="it">Submassiccio di Trun-Punteglias</skos:prefLabel>
	<skos:broader rdf:resource="https://dev-lexic.swissgeol.ch/TectonicUnits/InternalAarMassif"/>
	<status xmlns="http://www.w3.org/ns/adms#" rdf:resource="https://dev-lexic.swissgeol.ch/active"/>
</rdf:Description>

<rdf:Description rdf:about="https://dev-lexic.swissgeol.ch/TectonicUnits/KaminspitzSlice">
	<rdf:type rdf:resource="http://www.w3.org/2004/02/skos/core#Concept"/>
	<rdfs:isDefinedBy xml:lang="en">Gouffon Yves (Editor) (2024): Tectonic Map of Switzerland 1:500000, Explanatory notes. Federal Office of Topography swisstopo, Wabern</rdfs:isDefinedBy>
	<skos:definition xml:lang="en">The Kaminspitz Slice is the lowest post-nappe tectonic slice (due to a late out-of-sequence thrusting) of the parautochthonous cover of the northeastern end of the Aar Massif.</skos:definition>
	<skos:inScheme rdf:resource="https://dev-lexic.swissgeol.ch/TectonicUnits"/>
	<skos:prefLabel xml:lang="en">Kaminspitz Slice</skos:prefLabel>
	<skos:prefLabel xml:lang="de">Kaminspitz-Schuppe</skos:prefLabel>
	<skos:prefLabel xml:lang="fr">Écaille du Kaminspitz</skos:prefLabel>
	<skos:prefLabel xml:lang="it">Scaglia del Kaminspitz</skos:prefLabel>
	<skos:broader rdf:resource="https://dev-lexic.swissgeol.ch/TectonicUnits/AarMassif"/>
	<status xmlns="http://www.w3.org/ns/adms#" rdf:resource="https://dev-lexic.swissgeol.ch/active"/>
</rdf:Description>

<rdf:Description rdf:about="https://dev-lexic.swissgeol.ch/TectonicUnits/StelliSlice">
	<rdf:type rdf:resource="http://www.w3.org/2004/02/skos/core#Concept"/>
	<rdfs:isDefinedBy xml:lang="en">Gouffon Yves (Editor) (2024): Tectonic Map of Switzerland 1:500000, Explanatory notes. Federal Office of Topography swisstopo, Wabern</rdfs:isDefinedBy>
	<skos:definition xml:lang="en">The Stelli Slice is a post-nappe tectonic slice (due to a late out-of-sequence thrusting) of the parautochthonous cover of the northeastern end of the Aar Massif.</skos:definition>
	<skos:inScheme rdf:resource="https://dev-lexic.swissgeol.ch/TectonicUnits"/>
	<skos:prefLabel xml:lang="en">Stelli Slice</skos:prefLabel>
	<skos:prefLabel xml:lang="de">Stelli-Schuppe</skos:prefLabel>
	<skos:prefLabel xml:lang="fr">Écaille du Stelli</skos:prefLabel>
	<skos:prefLabel xml:lang="it">Scaglia dello Stelli</skos:prefLabel>
	<skos:broader rdf:resource="https://dev-lexic.swissgeol.ch/TectonicUnits/AarMassif"/>
	<status xmlns="http://www.w3.org/ns/adms#" rdf:resource="https://dev-lexic.swissgeol.ch/active"/>
</rdf:Description>

<rdf:Description rdf:about="https://dev-lexic.swissgeol.ch/TectonicUnits/TschepSlice">
	<rdf:type rdf:resource="http://www.w3.org/2004/02/skos/core#Concept"/>
	<rdfs:isDefinedBy xml:lang="en">Gouffon Yves (Editor) (2024): Tectonic Map of Switzerland 1:500000, Explanatory notes. Federal Office of Topography swisstopo, Wabern</rdfs:isDefinedBy>
	<skos:definition xml:lang="en">The Tschep Slice is the highest post-nappe tectonic slice (due to a late out-of-sequence thrusting) of the parautochthonous cover of the northeastern end of the Aar Massif. It comprises an upright stratigraphy reaching from Middle Jurassic to Early Cretaceous.</skos:definition>
	<skos:inScheme rdf:resource="https://dev-lexic.swissgeol.ch/TectonicUnits"/>
	<skos:prefLabel xml:lang="en">Tschep Slice</skos:prefLabel>
	<skos:prefLabel xml:lang="de">Tschep-Schuppe</skos:prefLabel>
	<skos:prefLabel xml:lang="fr">Écaille du Tschep</skos:prefLabel>
	<skos:prefLabel xml:lang="it">Scaglia del Tschep</skos:prefLabel>
	<skos:broader rdf:resource="https://dev-lexic.swissgeol.ch/TectonicUnits/AarMassif"/>
	<status xmlns="http://www.w3.org/ns/adms#" rdf:resource="https://dev-lexic.swissgeol.ch/active"/>
</rdf:Description>

<rdf:Description rdf:about="https://dev-lexic.swissgeol.ch/TectonicUnits/HochFulenSlice">
	<rdf:type rdf:resource="http://www.w3.org/2004/02/skos/core#Concept"/>
	<rdfs:isDefinedBy xml:lang="en">Gouffon Yves (Editor) (2024): Tectonic Map of Switzerland 1:500000, Explanatory notes. Federal Office of Topography swisstopo, Wabern</rdfs:isDefinedBy>
	<skos:definition xml:lang="en">The Hoch Fulen Slice is a Lower Helvetic parautochthonous tectonic slice made up of Late Jurassic to Paleogene series. It lies on top of the Paleogene series of the Aar Massif between Erstfeld (Reuss Valley) and the Klausenpass.</skos:definition>
	<skos:inScheme rdf:resource="https://dev-lexic.swissgeol.ch/TectonicUnits"/>
	<skos:prefLabel xml:lang="en">Hoch Fulen Slice</skos:prefLabel>
	<skos:prefLabel xml:lang="de">Hoch-Fulen-Schuppe</skos:prefLabel>
	<skos:prefLabel xml:lang="fr">Écaille du Hoch-Fulen</skos:prefLabel>
	<skos:prefLabel xml:lang="it">Scaglia del Hoch Fulen</skos:prefLabel>
	<skos:broader rdf:resource="https://dev-lexic.swissgeol.ch/TectonicUnits/AarMassif"/>
	<status xmlns="http://www.w3.org/ns/adms#" rdf:resource="https://dev-lexic.swissgeol.ch/active"/>
</rdf:Description>

<rdf:Description rdf:about="https://dev-lexic.swissgeol.ch/TectonicUnits/OrglenSlices_PartAarMassif">
	<rdf:type rdf:resource="http://www.w3.org/2004/02/skos/core#Concept"/>
	<rdfs:isDefinedBy xml:lang="en">Gouffon Yves (Editor) (2024): Tectonic Map of Switzerland 1:500000, Explanatory notes. Federal Office of Topography swisstopo, Wabern</rdfs:isDefinedBy>
	<skos:definition xml:lang="en">The Orglen Slices are post-nappe tectonic units (due to a late out-of-sequence thrusting) of the parautochthonous cover of the northeastern end of the Aar Massif.</skos:definition>
	<skos:inScheme rdf:resource="https://dev-lexic.swissgeol.ch/TectonicUnits"/>
	<skos:prefLabel xml:lang="en">Orglen Slices (part Aar Massif)</skos:prefLabel>
	<skos:prefLabel xml:lang="de">Orglen-Schuppen (Aar-Massiv-Anteil)</skos:prefLabel>
	<skos:prefLabel xml:lang="fr">Écailles de l'Orglen (partie Massif de l'Aar)</skos:prefLabel>
	<skos:prefLabel xml:lang="it">Scaglie dell'Orglen (parte Massiccio dell'Aare)</skos:prefLabel>
	<skos:broader rdf:resource="https://dev-lexic.swissgeol.ch/TectonicUnits/AarMassif"/>
	<skos:broader rdf:resource="https://dev-lexic.swissgeol.ch/TectonicUnits/OrglenSlices"/>
	<status xmlns="http://www.w3.org/ns/adms#" rdf:resource="https://dev-lexic.swissgeol.ch/active"/>
</rdf:Description>

<rdf:Description rdf:about="https://dev-lexic.swissgeol.ch/TectonicUnits/CalandaSlice_PartAarMassif">
	<rdf:type rdf:resource="http://www.w3.org/2004/02/skos/core#Concept"/>
	<rdfs:isDefinedBy xml:lang="en">Gouffon Yves (Editor) (2024): Tectonic Map of Switzerland 1:500000, Explanatory notes. Federal Office of Topography swisstopo, Wabern</rdfs:isDefinedBy>
	<skos:definition xml:lang="en">The Calanda Slice is a post-nappe tectonic slice (due to a late out-of-sequence thrusting) of the parautochthonous cover of the northeastern end of the Aar Massif.</skos:definition>
	<skos:inScheme rdf:resource="https://dev-lexic.swissgeol.ch/TectonicUnits"/>
	<skos:prefLabel xml:lang="en">Calanda Slice (part Aar Massif)</skos:prefLabel>
	<skos:prefLabel xml:lang="de">Calanda-Schuppe (Aar-Massiv-Anteil)</skos:prefLabel>
	<skos:prefLabel xml:lang="fr">Écaille du Calanda (partie Massif de l'Aar)</skos:prefLabel>
	<skos:prefLabel xml:lang="it">Scaglia del Calanda (parte Massiccio dell'Aare)</skos:prefLabel>
	<skos:broader rdf:resource="https://dev-lexic.swissgeol.ch/TectonicUnits/AarMassif"/>
	<skos:broader rdf:resource="https://dev-lexic.swissgeol.ch/TectonicUnits/CalandaSlice"/>
	<status xmlns="http://www.w3.org/ns/adms#" rdf:resource="https://dev-lexic.swissgeol.ch/active"/>
</rdf:Description>

<rdf:Description rdf:about="https://dev-lexic.swissgeol.ch/TectonicUnits/MiruttaSlice_PartAarMassif">
	<rdf:type rdf:resource="http://www.w3.org/2004/02/skos/core#Concept"/>
	<rdfs:isDefinedBy xml:lang="en">Gouffon Yves (Editor) (2024): Tectonic Map of Switzerland 1:500000, Explanatory notes. Federal Office of Topography swisstopo, Wabern</rdfs:isDefinedBy>
	<skos:definition xml:lang="en">The Mirutta Slices are post-nappe tectonic units (due to a late out-of-sequence thrusting) of the parautochthonous cover of the northeastern end of the Aar Massif.</skos:definition>
	<skos:inScheme rdf:resource="https://dev-lexic.swissgeol.ch/TectonicUnits"/>
	<skos:prefLabel xml:lang="en">Mirutta Slice (part Aar Massif)</skos:prefLabel>
	<skos:prefLabel xml:lang="de">Mirutta-Schuppe (Aar-Massiv-Anteil)</skos:prefLabel>
	<skos:prefLabel xml:lang="fr">Écaille du Mirutta (partie Massif de l'Aar)</skos:prefLabel>
	<skos:prefLabel xml:lang="it">Scaglia del Mirutta (parte Massiccio dell'Aare)</skos:prefLabel>
	<skos:broader rdf:resource="https://dev-lexic.swissgeol.ch/TectonicUnits/AarMassif"/>
	<skos:broader rdf:resource="https://dev-lexic.swissgeol.ch/TectonicUnits/MiruttaSlice"/>
	<status xmlns="http://www.w3.org/ns/adms#" rdf:resource="https://dev-lexic.swissgeol.ch/active"/>
</rdf:Description>

<rdf:Description rdf:about="https://dev-lexic.swissgeol.ch/TectonicUnits/PizDartgasSlice">
	<rdf:type rdf:resource="http://www.w3.org/2004/02/skos/core#Concept"/>
	<rdfs:isDefinedBy xml:lang="en">Gouffon Yves (Editor) (2024): Tectonic Map of Switzerland 1:500000, Explanatory notes. Federal Office of Topography swisstopo, Wabern</rdfs:isDefinedBy>
	<skos:definition xml:lang="en">The Piz d'Artgas Slice is a small tectonic unit of the southern rim of the Aar Massif in Surselva. It comprises dolomite of the Röti Formation, Dogger and limestone of the Quinten Formation.</skos:definition>
	<skos:inScheme rdf:resource="https://dev-lexic.swissgeol.ch/TectonicUnits"/>
	<skos:prefLabel xml:lang="en">Piz d'Artgas Slice</skos:prefLabel>
	<skos:prefLabel xml:lang="de">Piz-d'Artgas-Schuppe</skos:prefLabel>
	<skos:prefLabel xml:lang="fr">Écaille du Piz-d'Artgas</skos:prefLabel>
	<skos:prefLabel xml:lang="it">Scaglia del Piz d'Artgas</skos:prefLabel>
	<skos:broader rdf:resource="https://dev-lexic.swissgeol.ch/TectonicUnits/AarMassif"/>
	<status xmlns="http://www.w3.org/ns/adms#" rdf:resource="https://dev-lexic.swissgeol.ch/active"/>
</rdf:Description>

<rdf:Description rdf:about="https://dev-lexic.swissgeol.ch/TectonicUnits/KlausenpassSlices">
	<rdf:type rdf:resource="http://www.w3.org/2004/02/skos/core#Concept"/>
	<rdfs:isDefinedBy xml:lang="en">Gouffon Yves (Editor) (2024): Tectonic Map of Switzerland 1:500000, Explanatory notes. Federal Office of Topography swisstopo, Wabern</rdfs:isDefinedBy>
	<skos:inScheme rdf:resource="https://dev-lexic.swissgeol.ch/TectonicUnits"/>
	<skos:prefLabel xml:lang="en">Klausenpass Slices</skos:prefLabel>
	<skos:prefLabel xml:lang="de">Klausenpass-Schuppen</skos:prefLabel>
	<skos:prefLabel xml:lang="fr">Écailles du Col du Klausen</skos:prefLabel>
	<skos:prefLabel xml:lang="it">Scaglie del Klausenpass</skos:prefLabel>
	<skos:broader rdf:resource="https://dev-lexic.swissgeol.ch/TectonicUnits/ClaridenSliceComplex"/>
	<status xmlns="http://www.w3.org/ns/adms#" rdf:resource="https://dev-lexic.swissgeol.ch/active"/>
</rdf:Description>

<rdf:Description rdf:about="https://dev-lexic.swissgeol.ch/TectonicUnits/ChamerstockSlice">
	<rdf:type rdf:resource="http://www.w3.org/2004/02/skos/core#Concept"/>
	<rdfs:isDefinedBy xml:lang="en">Gouffon Yves (Editor) (2024): Tectonic Map of Switzerland 1:500000, Explanatory notes. Federal Office of Topography swisstopo, Wabern</rdfs:isDefinedBy>
	<skos:inScheme rdf:resource="https://dev-lexic.swissgeol.ch/TectonicUnits"/>
	<skos:prefLabel xml:lang="en">Chamerstock Slice</skos:prefLabel>
	<skos:prefLabel xml:lang="de">Chamerstock-Schuppe</skos:prefLabel>
	<skos:prefLabel xml:lang="fr">Écaille du Chamerstock</skos:prefLabel>
	<skos:prefLabel xml:lang="it">Scaglia del Chamerstock</skos:prefLabel>
	<skos:broader rdf:resource="https://dev-lexic.swissgeol.ch/TectonicUnits/ClaridenSliceComplex"/>
	<status xmlns="http://www.w3.org/ns/adms#" rdf:resource="https://dev-lexic.swissgeol.ch/active"/>
</rdf:Description>

<rdf:Description rdf:about="https://dev-lexic.swissgeol.ch/TectonicUnits/GeisstrittSlice">
	<rdf:type rdf:resource="http://www.w3.org/2004/02/skos/core#Concept"/>
	<rdfs:isDefinedBy xml:lang="en">Gouffon Yves (Editor) (2024): Tectonic Map of Switzerland 1:500000, Explanatory notes. Federal Office of Topography swisstopo, Wabern</rdfs:isDefinedBy>
	<skos:inScheme rdf:resource="https://dev-lexic.swissgeol.ch/TectonicUnits"/>
	<skos:prefLabel xml:lang="en">Geisstritt Slice</skos:prefLabel>
	<skos:prefLabel xml:lang="de">Geisstritt-Schuppe</skos:prefLabel>
	<skos:prefLabel xml:lang="fr">Écaille du Geisstritt</skos:prefLabel>
	<skos:prefLabel xml:lang="it">Scaglia del Geisstritt</skos:prefLabel>
	<skos:broader rdf:resource="https://dev-lexic.swissgeol.ch/TectonicUnits/ClaridenSliceComplex"/>
	<status xmlns="http://www.w3.org/ns/adms#" rdf:resource="https://dev-lexic.swissgeol.ch/active"/>
</rdf:Description>

<rdf:Description rdf:about="https://dev-lexic.swissgeol.ch/TectonicUnits/StichplattenSlice">
	<rdf:type rdf:resource="http://www.w3.org/2004/02/skos/core#Concept"/>
	<rdfs:isDefinedBy xml:lang="en">Gouffon Yves (Editor) (2024): Tectonic Map of Switzerland 1:500000, Explanatory notes. Federal Office of Topography swisstopo, Wabern</rdfs:isDefinedBy>
	<skos:inScheme rdf:resource="https://dev-lexic.swissgeol.ch/TectonicUnits"/>
	<skos:prefLabel xml:lang="en">Stichplatten Slice</skos:prefLabel>
	<skos:prefLabel xml:lang="de">Stichplatten-Schuppe</skos:prefLabel>
	<skos:prefLabel xml:lang="fr">Écaille de Stichplatten</skos:prefLabel>
	<skos:prefLabel xml:lang="it">Scaglia di Stichplatten</skos:prefLabel>
	<skos:broader rdf:resource="https://dev-lexic.swissgeol.ch/TectonicUnits/ClaridenSliceComplex"/>
	<status xmlns="http://www.w3.org/ns/adms#" rdf:resource="https://dev-lexic.swissgeol.ch/active"/>
</rdf:Description>

<rdf:Description rdf:about="https://dev-lexic.swissgeol.ch/TectonicUnits/GemsfairenSlice">
	<rdf:type rdf:resource="http://www.w3.org/2004/02/skos/core#Concept"/>
	<rdfs:isDefinedBy xml:lang="en">Gouffon Yves (Editor) (2024): Tectonic Map of Switzerland 1:500000, Explanatory notes. Federal Office of Topography swisstopo, Wabern</rdfs:isDefinedBy>
	<skos:inScheme rdf:resource="https://dev-lexic.swissgeol.ch/TectonicUnits"/>
	<skos:prefLabel xml:lang="en">Gemsfairen Slice</skos:prefLabel>
	<skos:prefLabel xml:lang="de">Gemsfairen-Schuppe</skos:prefLabel>
	<skos:prefLabel xml:lang="fr">Écaille du Gemsfairen</skos:prefLabel>
	<skos:prefLabel xml:lang="it">Scaglia del Gemsfairen</skos:prefLabel>
	<skos:broader rdf:resource="https://dev-lexic.swissgeol.ch/TectonicUnits/ClaridenSliceComplex"/>
	<status xmlns="http://www.w3.org/ns/adms#" rdf:resource="https://dev-lexic.swissgeol.ch/active"/>
</rdf:Description>

<rdf:Description rdf:about="https://dev-lexic.swissgeol.ch/TectonicUnits/RotstockSlice">
	<rdf:type rdf:resource="http://www.w3.org/2004/02/skos/core#Concept"/>
	<rdfs:isDefinedBy xml:lang="en">Gouffon Yves (Editor) (2024): Tectonic Map of Switzerland 1:500000, Explanatory notes. Federal Office of Topography swisstopo, Wabern</rdfs:isDefinedBy>
	<skos:inScheme rdf:resource="https://dev-lexic.swissgeol.ch/TectonicUnits"/>
	<skos:prefLabel xml:lang="en">Rotstock Slice</skos:prefLabel>
	<skos:prefLabel xml:lang="de">Rotstock-Schuppe</skos:prefLabel>
	<skos:prefLabel xml:lang="fr">Écaille du Rotstock</skos:prefLabel>
	<skos:prefLabel xml:lang="it">Scaglia del Rotstock</skos:prefLabel>
	<skos:broader rdf:resource="https://dev-lexic.swissgeol.ch/TectonicUnits/ClaridenSliceComplex"/>
	<status xmlns="http://www.w3.org/ns/adms#" rdf:resource="https://dev-lexic.swissgeol.ch/active"/>
</rdf:Description>

<rdf:Description rdf:about="https://dev-lexic.swissgeol.ch/TectonicUnits/LangfirnSlice">
	<rdf:type rdf:resource="http://www.w3.org/2004/02/skos/core#Concept"/>
	<rdfs:isDefinedBy xml:lang="en">Gouffon Yves (Editor) (2024): Tectonic Map of Switzerland 1:500000, Explanatory notes. Federal Office of Topography swisstopo, Wabern</rdfs:isDefinedBy>
	<skos:inScheme rdf:resource="https://dev-lexic.swissgeol.ch/TectonicUnits"/>
	<skos:prefLabel xml:lang="en">Langfirn Slice</skos:prefLabel>
	<skos:prefLabel xml:lang="de">Langfirn-Schuppe</skos:prefLabel>
	<skos:prefLabel xml:lang="fr">Écaille du Langfirn</skos:prefLabel>
	<skos:prefLabel xml:lang="it">Scaglia del Langfirn</skos:prefLabel>
	<skos:broader rdf:resource="https://dev-lexic.swissgeol.ch/TectonicUnits/ClaridenSliceComplex"/>
	<status xmlns="http://www.w3.org/ns/adms#" rdf:resource="https://dev-lexic.swissgeol.ch/active"/>
</rdf:Description>

<rdf:Description rdf:about="https://dev-lexic.swissgeol.ch/TectonicUnits/ChropfsbergSlice">
	<rdf:type rdf:resource="http://www.w3.org/2004/02/skos/core#Concept"/>
	<rdfs:isDefinedBy xml:lang="en">Gouffon Yves (Editor) (2024): Tectonic Map of Switzerland 1:500000, Explanatory notes. Federal Office of Topography swisstopo, Wabern</rdfs:isDefinedBy>
	<skos:inScheme rdf:resource="https://dev-lexic.swissgeol.ch/TectonicUnits"/>
	<skos:prefLabel xml:lang="en">Chropfsberg Slice</skos:prefLabel>
	<skos:prefLabel xml:lang="de">Chropfsberg-Schuppe</skos:prefLabel>
	<skos:prefLabel xml:lang="fr">Écaille de Chropfsberg</skos:prefLabel>
	<skos:prefLabel xml:lang="it">Scaglia di Chropfsberg</skos:prefLabel>
	<skos:broader rdf:resource="https://dev-lexic.swissgeol.ch/TectonicUnits/Chropfsberg-PizalunSlices"/>
	<status xmlns="http://www.w3.org/ns/adms#" rdf:resource="https://dev-lexic.swissgeol.ch/active"/>
</rdf:Description>

<rdf:Description rdf:about="https://dev-lexic.swissgeol.ch/TectonicUnits/PizalunSlice">
	<rdf:type rdf:resource="http://www.w3.org/2004/02/skos/core#Concept"/>
	<rdfs:isDefinedBy xml:lang="en">Gouffon Yves (Editor) (2024): Tectonic Map of Switzerland 1:500000, Explanatory notes. Federal Office of Topography swisstopo, Wabern</rdfs:isDefinedBy>
	<skos:inScheme rdf:resource="https://dev-lexic.swissgeol.ch/TectonicUnits"/>
	<skos:prefLabel xml:lang="en">Pizalun Slice</skos:prefLabel>
	<skos:prefLabel xml:lang="de">Pizalun-Schuppe</skos:prefLabel>
	<skos:prefLabel xml:lang="fr">Écaille du Pizalun</skos:prefLabel>
	<skos:prefLabel xml:lang="it">Scaglia del Pizalun</skos:prefLabel>
	<skos:broader rdf:resource="https://dev-lexic.swissgeol.ch/TectonicUnits/Chropfsberg-PizalunSlices"/>
	<status xmlns="http://www.w3.org/ns/adms#" rdf:resource="https://dev-lexic.swissgeol.ch/active"/>
</rdf:Description>

<rdf:Description rdf:about="https://dev-lexic.swissgeol.ch/TectonicUnits/GaffiaSlice">
	<rdf:type rdf:resource="http://www.w3.org/2004/02/skos/core#Concept"/>
	<rdfs:isDefinedBy xml:lang="en">Gouffon Yves (Editor) (2024): Tectonic Map of Switzerland 1:500000, Explanatory notes. Federal Office of Topography swisstopo, Wabern</rdfs:isDefinedBy>
	<skos:inScheme rdf:resource="https://dev-lexic.swissgeol.ch/TectonicUnits"/>
	<skos:prefLabel xml:lang="en">Gaffia Slice</skos:prefLabel>
	<skos:prefLabel xml:lang="de">Gaffia-Schuppe</skos:prefLabel>
	<skos:prefLabel xml:lang="fr">Écaille de Gaffia</skos:prefLabel>
	<skos:prefLabel xml:lang="it">Scaglia di Gaffia</skos:prefLabel>
	<skos:broader rdf:resource="https://dev-lexic.swissgeol.ch/TectonicUnits/Chropfsberg-PizalunSlices"/>
	<status xmlns="http://www.w3.org/ns/adms#" rdf:resource="https://dev-lexic.swissgeol.ch/active"/>
</rdf:Description>

<rdf:Description rdf:about="https://dev-lexic.swissgeol.ch/TectonicUnits/LogsbachSlice">
	<rdf:type rdf:resource="http://www.w3.org/2004/02/skos/core#Concept"/>
	<rdfs:isDefinedBy xml:lang="en">Gouffon Yves (Editor) (2024): Tectonic Map of Switzerland 1:500000, Explanatory notes. Federal Office of Topography swisstopo, Wabern</rdfs:isDefinedBy>
	<skos:inScheme rdf:resource="https://dev-lexic.swissgeol.ch/TectonicUnits"/>
	<skos:prefLabel xml:lang="en">Logsbach Slice</skos:prefLabel>
	<skos:prefLabel xml:lang="de">Logsbach-Schuppe</skos:prefLabel>
	<skos:prefLabel xml:lang="fr">Écaille du Logsbach</skos:prefLabel>
	<skos:prefLabel xml:lang="it">Scaglia del Logsbach</skos:prefLabel>
	<skos:broader rdf:resource="https://dev-lexic.swissgeol.ch/TectonicUnits/Chropfsberg-PizalunSlices"/>
	<status xmlns="http://www.w3.org/ns/adms#" rdf:resource="https://dev-lexic.swissgeol.ch/active"/>
</rdf:Description>

<rdf:Description rdf:about="https://dev-lexic.swissgeol.ch/TectonicUnits/MarchegghornSlice_PartBlattengrat">
	<rdf:type rdf:resource="http://www.w3.org/2004/02/skos/core#Concept"/>
	<rdfs:isDefinedBy xml:lang="en">Gouffon Yves (Editor) (2024): Tectonic Map of Switzerland 1:500000, Explanatory notes. Federal Office of Topography swisstopo, Wabern</rdfs:isDefinedBy>
	<skos:inScheme rdf:resource="https://dev-lexic.swissgeol.ch/TectonicUnits"/>
	<skos:prefLabel xml:lang="en">Marchegghorn Slice (part Blattengrat)</skos:prefLabel>
	<skos:prefLabel xml:lang="de">Marchegghorn-Schuppe (Blattengrat-Anteil)</skos:prefLabel>
	<skos:prefLabel xml:lang="fr">Écaille du Marchegghorn (partie Blattengrat)</skos:prefLabel>
	<skos:prefLabel xml:lang="it">Scaglia del Marchegghorn (parte Blattengrat)</skos:prefLabel>
	<skos:broader rdf:resource="https://dev-lexic.swissgeol.ch/TectonicUnits/BlattengratNappe"/>
	<skos:broader rdf:resource="https://dev-lexic.swissgeol.ch/TectonicUnits/MarchegghornSlice"/>
	<status xmlns="http://www.w3.org/ns/adms#" rdf:resource="https://dev-lexic.swissgeol.ch/active"/>
</rdf:Description>

<rdf:Description rdf:about="https://dev-lexic.swissgeol.ch/TectonicUnits/CalandaSlice_PartBlattengrat">
	<rdf:type rdf:resource="http://www.w3.org/2004/02/skos/core#Concept"/>
	<rdfs:isDefinedBy xml:lang="en">Gouffon Yves (Editor) (2024): Tectonic Map of Switzerland 1:500000, Explanatory notes. Federal Office of Topography swisstopo, Wabern</rdfs:isDefinedBy>
	<skos:inScheme rdf:resource="https://dev-lexic.swissgeol.ch/TectonicUnits"/>
	<skos:prefLabel xml:lang="en">Calanda Slice (part Blattengrat)</skos:prefLabel>
	<skos:prefLabel xml:lang="de">Calanda-Schuppe (Blattengrat-Anteil)</skos:prefLabel>
	<skos:prefLabel xml:lang="fr">Écaille du Calanda (partie Blattengrat)</skos:prefLabel>
	<skos:prefLabel xml:lang="it">Scaglia del Calanda (parte Blattengrat)</skos:prefLabel>
	<skos:broader rdf:resource="https://dev-lexic.swissgeol.ch/TectonicUnits/BlattengratNappe"/>
	<skos:broader rdf:resource="https://dev-lexic.swissgeol.ch/TectonicUnits/CalandaSlice"/>
	<status xmlns="http://www.w3.org/ns/adms#" rdf:resource="https://dev-lexic.swissgeol.ch/active"/>
</rdf:Description>

<rdf:Description rdf:about="https://dev-lexic.swissgeol.ch/TectonicUnits/MiruttaSlice_PartBlattengrat">
	<rdf:type rdf:resource="http://www.w3.org/2004/02/skos/core#Concept"/>
	<rdfs:isDefinedBy xml:lang="en">Gouffon Yves (Editor) (2024): Tectonic Map of Switzerland 1:500000, Explanatory notes. Federal Office of Topography swisstopo, Wabern</rdfs:isDefinedBy>
	<skos:inScheme rdf:resource="https://dev-lexic.swissgeol.ch/TectonicUnits"/>
	<skos:prefLabel xml:lang="en">Mirutta Slice (part Blattengrat)</skos:prefLabel>
	<skos:prefLabel xml:lang="de">Mirutta-Schuppe (Blattengrat-Anteil)</skos:prefLabel>
	<skos:prefLabel xml:lang="fr">Écaille du Mirutta (partie Blattengrat)</skos:prefLabel>
	<skos:prefLabel xml:lang="it">Scaglia del Mirutta (parte Blattengrat)</skos:prefLabel>
	<skos:broader rdf:resource="https://dev-lexic.swissgeol.ch/TectonicUnits/BlattengratNappe"/>
	<skos:broader rdf:resource="https://dev-lexic.swissgeol.ch/TectonicUnits/MiruttaSlice"/>
	<status xmlns="http://www.w3.org/ns/adms#" rdf:resource="https://dev-lexic.swissgeol.ch/active"/>
</rdf:Description>

<rdf:Description rdf:about="https://dev-lexic.swissgeol.ch/TectonicUnits/MarchegghornSlice_PartSardona">
	<rdf:type rdf:resource="http://www.w3.org/2004/02/skos/core#Concept"/>
	<rdfs:isDefinedBy xml:lang="en">Gouffon Yves (Editor) (2024): Tectonic Map of Switzerland 1:500000, Explanatory notes. Federal Office of Topography swisstopo, Wabern</rdfs:isDefinedBy>
	<skos:inScheme rdf:resource="https://dev-lexic.swissgeol.ch/TectonicUnits"/>
	<skos:prefLabel xml:lang="en">Marchegghorn Slice (part Sardona)</skos:prefLabel>
	<skos:prefLabel xml:lang="de">Marchegghorn-Schuppe (Sardona-Anteil)</skos:prefLabel>
	<skos:prefLabel xml:lang="fr">Écaille du Marchegghorn (partie Sardona)</skos:prefLabel>
	<skos:prefLabel xml:lang="it">Scaglia del Marchegghorn (parte Sardona)</skos:prefLabel>
	<skos:broader rdf:resource="https://dev-lexic.swissgeol.ch/TectonicUnits/SardonaNappe"/>
	<skos:broader rdf:resource="https://dev-lexic.swissgeol.ch/TectonicUnits/MarchegghornSlice"/>
	<status xmlns="http://www.w3.org/ns/adms#" rdf:resource="https://dev-lexic.swissgeol.ch/active"/>
</rdf:Description>

<rdf:Description rdf:about="https://dev-lexic.swissgeol.ch/TectonicUnits/OrglenSlices_PartSardona">
	<rdf:type rdf:resource="http://www.w3.org/2004/02/skos/core#Concept"/>
	<rdfs:isDefinedBy xml:lang="en">Gouffon Yves (Editor) (2024): Tectonic Map of Switzerland 1:500000, Explanatory notes. Federal Office of Topography swisstopo, Wabern</rdfs:isDefinedBy>
	<skos:inScheme rdf:resource="https://dev-lexic.swissgeol.ch/TectonicUnits"/>
	<skos:prefLabel xml:lang="en">Orglen Slices (part Sardona)</skos:prefLabel>
	<skos:prefLabel xml:lang="de">Orglen-Schuppen (Sardona-Anteil)</skos:prefLabel>
	<skos:prefLabel xml:lang="fr">Écailles de l'Orglen (partie Sardona)</skos:prefLabel>
	<skos:prefLabel xml:lang="it">Scaglie dell'Orglen (parte Sardona)</skos:prefLabel>
	<skos:broader rdf:resource="https://dev-lexic.swissgeol.ch/TectonicUnits/SardonaNappe"/>
	<skos:broader rdf:resource="https://dev-lexic.swissgeol.ch/TectonicUnits/OrglenSlices"/>
	<status xmlns="http://www.w3.org/ns/adms#" rdf:resource="https://dev-lexic.swissgeol.ch/active"/>
</rdf:Description>

<rdf:Description rdf:about="https://dev-lexic.swissgeol.ch/TectonicUnits/CalandaSlice_PartSardona">
	<rdf:type rdf:resource="http://www.w3.org/2004/02/skos/core#Concept"/>
	<rdfs:isDefinedBy xml:lang="en">Gouffon Yves (Editor) (2024): Tectonic Map of Switzerland 1:500000, Explanatory notes. Federal Office of Topography swisstopo, Wabern</rdfs:isDefinedBy>
	<skos:inScheme rdf:resource="https://dev-lexic.swissgeol.ch/TectonicUnits"/>
	<skos:prefLabel xml:lang="en">Calanda Slice (part Sardona)</skos:prefLabel>
	<skos:prefLabel xml:lang="de">Calanda-Schuppe (Sardona-Anteil)</skos:prefLabel>
	<skos:prefLabel xml:lang="fr">Écaille du Calanda (partie Sardona)</skos:prefLabel>
	<skos:prefLabel xml:lang="it">Scaglia del Calanda (parte Sardona)</skos:prefLabel>
	<skos:broader rdf:resource="https://dev-lexic.swissgeol.ch/TectonicUnits/SardonaNappe"/>
	<skos:broader rdf:resource="https://dev-lexic.swissgeol.ch/TectonicUnits/CalandaSlice"/>
	<status xmlns="http://www.w3.org/ns/adms#" rdf:resource="https://dev-lexic.swissgeol.ch/active"/>
</rdf:Description>

<rdf:Description rdf:about="https://dev-lexic.swissgeol.ch/TectonicUnits/MiruttaSlice_PartSardona">
	<rdf:type rdf:resource="http://www.w3.org/2004/02/skos/core#Concept"/>
	<rdfs:isDefinedBy xml:lang="en">Gouffon Yves (Editor) (2024): Tectonic Map of Switzerland 1:500000, Explanatory notes. Federal Office of Topography swisstopo, Wabern</rdfs:isDefinedBy>
	<skos:inScheme rdf:resource="https://dev-lexic.swissgeol.ch/TectonicUnits"/>
	<skos:prefLabel xml:lang="en">Mirutta Slice (part Sardona)</skos:prefLabel>
	<skos:prefLabel xml:lang="de">Mirutta-Schuppe (Sardona-Anteil)</skos:prefLabel>
	<skos:prefLabel xml:lang="fr">Écaille du Mirutta (partie Sardona)</skos:prefLabel>
	<skos:prefLabel xml:lang="it">Scaglia del Mirutta (parte Sardona)</skos:prefLabel>
	<skos:broader rdf:resource="https://dev-lexic.swissgeol.ch/TectonicUnits/SardonaNappe"/>
	<skos:broader rdf:resource="https://dev-lexic.swissgeol.ch/TectonicUnits/MiruttaSlice"/>
	<status xmlns="http://www.w3.org/ns/adms#" rdf:resource="https://dev-lexic.swissgeol.ch/active"/>
</rdf:Description>

<rdf:Description rdf:about="https://dev-lexic.swissgeol.ch/TectonicUnits/InternalAarMassif">
	<rdf:type rdf:resource="http://www.w3.org/2004/02/skos/core#Concept"/>
	<skos:definition xml:lang="en">The Internal Aar Massif is restricted to a thin band situated south of the Rote Kuh-Gampel Shear Zone and its possible continuation between Aletsch and Rhône glaciers. It is subdivied into two submassifs: the Baltschieder-Gletsch Submassif in upper Valais region, and the Trun-Punteglias Submassif in the Surselva (Graubünden), with an autochthonous sedimentary cover preserved in part locally.</skos:definition>
	<skos:inScheme rdf:resource="https://dev-lexic.swissgeol.ch/TectonicUnits"/>
	<skos:prefLabel xml:lang="en">Internal Aar Massif</skos:prefLabel>
	<skos:prefLabel xml:lang="de">Internes Aar-Massiv</skos:prefLabel>
	<skos:prefLabel xml:lang="fr">Massif de l'Aar interne</skos:prefLabel>
	<skos:prefLabel xml:lang="it">Massiccio dell'Aare interno</skos:prefLabel>
	<skos:broader rdf:resource="https://dev-lexic.swissgeol.ch/TectonicUnits/AarMassif"/>
</rdf:Description>

<rdf:Description rdf:about="https://dev-lexic.swissgeol.ch/TectonicUnits/DiableretsNappe">
	<rdf:type rdf:resource="http://www.w3.org/2004/02/skos/core#Concept"/>
	<rdfs:isDefinedBy xml:lang="en">Gouffon Yves (Editor) (2024): Tectonic Map of Switzerland 1:500000, Explanatory notes. Federal Office of Topography swisstopo, Wabern</rdfs:isDefinedBy>
	<skos:definition xml:lang="en">The Diablerets Nappe is an Upper Helvetic tectonic nappe in the Western Swiss Alps. Forming the base of the Wildhorn Nappe Complex, it is present only in the southwest and is linked by a tight syncline to the overlying Mont Gond Nappe.</skos:definition>
	<skos:inScheme rdf:resource="https://dev-lexic.swissgeol.ch/TectonicUnits"/>
	<skos:prefLabel xml:lang="en">Diablerets Nappe</skos:prefLabel>
	<skos:prefLabel xml:lang="de">Diablerets-Decke</skos:prefLabel>
	<skos:prefLabel xml:lang="fr">Nappe des Diablerets</skos:prefLabel>
	<skos:prefLabel xml:lang="it">Falda dei Diablerets</skos:prefLabel>
	<skos:broader rdf:resource="https://dev-lexic.swissgeol.ch/TectonicUnits/WildhornNappeComplex"/>
	<status xmlns="http://www.w3.org/ns/adms#" rdf:resource="https://dev-lexic.swissgeol.ch/active"/>
</rdf:Description>

<rdf:Description rdf:about="https://dev-lexic.swissgeol.ch/TectonicUnits/MontGondNappe">
	<rdf:type rdf:resource="http://www.w3.org/2004/02/skos/core#Concept"/>
	<rdfs:isDefinedBy xml:lang="en">Gouffon Yves (Editor) (2024): Tectonic Map of Switzerland 1:500000, Explanatory notes. Federal Office of Topography swisstopo, Wabern</rdfs:isDefinedBy>
	<skos:definition xml:lang="en">The Mont Gond Nappe is an Upper Helvetic tectonic nappe in the Western Swiss Alps. Forming the middle part of the Wildhorn Nappe Complex, it is present only in the southwest and is linked by a tight syncline to the underlying Diablerets Nappe.</skos:definition>
	<skos:inScheme rdf:resource="https://dev-lexic.swissgeol.ch/TectonicUnits"/>
	<skos:prefLabel xml:lang="en">Mont Gond Nappe</skos:prefLabel>
	<skos:prefLabel xml:lang="de">Mont-Gond-Decke</skos:prefLabel>
	<skos:prefLabel xml:lang="fr">Nappe du Mont Gond</skos:prefLabel>
	<skos:prefLabel xml:lang="it">Falda del Mont Gond</skos:prefLabel>
	<skos:broader rdf:resource="https://dev-lexic.swissgeol.ch/TectonicUnits/WildhornNappeComplex"/>
	<status xmlns="http://www.w3.org/ns/adms#" rdf:resource="https://dev-lexic.swissgeol.ch/active"/>
</rdf:Description>

<rdf:Description rdf:about="https://dev-lexic.swissgeol.ch/TectonicUnits/SublageNappe">
	<rdf:type rdf:resource="http://www.w3.org/2004/02/skos/core#Concept"/>
	<rdfs:isDefinedBy xml:lang="en">Gouffon Yves (Editor) (2024): Tectonic Map of Switzerland 1:500000, Explanatory notes. Federal Office of Topography swisstopo, Wabern</rdfs:isDefinedBy>
	<skos:definition xml:lang="en">The Sublage Nappe is an Upper Helvetic tectonic nappe in the Western Swiss Alps. It is the highest unit of the Wildhorn Nappe Complex and forms the main body of the complex. To the southwest it overlies the Mont Gond Nappe, whereas it overlies the thin Jägerchrüz Nappe north of Sierre and the Gellihorn Nappe further northeast.</skos:definition>
	<skos:inScheme rdf:resource="https://dev-lexic.swissgeol.ch/TectonicUnits"/>
	<skos:prefLabel xml:lang="en">Sublage Nappe</skos:prefLabel>
	<skos:prefLabel xml:lang="de">Sublage-Decke</skos:prefLabel>
	<skos:prefLabel xml:lang="fr">Nappe du Sublage</skos:prefLabel>
	<skos:prefLabel xml:lang="it">Falda del Sublage</skos:prefLabel>
	<skos:broader rdf:resource="https://dev-lexic.swissgeol.ch/TectonicUnits/WildhornNappeComplex"/>
	<status xmlns="http://www.w3.org/ns/adms#" rdf:resource="https://dev-lexic.swissgeol.ch/active"/>
</rdf:Description>

<rdf:Description rdf:about="https://dev-lexic.swissgeol.ch/TectonicUnits/WagetenSlice">
	<rdf:type rdf:resource="http://www.w3.org/2004/02/skos/core#Concept"/>
	<rdfs:isDefinedBy xml:lang="en">Gouffon Yves (Editor) (2024): Tectonic Map of Switzerland 1:500000, Explanatory notes. Federal Office of Topography swisstopo, Wabern</rdfs:isDefinedBy>
	<skos:inScheme rdf:resource="https://dev-lexic.swissgeol.ch/TectonicUnits"/>
	<skos:prefLabel xml:lang="en">Wageten Slice</skos:prefLabel>
	<skos:prefLabel xml:lang="de">Wageten-Schuppe</skos:prefLabel>
	<skos:prefLabel xml:lang="fr">Écaille de la Wageten</skos:prefLabel>
	<skos:prefLabel xml:lang="it">Scaglia della Wageten</skos:prefLabel>
	<skos:broader rdf:resource="https://dev-lexic.swissgeol.ch/TectonicUnits/GlarusNappeComplex"/>
	<status xmlns="http://www.w3.org/ns/adms#" rdf:resource="https://dev-lexic.swissgeol.ch/active"/>
</rdf:Description>

<rdf:Description rdf:about="https://dev-lexic.swissgeol.ch/TectonicUnits/Gonzen-WalenstadtSlices">
	<rdf:type rdf:resource="http://www.w3.org/2004/02/skos/core#Concept"/>
	<rdfs:isDefinedBy xml:lang="en">Gouffon Yves (Editor) (2024): Tectonic Map of Switzerland 1:500000, Explanatory notes. Federal Office of Topography swisstopo, Wabern</rdfs:isDefinedBy>
	<skos:inScheme rdf:resource="https://dev-lexic.swissgeol.ch/TectonicUnits"/>
	<skos:prefLabel xml:lang="en">Gonzen-Walenstadt Slices</skos:prefLabel>
	<skos:prefLabel xml:lang="de">Gonzen-Walenstadt-Schuppen</skos:prefLabel>
	<skos:prefLabel xml:lang="fr">Écailles du Gonzen-Walenstadt</skos:prefLabel>
	<skos:prefLabel xml:lang="it">Scaglie del Gonzen-Walenstadt</skos:prefLabel>
	<skos:broader rdf:resource="https://dev-lexic.swissgeol.ch/TectonicUnits/GlarusNappeComplex"/>
	<status xmlns="http://www.w3.org/ns/adms#" rdf:resource="https://dev-lexic.swissgeol.ch/active"/>
</rdf:Description>

<rdf:Description rdf:about="https://dev-lexic.swissgeol.ch/TectonicUnits/MuertschenNappe">
	<rdf:type rdf:resource="http://www.w3.org/2004/02/skos/core#Concept"/>
	<rdfs:isDefinedBy xml:lang="en">Gouffon Yves (Editor) (2024): Tectonic Map of Switzerland 1:500000, Explanatory notes. Federal Office of Topography swisstopo, Wabern</rdfs:isDefinedBy>
	<skos:inScheme rdf:resource="https://dev-lexic.swissgeol.ch/TectonicUnits"/>
	<skos:prefLabel xml:lang="en">Mürtschen Nappe</skos:prefLabel>
	<skos:prefLabel xml:lang="de">Mürtschen-Decke</skos:prefLabel>
	<skos:prefLabel xml:lang="fr">Nappe du Mürtschen</skos:prefLabel>
	<skos:prefLabel xml:lang="it">Falda del Mürtschen</skos:prefLabel>
	<skos:broader rdf:resource="https://dev-lexic.swissgeol.ch/TectonicUnits/GlarusNappeComplex"/>
	<status xmlns="http://www.w3.org/ns/adms#" rdf:resource="https://dev-lexic.swissgeol.ch/active"/>
</rdf:Description>

<rdf:Description rdf:about="https://dev-lexic.swissgeol.ch/TectonicUnits/ToralpSlice">
	<rdf:type rdf:resource="http://www.w3.org/2004/02/skos/core#Concept"/>
	<rdfs:isDefinedBy xml:lang="en">Gouffon Yves (Editor) (2024): Tectonic Map of Switzerland 1:500000, Explanatory notes. Federal Office of Topography swisstopo, Wabern</rdfs:isDefinedBy>
	<skos:inScheme rdf:resource="https://dev-lexic.swissgeol.ch/TectonicUnits"/>
	<skos:prefLabel xml:lang="en">Toralp Slice</skos:prefLabel>
	<skos:prefLabel xml:lang="de">Toralp-Schuppe</skos:prefLabel>
	<skos:prefLabel xml:lang="fr">Écaille de la Toralp</skos:prefLabel>
	<skos:prefLabel xml:lang="it">Scaglia della Toralp</skos:prefLabel>
	<skos:broader rdf:resource="https://dev-lexic.swissgeol.ch/TectonicUnits/AxenNappe"/>
	<status xmlns="http://www.w3.org/ns/adms#" rdf:resource="https://dev-lexic.swissgeol.ch/active"/>
</rdf:Description>

<rdf:Description rdf:about="https://dev-lexic.swissgeol.ch/TectonicUnits/SilberenSlices">
	<rdf:type rdf:resource="http://www.w3.org/2004/02/skos/core#Concept"/>
	<rdfs:isDefinedBy xml:lang="en">Gouffon Yves (Editor) (2024): Tectonic Map of Switzerland 1:500000, Explanatory notes. Federal Office of Topography swisstopo, Wabern</rdfs:isDefinedBy>
	<skos:inScheme rdf:resource="https://dev-lexic.swissgeol.ch/TectonicUnits"/>
	<skos:prefLabel xml:lang="en">Silberen Slices</skos:prefLabel>
	<skos:prefLabel xml:lang="de">Silberen-Schuppen</skos:prefLabel>
	<skos:prefLabel xml:lang="fr">Écaille du Silberen</skos:prefLabel>
	<skos:prefLabel xml:lang="it">Scaglia del Silberen</skos:prefLabel>
	<skos:broader rdf:resource="https://dev-lexic.swissgeol.ch/TectonicUnits/AxenNappe"/>
	<status xmlns="http://www.w3.org/ns/adms#" rdf:resource="https://dev-lexic.swissgeol.ch/active"/>
</rdf:Description>

<rdf:Description rdf:about="https://dev-lexic.swissgeol.ch/TectonicUnits/BaechistockSlice">
	<rdf:type rdf:resource="http://www.w3.org/2004/02/skos/core#Concept"/>
	<rdfs:isDefinedBy xml:lang="en">Gouffon Yves (Editor) (2024): Tectonic Map of Switzerland 1:500000, Explanatory notes. Federal Office of Topography swisstopo, Wabern</rdfs:isDefinedBy>
	<skos:inScheme rdf:resource="https://dev-lexic.swissgeol.ch/TectonicUnits"/>
	<skos:prefLabel xml:lang="en">Bächistock Slice</skos:prefLabel>
	<skos:prefLabel xml:lang="de">Bächistock-Schuppe</skos:prefLabel>
	<skos:prefLabel xml:lang="fr">Écaille du Bächistock</skos:prefLabel>
	<skos:prefLabel xml:lang="it">Scaglia del Bächistock</skos:prefLabel>
	<skos:broader rdf:resource="https://dev-lexic.swissgeol.ch/TectonicUnits/AxenNappe"/>
	<status xmlns="http://www.w3.org/ns/adms#" rdf:resource="https://dev-lexic.swissgeol.ch/active"/>
</rdf:Description>

<rdf:Description rdf:about="https://dev-lexic.swissgeol.ch/TectonicUnits/WissbergSlice">
	<rdf:type rdf:resource="http://www.w3.org/2004/02/skos/core#Concept"/>
	<rdfs:isDefinedBy xml:lang="en">Gouffon Yves (Editor) (2024): Tectonic Map of Switzerland 1:500000, Explanatory notes. Federal Office of Topography swisstopo, Wabern</rdfs:isDefinedBy>
	<skos:inScheme rdf:resource="https://dev-lexic.swissgeol.ch/TectonicUnits"/>
	<skos:prefLabel xml:lang="en">Wissberg Slice</skos:prefLabel>
	<skos:prefLabel xml:lang="de">Wissberg-Schuppe</skos:prefLabel>
	<skos:prefLabel xml:lang="fr">Écaille du Wissberg</skos:prefLabel>
	<skos:prefLabel xml:lang="it">Scaglia del Wissberg</skos:prefLabel>
	<skos:broader rdf:resource="https://dev-lexic.swissgeol.ch/TectonicUnits/AxenNappe"/>
	<status xmlns="http://www.w3.org/ns/adms#" rdf:resource="https://dev-lexic.swissgeol.ch/active"/>
</rdf:Description>

<rdf:Description rdf:about="https://dev-lexic.swissgeol.ch/TectonicUnits/SchaechentalerWindgaellenSlices">
	<rdf:type rdf:resource="http://www.w3.org/2004/02/skos/core#Concept"/>
	<rdfs:isDefinedBy xml:lang="en">Gouffon Yves (Editor) (2024): Tectonic Map of Switzerland 1:500000, Explanatory notes. Federal Office of Topography swisstopo, Wabern</rdfs:isDefinedBy>
	<skos:inScheme rdf:resource="https://dev-lexic.swissgeol.ch/TectonicUnits"/>
	<skos:prefLabel xml:lang="en">Schächentaler Windgällen Slices</skos:prefLabel>
	<skos:prefLabel xml:lang="de">Schächentaler Windgällen-Schuppen</skos:prefLabel>
	<skos:prefLabel xml:lang="fr">Écaille des Schächentaler Windgällen</skos:prefLabel>
	<skos:prefLabel xml:lang="it">Scaglia delle Schächentaler Windgällen</skos:prefLabel>
	<skos:broader rdf:resource="https://dev-lexic.swissgeol.ch/TectonicUnits/AxenNappe"/>
	<status xmlns="http://www.w3.org/ns/adms#" rdf:resource="https://dev-lexic.swissgeol.ch/active"/>
</rdf:Description>

<rdf:Description rdf:about="https://dev-lexic.swissgeol.ch/TectonicUnits/HoechTurmSlices">
	<rdf:type rdf:resource="http://www.w3.org/2004/02/skos/core#Concept"/>
	<rdfs:isDefinedBy xml:lang="en">Gouffon Yves (Editor) (2024): Tectonic Map of Switzerland 1:500000, Explanatory notes. Federal Office of Topography swisstopo, Wabern</rdfs:isDefinedBy>
	<skos:inScheme rdf:resource="https://dev-lexic.swissgeol.ch/TectonicUnits"/>
	<skos:prefLabel xml:lang="en">Höch Turm Slices</skos:prefLabel>
	<skos:prefLabel xml:lang="de">Höch-Turm-Schuppen</skos:prefLabel>
	<skos:prefLabel xml:lang="fr">Écaille du Höch Turm</skos:prefLabel>
	<skos:prefLabel xml:lang="it">Scaglia del Höch Turm</skos:prefLabel>
	<skos:broader rdf:resource="https://dev-lexic.swissgeol.ch/TectonicUnits/AxenNappe"/>
	<status xmlns="http://www.w3.org/ns/adms#" rdf:resource="https://dev-lexic.swissgeol.ch/active"/>
</rdf:Description>

<rdf:Description rdf:about="https://dev-lexic.swissgeol.ch/TectonicUnits/FriterenSlice">
	<rdf:type rdf:resource="http://www.w3.org/2004/02/skos/core#Concept"/>
	<rdfs:isDefinedBy xml:lang="en">Gouffon Yves (Editor) (2024): Tectonic Map of Switzerland 1:500000, Explanatory notes. Federal Office of Topography swisstopo, Wabern</rdfs:isDefinedBy>
	<skos:inScheme rdf:resource="https://dev-lexic.swissgeol.ch/TectonicUnits"/>
	<skos:prefLabel xml:lang="en">Friteren Slice</skos:prefLabel>
	<skos:prefLabel xml:lang="de">Friteren-Schuppe</skos:prefLabel>
	<skos:prefLabel xml:lang="fr">Écaille de Friteren</skos:prefLabel>
	<skos:prefLabel xml:lang="it">Scaglia di Friteren</skos:prefLabel>
	<skos:broader rdf:resource="https://dev-lexic.swissgeol.ch/TectonicUnits/AxenNappe"/>
	<status xmlns="http://www.w3.org/ns/adms#" rdf:resource="https://dev-lexic.swissgeol.ch/active"/>
</rdf:Description>

<rdf:Description rdf:about="https://dev-lexic.swissgeol.ch/TectonicUnits/AxenNorthSlice">
	<rdf:type rdf:resource="http://www.w3.org/2004/02/skos/core#Concept"/>
	<rdfs:isDefinedBy xml:lang="en">Gouffon Yves (Editor) (2024): Tectonic Map of Switzerland 1:500000, Explanatory notes. Federal Office of Topography swisstopo, Wabern</rdfs:isDefinedBy>
	<skos:inScheme rdf:resource="https://dev-lexic.swissgeol.ch/TectonicUnits"/>
	<skos:prefLabel xml:lang="en">Axen north Slice</skos:prefLabel>
	<skos:prefLabel xml:lang="de">Axen-Nordschuppe</skos:prefLabel>
	<skos:prefLabel xml:lang="fr">Écaille nord de l'Axen</skos:prefLabel>
	<skos:prefLabel xml:lang="it">Scaglia nord dell'Axen</skos:prefLabel>
	<skos:broader rdf:resource="https://dev-lexic.swissgeol.ch/TectonicUnits/AxenNappe"/>
	<status xmlns="http://www.w3.org/ns/adms#" rdf:resource="https://dev-lexic.swissgeol.ch/active"/>
</rdf:Description>

<rdf:Description rdf:about="https://dev-lexic.swissgeol.ch/TectonicUnits/AxenSouthSlice">
	<rdf:type rdf:resource="http://www.w3.org/2004/02/skos/core#Concept"/>
	<rdfs:isDefinedBy xml:lang="en">Gouffon Yves (Editor) (2024): Tectonic Map of Switzerland 1:500000, Explanatory notes. Federal Office of Topography swisstopo, Wabern</rdfs:isDefinedBy>
	<skos:inScheme rdf:resource="https://dev-lexic.swissgeol.ch/TectonicUnits"/>
	<skos:prefLabel xml:lang="en">Axen south Slice</skos:prefLabel>
	<skos:prefLabel xml:lang="de">Axen-Südschuppe</skos:prefLabel>
	<skos:prefLabel xml:lang="fr">Écaille sud de l'Axen</skos:prefLabel>
	<skos:prefLabel xml:lang="it">Scaglia sud dell'Axen</skos:prefLabel>
	<skos:broader rdf:resource="https://dev-lexic.swissgeol.ch/TectonicUnits/AxenNappe"/>
	<status xmlns="http://www.w3.org/ns/adms#" rdf:resource="https://dev-lexic.swissgeol.ch/active"/>
</rdf:Description>

<rdf:Description rdf:about="https://dev-lexic.swissgeol.ch/TectonicUnits/WissenwandSlice">
	<rdf:type rdf:resource="http://www.w3.org/2004/02/skos/core#Concept"/>
	<rdfs:isDefinedBy xml:lang="en">Gouffon Yves (Editor) (2024): Tectonic Map of Switzerland 1:500000, Explanatory notes. Federal Office of Topography swisstopo, Wabern</rdfs:isDefinedBy>
	<skos:definition xml:lang="en">The Wissenwand Slice, composed of Late Jurassic limestone (Quinten Formation), forms the base of the Drusberg Nappe in the Muotatal, where it underlies the Palfris Formation of the main part of the nappe.</skos:definition>
	<skos:inScheme rdf:resource="https://dev-lexic.swissgeol.ch/TectonicUnits"/>
	<skos:prefLabel xml:lang="en">Wissenwand Slice</skos:prefLabel>
	<skos:prefLabel xml:lang="de">Wissenwand-Schuppe</skos:prefLabel>
	<skos:prefLabel xml:lang="fr">Écaille de la Wissenwand</skos:prefLabel>
	<skos:prefLabel xml:lang="it">Scaglia della Wissenwand</skos:prefLabel>
	<skos:broader rdf:resource="https://dev-lexic.swissgeol.ch/TectonicUnits/DrusbergNappe"/>
	<status xmlns="http://www.w3.org/ns/adms#" rdf:resource="https://dev-lexic.swissgeol.ch/active"/>
</rdf:Description>

<rdf:Description rdf:about="https://dev-lexic.swissgeol.ch/TectonicUnits/Niederhorn-PilatusSlice">
	<rdf:type rdf:resource="http://www.w3.org/2004/02/skos/core#Concept"/>
	<rdfs:isDefinedBy xml:lang="en">Gouffon Yves (Editor) (2024): Tectonic Map of Switzerland 1:500000, Explanatory notes. Federal Office of Topography swisstopo, Wabern</rdfs:isDefinedBy>
	<skos:inScheme rdf:resource="https://dev-lexic.swissgeol.ch/TectonicUnits"/>
	<skos:prefLabel xml:lang="en">Niederhorn-Pilatus Slice</skos:prefLabel>
	<skos:prefLabel xml:lang="de">Niederhorn-Pilatus-Schuppe</skos:prefLabel>
	<skos:prefLabel xml:lang="fr">Écaille du Niederhorn-Pilatus</skos:prefLabel>
	<skos:prefLabel xml:lang="it">Scaglia del Niederhorn-Pilatus</skos:prefLabel>
	<skos:altLabel xml:lang="de">Niederhorn-Decke</skos:altLabel>
	<skos:broader rdf:resource="https://dev-lexic.swissgeol.ch/TectonicUnits/DrusbergNappe"/>
	<status xmlns="http://www.w3.org/ns/adms#" rdf:resource="https://dev-lexic.swissgeol.ch/active"/>
</rdf:Description>

<rdf:Description rdf:about="https://dev-lexic.swissgeol.ch/TectonicUnits/Buergenstock-UrmibergSlice">
	<rdf:type rdf:resource="http://www.w3.org/2004/02/skos/core#Concept"/>
	<rdfs:isDefinedBy xml:lang="en">Gouffon Yves (Editor) (2024): Tectonic Map of Switzerland 1:500000, Explanatory notes. Federal Office of Topography swisstopo, Wabern</rdfs:isDefinedBy>
	<skos:inScheme rdf:resource="https://dev-lexic.swissgeol.ch/TectonicUnits"/>
	<skos:prefLabel xml:lang="en">Bürgenstock-Urmiberg Slice</skos:prefLabel>
	<skos:prefLabel xml:lang="de">Bürgenstock-Urmiberg-Schuppe</skos:prefLabel>
	<skos:prefLabel xml:lang="fr">Écaille du Bürgenstock-Urmiberg</skos:prefLabel>
	<skos:prefLabel xml:lang="it">Scaglia del Bürgenstock-Urmiberg</skos:prefLabel>
	<skos:broader rdf:resource="https://dev-lexic.swissgeol.ch/TectonicUnits/DrusbergNappe"/>
	<status xmlns="http://www.w3.org/ns/adms#" rdf:resource="https://dev-lexic.swissgeol.ch/active"/>
</rdf:Description>

<rdf:Description rdf:about="https://dev-lexic.swissgeol.ch/TectonicUnits/HochflueSlice">
	<rdf:type rdf:resource="http://www.w3.org/2004/02/skos/core#Concept"/>
	<rdfs:isDefinedBy xml:lang="en">Gouffon Yves (Editor) (2024): Tectonic Map of Switzerland 1:500000, Explanatory notes. Federal Office of Topography swisstopo, Wabern</rdfs:isDefinedBy>
	<skos:inScheme rdf:resource="https://dev-lexic.swissgeol.ch/TectonicUnits"/>
	<skos:prefLabel xml:lang="en">Hochflue Slice</skos:prefLabel>
	<skos:prefLabel xml:lang="de">Hochflue-Schuppe</skos:prefLabel>
	<skos:prefLabel xml:lang="fr">Écaille de la Hochflue</skos:prefLabel>
	<skos:prefLabel xml:lang="it">Scaglia della Hochflue</skos:prefLabel>
	<skos:broader rdf:resource="https://dev-lexic.swissgeol.ch/TectonicUnits/DrusbergNappe"/>
	<status xmlns="http://www.w3.org/ns/adms#" rdf:resource="https://dev-lexic.swissgeol.ch/active"/>
</rdf:Description>

<rdf:Description rdf:about="https://dev-lexic.swissgeol.ch/TectonicUnits/MaisanderSlice">
	<rdf:type rdf:resource="http://www.w3.org/2004/02/skos/core#Concept"/>
	<rdfs:isDefinedBy xml:lang="en">Gouffon Yves (Editor) (2024): Tectonic Map of Switzerland 1:500000, Explanatory notes. Federal Office of Topography swisstopo, Wabern</rdfs:isDefinedBy>
	<skos:definition xml:lang="en">The Maisander Slices are composed of Late Jurassic limestone (Quinten Formation) intercalated into the Palfris Formation of the Axen Nappe between the Engelberg Valley and the Vierwaldstättersee.</skos:definition>
	<skos:inScheme rdf:resource="https://dev-lexic.swissgeol.ch/TectonicUnits"/>
	<skos:prefLabel xml:lang="en">Maisander Slice</skos:prefLabel>
	<skos:prefLabel xml:lang="de">Maisander-Schuppe</skos:prefLabel>
	<skos:prefLabel xml:lang="fr">Écaille du Maisander</skos:prefLabel>
	<skos:prefLabel xml:lang="it">Scaglia del Maisander</skos:prefLabel>
	<skos:broader rdf:resource="https://dev-lexic.swissgeol.ch/TectonicUnits/DrusbergNappe"/>
	<status xmlns="http://www.w3.org/ns/adms#" rdf:resource="https://dev-lexic.swissgeol.ch/active"/>
</rdf:Description>

<rdf:Description rdf:about="https://dev-lexic.swissgeol.ch/TectonicUnits/AubrigSlice">
	<rdf:type rdf:resource="http://www.w3.org/2004/02/skos/core#Concept"/>
	<rdfs:isDefinedBy xml:lang="en">Gouffon Yves (Editor) (2024): Tectonic Map of Switzerland 1:500000, Explanatory notes. Federal Office of Topography swisstopo, Wabern</rdfs:isDefinedBy>
	<skos:inScheme rdf:resource="https://dev-lexic.swissgeol.ch/TectonicUnits"/>
	<skos:prefLabel xml:lang="en">Aubrig Slice</skos:prefLabel>
	<skos:prefLabel xml:lang="de">Aubrig-Schuppe</skos:prefLabel>
	<skos:prefLabel xml:lang="fr">Écaille de l'Aubrig</skos:prefLabel>
	<skos:prefLabel xml:lang="it">Scaglia dell'Aubrig</skos:prefLabel>
	<skos:broader rdf:resource="https://dev-lexic.swissgeol.ch/TectonicUnits/DrusbergNappe"/>
	<status xmlns="http://www.w3.org/ns/adms#" rdf:resource="https://dev-lexic.swissgeol.ch/active"/>
</rdf:Description>

<rdf:Description rdf:about="https://dev-lexic.swissgeol.ch/TectonicUnits/InfraprealpineMelange">
	<rdf:type rdf:resource="http://www.w3.org/2004/02/skos/core#Concept"/>
	<rdfs:isDefinedBy xml:lang="en">Gouffon Yves (Editor) (2024): Tectonic Map of Switzerland 1:500000, Explanatory notes. Federal Office of Topography swisstopo, Wabern</rdfs:isDefinedBy>
	<skos:inScheme rdf:resource="https://dev-lexic.swissgeol.ch/TectonicUnits"/>
	<skos:prefLabel xml:lang="en">Infraprealpine Mélange</skos:prefLabel>
	<skos:prefLabel xml:lang="de">Infrapräalpines Melange</skos:prefLabel>
	<skos:prefLabel xml:lang="fr">Mélange Infrapréalpin</skos:prefLabel>
	<skos:prefLabel xml:lang="it">Mélange infraprealpino</skos:prefLabel>
	<skos:broader rdf:resource="https://dev-lexic.swissgeol.ch/TectonicUnits/BulleMelangeZone"/>
	<status xmlns="http://www.w3.org/ns/adms#" rdf:resource="https://dev-lexic.swissgeol.ch/active"/>
</rdf:Description>

<rdf:Description rdf:about="https://dev-lexic.swissgeol.ch/TectonicUnits/MontsalvensSlice">
	<rdf:type rdf:resource="http://www.w3.org/2004/02/skos/core#Concept"/>
	<rdfs:isDefinedBy xml:lang="en">Gouffon Yves (Editor) (2024): Tectonic Map of Switzerland 1:500000, Explanatory notes. Federal Office of Topography swisstopo, Wabern</rdfs:isDefinedBy>
	<skos:inScheme rdf:resource="https://dev-lexic.swissgeol.ch/TectonicUnits"/>
	<skos:prefLabel xml:lang="en">Montsalvens Slice</skos:prefLabel>
	<skos:prefLabel xml:lang="de">Montsalvens-Schuppe</skos:prefLabel>
	<skos:prefLabel xml:lang="fr">Écaille de Montsalvens</skos:prefLabel>
	<skos:prefLabel xml:lang="it">Scaglia di Montsalvens</skos:prefLabel>
	<skos:broader rdf:resource="https://dev-lexic.swissgeol.ch/TectonicUnits/BulleMelangeZone"/>
	<status xmlns="http://www.w3.org/ns/adms#" rdf:resource="https://dev-lexic.swissgeol.ch/active"/>
</rdf:Description>

<rdf:Description rdf:about="https://dev-lexic.swissgeol.ch/TectonicUnits/LesPleiadesSlice">
	<rdf:type rdf:resource="http://www.w3.org/2004/02/skos/core#Concept"/>
	<rdfs:isDefinedBy xml:lang="en">Gouffon Yves (Editor) (2024): Tectonic Map of Switzerland 1:500000, Explanatory notes. Federal Office of Topography swisstopo, Wabern</rdfs:isDefinedBy>
	<skos:inScheme rdf:resource="https://dev-lexic.swissgeol.ch/TectonicUnits"/>
	<skos:prefLabel xml:lang="en">Les Pléiades Slice</skos:prefLabel>
	<skos:prefLabel xml:lang="de">Les-Pléiades-Schuppe</skos:prefLabel>
	<skos:prefLabel xml:lang="fr">Écaille des Pléiades</skos:prefLabel>
	<skos:prefLabel xml:lang="it">Scaglia delle Pléiades</skos:prefLabel>
	<skos:broader rdf:resource="https://dev-lexic.swissgeol.ch/TectonicUnits/BulleMelangeZone"/>
	<status xmlns="http://www.w3.org/ns/adms#" rdf:resource="https://dev-lexic.swissgeol.ch/active"/>
</rdf:Description>

<rdf:Description rdf:about="https://dev-lexic.swissgeol.ch/TectonicUnits/FaucignySlices">
	<rdf:type rdf:resource="http://www.w3.org/2004/02/skos/core#Concept"/>
	<rdfs:isDefinedBy xml:lang="en">Gouffon Yves (Editor) (2024): Tectonic Map of Switzerland 1:500000, Explanatory notes. Federal Office of Topography swisstopo, Wabern</rdfs:isDefinedBy>
	<skos:inScheme rdf:resource="https://dev-lexic.swissgeol.ch/TectonicUnits"/>
	<skos:prefLabel xml:lang="en">Faucigny Slices</skos:prefLabel>
	<skos:prefLabel xml:lang="de">Faucigny-Schuppen</skos:prefLabel>
	<skos:prefLabel xml:lang="fr">Écailles du Faucigny</skos:prefLabel>
	<skos:prefLabel xml:lang="it">Scaglie del Faucigny</skos:prefLabel>
	<skos:broader rdf:resource="https://dev-lexic.swissgeol.ch/TectonicUnits/BulleMelangeZone"/>
	<status xmlns="http://www.w3.org/ns/adms#" rdf:resource="https://dev-lexic.swissgeol.ch/active"/>
</rdf:Description>

<rdf:Description rdf:about="https://dev-lexic.swissgeol.ch/TectonicUnits/BoisDeBouleyresSlice">
	<rdf:type rdf:resource="http://www.w3.org/2004/02/skos/core#Concept"/>
	<rdfs:isDefinedBy xml:lang="en">Gouffon Yves (Editor) (2024): Tectonic Map of Switzerland 1:500000, Explanatory notes. Federal Office of Topography swisstopo, Wabern</rdfs:isDefinedBy>
	<skos:inScheme rdf:resource="https://dev-lexic.swissgeol.ch/TectonicUnits"/>
	<skos:prefLabel xml:lang="en">Bois de Bouleyres Slice</skos:prefLabel>
	<skos:prefLabel xml:lang="de">Bois-de-Bouleyres-Schuppe</skos:prefLabel>
	<skos:prefLabel xml:lang="fr">Écaille du Bois de Bouleyres</skos:prefLabel>
	<skos:prefLabel xml:lang="it">Scaglia del Bois de Bouleyres</skos:prefLabel>
	<skos:broader rdf:resource="https://dev-lexic.swissgeol.ch/TectonicUnits/BulleMelangeZone"/>
	<status xmlns="http://www.w3.org/ns/adms#" rdf:resource="https://dev-lexic.swissgeol.ch/active"/>
</rdf:Description>

<rdf:Description rdf:about="https://dev-lexic.swissgeol.ch/TectonicUnits/Lepontic">
	<rdf:type rdf:resource="http://www.w3.org/2004/02/skos/core#Concept"/>
	<rdfs:isDefinedBy xml:lang="en">Gouffon Yves (Editor) (2024): Tectonic Map of Switzerland 1:500000, Explanatory notes. Federal Office of Topography swisstopo, Wabern</rdfs:isDefinedBy>
	<rdfs:comment rdf:datatype="http://www.w3.org/1999/02/22-rdf-syntax-ns#HTML">https://data.geo.admin.ch/ch.swisstopo.geologie-tektonische_karte/pdf/Erl-TK500_2024.pdf</rdfs:comment>
	<rdfs:comment rdf:datatype="http://www.w3.org/1999/02/22-rdf-syntax-ns#HTML">https://www.strati.ch/en/tectonic/lepontic</rdfs:comment>
	<skos:definition xml:lang="en">The Lepontic tectonic domain is situated between the Helvetic and Penninic units in the internal part of the Central Alps. It is characterized by the presence of a structural and metamorphic dome (Lepontine Dome). Most of these units are derived from the most distal part of the thinned European continental margin.</skos:definition>
	<skos:inScheme rdf:resource="https://dev-lexic.swissgeol.ch/TectonicUnits"/>
	<skos:topConceptOf rdf:resource="https://dev-lexic.swissgeol.ch/TectonicUnits"/>
	<skos:prefLabel xml:lang="en">Lepontic</skos:prefLabel>
	<skos:prefLabel xml:lang="de">Lepontikum</skos:prefLabel>
	<skos:prefLabel xml:lang="fr">Lépontique</skos:prefLabel>
	<skos:prefLabel xml:lang="it">Lepontico</skos:prefLabel>
	<skos:narrower rdf:resource="https://dev-lexic.swissgeol.ch/TectonicUnits/VerampioNappe"/>
	<skos:narrower rdf:resource="https://dev-lexic.swissgeol.ch/TectonicUnits/AntigorioNappeComplex"/>
	<skos:narrower rdf:resource="https://dev-lexic.swissgeol.ch/TectonicUnits/LebendunNappe"/>
	<skos:narrower rdf:resource="https://dev-lexic.swissgeol.ch/TectonicUnits/MonteLeoneNappe"/>
	<skos:narrower rdf:resource="https://dev-lexic.swissgeol.ch/TectonicUnits/MoncuccoNappe"/>
	<skos:narrower rdf:resource="https://dev-lexic.swissgeol.ch/TectonicUnits/IsornoZone"/>
	<skos:narrower rdf:resource="https://dev-lexic.swissgeol.ch/TectonicUnits/Orselina-BellinzonaZone"/>
	<skos:narrower rdf:resource="https://dev-lexic.swissgeol.ch/TectonicUnits/BoscoZone"/>
	<skos:narrower rdf:resource="https://dev-lexic.swissgeol.ch/TectonicUnits/BombognoZone"/>
	<skos:narrower rdf:resource="https://dev-lexic.swissgeol.ch/TectonicUnits/MaggiaNappe"/>
	<skos:narrower rdf:resource="https://dev-lexic.swissgeol.ch/TectonicUnits/SambucoNappe"/>
	<skos:narrower rdf:resource="https://dev-lexic.swissgeol.ch/TectonicUnits/SanGiorgioSlice"/>
	<skos:narrower rdf:resource="https://dev-lexic.swissgeol.ch/TectonicUnits/Leventina-LucomagnoNappe"/>
	<skos:narrower rdf:resource="https://dev-lexic.swissgeol.ch/TectonicUnits/SimanoNappe"/>
	<skos:narrower rdf:resource="https://dev-lexic.swissgeol.ch/TectonicUnits/CimaLungaNappe"/>
	<skos:narrower rdf:resource="https://dev-lexic.swissgeol.ch/TectonicUnits/AdulaNappe"/>
	<skos:narrower rdf:resource="https://dev-lexic.swissgeol.ch/TectonicUnits/GrufComplex"/>
	<skos:narrower rdf:resource="https://dev-lexic.swissgeol.ch/TectonicUnits/SojaNappe"/>
	<skos:narrower rdf:resource="https://dev-lexic.swissgeol.ch/TectonicUnits/PizTerri-LunschaniaNappe"/>
	<skos:narrower rdf:resource="https://dev-lexic.swissgeol.ch/TectonicUnits/PizzoDelValloneNappe"/>
	<status xmlns="http://www.w3.org/ns/adms#" rdf:resource="https://dev-lexic.swissgeol.ch/active"/>
</rdf:Description>

<rdf:Description rdf:about="https://dev-lexic.swissgeol.ch/TectonicUnits/VerampioNappe">
	<rdf:type rdf:resource="http://www.w3.org/2004/02/skos/core#Concept"/>
	<rdfs:isDefinedBy xml:lang="en">Gouffon Yves (Editor) (2024): Tectonic Map of Switzerland 1:500000, Explanatory notes. Federal Office of Topography swisstopo, Wabern</rdfs:isDefinedBy>
	<skos:definition xml:lang="en">The Verampio Nappe is the lowest Lepontic tectonic unit of the Toce Culmination, cropping out as a tectonic window beneath the Antigorio Nappe in the Valle Antigorio and Valle Devero (Italy).</skos:definition>
	<skos:inScheme rdf:resource="https://dev-lexic.swissgeol.ch/TectonicUnits"/>
	<skos:prefLabel xml:lang="en">Verampio Nappe</skos:prefLabel>
	<skos:prefLabel xml:lang="de">Verampio-Decke</skos:prefLabel>
	<skos:prefLabel xml:lang="fr">Nappe de Verampio</skos:prefLabel>
	<skos:prefLabel xml:lang="it">Falda di Verampio</skos:prefLabel>
	<skos:broader rdf:resource="https://dev-lexic.swissgeol.ch/TectonicUnits/Lepontic"/>
	<status xmlns="http://www.w3.org/ns/adms#" rdf:resource="https://dev-lexic.swissgeol.ch/active"/>
</rdf:Description>

<rdf:Description rdf:about="https://dev-lexic.swissgeol.ch/TectonicUnits/AntigorioNappeComplex">
	<rdf:type rdf:resource="http://www.w3.org/2004/02/skos/core#Concept"/>
	<rdfs:isDefinedBy xml:lang="en">Gouffon Yves (Editor) (2024): Tectonic Map of Switzerland 1:500000, Explanatory notes. Federal Office of Topography swisstopo, Wabern</rdfs:isDefinedBy>
	<skos:definition xml:lang="en">The Antigorio Nappe Complex is a composite tectonic unit of the Western Lepontic (Toce Culmination) grouping together the Antigorio Nappe and the Mergoscia Zone. The boundary between these two units, affected by isoclinal folds, has been defined differently by the authors and is even completely unidentifiable in the Southern Steep Belt (or “root zone” north of the Tonale Fault), where the rocks of each of these units are no longer recognizable due to their migmatization.</skos:definition>
	<skos:inScheme rdf:resource="https://dev-lexic.swissgeol.ch/TectonicUnits"/>
	<skos:prefLabel xml:lang="en">Antigorio Nappe Complex</skos:prefLabel>
	<skos:prefLabel xml:lang="de">Antigorio-Deckenkomplex</skos:prefLabel>
	<skos:prefLabel xml:lang="fr">Complexe de nappes d'Antigorio</skos:prefLabel>
	<skos:prefLabel xml:lang="it">Complesso di falde di Antigorio</skos:prefLabel>
	<skos:broader rdf:resource="https://dev-lexic.swissgeol.ch/TectonicUnits/Lepontic"/>
	<skos:narrower rdf:resource="https://dev-lexic.swissgeol.ch/TectonicUnits/AntigorioNappe"/>
	<skos:narrower rdf:resource="https://dev-lexic.swissgeol.ch/TectonicUnits/MergosciaZone"/>
	<status xmlns="http://www.w3.org/ns/adms#" rdf:resource="https://dev-lexic.swissgeol.ch/active"/>
</rdf:Description>

<rdf:Description rdf:about="https://dev-lexic.swissgeol.ch/TectonicUnits/LebendunNappe">
	<rdf:type rdf:resource="http://www.w3.org/2004/02/skos/core#Concept"/>
	<rdfs:isDefinedBy xml:lang="en">Gouffon Yves (Editor) (2024): Tectonic Map of Switzerland 1:500000, Explanatory notes. Federal Office of Topography swisstopo, Wabern</rdfs:isDefinedBy>
	<skos:definition xml:lang="en">The Lebendun Nappe is a tectonic unit of the Western Lepontic (Toce Culmination). It overlaps the Antigorio Nappe on its northwestern edge and is overlapped by the Pizzo del Vallone in the west and by the Sambuco Nappe in the northeast. In the north, it is bordered by the calcschists of the Sion-Courmayeur Nappe. The end of the Lebendun Nappe to the east is not clearly established, as its rocks around the Sambuco Nappe – mainly siliceous and carbonate schists – are quite similar to the metasediments of neighboring units.</skos:definition>
	<skos:inScheme rdf:resource="https://dev-lexic.swissgeol.ch/TectonicUnits"/>
	<skos:prefLabel xml:lang="en">Lebendun Nappe</skos:prefLabel>
	<skos:prefLabel xml:lang="de">Lebendun-Decke</skos:prefLabel>
	<skos:prefLabel xml:lang="fr">Nappe du Lebendun</skos:prefLabel>
	<skos:prefLabel xml:lang="it">Falda del Lebendun</skos:prefLabel>
	<skos:broader rdf:resource="https://dev-lexic.swissgeol.ch/TectonicUnits/Lepontic"/>
	<status xmlns="http://www.w3.org/ns/adms#" rdf:resource="https://dev-lexic.swissgeol.ch/active"/>
</rdf:Description>

<rdf:Description rdf:about="https://dev-lexic.swissgeol.ch/TectonicUnits/MonteLeoneNappe">
	<rdf:type rdf:resource="http://www.w3.org/2004/02/skos/core#Concept"/>
	<rdfs:isDefinedBy xml:lang="en">Gouffon Yves (Editor) (2024): Tectonic Map of Switzerland 1:500000, Explanatory notes. Federal Office of Topography swisstopo, Wabern</rdfs:isDefinedBy>
	<skos:definition xml:lang="en">The Monte Leone Nappe is the highest of the Lepontic units in the Toce Culmination. It is involved in the large synformal Berisal Backfold and further east, after following the Rhône-Simplon Fault, in the Alpe Bosa-Wandfluhhorn double fold. This nappe consists mainly of a crystalline basement made of various orthogneisses (Ordovician and Permo-Carboniferous) and paragneisses, covered by a relatively reduced  Triassic–Cretaceous(–Paleogene?) sedimentary series. A particularity of this nappe is the presence of a large ultramafic body (Geisspfad) within the gneisses.</skos:definition>
	<skos:inScheme rdf:resource="https://dev-lexic.swissgeol.ch/TectonicUnits"/>
	<skos:prefLabel xml:lang="en">Monte Leone Nappe</skos:prefLabel>
	<skos:prefLabel xml:lang="de">Monte-Leone-Decke</skos:prefLabel>
	<skos:prefLabel xml:lang="fr">Nappe du Monte Leone</skos:prefLabel>
	<skos:prefLabel xml:lang="it">Falda del Monte Leone</skos:prefLabel>
	<skos:broader rdf:resource="https://dev-lexic.swissgeol.ch/TectonicUnits/Lepontic"/>
	<status xmlns="http://www.w3.org/ns/adms#" rdf:resource="https://dev-lexic.swissgeol.ch/active"/>
</rdf:Description>

<rdf:Description rdf:about="https://dev-lexic.swissgeol.ch/TectonicUnits/MoncuccoNappe">
	<rdf:type rdf:resource="http://www.w3.org/2004/02/skos/core#Concept"/>
	<rdfs:isDefinedBy xml:lang="en">Gouffon Yves (Editor) (2024): Tectonic Map of Switzerland 1:500000, Explanatory notes. Federal Office of Topography swisstopo, Wabern</rdfs:isDefinedBy>
	<skos:definition xml:lang="en">The Moncucco Nappe occupies the core of the Vanzone Antiform in the Valle d’Ossola. It consists of a crystalline basement intruded by a Permian granite and is interpreted as the equivalent of the Monte Leone Nappe in the hangingwall of the Simplon Fault. Similar to that nappe, the Moncucco Nappe contains a large ultramafic body at its top.</skos:definition>
	<skos:inScheme rdf:resource="https://dev-lexic.swissgeol.ch/TectonicUnits"/>
	<skos:prefLabel xml:lang="en">Moncucco Nappe</skos:prefLabel>
	<skos:prefLabel xml:lang="de">Moncucco-Decke</skos:prefLabel>
	<skos:prefLabel xml:lang="fr">Nappe du Moncucco</skos:prefLabel>
	<skos:prefLabel xml:lang="it">Falda del Moncucco</skos:prefLabel>
	<skos:broader rdf:resource="https://dev-lexic.swissgeol.ch/TectonicUnits/Lepontic"/>
	<status xmlns="http://www.w3.org/ns/adms#" rdf:resource="https://dev-lexic.swissgeol.ch/active"/>
</rdf:Description>

<rdf:Description rdf:about="https://dev-lexic.swissgeol.ch/TectonicUnits/IsornoZone">
	<rdf:type rdf:resource="http://www.w3.org/2004/02/skos/core#Concept"/>
	<rdfs:isDefinedBy xml:lang="en">Gouffon Yves (Editor) (2024): Tectonic Map of Switzerland 1:500000, Explanatory notes. Federal Office of Topography swisstopo, Wabern</rdfs:isDefinedBy>
	<skos:definition xml:lang="en">The Isorno Zone corresponds to the Bosco and Bombogno zones in the southern part of the eastern (upper) limb of the large polyphase Alpe Bosa-Wandfluhhorn Fold (located between the Maggia and Antigorio valleys), where these two zones cannot be distinguished.</skos:definition>
	<skos:inScheme rdf:resource="https://dev-lexic.swissgeol.ch/TectonicUnits"/>
	<skos:prefLabel xml:lang="en">Isorno Zone</skos:prefLabel>
	<skos:prefLabel xml:lang="de">Isorno-Zone</skos:prefLabel>
	<skos:prefLabel xml:lang="fr">Zone de l'Isorno</skos:prefLabel>
	<skos:prefLabel xml:lang="it">Zona dell'Isorno</skos:prefLabel>
	<skos:broader rdf:resource="https://dev-lexic.swissgeol.ch/TectonicUnits/Lepontic"/>
	<skos:related rdf:resource="https://dev-lexic.swissgeol.ch/TectonicUnits/BoscoZone"/>
	<status xmlns="http://www.w3.org/ns/adms#" rdf:resource="https://dev-lexic.swissgeol.ch/active"/>
</rdf:Description>

<rdf:Description rdf:about="https://dev-lexic.swissgeol.ch/TectonicUnits/Orselina-BellinzonaZone">
	<rdf:type rdf:resource="http://www.w3.org/2004/02/skos/core#Concept"/>
	<rdfs:isDefinedBy xml:lang="en">Gouffon Yves (Editor) (2024): Tectonic Map of Switzerland 1:500000, Explanatory notes. Federal Office of Topography swisstopo, Wabern</rdfs:isDefinedBy>
	<skos:definition xml:lang="en">The Orselina-Bellinzona Zone is continuous between the Valle d’Ossola and Bellinzona. It is located between the Antigorio Nappe and the Centovalli Fault west of Locarno and between the Mergoscia Zone and the Tonale Fault further east. It is lithologically similar to the Isorno Zone.</skos:definition>
	<skos:inScheme rdf:resource="https://dev-lexic.swissgeol.ch/TectonicUnits"/>
	<skos:prefLabel xml:lang="en">Orselina-Bellinzona Zone</skos:prefLabel>
	<skos:prefLabel xml:lang="de">Orselina-Bellinzona-Zone</skos:prefLabel>
	<skos:prefLabel xml:lang="fr">Zone d'Orselina-Bellinzona</skos:prefLabel>
	<skos:prefLabel xml:lang="it">Zona di Orselina-Bellinzona</skos:prefLabel>
	<skos:broader rdf:resource="https://dev-lexic.swissgeol.ch/TectonicUnits/Lepontic"/>
	<status xmlns="http://www.w3.org/ns/adms#" rdf:resource="https://dev-lexic.swissgeol.ch/active"/>
</rdf:Description>

<rdf:Description rdf:about="https://dev-lexic.swissgeol.ch/TectonicUnits/BoscoZone">
	<rdf:type rdf:resource="http://www.w3.org/2004/02/skos/core#Concept"/>
	<rdfs:isDefinedBy xml:lang="en">Gouffon Yves (Editor) (2024): Tectonic Map of Switzerland 1:500000, Explanatory notes. Federal Office of Topography swisstopo, Wabern</rdfs:isDefinedBy>
	<skos:definition xml:lang="en">The Bosco Zone (Western Lepontic) is situated in the western (lower) limb of the large polyphase Alpe Bosa-Wandfluhhorn Fold (located between the Maggia and Antigorio valleys), where it is surrounded by the Bombogno Zone (resp. the Antigorio and Monte Leone nappes). It consists of a crystalline basement of sedimentary origin (micaschists) intruded by orthogneiss masses and veins. It underwent an Oligocene amphibolite facies metamorphism.</skos:definition>
	<skos:inScheme rdf:resource="https://dev-lexic.swissgeol.ch/TectonicUnits"/>
	<skos:prefLabel xml:lang="en">Bosco Zone</skos:prefLabel>
	<skos:prefLabel xml:lang="de">Bosco-Zone</skos:prefLabel>
	<skos:prefLabel xml:lang="fr">Zone de Bosco</skos:prefLabel>
	<skos:prefLabel xml:lang="it">Zona di Bosco</skos:prefLabel>
	<skos:broader rdf:resource="https://dev-lexic.swissgeol.ch/TectonicUnits/Lepontic"/>
	<skos:related rdf:resource="https://dev-lexic.swissgeol.ch/TectonicUnits/IsornoZone"/>
	<status xmlns="http://www.w3.org/ns/adms#" rdf:resource="https://dev-lexic.swissgeol.ch/active"/>
</rdf:Description>

<rdf:Description rdf:about="https://dev-lexic.swissgeol.ch/TectonicUnits/BombognoZone">
	<rdf:type rdf:resource="http://www.w3.org/2004/02/skos/core#Concept"/>
	<rdfs:isDefinedBy xml:lang="en">Gouffon Yves (Editor) (2024): Tectonic Map of Switzerland 1:500000, Explanatory notes. Federal Office of Topography swisstopo, Wabern</rdfs:isDefinedBy>
	<skos:definition xml:lang="en">The Bombogno Zone (Western Lepontic) is situated in the western (lower) limb of the large polyphase Alpe Bosa-Wandfluhhorn Fold (located between the Maggia and Antigorio valleys), where it surrounds the Bosco Zone. It consists of a very heterogeneous series mainly of metasedimentary origin (calcschists, micaschists, paragneiss), with subordinated mafic and ultramafic bodies. It underwent an Oligocene amphibolite facies metamorphism.</skos:definition>
	<skos:inScheme rdf:resource="https://dev-lexic.swissgeol.ch/TectonicUnits"/>
	<skos:prefLabel xml:lang="en">Bombogno Zone</skos:prefLabel>
	<skos:prefLabel xml:lang="de">Bombogno-Zone</skos:prefLabel>
	<skos:prefLabel xml:lang="fr">Zone du Bombogno</skos:prefLabel>
	<skos:prefLabel xml:lang="it">Zona del Bombogno</skos:prefLabel>
	<skos:broader rdf:resource="https://dev-lexic.swissgeol.ch/TectonicUnits/Lepontic"/>
	<skos:related rdf:resource="https://dev-lexic.swissgeol.ch/TectonicUnits/IsornoZone"/>
	<status xmlns="http://www.w3.org/ns/adms#" rdf:resource="https://dev-lexic.swissgeol.ch/active"/>
</rdf:Description>

<rdf:Description rdf:about="https://dev-lexic.swissgeol.ch/TectonicUnits/MaggiaNappe">
	<rdf:type rdf:resource="http://www.w3.org/2004/02/skos/core#Concept"/>
	<rdfs:isDefinedBy xml:lang="en">Gouffon Yves (Editor) (2024): Tectonic Map of Switzerland 1:500000, Explanatory notes. Federal Office of Topography swisstopo, Wabern</rdfs:isDefinedBy>
	<skos:definition xml:lang="en">The Maggia Nappe (together with the cartographic disjunct Sambuco Nappe) occupies the NNW–SSE oriented transverse synformal zone in the middle of the structural Lepontine Dome. It is made up of basement rocks intruded by Variscan granitoids (Late Carboniferous).</skos:definition>
	<skos:inScheme rdf:resource="https://dev-lexic.swissgeol.ch/TectonicUnits"/>
	<skos:prefLabel xml:lang="en">Maggia Nappe</skos:prefLabel>
	<skos:prefLabel xml:lang="de">Maggia-Decke</skos:prefLabel>
	<skos:prefLabel xml:lang="fr">Nappe de la Maggia</skos:prefLabel>
	<skos:prefLabel xml:lang="it">Falda della Maggia</skos:prefLabel>
	<skos:broader rdf:resource="https://dev-lexic.swissgeol.ch/TectonicUnits/Lepontic"/>
	<status xmlns="http://www.w3.org/ns/adms#" rdf:resource="https://dev-lexic.swissgeol.ch/active"/>
</rdf:Description>

<rdf:Description rdf:about="https://dev-lexic.swissgeol.ch/TectonicUnits/SambucoNappe">
	<rdf:type rdf:resource="http://www.w3.org/2004/02/skos/core#Concept"/>
	<rdfs:isDefinedBy xml:lang="en">Gouffon Yves (Editor) (2024): Tectonic Map of Switzerland 1:500000, Explanatory notes. Federal Office of Topography swisstopo, Wabern</rdfs:isDefinedBy>
	<skos:definition xml:lang="en">The Sambuco Nappe (together with the cartographic disjunct Maggia Nappe) occupies the NNW–SSE oriented transverse synformal zone in the middle of the structural Lepontine Dome. It is made up of basement rocks intruded by Variscan granitoids (Late Carboniferous) with a thin sedimentary cover of Helvetic facies affinity.</skos:definition>
	<skos:inScheme rdf:resource="https://dev-lexic.swissgeol.ch/TectonicUnits"/>
	<skos:prefLabel xml:lang="en">Sambuco Nappe</skos:prefLabel>
	<skos:prefLabel xml:lang="de">Sambuco-Decke</skos:prefLabel>
	<skos:prefLabel xml:lang="fr">Nappe du Sambuco</skos:prefLabel>
	<skos:prefLabel xml:lang="it">Falda del Sambuco</skos:prefLabel>
	<skos:broader rdf:resource="https://dev-lexic.swissgeol.ch/TectonicUnits/Lepontic"/>
	<status xmlns="http://www.w3.org/ns/adms#" rdf:resource="https://dev-lexic.swissgeol.ch/active"/>
</rdf:Description>

<rdf:Description rdf:about="https://dev-lexic.swissgeol.ch/TectonicUnits/SanGiorgioSlice">
	<rdf:type rdf:resource="http://www.w3.org/2004/02/skos/core#Concept"/>
	<rdfs:isDefinedBy xml:lang="en">Gouffon Yves (Editor) (2024): Tectonic Map of Switzerland 1:500000, Explanatory notes. Federal Office of Topography swisstopo, Wabern</rdfs:isDefinedBy>
	<skos:definition xml:lang="en">The San Giorgio Slice, located in the Valle Leventina, is a small tectonic unit of the Eastern Lepontic (Ticino Culmination) similar to the Soja Nappe. It consists of a crystalline basement (micaschists with metaconglomerate layers) and its Triassic sedimentary cover.</skos:definition>
	<skos:inScheme rdf:resource="https://dev-lexic.swissgeol.ch/TectonicUnits"/>
	<skos:prefLabel xml:lang="en">San Giorgio Slice</skos:prefLabel>
	<skos:prefLabel xml:lang="de">San-Giorgio-Schuppe</skos:prefLabel>
	<skos:prefLabel xml:lang="fr">Écaille de San Giorgio</skos:prefLabel>
	<skos:prefLabel xml:lang="it">Scaglia di San Giorgio</skos:prefLabel>
	<skos:broader rdf:resource="https://dev-lexic.swissgeol.ch/TectonicUnits/Lepontic"/>
	<status xmlns="http://www.w3.org/ns/adms#" rdf:resource="https://dev-lexic.swissgeol.ch/active"/>
</rdf:Description>

<rdf:Description rdf:about="https://dev-lexic.swissgeol.ch/TectonicUnits/Leventina-LucomagnoNappe">
	<rdf:type rdf:resource="http://www.w3.org/2004/02/skos/core#Concept"/>
	<rdfs:isDefinedBy xml:lang="en">Gouffon Yves (Editor) (2024): Tectonic Map of Switzerland 1:500000, Explanatory notes. Federal Office of Topography swisstopo, Wabern</rdfs:isDefinedBy>
	<skos:definition xml:lang="en">The Leventina-Lucomagno Nappe is the lowest unit of the Ticino Culmination. It consists of a Late Variscan magmatic edifice (“Leventina Unit”) covered by a thick stack of paragneisses and micaschists (“Lucomagno Unit”). Sparse quartzitic gneisses (“roof quartzites”) occur at the boundariy between these units and were interpreted as being Mesozoic in age by several authors and hence used to discriminate between a “Leventina Nappe” and a “Lucomagno Nappe”. However, these quartz-rich horizons above the orthogneisses form metasomatically altered zones – in places sheared – and cannot be considered as Mesozoic metasediments.</skos:definition>
	<skos:inScheme rdf:resource="https://dev-lexic.swissgeol.ch/TectonicUnits"/>
	<skos:prefLabel xml:lang="en">Leventina-Lucomagno Nappe</skos:prefLabel>
	<skos:prefLabel xml:lang="de">Leventina-Lucomagno-Decke</skos:prefLabel>
	<skos:prefLabel xml:lang="fr">Nappe de la Leventina-Lucomagno</skos:prefLabel>
	<skos:prefLabel xml:lang="it">Falda della Leventina-Lucomagno</skos:prefLabel>
	<skos:altLabel xml:lang="fr">nappe du Lukmanier</skos:altLabel>
	<skos:broader rdf:resource="https://dev-lexic.swissgeol.ch/TectonicUnits/Lepontic"/>
	<status xmlns="http://www.w3.org/ns/adms#" rdf:resource="https://dev-lexic.swissgeol.ch/active"/>
</rdf:Description>

<rdf:Description rdf:about="https://dev-lexic.swissgeol.ch/TectonicUnits/SimanoNappe">
	<rdf:type rdf:resource="http://www.w3.org/2004/02/skos/core#Concept"/>
	<rdfs:isDefinedBy xml:lang="en">Gouffon Yves (Editor) (2024): Tectonic Map of Switzerland 1:500000, Explanatory notes. Federal Office of Topography swisstopo, Wabern</rdfs:isDefinedBy>
	<skos:definition xml:lang="en">The Simano Nappe consists of a heterogenous metamorphosed magmatic complex intruded into pre-Variscan paragneisses, forming today the orthogneisses that dominate the southern and the western part of the nappe. The eastern part contains Ordovician orthogneisses within paragneisses and the northern part consists of semi- to metapelitic gneisses, micaschists, amphibolites and sporadic lenses of ultramafic rocks, locally covered by Permian and Triassic sedimentary rocks. The frontal part of the Simano Nappe, forming a large-scale recumbent fold, is bordered by metacarbonates, considered to be the Mesozoic sedimentary cover of the nappe.</skos:definition>
	<skos:inScheme rdf:resource="https://dev-lexic.swissgeol.ch/TectonicUnits"/>
	<skos:prefLabel xml:lang="en">Simano Nappe</skos:prefLabel>
	<skos:prefLabel xml:lang="de">Simano-Decke</skos:prefLabel>
	<skos:prefLabel xml:lang="fr">Nappe du Simano</skos:prefLabel>
	<skos:prefLabel xml:lang="it">Falda del Simano</skos:prefLabel>
	<skos:broader rdf:resource="https://dev-lexic.swissgeol.ch/TectonicUnits/Lepontic"/>
	<status xmlns="http://www.w3.org/ns/adms#" rdf:resource="https://dev-lexic.swissgeol.ch/active"/>
</rdf:Description>

<rdf:Description rdf:about="https://dev-lexic.swissgeol.ch/TectonicUnits/CimaLungaNappe">
	<rdf:type rdf:resource="http://www.w3.org/2004/02/skos/core#Concept"/>
	<rdfs:isDefinedBy xml:lang="en">Gouffon Yves (Editor) (2024): Tectonic Map of Switzerland 1:500000, Explanatory notes. Federal Office of Topography swisstopo, Wabern</rdfs:isDefinedBy>
	<skos:definition xml:lang="en">The Cima Lunga Nappe is a tectonic unit of the Eastern Lepontic (Ticino Culmination). It is made up of paragneisses, orthogneisses, sheets of marble and calcschist as well as lenses of mafic and ultramafic rocks that locally have an incoherent character. Eclogitic mineral assemblages are widespread in the mafic and ultramafic rocks. Sheath folds around the disrupted competent mafic and ultramafic lenses suggest intense shearing within a shear zone at the base of the Maggia Nappe. According to most authors, the Cima Lunga Nappe is connected in the east, to the Adula Nappe in the lower Valle Mesolcina.</skos:definition>
	<skos:inScheme rdf:resource="https://dev-lexic.swissgeol.ch/TectonicUnits"/>
	<skos:prefLabel xml:lang="en">Cima Lunga Nappe</skos:prefLabel>
	<skos:prefLabel xml:lang="de">Cima-Lunga-Decke</skos:prefLabel>
	<skos:prefLabel xml:lang="fr">Nappe de la Cima Lunga</skos:prefLabel>
	<skos:prefLabel xml:lang="it">Falda della Cima Lunga</skos:prefLabel>
	<skos:broader rdf:resource="https://dev-lexic.swissgeol.ch/TectonicUnits/Lepontic"/>
	<status xmlns="http://www.w3.org/ns/adms#" rdf:resource="https://dev-lexic.swissgeol.ch/active"/>
</rdf:Description>

<rdf:Description rdf:about="https://dev-lexic.swissgeol.ch/TectonicUnits/AdulaNappe">
	<rdf:type rdf:resource="http://www.w3.org/2004/02/skos/core#Concept"/>
	<rdfs:isDefinedBy xml:lang="en">Gouffon Yves (Editor) (2024): Tectonic Map of Switzerland 1:500000, Explanatory notes. Federal Office of Topography swisstopo, Wabern</rdfs:isDefinedBy>
	<skos:definition xml:lang="en">The Adula Nappe is a tectonic unit of the Eastern Lepontic (Ticino Culmination). It consists of a Paleozoic crystalline basement (orthogneisses, paragneisses and lenses of mafic and ultramafic rock) which experienced high-pressure Alpine metamorphism under eclogite-facies conditions. A reduced series of Mesozoic sediments is locally preserved in the cores of the synclines.</skos:definition>
	<skos:inScheme rdf:resource="https://dev-lexic.swissgeol.ch/TectonicUnits"/>
	<skos:prefLabel xml:lang="en">Adula Nappe</skos:prefLabel>
	<skos:prefLabel xml:lang="de">Adula-Decke</skos:prefLabel>
	<skos:prefLabel xml:lang="fr">Nappe de l'Adula</skos:prefLabel>
	<skos:prefLabel xml:lang="it">Falda dell'Adula</skos:prefLabel>
	<skos:broader rdf:resource="https://dev-lexic.swissgeol.ch/TectonicUnits/Lepontic"/>
	<status xmlns="http://www.w3.org/ns/adms#" rdf:resource="https://dev-lexic.swissgeol.ch/active"/>
</rdf:Description>

<rdf:Description rdf:about="https://dev-lexic.swissgeol.ch/TectonicUnits/GrufComplex">
	<rdf:type rdf:resource="http://www.w3.org/2004/02/skos/core#Concept"/>
	<rdfs:isDefinedBy xml:lang="en">Gouffon Yves (Editor) (2024): Tectonic Map of Switzerland 1:500000, Explanatory notes. Federal Office of Topography swisstopo, Wabern</rdfs:isDefinedBy>
	<skos:definition xml:lang="en">The Gruf Complex is a polymetamorphic migmatitic unit of the Eastern Lepontic (Ticino Culmination), interpreted as a lower crust compartment (possibly related to the Adula Nappe) that was dragged up by the rise of the Bregaglia Intrusion. It directly underlies the Tambo Nappe and the ophiolitic Chiavenna Nappe to the north along a steeply N-dipping fault and follows the base of the Bregaglia Intrusion to the south.</skos:definition>
	<skos:inScheme rdf:resource="https://dev-lexic.swissgeol.ch/TectonicUnits"/>
	<skos:prefLabel xml:lang="en">Gruf Complex</skos:prefLabel>
	<skos:prefLabel xml:lang="de">Gruf-Komplex</skos:prefLabel>
	<skos:prefLabel xml:lang="fr">Complexe du Gruf</skos:prefLabel>
	<skos:prefLabel xml:lang="it">Complesso del Gruf</skos:prefLabel>
	<skos:broader rdf:resource="https://dev-lexic.swissgeol.ch/TectonicUnits/Lepontic"/>
	<status xmlns="http://www.w3.org/ns/adms#" rdf:resource="https://dev-lexic.swissgeol.ch/active"/>
</rdf:Description>

<rdf:Description rdf:about="https://dev-lexic.swissgeol.ch/TectonicUnits/SojaNappe">
	<rdf:type rdf:resource="http://www.w3.org/2004/02/skos/core#Concept"/>
	<rdfs:isDefinedBy xml:lang="en">Gouffon Yves (Editor) (2024): Tectonic Map of Switzerland 1:500000, Explanatory notes. Federal Office of Topography swisstopo, Wabern</rdfs:isDefinedBy>
	<skos:definition xml:lang="en">The Soja Nappe is a small tectonic unit of the Eastern Lepontic (Ticino Culmination) located between the overlying frontal part of Adula Nappe and the underlying Simano Nappe. To the north, it extends into the Garzott Slices located in the core of the Lunschania Antiform and surrounded by the Piz Terri-Lunschania Nappe. It includes a polycyclic crystalline basement covered by Permian to Jurassic sediments.</skos:definition>
	<skos:inScheme rdf:resource="https://dev-lexic.swissgeol.ch/TectonicUnits"/>
	<skos:prefLabel xml:lang="en">Soja Nappe</skos:prefLabel>
	<skos:prefLabel xml:lang="de">Soja-Decke</skos:prefLabel>
	<skos:prefLabel xml:lang="fr">Nappe de Soja</skos:prefLabel>
	<skos:prefLabel xml:lang="it">Falda di Soja</skos:prefLabel>
	<skos:broader rdf:resource="https://dev-lexic.swissgeol.ch/TectonicUnits/Lepontic"/>
	<skos:narrower rdf:resource="https://dev-lexic.swissgeol.ch/TectonicUnits/GarzottSlices"/>
	<status xmlns="http://www.w3.org/ns/adms#" rdf:resource="https://dev-lexic.swissgeol.ch/active"/>
</rdf:Description>

<rdf:Description rdf:about="https://dev-lexic.swissgeol.ch/TectonicUnits/PizTerri-LunschaniaNappe">
	<rdf:type rdf:resource="http://www.w3.org/2004/02/skos/core#Concept"/>
	<rdfs:isDefinedBy xml:lang="en">Gouffon Yves (Editor) (2024): Tectonic Map of Switzerland 1:500000, Explanatory notes. Federal Office of Topography swisstopo, Wabern</rdfs:isDefinedBy>
	<skos:definition xml:lang="en">The Piz Terri-Lunschania Nappe (Eastern Lepontic) consists of several slices made up of Permian and Mesozoic sediments. This nappe forms the large isoclinal Lunschania Antiform situated in front of the Adula Nappe and surrounded by the Grava Nappe.</skos:definition>
	<skos:inScheme rdf:resource="https://dev-lexic.swissgeol.ch/TectonicUnits"/>
	<skos:prefLabel xml:lang="en">Piz Terri - Lunschania Nappe</skos:prefLabel>
	<skos:prefLabel xml:lang="de">Piz-Terri-Lunschania-Decke</skos:prefLabel>
	<skos:prefLabel xml:lang="fr">Nappe du Piz Terri - Lunschania</skos:prefLabel>
	<skos:prefLabel xml:lang="it">Falda del Piz Terri - Lunschania</skos:prefLabel>
	<skos:broader rdf:resource="https://dev-lexic.swissgeol.ch/TectonicUnits/Lepontic"/>
	<skos:narrower rdf:resource="https://dev-lexic.swissgeol.ch/TectonicUnits/TerriSlice"/>
	<skos:narrower rdf:resource="https://dev-lexic.swissgeol.ch/TectonicUnits/Gueida-AlpettasSlices"/>
	<skos:narrower rdf:resource="https://dev-lexic.swissgeol.ch/TectonicUnits/DarlunSlice"/>
	<status xmlns="http://www.w3.org/ns/adms#" rdf:resource="https://dev-lexic.swissgeol.ch/active"/>
</rdf:Description>

<rdf:Description rdf:about="https://dev-lexic.swissgeol.ch/TectonicUnits/PizzoDelValloneNappe">
	<rdf:type rdf:resource="http://www.w3.org/2004/02/skos/core#Concept"/>
	<rdfs:isDefinedBy xml:lang="en">Gouffon Yves (Editor) (2024): Tectonic Map of Switzerland 1:500000, Explanatory notes. Federal Office of Topography swisstopo, Wabern</rdfs:isDefinedBy>
	<skos:definition xml:lang="en">The Pizzo del Vallone Nappe surrounds the Monte Leone Nappe mainly in the large synformal Berisal Backfold. It is composed of a detrital sedimentary series covering the entire Mesozoic and possibly the Paleogene, characterized by Jurassic basaltic rocks. In the western part of the nappe, both north and south of the Monte Leone Nappe, occur the crystalline basement of these metasediments.</skos:definition>
	<skos:inScheme rdf:resource="https://dev-lexic.swissgeol.ch/TectonicUnits"/>
	<skos:prefLabel xml:lang="en">Pizzo del Vallone Nappe</skos:prefLabel>
	<skos:prefLabel xml:lang="de">Pizzo-del-Vallone-Decke</skos:prefLabel>
	<skos:prefLabel xml:lang="fr">Nappe du Pizzo del Vallone</skos:prefLabel>
	<skos:prefLabel xml:lang="it">Falda del Pizzo del Vallone</skos:prefLabel>
	<skos:broader rdf:resource="https://dev-lexic.swissgeol.ch/TectonicUnits/Lepontic"/>
	<status xmlns="http://www.w3.org/ns/adms#" rdf:resource="https://dev-lexic.swissgeol.ch/active"/>
</rdf:Description>

<rdf:Description rdf:about="https://dev-lexic.swissgeol.ch/TectonicUnits/AntigorioNappe">
	<rdf:type rdf:resource="http://www.w3.org/2004/02/skos/core#Concept"/>
	<rdfs:isDefinedBy xml:lang="en">Gouffon Yves (Editor) (2024): Tectonic Map of Switzerland 1:500000, Explanatory notes. Federal Office of Topography swisstopo, Wabern</rdfs:isDefinedBy>
	<skos:definition xml:lang="en">The Antigorio Nappe is a tectonic nappe of the Western Lepontic (Toce Culimnation) consisting mainly of Variscan granitoids. In its northwestern part, this basement is surrounded by an autochthonous Mesozoic–Paleogene sedimentary cover, which could be connected to the cover of the Verampio Nappe via an early thrust syncline. Late folding is responsible for two multi-kilometer-scale isoclinal structures: the Alpe Bosa-Wandfluhhorn fold and the Ziccher fold.</skos:definition>
	<skos:inScheme rdf:resource="https://dev-lexic.swissgeol.ch/TectonicUnits"/>
	<skos:prefLabel xml:lang="en">Antigorio Nappe</skos:prefLabel>
	<skos:prefLabel xml:lang="de">Antigorio-Decke</skos:prefLabel>
	<skos:prefLabel xml:lang="fr">Nappe d'Antigorio</skos:prefLabel>
	<skos:prefLabel xml:lang="it">Falda di Antigorio</skos:prefLabel>
	<skos:broader rdf:resource="https://dev-lexic.swissgeol.ch/TectonicUnits/AntigorioNappeComplex"/>
	<status xmlns="http://www.w3.org/ns/adms#" rdf:resource="https://dev-lexic.swissgeol.ch/active"/>
</rdf:Description>

<rdf:Description rdf:about="https://dev-lexic.swissgeol.ch/TectonicUnits/MergosciaZone">
	<rdf:type rdf:resource="http://www.w3.org/2004/02/skos/core#Concept"/>
	<rdfs:isDefinedBy xml:lang="en">Gouffon Yves (Editor) (2024): Tectonic Map of Switzerland 1:500000, Explanatory notes. Federal Office of Topography swisstopo, Wabern</rdfs:isDefinedBy>
	<skos:definition xml:lang="en">The Mergoscia Zone is a heterogeneous tectonic unit of the Western Lepontic (Toce Culimnation). It is composed of ortho- and paragneisses, metapelites, calcschists, metabasites and meta-ultrabasites. Both metabasites and meta-ultrabasites contain rare relics of high-pressure metamorphism (retrogressed eclogites and garnet-metaperidotites). This zone, displaying a high degree of deformation, is also interpreted as a mélange rather than as an originally stratified framework.</skos:definition>
	<skos:inScheme rdf:resource="https://dev-lexic.swissgeol.ch/TectonicUnits"/>
	<skos:prefLabel xml:lang="en">Mergoscia Zone</skos:prefLabel>
	<skos:prefLabel xml:lang="de">Mergoscia-Zone</skos:prefLabel>
	<skos:prefLabel xml:lang="fr">Zone de Mergoscia</skos:prefLabel>
	<skos:prefLabel xml:lang="it">Zona di Mergoscia</skos:prefLabel>
	<skos:broader rdf:resource="https://dev-lexic.swissgeol.ch/TectonicUnits/AntigorioNappeComplex"/>
	<status xmlns="http://www.w3.org/ns/adms#" rdf:resource="https://dev-lexic.swissgeol.ch/active"/>
</rdf:Description>

<rdf:Description rdf:about="https://dev-lexic.swissgeol.ch/TectonicUnits/GarzottSlices">
	<rdf:type rdf:resource="http://www.w3.org/2004/02/skos/core#Concept"/>
	<rdfs:isDefinedBy xml:lang="en">Gouffon Yves (Editor) (2024): Tectonic Map of Switzerland 1:500000, Explanatory notes. Federal Office of Topography swisstopo, Wabern</rdfs:isDefinedBy>
	<skos:definition xml:lang="en">The Garzott Slices are considered as a northern extension of the Soja Nappe in the core of the Lunschania Antiform, where they are surrounded by the Piz Terri-Lunschania Nappe. Due to this structural position, Galster et al. (2012) attached the Garzott Slices to the Piz Terri-Lunschania Nappe, but the facies analogies bring them closer to the Soja Nappe (Vögeli et al. 2013).</skos:definition>
	<skos:inScheme rdf:resource="https://dev-lexic.swissgeol.ch/TectonicUnits"/>
	<skos:prefLabel xml:lang="en">Garzott Slices</skos:prefLabel>
	<skos:prefLabel xml:lang="de">Garzott-Schuppen</skos:prefLabel>
	<skos:prefLabel xml:lang="fr">Écailles de Garzott</skos:prefLabel>
	<skos:prefLabel xml:lang="it">Scaglie di Garzott</skos:prefLabel>
	<skos:broader rdf:resource="https://dev-lexic.swissgeol.ch/TectonicUnits/SojaNappe"/>
	<status xmlns="http://www.w3.org/ns/adms#" rdf:resource="https://dev-lexic.swissgeol.ch/active"/>
</rdf:Description>

<rdf:Description rdf:about="https://dev-lexic.swissgeol.ch/TectonicUnits/TerriSlice">
	<rdf:type rdf:resource="http://www.w3.org/2004/02/skos/core#Concept"/>
	<rdfs:isDefinedBy xml:lang="en">Gouffon Yves (Editor) (2024): Tectonic Map of Switzerland 1:500000, Explanatory notes. Federal Office of Topography swisstopo, Wabern</rdfs:isDefinedBy>
	<skos:inScheme rdf:resource="https://dev-lexic.swissgeol.ch/TectonicUnits"/>
	<skos:prefLabel xml:lang="en">Terri Slice</skos:prefLabel>
	<skos:prefLabel xml:lang="de">Terri-Schuppe</skos:prefLabel>
	<skos:prefLabel xml:lang="fr">Écaille du Terri</skos:prefLabel>
	<skos:prefLabel xml:lang="it">Scaglia del Terri</skos:prefLabel>
	<skos:broader rdf:resource="https://dev-lexic.swissgeol.ch/TectonicUnits/PizTerri-LunschaniaNappe"/>
	<status xmlns="http://www.w3.org/ns/adms#" rdf:resource="https://dev-lexic.swissgeol.ch/active"/>
</rdf:Description>

<rdf:Description rdf:about="https://dev-lexic.swissgeol.ch/TectonicUnits/Gueida-AlpettasSlices">
	<rdf:type rdf:resource="http://www.w3.org/2004/02/skos/core#Concept"/>
	<rdfs:isDefinedBy xml:lang="en">Gouffon Yves (Editor) (2024): Tectonic Map of Switzerland 1:500000, Explanatory notes. Federal Office of Topography swisstopo, Wabern</rdfs:isDefinedBy>
	<skos:inScheme rdf:resource="https://dev-lexic.swissgeol.ch/TectonicUnits"/>
	<skos:prefLabel xml:lang="en">Güida-Alpettas Slices</skos:prefLabel>
	<skos:prefLabel xml:lang="de">Güida-Alpettas-Schuppen</skos:prefLabel>
	<skos:prefLabel xml:lang="fr">Écailles de Güida-Alpettas</skos:prefLabel>
	<skos:prefLabel xml:lang="it">Scaglie di Güida-Alpettas</skos:prefLabel>
	<skos:broader rdf:resource="https://dev-lexic.swissgeol.ch/TectonicUnits/PizTerri-LunschaniaNappe"/>
	<status xmlns="http://www.w3.org/ns/adms#" rdf:resource="https://dev-lexic.swissgeol.ch/active"/>
</rdf:Description>

<rdf:Description rdf:about="https://dev-lexic.swissgeol.ch/TectonicUnits/DarlunSlice">
	<rdf:type rdf:resource="http://www.w3.org/2004/02/skos/core#Concept"/>
	<rdfs:isDefinedBy xml:lang="en">Gouffon Yves (Editor) (2024): Tectonic Map of Switzerland 1:500000, Explanatory notes. Federal Office of Topography swisstopo, Wabern</rdfs:isDefinedBy>
	<skos:inScheme rdf:resource="https://dev-lexic.swissgeol.ch/TectonicUnits"/>
	<skos:prefLabel xml:lang="en">Darlun Slice</skos:prefLabel>
	<skos:prefLabel xml:lang="de">Darlun-Schuppe</skos:prefLabel>
	<skos:prefLabel xml:lang="fr">Écaille de Darlun</skos:prefLabel>
	<skos:prefLabel xml:lang="it">Scaglia di Darlun</skos:prefLabel>
	<skos:broader rdf:resource="https://dev-lexic.swissgeol.ch/TectonicUnits/PizTerri-LunschaniaNappe"/>
	<status xmlns="http://www.w3.org/ns/adms#" rdf:resource="https://dev-lexic.swissgeol.ch/active"/>
</rdf:Description>

<rdf:Description rdf:about="https://dev-lexic.swissgeol.ch/TectonicUnits/Penninic">
	<rdf:type rdf:resource="http://www.w3.org/2004/02/skos/core#Concept"/>
	<rdfs:isDefinedBy xml:lang="en">Gouffon Yves (Editor) (2024): Tectonic Map of Switzerland 1:500000, Explanatory notes. Federal Office of Topography swisstopo, Wabern</rdfs:isDefinedBy>
	<rdfs:comment rdf:datatype="http://www.w3.org/1999/02/22-rdf-syntax-ns#HTML">https://data.geo.admin.ch/ch.swisstopo.geologie-tektonische_karte/pdf/Erl-TK500_2024.pdf</rdfs:comment>
	<skos:definition xml:lang="en">The Penninic domain comprises all tectonic units situated between the Helvetic or the Lepontic domains and the Austroalpine or the Salassic domains. It also includes units that were transported further north on the Helvetic and which are currently found as klippen on top or in front of this domain (e.g. Prealps).</skos:definition>
	<skos:inScheme rdf:resource="https://dev-lexic.swissgeol.ch/TectonicUnits"/>
	<skos:topConceptOf rdf:resource="https://dev-lexic.swissgeol.ch/TectonicUnits"/>
	<skos:prefLabel xml:lang="en">Penninic</skos:prefLabel>
	<skos:prefLabel xml:lang="de">Penninikum</skos:prefLabel>
	<skos:prefLabel xml:lang="fr">Pennique</skos:prefLabel>
	<skos:prefLabel xml:lang="it">Pennidico</skos:prefLabel>
	<skos:narrower rdf:resource="https://dev-lexic.swissgeol.ch/TectonicUnits/LowerPenninic"/>
	<skos:narrower rdf:resource="https://dev-lexic.swissgeol.ch/TectonicUnits/MiddlePenninic"/>
	<skos:narrower rdf:resource="https://dev-lexic.swissgeol.ch/TectonicUnits/UpperPenninic"/>
	<status xmlns="http://www.w3.org/ns/adms#" rdf:resource="https://dev-lexic.swissgeol.ch/active"/>
</rdf:Description>

<rdf:Description rdf:about="https://dev-lexic.swissgeol.ch/TectonicUnits/LowerPenninic">
	<rdf:type rdf:resource="http://www.w3.org/2004/02/skos/core#Concept"/>
	<rdfs:isDefinedBy xml:lang="en">Gouffon Yves (Editor) (2024): Tectonic Map of Switzerland 1:500000, Explanatory notes. Federal Office of Topography swisstopo, Wabern</rdfs:isDefinedBy>
	<skos:definition xml:lang="en">The Lower Penninic tectonic units are derived paleogeographically from the Cretaceous-Paleogene Valaisan Ocean. The remains of this basin are now at the base of the Penninic nappe stack and were overthrust by units that were originally deposited further south.</skos:definition>
	<skos:inScheme rdf:resource="https://dev-lexic.swissgeol.ch/TectonicUnits"/>
	<skos:prefLabel xml:lang="en">Lower Penninic</skos:prefLabel>
	<skos:prefLabel xml:lang="de">Unterpenninikum</skos:prefLabel>
	<skos:prefLabel xml:lang="fr">Pennique inférieur</skos:prefLabel>
	<skos:prefLabel xml:lang="it">Pennidico inferiore</skos:prefLabel>
	<skos:broader rdf:resource="https://dev-lexic.swissgeol.ch/TectonicUnits/Penninic"/>
	<skos:narrower rdf:resource="https://dev-lexic.swissgeol.ch/TectonicUnits/NiesenNappe"/>
	<skos:narrower rdf:resource="https://dev-lexic.swissgeol.ch/TectonicUnits/VoironsNappe"/>
	<skos:narrower rdf:resource="https://dev-lexic.swissgeol.ch/TectonicUnits/GurnigelNappe"/>
	<skos:narrower rdf:resource="https://dev-lexic.swissgeol.ch/TectonicUnits/SchlierenNappe"/>
	<skos:narrower rdf:resource="https://dev-lexic.swissgeol.ch/TectonicUnits/WaegitalNappe"/>
	<skos:narrower rdf:resource="https://dev-lexic.swissgeol.ch/TectonicUnits/UentschenNappe"/>
	<skos:narrower rdf:resource="https://dev-lexic.swissgeol.ch/TectonicUnits/SigiswangNappe"/>
	<skos:narrower rdf:resource="https://dev-lexic.swissgeol.ch/TectonicUnits/TriesenbergSliceComplex"/>
	<skos:narrower rdf:resource="https://dev-lexic.swissgeol.ch/TectonicUnits/OberstdorfNappe"/>
	<skos:narrower rdf:resource="https://dev-lexic.swissgeol.ch/TectonicUnits/Sion-CourmayeurNappe"/>
	<skos:narrower rdf:resource="https://dev-lexic.swissgeol.ch/TectonicUnits/ChiavennaNappe"/>
	<skos:narrower rdf:resource="https://dev-lexic.swissgeol.ch/TectonicUnits/ValsSlices"/>
	<skos:narrower rdf:resource="https://dev-lexic.swissgeol.ch/TectonicUnits/AulNappe"/>
	<skos:narrower rdf:resource="https://dev-lexic.swissgeol.ch/TectonicUnits/GravaNappe"/>
	<skos:narrower rdf:resource="https://dev-lexic.swissgeol.ch/TectonicUnits/TomuelNappe"/>
	<skos:narrower rdf:resource="https://dev-lexic.swissgeol.ch/TectonicUnits/Roz-ChampatschMelange"/>
	<skos:narrower rdf:resource="https://dev-lexic.swissgeol.ch/TectonicUnits/RamoschZone"/>
	<skos:narrower rdf:resource="https://dev-lexic.swissgeol.ch/TectonicUnits/PfundsNappe"/>
	<status xmlns="http://www.w3.org/ns/adms#" rdf:resource="https://dev-lexic.swissgeol.ch/active"/>
</rdf:Description>

<rdf:Description rdf:about="https://dev-lexic.swissgeol.ch/TectonicUnits/MiddlePenninic">
	<rdf:type rdf:resource="http://www.w3.org/2004/02/skos/core#Concept"/>
	<rdfs:isDefinedBy xml:lang="en">Gouffon Yves (Editor) (2024): Tectonic Map of Switzerland 1:500000, Explanatory notes. Federal Office of Topography swisstopo, Wabern</rdfs:isDefinedBy>
	<skos:definition xml:lang="en">The Middle Penninic subdomain comprises tectonic units located between the Lower Penninic subduction surface and the major thrust of the Upper Penninic. Paleogeographically, these units are derived from the Briançonnais Terrane. They are formed of a polycyclic crystalline basement, cut by Late Cambrian (ca. 500 Ma) and Permian (ca. 270 Ma) granitic intrusions, by Permo-Carboniferous sediments that filled narrow basins and a characteristic Mesozoic – Paleogene sedimentary cover (much of it detached at the level of the Triassic evaporites to form some of the nappes in the Prealps).</skos:definition>
	<skos:inScheme rdf:resource="https://dev-lexic.swissgeol.ch/TectonicUnits"/>
	<skos:prefLabel xml:lang="en">Middle Penninic</skos:prefLabel>
	<skos:prefLabel xml:lang="de">Mittelpenninikum</skos:prefLabel>
	<skos:prefLabel xml:lang="fr">Pennique moyen</skos:prefLabel>
	<skos:prefLabel xml:lang="it">Pennidico medio</skos:prefLabel>
	<skos:broader rdf:resource="https://dev-lexic.swissgeol.ch/TectonicUnits/Penninic"/>
	<skos:narrower rdf:resource="https://dev-lexic.swissgeol.ch/TectonicUnits/ZoneSubmediane"/>
	<skos:narrower rdf:resource="https://dev-lexic.swissgeol.ch/TectonicUnits/PrealpesMedianesNappe"/>
	<skos:narrower rdf:resource="https://dev-lexic.swissgeol.ch/TectonicUnits/BrecciaNappe"/>
	<skos:narrower rdf:resource="https://dev-lexic.swissgeol.ch/TectonicUnits/ZoneHouillere"/>
	<skos:narrower rdf:resource="https://dev-lexic.swissgeol.ch/TectonicUnits/GaelmjiZone"/>
	<skos:narrower rdf:resource="https://dev-lexic.swissgeol.ch/TectonicUnits/RuginentaNappe"/>
	<skos:narrower rdf:resource="https://dev-lexic.swissgeol.ch/TectonicUnits/RuitorNappe"/>
	<skos:narrower rdf:resource="https://dev-lexic.swissgeol.ch/TectonicUnits/UpperStaldenNappe"/>
	<skos:narrower rdf:resource="https://dev-lexic.swissgeol.ch/TectonicUnits/BerisalNappe"/>
	<skos:narrower rdf:resource="https://dev-lexic.swissgeol.ch/TectonicUnits/CamugheraNappe"/>
	<skos:narrower rdf:resource="https://dev-lexic.swissgeol.ch/TectonicUnits/Siviez-MischabelNappe"/>
	<skos:narrower rdf:resource="https://dev-lexic.swissgeol.ch/TectonicUnits/MontFortNappe"/>
	<skos:narrower rdf:resource="https://dev-lexic.swissgeol.ch/TectonicUnits/PortjengratNappe"/>
	<skos:narrower rdf:resource="https://dev-lexic.swissgeol.ch/TectonicUnits/StockhornNappe"/>
	<skos:narrower rdf:resource="https://dev-lexic.swissgeol.ch/TectonicUnits/MonteRosaNappe"/>
	<skos:narrower rdf:resource="https://dev-lexic.swissgeol.ch/TectonicUnits/TamboNappe"/>
	<skos:narrower rdf:resource="https://dev-lexic.swissgeol.ch/TectonicUnits/SurettaNappe"/>
	<skos:narrower rdf:resource="https://dev-lexic.swissgeol.ch/TectonicUnits/SchamsNappeComplex"/>
	<skos:narrower rdf:resource="https://dev-lexic.swissgeol.ch/TectonicUnits/FalknisNappe"/>
	<skos:narrower rdf:resource="https://dev-lexic.swissgeol.ch/TectonicUnits/SulzfluhNappe"/>
	<skos:narrower rdf:resource="https://dev-lexic.swissgeol.ch/TectonicUnits/FimberZone"/>
	<skos:narrower rdf:resource="https://dev-lexic.swissgeol.ch/TectonicUnits/TasnaNappe"/>
	<status xmlns="http://www.w3.org/ns/adms#" rdf:resource="https://dev-lexic.swissgeol.ch/active"/>
</rdf:Description>

<rdf:Description rdf:about="https://dev-lexic.swissgeol.ch/TectonicUnits/UpperPenninic">
	<rdf:type rdf:resource="http://www.w3.org/2004/02/skos/core#Concept"/>
	<rdfs:isDefinedBy xml:lang="en">Gouffon Yves (Editor) (2024): Tectonic Map of Switzerland 1:500000, Explanatory notes. Federal Office of Topography swisstopo, Wabern</rdfs:isDefinedBy>
	<skos:definition xml:lang="en">The Upper Penninic subdomain contains mainly magmatic and sedimentary rocks derived from the Piemonte-Liguria Ocean. Some thin continental margin sedimentary series and small continental crust slices are intercalated within these units. All of these units were driven into a subduction zone under the Salassic nappes, some exposed to high-pressure metamorphic conditions, others remaining under lower pressure conditions.</skos:definition>
	<skos:inScheme rdf:resource="https://dev-lexic.swissgeol.ch/TectonicUnits"/>
	<skos:prefLabel xml:lang="en">Upper Penninic</skos:prefLabel>
	<skos:prefLabel xml:lang="de">Oberpenninikum</skos:prefLabel>
	<skos:prefLabel xml:lang="fr">Pennique supérieur</skos:prefLabel>
	<skos:prefLabel xml:lang="it">Pennidico superiore</skos:prefLabel>
	<skos:broader rdf:resource="https://dev-lexic.swissgeol.ch/TectonicUnits/Penninic"/>
	<skos:narrower rdf:resource="https://dev-lexic.swissgeol.ch/TectonicUnits/GetsNappe"/>
	<skos:narrower rdf:resource="https://dev-lexic.swissgeol.ch/TectonicUnits/SimmeNappe"/>
	<skos:narrower rdf:resource="https://dev-lexic.swissgeol.ch/TectonicUnits/DransesNappe"/>
	<skos:narrower rdf:resource="https://dev-lexic.swissgeol.ch/TectonicUnits/SarineNappe"/>
	<skos:narrower rdf:resource="https://dev-lexic.swissgeol.ch/TectonicUnits/AntronaNappe"/>
	<skos:narrower rdf:resource="https://dev-lexic.swissgeol.ch/TectonicUnits/Zermatt-SaasFeeNappe"/>
	<skos:narrower rdf:resource="https://dev-lexic.swissgeol.ch/TectonicUnits/TheodulgletscherSlice"/>
	<skos:narrower rdf:resource="https://dev-lexic.swissgeol.ch/TectonicUnits/MontEmiliusNappe"/>
	<skos:narrower rdf:resource="https://dev-lexic.swissgeol.ch/TectonicUnits/Etirol-LevazSlice"/>
	<skos:narrower rdf:resource="https://dev-lexic.swissgeol.ch/TectonicUnits/Chatillon-St-VincentSlices"/>
	<skos:narrower rdf:resource="https://dev-lexic.swissgeol.ch/TectonicUnits/GornergratNappe"/>
	<skos:narrower rdf:resource="https://dev-lexic.swissgeol.ch/TectonicUnits/CimesBlanchesNappe"/>
	<skos:narrower rdf:resource="https://dev-lexic.swissgeol.ch/TectonicUnits/FrilihornNappe"/>
	<skos:narrower rdf:resource="https://dev-lexic.swissgeol.ch/TectonicUnits/TsateNappe"/>
	<skos:narrower rdf:resource="https://dev-lexic.swissgeol.ch/TectonicUnits/AversNappe"/>
	<skos:narrower rdf:resource="https://dev-lexic.swissgeol.ch/TectonicUnits/Malenco-Forno-LizunNappe"/>
	<skos:narrower rdf:resource="https://dev-lexic.swissgeol.ch/TectonicUnits/PlattaNappe"/>
	<skos:narrower rdf:resource="https://dev-lexic.swissgeol.ch/TectonicUnits/ArosaZone"/>
	<status xmlns="http://www.w3.org/ns/adms#" rdf:resource="https://dev-lexic.swissgeol.ch/active"/>
</rdf:Description>

<rdf:Description rdf:about="https://dev-lexic.swissgeol.ch/TectonicUnits/NiesenNappe">
	<rdf:type rdf:resource="http://www.w3.org/2004/02/skos/core#Concept"/>
	<rdfs:isDefinedBy xml:lang="en">Gouffon Yves (Editor) (2024): Tectonic Map of Switzerland 1:500000, Explanatory notes. Federal Office of Topography swisstopo, Wabern</rdfs:isDefinedBy>
	<skos:definition xml:lang="en">The Niesen Nappe is a Lower Penninic tectonic unit located at the rear of the Romandes Prealps, in front of the Helvetic nappes and on top of the Pillon Mélange Zone. It is composed of flysch deposits of Late Cretaceous to Paleocene age.</skos:definition>
	<skos:inScheme rdf:resource="https://dev-lexic.swissgeol.ch/TectonicUnits"/>
	<skos:prefLabel xml:lang="en">Niesen Nappe</skos:prefLabel>
	<skos:prefLabel xml:lang="de">Niesen-Decke</skos:prefLabel>
	<skos:prefLabel xml:lang="fr">Nappe du Niesen</skos:prefLabel>
	<skos:prefLabel xml:lang="it">Falda del Niesen</skos:prefLabel>
	<skos:broader rdf:resource="https://dev-lexic.swissgeol.ch/TectonicUnits/LowerPenninic"/>
	<skos:narrower rdf:resource="https://dev-lexic.swissgeol.ch/TectonicUnits/Infra-NiesenMelange"/>
	<status xmlns="http://www.w3.org/ns/adms#" rdf:resource="https://dev-lexic.swissgeol.ch/active"/>
</rdf:Description>

<rdf:Description rdf:about="https://dev-lexic.swissgeol.ch/TectonicUnits/VoironsNappe">
	<rdf:type rdf:resource="http://www.w3.org/2004/02/skos/core#Concept"/>
	<rdfs:isDefinedBy xml:lang="en">Gouffon Yves (Editor) (2024): Tectonic Map of Switzerland 1:500000, Explanatory notes. Federal Office of Topography swisstopo, Wabern</rdfs:isDefinedBy>
	<skos:definition xml:lang="en">The Voirons Nappe is a Lower Penninic tectonic unit located at the front of the Chablais Prealps. It is composed of flysch deposits of Paleogene age.</skos:definition>
	<skos:inScheme rdf:resource="https://dev-lexic.swissgeol.ch/TectonicUnits"/>
	<skos:prefLabel xml:lang="en">Voirons Nappe</skos:prefLabel>
	<skos:prefLabel xml:lang="de">Voirons-Decke</skos:prefLabel>
	<skos:prefLabel xml:lang="fr">Nappe des Voirons</skos:prefLabel>
	<skos:prefLabel xml:lang="it">Falda dei Voirons</skos:prefLabel>
	<skos:broader rdf:resource="https://dev-lexic.swissgeol.ch/TectonicUnits/LowerPenninic"/>
	<status xmlns="http://www.w3.org/ns/adms#" rdf:resource="https://dev-lexic.swissgeol.ch/active"/>
</rdf:Description>

<rdf:Description rdf:about="https://dev-lexic.swissgeol.ch/TectonicUnits/GurnigelNappe">
	<rdf:type rdf:resource="http://www.w3.org/2004/02/skos/core#Concept"/>
	<rdfs:isDefinedBy xml:lang="en">Gouffon Yves (Editor) (2024): Tectonic Map of Switzerland 1:500000, Explanatory notes. Federal Office of Topography swisstopo, Wabern</rdfs:isDefinedBy>
	<skos:definition xml:lang="en">The Gurnigel Nappe is a Lower Penninic tectonic unit located at the front of the Romandes Prealps. It is composed of flysch deposits of Late Cretaceous to Eocene age.</skos:definition>
	<skos:inScheme rdf:resource="https://dev-lexic.swissgeol.ch/TectonicUnits"/>
	<skos:prefLabel xml:lang="en">Gurnigel Nappe</skos:prefLabel>
	<skos:prefLabel xml:lang="de">Gurnigel-Decke</skos:prefLabel>
	<skos:prefLabel xml:lang="fr">Nappe du Gurnigel</skos:prefLabel>
	<skos:prefLabel xml:lang="it">Falda del Gurnigel</skos:prefLabel>
	<skos:broader rdf:resource="https://dev-lexic.swissgeol.ch/TectonicUnits/LowerPenninic"/>
	<status xmlns="http://www.w3.org/ns/adms#" rdf:resource="https://dev-lexic.swissgeol.ch/active"/>
</rdf:Description>

<rdf:Description rdf:about="https://dev-lexic.swissgeol.ch/TectonicUnits/SchlierenNappe">
	<rdf:type rdf:resource="http://www.w3.org/2004/02/skos/core#Concept"/>
	<rdfs:isDefinedBy xml:lang="en">Gouffon Yves (Editor) (2024): Tectonic Map of Switzerland 1:500000, Explanatory notes. Federal Office of Topography swisstopo, Wabern</rdfs:isDefinedBy>
	<skos:definition xml:lang="en">The Schlieren Nappe is a Lower Penninic tectonic unit occuring between Thunersee and Vierwaldstättersee in a large synform of the Upper Helvetic Drusberg Nappe (with intercalated Habkern Mélange Zone). This nappe only consists of Cretaceous–Paleogene flysch very similar to the Voirons and Gurnigel flysches in the Prealps and to the Wägital flysch further east.</skos:definition>
	<skos:inScheme rdf:resource="https://dev-lexic.swissgeol.ch/TectonicUnits"/>
	<skos:prefLabel xml:lang="en">Schlieren Nappe</skos:prefLabel>
	<skos:prefLabel xml:lang="de">Schlieren-Decke</skos:prefLabel>
	<skos:prefLabel xml:lang="fr">Nappe des Schlieren</skos:prefLabel>
	<skos:prefLabel xml:lang="it">Falda delle Schlieren</skos:prefLabel>
	<skos:broader rdf:resource="https://dev-lexic.swissgeol.ch/TectonicUnits/LowerPenninic"/>
	<status xmlns="http://www.w3.org/ns/adms#" rdf:resource="https://dev-lexic.swissgeol.ch/active"/>
</rdf:Description>

<rdf:Description rdf:about="https://dev-lexic.swissgeol.ch/TectonicUnits/WaegitalNappe">
	<rdf:type rdf:resource="http://www.w3.org/2004/02/skos/core#Concept"/>
	<rdfs:isDefinedBy xml:lang="en">Gouffon Yves (Editor) (2024): Tectonic Map of Switzerland 1:500000, Explanatory notes. Federal Office of Topography swisstopo, Wabern</rdfs:isDefinedBy>
	<skos:definition xml:lang="en">The Wägital Nappe, occuring between Vierwaldstättersee and Walensee, is a Lower Penninic tectonic unit similar to the Schlieren Nappe but located at the front of the Drusberg Nappe and surrounded by the Iberg Mélange and the Internal Einsiedeln Slices of the Upper Helvetic.</skos:definition>
	<skos:inScheme rdf:resource="https://dev-lexic.swissgeol.ch/TectonicUnits"/>
	<skos:prefLabel xml:lang="en">Wägital Nappe</skos:prefLabel>
	<skos:prefLabel xml:lang="de">Wägital-Decke</skos:prefLabel>
	<skos:prefLabel xml:lang="fr">Nappe du Wägital</skos:prefLabel>
	<skos:prefLabel xml:lang="it">Falda del Wägital</skos:prefLabel>
	<skos:broader rdf:resource="https://dev-lexic.swissgeol.ch/TectonicUnits/LowerPenninic"/>
	<status xmlns="http://www.w3.org/ns/adms#" rdf:resource="https://dev-lexic.swissgeol.ch/active"/>
</rdf:Description>

<rdf:Description rdf:about="https://dev-lexic.swissgeol.ch/TectonicUnits/UentschenNappe">
	<rdf:type rdf:resource="http://www.w3.org/2004/02/skos/core#Concept"/>
	<rdfs:isDefinedBy xml:lang="en">Gouffon Yves (Editor) (2024): Tectonic Map of Switzerland 1:500000, Explanatory notes. Federal Office of Topography swisstopo, Wabern</rdfs:isDefinedBy>
	<skos:definition xml:lang="en">The Lower Penninic Üntschen Nappe, occuring east of the Rhine, is located south of the Säntis Nappe. It is made up of the Late Cretaceous Vorarlberg Flysch and is one of the westernmost occurrences of a flysch belt referred to as the Rhenodanubian Flysch Zone (Mattern 1999). Several klippes overlying the Wildhaus Mélange in a few synforms within the Upper Helvetic Säntis Nappe are also attributed to the Üntschen Nappe (from east to west: Gamserberg, Vorder and Hinder Höhi north of Amden).</skos:definition>
	<skos:inScheme rdf:resource="https://dev-lexic.swissgeol.ch/TectonicUnits"/>
	<skos:prefLabel xml:lang="en">Üntschen Nappe</skos:prefLabel>
	<skos:prefLabel xml:lang="de">Üntschen-Decke</skos:prefLabel>
	<skos:prefLabel xml:lang="fr">Nappe de l'Üntschen</skos:prefLabel>
	<skos:prefLabel xml:lang="it">Falda dell'Üntschen</skos:prefLabel>
	<skos:broader rdf:resource="https://dev-lexic.swissgeol.ch/TectonicUnits/LowerPenninic"/>
	<status xmlns="http://www.w3.org/ns/adms#" rdf:resource="https://dev-lexic.swissgeol.ch/active"/>
</rdf:Description>

<rdf:Description rdf:about="https://dev-lexic.swissgeol.ch/TectonicUnits/SigiswangNappe">
	<rdf:type rdf:resource="http://www.w3.org/2004/02/skos/core#Concept"/>
	<rdfs:isDefinedBy xml:lang="en">Gouffon Yves (Editor) (2024): Tectonic Map of Switzerland 1:500000, Explanatory notes. Federal Office of Topography swisstopo, Wabern</rdfs:isDefinedBy>
	<skos:definition xml:lang="en">The Lower Penninic Sigiswang Nappe, occuring east of the Rhine, is located north of the Säntis Nappe. It is made up of the Late Cretaceous Vorarlberg Flysch and is one of the westernmost occurrences of a flysch belt referred to as the Rhenodanubian Flysch Zone (Mattern 1999). Several klippes overlying the Liebenstein Nappe, resp. the Wildhaus Mélange in a few synforms within the Upper Helvetic Säntis Nappe are also attributed to the Sigiswang Nappe (from east to west: Müselalpe, Hohe Kugel and Fähnerenspitz).</skos:definition>
	<skos:inScheme rdf:resource="https://dev-lexic.swissgeol.ch/TectonicUnits"/>
	<skos:prefLabel xml:lang="en">Sigiswang Nappe</skos:prefLabel>
	<skos:prefLabel xml:lang="de">Sigiswang-Decke</skos:prefLabel>
	<skos:prefLabel xml:lang="fr">Nappe de Sigiswang</skos:prefLabel>
	<skos:prefLabel xml:lang="it">Falda di Sigiswang</skos:prefLabel>
	<skos:broader rdf:resource="https://dev-lexic.swissgeol.ch/TectonicUnits/LowerPenninic"/>
	<status xmlns="http://www.w3.org/ns/adms#" rdf:resource="https://dev-lexic.swissgeol.ch/active"/>
</rdf:Description>

<rdf:Description rdf:about="https://dev-lexic.swissgeol.ch/TectonicUnits/TriesenbergSliceComplex">
	<rdf:type rdf:resource="http://www.w3.org/2004/02/skos/core#Concept"/>
	<rdfs:isDefinedBy xml:lang="en">Gouffon Yves (Editor) (2024): Tectonic Map of Switzerland 1:500000, Explanatory notes. Federal Office of Topography swisstopo, Wabern</rdfs:isDefinedBy>
	<skos:definition xml:lang="en">The small Triesenberg Slice Complex (formerly «Liechtenstein Flysch») is a Lower Penninic tectonic unit occuring in Liechtenstein and located at the base of the Austroalpine units, the Arosa Nappe or the Falknis Nappe. It comprises two slices, the northern one composed of the Vaduz Flysch (Late Cretaceous), more or less equivalent to that of the Oberstdorf Nappe, and the southern one of the Triesen Flysch (Late Cretaceous to Paleogene), which has an affinity with the Prättigau Flysch.</skos:definition>
	<skos:inScheme rdf:resource="https://dev-lexic.swissgeol.ch/TectonicUnits"/>
	<skos:prefLabel xml:lang="en">Triesenberg Slice Complex</skos:prefLabel>
	<skos:prefLabel xml:lang="de">Triesenberg-Schuppenkomplex</skos:prefLabel>
	<skos:prefLabel xml:lang="fr">Complexe d'écailles de Triesenberg</skos:prefLabel>
	<skos:prefLabel xml:lang="it">Complesso di scaglie di Triesenberg</skos:prefLabel>
	<skos:broader rdf:resource="https://dev-lexic.swissgeol.ch/TectonicUnits/LowerPenninic"/>
	<status xmlns="http://www.w3.org/ns/adms#" rdf:resource="https://dev-lexic.swissgeol.ch/active"/>
</rdf:Description>

<rdf:Description rdf:about="https://dev-lexic.swissgeol.ch/TectonicUnits/OberstdorfNappe">
	<rdf:type rdf:resource="http://www.w3.org/2004/02/skos/core#Concept"/>
	<rdfs:isDefinedBy xml:lang="en">Gouffon Yves (Editor) (2024): Tectonic Map of Switzerland 1:500000, Explanatory notes. Federal Office of Topography swisstopo, Wabern</rdfs:isDefinedBy>
	<skos:definition xml:lang="en">The Lower Penninic Oberstdorf Nappe overlies the Üntschen and Sigiswang nappes in their eastern part. It is made up of the Rhenodanubian Flysch as the other two nappes.</skos:definition>
	<skos:inScheme rdf:resource="https://dev-lexic.swissgeol.ch/TectonicUnits"/>
	<skos:prefLabel xml:lang="en">Oberstdorf Nappe</skos:prefLabel>
	<skos:prefLabel xml:lang="de">Oberstdorf-Decke</skos:prefLabel>
	<skos:prefLabel xml:lang="fr">Nappe d'Oberstdorf</skos:prefLabel>
	<skos:prefLabel xml:lang="it">Falda di Oberstdorf</skos:prefLabel>
	<skos:broader rdf:resource="https://dev-lexic.swissgeol.ch/TectonicUnits/LowerPenninic"/>
	<status xmlns="http://www.w3.org/ns/adms#" rdf:resource="https://dev-lexic.swissgeol.ch/active"/>
</rdf:Description>

<rdf:Description rdf:about="https://dev-lexic.swissgeol.ch/TectonicUnits/Sion-CourmayeurNappe">
	<rdf:type rdf:resource="http://www.w3.org/2004/02/skos/core#Concept"/>
	<rdfs:isDefinedBy xml:lang="en">Gouffon Yves (Editor) (2024): Tectonic Map of Switzerland 1:500000, Explanatory notes. Federal Office of Topography swisstopo, Wabern</rdfs:isDefinedBy>
	<skos:definition xml:lang="en">The Sion-Courmayeur Nappe is a Lower Penninic tectonic unit of Western Switzerland. It is dominated by flysch-type rocks, deposited during the Cretaceous in the Valaisan Basin, and has undergone high-pressure / low-temperature metamorphism.</skos:definition>
	<skos:inScheme rdf:resource="https://dev-lexic.swissgeol.ch/TectonicUnits"/>
	<skos:prefLabel xml:lang="en">Sion-Courmayeur Nappe</skos:prefLabel>
	<skos:prefLabel xml:lang="de">Sion-Courmayeur-Decke</skos:prefLabel>
	<skos:prefLabel xml:lang="fr">Nappe de Sion-Courmayeur</skos:prefLabel>
	<skos:prefLabel xml:lang="it">Falda di Sion-Courmayeur</skos:prefLabel>
	<skos:broader rdf:resource="https://dev-lexic.swissgeol.ch/TectonicUnits/LowerPenninic"/>
	<skos:narrower rdf:resource="https://dev-lexic.swissgeol.ch/TectonicUnits/RosswaldSlice"/>
	<skos:narrower rdf:resource="https://dev-lexic.swissgeol.ch/TectonicUnits/FerretSlice"/>
	<skos:narrower rdf:resource="https://dev-lexic.swissgeol.ch/TectonicUnits/MoutiersSlice"/>
	<skos:narrower rdf:resource="https://dev-lexic.swissgeol.ch/TectonicUnits/Roignais-VersoyenSlice"/>
	<skos:narrower rdf:resource="https://dev-lexic.swissgeol.ch/TectonicUnits/PierreAvoiSlice"/>
	<skos:narrower rdf:resource="https://dev-lexic.swissgeol.ch/TectonicUnits/PetitSt-BernardSlice"/>
	<status xmlns="http://www.w3.org/ns/adms#" rdf:resource="https://dev-lexic.swissgeol.ch/active"/>
</rdf:Description>

<rdf:Description rdf:about="https://dev-lexic.swissgeol.ch/TectonicUnits/ChiavennaNappe">
	<rdf:type rdf:resource="http://www.w3.org/2004/02/skos/core#Concept"/>
	<rdfs:isDefinedBy xml:lang="en">Gouffon Yves (Editor) (2024): Tectonic Map of Switzerland 1:500000, Explanatory notes. Federal Office of Topography swisstopo, Wabern</rdfs:isDefinedBy>
	<skos:definition xml:lang="en">The Lower Penninic Chiavenna Nappe is a large ophiolitic slice found below the Middle Penninic Tambo Nappe and against the Gruf Complex, and thus considered as a remnant of the Valaisan oceanic crust.</skos:definition>
	<skos:inScheme rdf:resource="https://dev-lexic.swissgeol.ch/TectonicUnits"/>
	<skos:prefLabel xml:lang="en">Chiavenna Nappe</skos:prefLabel>
	<skos:prefLabel xml:lang="de">Chiavenna-Decke</skos:prefLabel>
	<skos:prefLabel xml:lang="fr">Nappe de Chiavenna</skos:prefLabel>
	<skos:prefLabel xml:lang="it">Falda di Chiavenna</skos:prefLabel>
	<skos:broader rdf:resource="https://dev-lexic.swissgeol.ch/TectonicUnits/LowerPenninic"/>
	<status xmlns="http://www.w3.org/ns/adms#" rdf:resource="https://dev-lexic.swissgeol.ch/active"/>
</rdf:Description>

<rdf:Description rdf:about="https://dev-lexic.swissgeol.ch/TectonicUnits/ValsSlices">
	<rdf:type rdf:resource="http://www.w3.org/2004/02/skos/core#Concept"/>
	<rdfs:isDefinedBy xml:lang="en">Gouffon Yves (Editor) (2024): Tectonic Map of Switzerland 1:500000, Explanatory notes. Federal Office of Topography swisstopo, Wabern</rdfs:isDefinedBy>
	<skos:definition xml:lang="en">The Lower Penninic Vals Slices (former «Upper Vals Slices») overly the Adula Nappe in its northeastern frontal part. They are mainly composed of Mesozoic shaly-calcareous-sandy marine sedimentary rocks («Bündnerschiefer») with some ophiolitic rocks of Late Jurassic age, similarly to the overlying Aul, Grava and Tomül nappes (all rooted in the «Misox Zone» between the Adula and Tambo nappes).</skos:definition>
	<skos:inScheme rdf:resource="https://dev-lexic.swissgeol.ch/TectonicUnits"/>
	<skos:prefLabel xml:lang="en">Vals Slices</skos:prefLabel>
	<skos:prefLabel xml:lang="de">Vals-Schuppen</skos:prefLabel>
	<skos:prefLabel xml:lang="fr">Écailles de Vals</skos:prefLabel>
	<skos:prefLabel xml:lang="it">Scaglie di Vals</skos:prefLabel>
	<skos:altLabel xml:lang="de">Obere Valser Schuppen</skos:altLabel>
	<skos:altLabel xml:lang="en">Upper Vals Slices</skos:altLabel>
	<skos:broader rdf:resource="https://dev-lexic.swissgeol.ch/TectonicUnits/LowerPenninic"/>
	<status xmlns="http://www.w3.org/ns/adms#" rdf:resource="https://dev-lexic.swissgeol.ch/active"/>
</rdf:Description>

<rdf:Description rdf:about="https://dev-lexic.swissgeol.ch/TectonicUnits/AulNappe">
	<rdf:type rdf:resource="http://www.w3.org/2004/02/skos/core#Concept"/>
	<rdfs:isDefinedBy xml:lang="en">Gouffon Yves (Editor) (2024): Tectonic Map of Switzerland 1:500000, Explanatory notes. Federal Office of Topography swisstopo, Wabern</rdfs:isDefinedBy>
	<skos:definition xml:lang="en">The Aul Nappe consists of an ophiolitic mélange complex at its base, including serpentinite and pillow basalts, overlain by a marble whose age is not younger than Jurassic. It structurally overlies the Vals Slices and roots, together with the it and the Grava and Tomül nappes, in the «Misox Zone».</skos:definition>
	<skos:inScheme rdf:resource="https://dev-lexic.swissgeol.ch/TectonicUnits"/>
	<skos:prefLabel xml:lang="en">Aul Nappe</skos:prefLabel>
	<skos:prefLabel xml:lang="de">Aul-Decke</skos:prefLabel>
	<skos:prefLabel xml:lang="fr">Nappe de l'Aul</skos:prefLabel>
	<skos:prefLabel xml:lang="it">Falda dell'Aul</skos:prefLabel>
	<skos:broader rdf:resource="https://dev-lexic.swissgeol.ch/TectonicUnits/LowerPenninic"/>
	<status xmlns="http://www.w3.org/ns/adms#" rdf:resource="https://dev-lexic.swissgeol.ch/active"/>
</rdf:Description>

<rdf:Description rdf:about="https://dev-lexic.swissgeol.ch/TectonicUnits/GravaNappe">
	<rdf:type rdf:resource="http://www.w3.org/2004/02/skos/core#Concept"/>
	<rdfs:isDefinedBy xml:lang="en">Gouffon Yves (Editor) (2024): Tectonic Map of Switzerland 1:500000, Explanatory notes. Federal Office of Topography swisstopo, Wabern</rdfs:isDefinedBy>
	<skos:definition xml:lang="en">The Lower Penninic Grava Nappe is folded around the front of the Adula Nappe and the Lunschania Antiform. In an overturned tectonic position, it can be followed all the way into a synform located between the Simano and Leventina-Lucomagno nappes. Westward it is found as a klippe in the core of the Molare Syncline and possibly pinches out in the Piora-Peiden Slice Complex between Lago Ritom and Airolo.
The Grava Nappe overlies the Aul Nappe with a basal mélange zone, which contains Early Jurassic Gryphaea-bearing limestones, metabasalts and dark shales. The rest of the nappe consists of Cretaceous «Bündnerschiefer».</skos:definition>
	<skos:inScheme rdf:resource="https://dev-lexic.swissgeol.ch/TectonicUnits"/>
	<skos:prefLabel xml:lang="en">Grava Nappe</skos:prefLabel>
	<skos:prefLabel xml:lang="de">Grava-Decke</skos:prefLabel>
	<skos:prefLabel xml:lang="fr">Nappe de la Grava</skos:prefLabel>
	<skos:prefLabel xml:lang="it">Falda della Grava</skos:prefLabel>
	<skos:broader rdf:resource="https://dev-lexic.swissgeol.ch/TectonicUnits/LowerPenninic"/>
	<skos:related rdf:resource="https://dev-lexic.swissgeol.ch/TectonicUnits/TomuelNappe"/>
	<status xmlns="http://www.w3.org/ns/adms#" rdf:resource="https://dev-lexic.swissgeol.ch/active"/>
</rdf:Description>

<rdf:Description rdf:about="https://dev-lexic.swissgeol.ch/TectonicUnits/TomuelNappe">
	<rdf:type rdf:resource="http://www.w3.org/2004/02/skos/core#Concept"/>
	<rdfs:isDefinedBy xml:lang="en">Gouffon Yves (Editor) (2024): Tectonic Map of Switzerland 1:500000, Explanatory notes. Federal Office of Topography swisstopo, Wabern</rdfs:isDefinedBy>
	<skos:definition xml:lang="en">The Lower Penninic Tomül Nappe is the highest of the “Bündnerschiefer” nappes rooting in the «Misox Zone». It can be followed eastward, below the Middle Penninic Schams Nappe Complex, and is then backfolded, together with the latter, around the front of the Suretta Nappe in order to come to lie in an overturned position on top of the Schams Nappe Complex in the upper limb of the Niemet-Beverin Backfold. East of Lenzerheide, the Tomül Nappe can be followed even further to the east and into the Prättigau Half-Window where it underlies the Middle Penninic Falknis and Sulzfluh nappes.
The Tomül Nappe locally has an ophiolite-bearing mélange at its base, overlain by very thick (over 2 km-thick) and multiply folded «Bündnerschiefer» and flysch sequence of Cretaceous–Paleogene age.</skos:definition>
	<skos:inScheme rdf:resource="https://dev-lexic.swissgeol.ch/TectonicUnits"/>
	<skos:prefLabel xml:lang="en">Tomül Nappe</skos:prefLabel>
	<skos:prefLabel xml:lang="de">Tomül-Decke</skos:prefLabel>
	<skos:prefLabel xml:lang="fr">Nappe du Tomül</skos:prefLabel>
	<skos:prefLabel xml:lang="it">Falda del Tomül</skos:prefLabel>
	<skos:broader rdf:resource="https://dev-lexic.swissgeol.ch/TectonicUnits/LowerPenninic"/>
	<skos:narrower rdf:resource="https://dev-lexic.swissgeol.ch/TectonicUnits/ForbeschSlice"/>
	<skos:related rdf:resource="https://dev-lexic.swissgeol.ch/TectonicUnits/GravaNappe"/>
	<status xmlns="http://www.w3.org/ns/adms#" rdf:resource="https://dev-lexic.swissgeol.ch/active"/>
</rdf:Description>

<rdf:Description rdf:about="https://dev-lexic.swissgeol.ch/TectonicUnits/Roz-ChampatschMelange">
	<rdf:type rdf:resource="http://www.w3.org/2004/02/skos/core#Concept"/>
	<rdfs:isDefinedBy xml:lang="en">Gouffon Yves (Editor) (2024): Tectonic Map of Switzerland 1:500000, Explanatory notes. Federal Office of Topography swisstopo, Wabern</rdfs:isDefinedBy>
	<skos:definition xml:lang="en">The Lower Penninic Roz-Champatsch Mélange directly overlies the Pfunds Nappe in the Lower Engadine Window and is dominated by flysch-type sedimentary rocks. Although having formerly been considered an equivalent of the «North Penninic flysch» of the Prättigau (Tomül Nappe), it differs from this nappe in that it includes slivers of various rocks, such as crystalline basement, Triassic sediments and occasional serpentinite.</skos:definition>
	<skos:inScheme rdf:resource="https://dev-lexic.swissgeol.ch/TectonicUnits"/>
	<skos:prefLabel xml:lang="en">Roz-Champatsch Mélange</skos:prefLabel>
	<skos:prefLabel xml:lang="de">Roz-Champatsch-Melange</skos:prefLabel>
	<skos:prefLabel xml:lang="fr">Mélange de Roz-Champatsch</skos:prefLabel>
	<skos:prefLabel xml:lang="it">Mélange di Roz-Champatsch</skos:prefLabel>
	<skos:broader rdf:resource="https://dev-lexic.swissgeol.ch/TectonicUnits/LowerPenninic"/>
	<status xmlns="http://www.w3.org/ns/adms#" rdf:resource="https://dev-lexic.swissgeol.ch/active"/>
</rdf:Description>

<rdf:Description rdf:about="https://dev-lexic.swissgeol.ch/TectonicUnits/RamoschZone">
	<rdf:type rdf:resource="http://www.w3.org/2004/02/skos/core#Concept"/>
	<rdfs:isDefinedBy xml:lang="en">Gouffon Yves (Editor) (2024): Tectonic Map of Switzerland 1:500000, Explanatory notes. Federal Office of Topography swisstopo, Wabern</rdfs:isDefinedBy>
	<skos:definition xml:lang="en">The Ramosch Zone is the highest Lower Penninic ophiolite-bearing unit of the Lower Engadine Window, directly underlying the Middle Penninic Tasna Nappe. It forms a discontinuous band (locally with the character of a mélange) restricted to the western and southwestern rim of tectonic window and is largely dominated by mafic and ultramafic rocks, including metabasalts. The Ramosch Zone is interpreted as the most oceanward part of the ocean-continent transition visible in the Tasna Nappe, and is considered as the lowest subunit of the Tasna Nappe by some authors.</skos:definition>
	<skos:inScheme rdf:resource="https://dev-lexic.swissgeol.ch/TectonicUnits"/>
	<skos:prefLabel xml:lang="en">Ramosch Zone</skos:prefLabel>
	<skos:prefLabel xml:lang="de">Ramosch-Zone</skos:prefLabel>
	<skos:prefLabel xml:lang="fr">Zone de Ramosch</skos:prefLabel>
	<skos:prefLabel xml:lang="it">Zona di Ramosch</skos:prefLabel>
	<skos:broader rdf:resource="https://dev-lexic.swissgeol.ch/TectonicUnits/LowerPenninic"/>
	<status xmlns="http://www.w3.org/ns/adms#" rdf:resource="https://dev-lexic.swissgeol.ch/active"/>
</rdf:Description>

<rdf:Description rdf:about="https://dev-lexic.swissgeol.ch/TectonicUnits/PfundsNappe">
	<rdf:type rdf:resource="http://www.w3.org/2004/02/skos/core#Concept"/>
	<rdfs:isDefinedBy xml:lang="en">Gouffon Yves (Editor) (2024): Tectonic Map of Switzerland 1:500000, Explanatory notes. Federal Office of Topography swisstopo, Wabern</rdfs:isDefinedBy>
	<skos:definition xml:lang="en">The Lower Penninic Pfunds Nappe is the lowest and largest tectonic unit in the core of the Lower Engadine Window. It consists of kilometer-thick Mesozoic shaly-calcareous-sandy marine sedimentary rocks of Cretaceous age («Bündnerschiefer»), which contain some metabasalt bodies (incl. the large body of metabasalts at Piz Mundin which forms the stratigraphic basis of the «Bündnerschiefer» in the center of the window).</skos:definition>
	<skos:inScheme rdf:resource="https://dev-lexic.swissgeol.ch/TectonicUnits"/>
	<skos:prefLabel xml:lang="en">Pfunds Nappe</skos:prefLabel>
	<skos:prefLabel xml:lang="de">Pfunds-Decke</skos:prefLabel>
	<skos:prefLabel xml:lang="fr">Nappe de Pfunds</skos:prefLabel>
	<skos:prefLabel xml:lang="it">Falda di Pfunds</skos:prefLabel>
	<skos:altLabel xml:lang="de">Muttler-Decke</skos:altLabel>
	<skos:broader rdf:resource="https://dev-lexic.swissgeol.ch/TectonicUnits/LowerPenninic"/>
	<status xmlns="http://www.w3.org/ns/adms#" rdf:resource="https://dev-lexic.swissgeol.ch/active"/>
</rdf:Description>

<rdf:Description rdf:about="https://dev-lexic.swissgeol.ch/TectonicUnits/ZoneSubmediane">
	<rdf:type rdf:resource="http://www.w3.org/2004/02/skos/core#Concept"/>
	<rdfs:isDefinedBy xml:lang="en">Gouffon Yves (Editor) (2024): Tectonic Map of Switzerland 1:500000, Explanatory notes. Federal Office of Topography swisstopo, Wabern</rdfs:isDefinedBy>
	<skos:definition xml:lang="en">The Zone Submédiane is a mélange zone that is generally found at the base of the Préalpes Médianes Nappe and morphologically determines a succession of mountain passes and valleys. It contains slivers of varying composition, size and origin (from the Ultrahelvetic to the Subbriançonnais realms) within a matrix comprising evaporites or «wildflysch».</skos:definition>
	<skos:inScheme rdf:resource="https://dev-lexic.swissgeol.ch/TectonicUnits"/>
	<skos:prefLabel xml:lang="en">Zone Submédiane</skos:prefLabel>
	<skos:prefLabel xml:lang="de">Zone Submédiane</skos:prefLabel>
	<skos:prefLabel xml:lang="fr">Zone Submédiane</skos:prefLabel>
	<skos:prefLabel xml:lang="it">Zona Submédiane</skos:prefLabel>
	<skos:broader rdf:resource="https://dev-lexic.swissgeol.ch/TectonicUnits/MiddlePenninic"/>
	<status xmlns="http://www.w3.org/ns/adms#" rdf:resource="https://dev-lexic.swissgeol.ch/active"/>
</rdf:Description>

<rdf:Description rdf:about="https://dev-lexic.swissgeol.ch/TectonicUnits/PrealpesMedianesNappe">
	<rdf:type rdf:resource="http://www.w3.org/2004/02/skos/core#Concept"/>
	<rdfs:isDefinedBy xml:lang="en">Gouffon Yves (Editor) (2024): Tectonic Map of Switzerland 1:500000, Explanatory notes. Federal Office of Topography swisstopo, Wabern</rdfs:isDefinedBy>
	<skos:definition xml:lang="en">The Préalpes Médianes Nappe (also called Klippen-Decke in German) is a Middle Penninic tectonic unit located in the central part of the Prealps. It is subdivided into an external part, called the Préalpes Médianes Plastiques, and an internal part, the Préalpes Médianes Rigides.</skos:definition>
	<skos:inScheme rdf:resource="https://dev-lexic.swissgeol.ch/TectonicUnits"/>
	<skos:prefLabel xml:lang="en">Préalpes Médianes Nappe</skos:prefLabel>
	<skos:prefLabel xml:lang="de">Klippen-Decke</skos:prefLabel>
	<skos:prefLabel xml:lang="fr">Nappe des Préalpes Médianes</skos:prefLabel>
	<skos:prefLabel xml:lang="it">Falda delle Préalpes Médianes</skos:prefLabel>
	<skos:broader rdf:resource="https://dev-lexic.swissgeol.ch/TectonicUnits/MiddlePenninic"/>
	<skos:narrower rdf:resource="https://dev-lexic.swissgeol.ch/TectonicUnits/PrealpesMedianesPlastiques"/>
	<skos:narrower rdf:resource="https://dev-lexic.swissgeol.ch/TectonicUnits/PrealpesMedianesRigides"/>
	<skos:narrower rdf:resource="https://dev-lexic.swissgeol.ch/TectonicUnits/Mythen-RoggeneggSlice"/>
	<skos:narrower rdf:resource="https://dev-lexic.swissgeol.ch/TectonicUnits/ObereRotenflueSlice"/>
	<skos:narrower rdf:resource="https://dev-lexic.swissgeol.ch/TectonicUnits/Staeglerenegg-BruennelistockSlices"/>
	<status xmlns="http://www.w3.org/ns/adms#" rdf:resource="https://dev-lexic.swissgeol.ch/active"/>
</rdf:Description>

<rdf:Description rdf:about="https://dev-lexic.swissgeol.ch/TectonicUnits/BrecciaNappe">
	<rdf:type rdf:resource="http://www.w3.org/2004/02/skos/core#Concept"/>
	<rdfs:isDefinedBy xml:lang="en">Gouffon Yves (Editor) (2024): Tectonic Map of Switzerland 1:500000, Explanatory notes. Federal Office of Topography swisstopo, Wabern</rdfs:isDefinedBy>
	<skos:definition xml:lang="en">The Breccia Nappe is a Middle Penninic tectonic unit of the Prealps, overlying the Préalpes Médianes Nappe and being itself overlain by Upper Penninic units. Its stratigraphic sequence spans the Triassic to the Paleocene and is characterized by two thick formations of Jurassic breccias giving the nappe its name.</skos:definition>
	<skos:inScheme rdf:resource="https://dev-lexic.swissgeol.ch/TectonicUnits"/>
	<skos:prefLabel xml:lang="en">Breccia Nappe</skos:prefLabel>
	<skos:prefLabel xml:lang="de">Brekzien-Decke</skos:prefLabel>
	<skos:prefLabel xml:lang="fr">Nappe de la Brèche</skos:prefLabel>
	<skos:prefLabel xml:lang="it">Falda della Breccia</skos:prefLabel>
	<skos:broader rdf:resource="https://dev-lexic.swissgeol.ch/TectonicUnits/MiddlePenninic"/>
	<status xmlns="http://www.w3.org/ns/adms#" rdf:resource="https://dev-lexic.swissgeol.ch/active"/>
</rdf:Description>

<rdf:Description rdf:about="https://dev-lexic.swissgeol.ch/TectonicUnits/ZoneHouillere">
	<rdf:type rdf:resource="http://www.w3.org/2004/02/skos/core#Concept"/>
	<rdfs:isDefinedBy xml:lang="en">Gouffon Yves (Editor) (2024): Tectonic Map of Switzerland 1:500000, Explanatory notes. Federal Office of Topography swisstopo, Wabern</rdfs:isDefinedBy>
	<skos:definition xml:lang="en">The Zone Houillère is the lowest tectonic unit of the Middle Penninic of the Western Alps. It is subdivided by a thrust fault into an external part, dissected into numerous slices, and a more continuous internal part. It comprises mainly Late Carboniferous to Permian metasediments, locally rich in coal (as its name implies), accompanied by Early and Middle Triassic sediments. The rest of the series, from the Middle Triassic upward, was detached to form the Préalpes Médianes Plastiques.</skos:definition>
	<skos:inScheme rdf:resource="https://dev-lexic.swissgeol.ch/TectonicUnits"/>
	<skos:prefLabel xml:lang="en">Zone Houillère</skos:prefLabel>
	<skos:prefLabel xml:lang="de">Zone Houillère</skos:prefLabel>
	<skos:prefLabel xml:lang="fr">Zone Houillère</skos:prefLabel>
	<skos:prefLabel xml:lang="it">Zona Houillère</skos:prefLabel>
	<skos:broader rdf:resource="https://dev-lexic.swissgeol.ch/TectonicUnits/MiddlePenninic"/>
	<skos:narrower rdf:resource="https://dev-lexic.swissgeol.ch/TectonicUnits/ExternalZoneHouillere"/>
	<skos:narrower rdf:resource="https://dev-lexic.swissgeol.ch/TectonicUnits/InternalZoneHouillere"/>
	<skos:narrower rdf:resource="https://dev-lexic.swissgeol.ch/TectonicUnits/VisperterminenSlice"/>
	<skos:narrower rdf:resource="https://dev-lexic.swissgeol.ch/TectonicUnits/LowerStaldenSlice"/>
	<skos:related rdf:resource="https://dev-lexic.swissgeol.ch/TectonicUnits/PrealpesMedianesPlastiques"/>
	<status xmlns="http://www.w3.org/ns/adms#" rdf:resource="https://dev-lexic.swissgeol.ch/active"/>
</rdf:Description>

<rdf:Description rdf:about="https://dev-lexic.swissgeol.ch/TectonicUnits/GaelmjiZone">
	<rdf:type rdf:resource="http://www.w3.org/2004/02/skos/core#Concept"/>
	<rdfs:isDefinedBy xml:lang="en">Gouffon Yves (Editor) (2024): Tectonic Map of Switzerland 1:500000, Explanatory notes. Federal Office of Topography swisstopo, Wabern</rdfs:isDefinedBy>
	<skos:definition xml:lang="en">The Gälmji Zone is a Middle Penninic tectonic unit of the Western Alps, lying between the Sion-Courmayeur Nappe and the Berisal Nappe in the large synformal Berisal Backfold, to the northeast of the Simplonpass. It forms a thin band of green gneisses and micaschists comparable to those of the Visperterminen and Lower Stalden slices (Zone Houillère). Thick amphibolite layers are interbedded in these metasediments, and scarce remains of Triassic sediments represent the rest of the sedimentary cover. This unit is interpreted to be a metamorphic equivalent of the Zone Houillère east of the Rhône-Simplon Fault.</skos:definition>
	<skos:inScheme rdf:resource="https://dev-lexic.swissgeol.ch/TectonicUnits"/>
	<skos:prefLabel xml:lang="en">Gälmji Zone</skos:prefLabel>
	<skos:prefLabel xml:lang="de">Gälmji-Zone</skos:prefLabel>
	<skos:prefLabel xml:lang="fr">Zone de Gälmji</skos:prefLabel>
	<skos:prefLabel xml:lang="it">Zona di Gälmji</skos:prefLabel>
	<skos:broader rdf:resource="https://dev-lexic.swissgeol.ch/TectonicUnits/MiddlePenninic"/>
	<skos:related rdf:resource="https://dev-lexic.swissgeol.ch/TectonicUnits/ZoneHouillere"/>
	<status xmlns="http://www.w3.org/ns/adms#" rdf:resource="https://dev-lexic.swissgeol.ch/active"/>
</rdf:Description>

<rdf:Description rdf:about="https://dev-lexic.swissgeol.ch/TectonicUnits/RuginentaNappe">
	<rdf:type rdf:resource="http://www.w3.org/2004/02/skos/core#Concept"/>
	<rdfs:isDefinedBy xml:lang="en">Gouffon Yves (Editor) (2024): Tectonic Map of Switzerland 1:500000, Explanatory notes. Federal Office of Topography swisstopo, Wabern</rdfs:isDefinedBy>
	<skos:definition xml:lang="en">The Ruginenta Nappe is a Middle Penninic tectonic unit of the Western Alps, occuring between the Moncucco Nappe and the Camughera Nappe in the huge Vanzone Antiform (south of the Simplonpass). It consists of a polycyclic basement intruded by a granite and overlain by a Carboniferous–Triassic sedimentary cover.</skos:definition>
	<skos:inScheme rdf:resource="https://dev-lexic.swissgeol.ch/TectonicUnits"/>
	<skos:prefLabel xml:lang="en">Ruginenta Nappe</skos:prefLabel>
	<skos:prefLabel xml:lang="de">Ruginenta-Decke</skos:prefLabel>
	<skos:prefLabel xml:lang="fr">Nappe de Ruginenta</skos:prefLabel>
	<skos:prefLabel xml:lang="it">Falda di Ruginenta</skos:prefLabel>
	<skos:broader rdf:resource="https://dev-lexic.swissgeol.ch/TectonicUnits/MiddlePenninic"/>
	<status xmlns="http://www.w3.org/ns/adms#" rdf:resource="https://dev-lexic.swissgeol.ch/active"/>
</rdf:Description>

<rdf:Description rdf:about="https://dev-lexic.swissgeol.ch/TectonicUnits/RuitorNappe">
	<rdf:type rdf:resource="http://www.w3.org/2004/02/skos/core#Concept"/>
	<rdfs:isDefinedBy xml:lang="en">Gouffon Yves (Editor) (2024): Tectonic Map of Switzerland 1:500000, Explanatory notes. Federal Office of Topography swisstopo, Wabern</rdfs:isDefinedBy>
	<skos:definition xml:lang="en">The Ruitor Nappe is a Middle Penninic tectonic unit of the Western Alps, extending from the Valle d’Aosta into the Val de Bagnes, where it pinches out between the Zone Houillère and the Siviez-Mischabel Nappe. It is characterized by a polycyclic basement with numerous pre-Alpine relics, covered by Permian clastic rocks. These latter lithologies are in contact with the Permian cover of the Siviez-Mischabel Nappe, so that the tectonic contact that separates these two nappes is rarely recognizable in the field.</skos:definition>
	<skos:inScheme rdf:resource="https://dev-lexic.swissgeol.ch/TectonicUnits"/>
	<skos:prefLabel xml:lang="en">Ruitor Nappe</skos:prefLabel>
	<skos:prefLabel xml:lang="de">Ruitor-Decke</skos:prefLabel>
	<skos:prefLabel xml:lang="fr">Nappe du Ruitor</skos:prefLabel>
	<skos:prefLabel xml:lang="it">Falda del Ruitor</skos:prefLabel>
	<skos:broader rdf:resource="https://dev-lexic.swissgeol.ch/TectonicUnits/MiddlePenninic"/>
	<status xmlns="http://www.w3.org/ns/adms#" rdf:resource="https://dev-lexic.swissgeol.ch/active"/>
</rdf:Description>

<rdf:Description rdf:about="https://dev-lexic.swissgeol.ch/TectonicUnits/UpperStaldenNappe">
	<rdf:type rdf:resource="http://www.w3.org/2004/02/skos/core#Concept"/>
	<rdfs:isDefinedBy xml:lang="en">Gouffon Yves (Editor) (2024): Tectonic Map of Switzerland 1:500000, Explanatory notes. Federal Office of Topography swisstopo, Wabern</rdfs:isDefinedBy>
	<skos:definition xml:lang="en">The Upper Stalden Nappe is a Middle Penninic tectonic unit of the upper Valais region, between Visp and the Simplonpass, with a similar in structural position as that of the Ruitor Nappe (between the Zone Houillère and the Siviez-Mischabel Nappe). It is composed of a polycyclic basement with numerous pre-Alpine relics, seemingly lacking a sedimentary cover.</skos:definition>
	<skos:inScheme rdf:resource="https://dev-lexic.swissgeol.ch/TectonicUnits"/>
	<skos:prefLabel xml:lang="en">Upper Stalden Nappe</skos:prefLabel>
	<skos:prefLabel xml:lang="de">Obere Stalden-Decke</skos:prefLabel>
	<skos:prefLabel xml:lang="fr">Nappe supérieure de Stalden</skos:prefLabel>
	<skos:prefLabel xml:lang="it">Falda superiore di Stalden</skos:prefLabel>
	<skos:broader rdf:resource="https://dev-lexic.swissgeol.ch/TectonicUnits/MiddlePenninic"/>
	<status xmlns="http://www.w3.org/ns/adms#" rdf:resource="https://dev-lexic.swissgeol.ch/active"/>
</rdf:Description>

<rdf:Description rdf:about="https://dev-lexic.swissgeol.ch/TectonicUnits/BerisalNappe">
	<rdf:type rdf:resource="http://www.w3.org/2004/02/skos/core#Concept"/>
	<rdfs:isDefinedBy xml:lang="en">Gouffon Yves (Editor) (2024): Tectonic Map of Switzerland 1:500000, Explanatory notes. Federal Office of Topography swisstopo, Wabern</rdfs:isDefinedBy>
	<skos:definition xml:lang="en">The Berisal Nappe is a Middle Penninic tectonic unit occupying the core of the large synformal Berisal Backfold. It consists of a polycyclic basement with numerous pre-Alpine relics. It is thus lithologically similar to the Upper Stalden Nappe and interpreted as the continuation of this unit to the east, in the footwall of the Rhône-Simplon Fault.</skos:definition>
	<skos:inScheme rdf:resource="https://dev-lexic.swissgeol.ch/TectonicUnits"/>
	<skos:prefLabel xml:lang="en">Berisal Nappe</skos:prefLabel>
	<skos:prefLabel xml:lang="de">Berisal-Decke</skos:prefLabel>
	<skos:prefLabel xml:lang="fr">Nappe de Berisal</skos:prefLabel>
	<skos:prefLabel xml:lang="it">Falda di Berisal</skos:prefLabel>
	<skos:broader rdf:resource="https://dev-lexic.swissgeol.ch/TectonicUnits/MiddlePenninic"/>
	<status xmlns="http://www.w3.org/ns/adms#" rdf:resource="https://dev-lexic.swissgeol.ch/active"/>
</rdf:Description>

<rdf:Description rdf:about="https://dev-lexic.swissgeol.ch/TectonicUnits/CamugheraNappe">
	<rdf:type rdf:resource="http://www.w3.org/2004/02/skos/core#Concept"/>
	<rdfs:isDefinedBy xml:lang="en">Gouffon Yves (Editor) (2024): Tectonic Map of Switzerland 1:500000, Explanatory notes. Federal Office of Topography swisstopo, Wabern</rdfs:isDefinedBy>
	<skos:definition xml:lang="en">The Camughera Nappe is a Middle Penninic tectonic unit located in the region of Domodossola. It consists of rocks similar to the crystalline basement of the Siviez-Mischabel Nappe and may be the continuation of this nappe. It is folded by the large Vanzone Antiform and overlies the Ruginenta Nappe.</skos:definition>
	<skos:inScheme rdf:resource="https://dev-lexic.swissgeol.ch/TectonicUnits"/>
	<skos:prefLabel xml:lang="en">Camughera Nappe</skos:prefLabel>
	<skos:prefLabel xml:lang="de">Camughera-Decke</skos:prefLabel>
	<skos:prefLabel xml:lang="fr">Nappe de la Camughera</skos:prefLabel>
	<skos:prefLabel xml:lang="it">Falda della Camughera</skos:prefLabel>
	<skos:broader rdf:resource="https://dev-lexic.swissgeol.ch/TectonicUnits/MiddlePenninic"/>
	<status xmlns="http://www.w3.org/ns/adms#" rdf:resource="https://dev-lexic.swissgeol.ch/active"/>
</rdf:Description>

<rdf:Description rdf:about="https://dev-lexic.swissgeol.ch/TectonicUnits/Siviez-MischabelNappe">
	<rdf:type rdf:resource="http://www.w3.org/2004/02/skos/core#Concept"/>
	<rdfs:isDefinedBy xml:lang="en">Gouffon Yves (Editor) (2024): Tectonic Map of Switzerland 1:500000, Explanatory notes. Federal Office of Topography swisstopo, Wabern</rdfs:isDefinedBy>
	<skos:definition xml:lang="en">The Siviez-Mischabel Nappe is a Middle Penninic tectonic unit of the Western Alps. It is made up of a crystalline basement with rocks of sedimentary and magmatic origin (Proterozoic to Ordovician), covered by a typical Briançonnais sedimentary cover. A Permian metagranite (Randa Orthogneiss) intruded the crystalline basement and the Permian cover. The sedimentary cover includes Permian to Triassic formations, completed by Jurassic to Eocene formations only in the normal limb of the nappe between Zermatt and the Val d’Anniviers, especially well developed in the Barrhorn region. Further west, the sedimentary cover is detached at the level of the Middle Triassic evaporites and form the Préalpes Médianes Rigides.</skos:definition>
	<skos:inScheme rdf:resource="https://dev-lexic.swissgeol.ch/TectonicUnits"/>
	<skos:prefLabel xml:lang="en">Siviez-Mischabel Nappe</skos:prefLabel>
	<skos:prefLabel xml:lang="de">Siviez-Mischabel-Decke</skos:prefLabel>
	<skos:prefLabel xml:lang="fr">Nappe de Siviez-Mischabel</skos:prefLabel>
	<skos:prefLabel xml:lang="it">Falda di Siviez-Mischabel</skos:prefLabel>
	<skos:broader rdf:resource="https://dev-lexic.swissgeol.ch/TectonicUnits/MiddlePenninic"/>
	<status xmlns="http://www.w3.org/ns/adms#" rdf:resource="https://dev-lexic.swissgeol.ch/active"/>
</rdf:Description>

<rdf:Description rdf:about="https://dev-lexic.swissgeol.ch/TectonicUnits/MontFortNappe">
	<rdf:type rdf:resource="http://www.w3.org/2004/02/skos/core#Concept"/>
	<rdfs:isDefinedBy xml:lang="en">Gouffon Yves (Editor) (2024): Tectonic Map of Switzerland 1:500000, Explanatory notes. Federal Office of Topography swisstopo, Wabern</rdfs:isDefinedBy>
	<skos:definition xml:lang="en">The Mont Fort Nappe is a Middle Penninic tectonic unit of the Western Alps extending from the Valle d’Aosta in the SSW to the Val d’Anniviers in the NNE. Its basement (similar to the upper, monocyclic part of that of the Siviez-Mischabel Nappe) ends as an anticline in the Val d’Hérémence, just downstream of the Grande Dixence Dam, but its Permian–Mesozoic sedimentary cover (characteristically including a large accumulation of breccias;) continues towards the east and forms pinched recumbent frontal folds with the lower part of the Tsaté Nappe up to the Lac de Moiry. Southward, the Mont Fort Nappe is interrupted by the Col de Bard Fault, but equivalent units are found further south in the Valle d’Aosta and in the Vanoise mountain range.</skos:definition>
	<skos:inScheme rdf:resource="https://dev-lexic.swissgeol.ch/TectonicUnits"/>
	<skos:prefLabel xml:lang="en">Mont Fort Nappe</skos:prefLabel>
	<skos:prefLabel xml:lang="de">Mont-Fort-Decke</skos:prefLabel>
	<skos:prefLabel xml:lang="fr">Nappe du Mont Fort</skos:prefLabel>
	<skos:prefLabel xml:lang="it">Falda del Mont Fort</skos:prefLabel>
	<skos:broader rdf:resource="https://dev-lexic.swissgeol.ch/TectonicUnits/MiddlePenninic"/>
	<status xmlns="http://www.w3.org/ns/adms#" rdf:resource="https://dev-lexic.swissgeol.ch/active"/>
</rdf:Description>

<rdf:Description rdf:about="https://dev-lexic.swissgeol.ch/TectonicUnits/PortjengratNappe">
	<rdf:type rdf:resource="http://www.w3.org/2004/02/skos/core#Concept"/>
	<rdfs:isDefinedBy xml:lang="en">Gouffon Yves (Editor) (2024): Tectonic Map of Switzerland 1:500000, Explanatory notes. Federal Office of Topography swisstopo, Wabern</rdfs:isDefinedBy>
	<skos:definition xml:lang="en">The Portjengrat Nappe, exposed east of Saas Fee, is a Middle Penninic tectonic unit that underwent a Alpine high-pressure metamorphism and occupies a special position as a buffer zone between the Siviez-Mischabel and Monte Rosa nappes on the one side and between the Zermatt - Saas Fee and Antrona nappes on the other side. It consists mainly of a crystalline basement resembling that of the Siviez-Mischabel and Monte Rosa nappes, overlain by a very thin Mesozoic sedimentary cover. Both basement and cover are crosscut by mafic veins, such as in the adjacent «Furgg Zone».</skos:definition>
	<skos:inScheme rdf:resource="https://dev-lexic.swissgeol.ch/TectonicUnits"/>
	<skos:prefLabel xml:lang="en">Portjengrat Nappe</skos:prefLabel>
	<skos:prefLabel xml:lang="de">Portjengrat-Decke</skos:prefLabel>
	<skos:prefLabel xml:lang="fr">Nappe du Portjengrat</skos:prefLabel>
	<skos:prefLabel xml:lang="it">Falda del Portjengrat</skos:prefLabel>
	<skos:broader rdf:resource="https://dev-lexic.swissgeol.ch/TectonicUnits/MiddlePenninic"/>
	<status xmlns="http://www.w3.org/ns/adms#" rdf:resource="https://dev-lexic.swissgeol.ch/active"/>
</rdf:Description>

<rdf:Description rdf:about="https://dev-lexic.swissgeol.ch/TectonicUnits/StockhornNappe">
	<rdf:type rdf:resource="http://www.w3.org/2004/02/skos/core#Concept"/>
	<rdfs:isDefinedBy xml:lang="en">Gouffon Yves (Editor) (2024): Tectonic Map of Switzerland 1:500000, Explanatory notes. Federal Office of Topography swisstopo, Wabern</rdfs:isDefinedBy>
	<skos:definition xml:lang="en">The Stockhorn Nappe is a small tectonic unit of the Middle Penninic, located on top of the Monte Rosa Nappe and separated from the Zermatt - Saas Fee Nappe by the thin Gornergrat Nappe. It is lithologically similar to the Portjengrat Nappe and can thus be correlated with it.</skos:definition>
	<skos:inScheme rdf:resource="https://dev-lexic.swissgeol.ch/TectonicUnits"/>
	<skos:prefLabel xml:lang="en">Stockhorn Nappe</skos:prefLabel>
	<skos:prefLabel xml:lang="de">Stockhorn-Decke</skos:prefLabel>
	<skos:prefLabel xml:lang="fr">Nappe du Stockhorn</skos:prefLabel>
	<skos:prefLabel xml:lang="it">Falda dello Stockhorn</skos:prefLabel>
	<skos:broader rdf:resource="https://dev-lexic.swissgeol.ch/TectonicUnits/MiddlePenninic"/>
	<status xmlns="http://www.w3.org/ns/adms#" rdf:resource="https://dev-lexic.swissgeol.ch/active"/>
</rdf:Description>

<rdf:Description rdf:about="https://dev-lexic.swissgeol.ch/TectonicUnits/MonteRosaNappe">
	<rdf:type rdf:resource="http://www.w3.org/2004/02/skos/core#Concept"/>
	<rdfs:isDefinedBy xml:lang="en">Gouffon Yves (Editor) (2024): Tectonic Map of Switzerland 1:500000, Explanatory notes. Federal Office of Topography swisstopo, Wabern</rdfs:isDefinedBy>
	<skos:definition xml:lang="en">The Monte Rosa Nappe is a Middle Penninic tectonic unit of the Western Alps mainly comprising a polycyclic crystalline basement (paragneisses and orthogneisses of Carboniferous and Permian intrusion age). This basement is subdivided in two parts by the thick Stellihorn Shear Zone. A sedimentary series, known as the «Furgg Zone» (Permian to Jurassic metasediments, crosscut by mafic sills and dykes), surrounds the crystalline basement in a discontinuous manner, and separates in particular the Monte Rosa gneisses from those of the Portjengrat Nappe. All the rocks of the Monte Rosa Nappe have undergone a high pressure metamorphism (eclogite facies).</skos:definition>
	<skos:inScheme rdf:resource="https://dev-lexic.swissgeol.ch/TectonicUnits"/>
	<skos:prefLabel xml:lang="en">Monte Rosa Nappe</skos:prefLabel>
	<skos:prefLabel xml:lang="de">Monte-Rosa-Decke</skos:prefLabel>
	<skos:prefLabel xml:lang="fr">Nappe du Mont Rose</skos:prefLabel>
	<skos:prefLabel xml:lang="it">Falda del Monte Rosa</skos:prefLabel>
	<skos:broader rdf:resource="https://dev-lexic.swissgeol.ch/TectonicUnits/MiddlePenninic"/>
	<status xmlns="http://www.w3.org/ns/adms#" rdf:resource="https://dev-lexic.swissgeol.ch/active"/>
</rdf:Description>

<rdf:Description rdf:about="https://dev-lexic.swissgeol.ch/TectonicUnits/TamboNappe">
	<rdf:type rdf:resource="http://www.w3.org/2004/02/skos/core#Concept"/>
	<rdfs:isDefinedBy xml:lang="en">Gouffon Yves (Editor) (2024): Tectonic Map of Switzerland 1:500000, Explanatory notes. Federal Office of Topography swisstopo, Wabern</rdfs:isDefinedBy>
	<skos:definition xml:lang="en">The Tambo Nappe is a Middle Penninic tectonic unit of eastern Switzerland made up of polymetamorphic paragneisses intruded by the Permian Truzzo Granite that escaped Paleozoic deformation and metamorphism. This crystalline basement is unconformably overlain by a Permian–Mesozoic cover roughly comparable to the Briançonnais facies of the Barrhorn (Siviez-Mischabel Nappe) and Vanoise series.</skos:definition>
	<skos:inScheme rdf:resource="https://dev-lexic.swissgeol.ch/TectonicUnits"/>
	<skos:prefLabel xml:lang="en">Tambo Nappe</skos:prefLabel>
	<skos:prefLabel xml:lang="de">Tambo-Decke</skos:prefLabel>
	<skos:prefLabel xml:lang="fr">Nappe du Tambo</skos:prefLabel>
	<skos:prefLabel xml:lang="it">Falda del Tambo</skos:prefLabel>
	<skos:broader rdf:resource="https://dev-lexic.swissgeol.ch/TectonicUnits/MiddlePenninic"/>
	<status xmlns="http://www.w3.org/ns/adms#" rdf:resource="https://dev-lexic.swissgeol.ch/active"/>
</rdf:Description>

<rdf:Description rdf:about="https://dev-lexic.swissgeol.ch/TectonicUnits/SurettaNappe">
	<rdf:type rdf:resource="http://www.w3.org/2004/02/skos/core#Concept"/>
	<rdfs:isDefinedBy xml:lang="en">Gouffon Yves (Editor) (2024): Tectonic Map of Switzerland 1:500000, Explanatory notes. Federal Office of Topography swisstopo, Wabern</rdfs:isDefinedBy>
	<skos:definition xml:lang="en">The Suretta Nappe is a Middle Penninic tectonic unit of eastern Switzerland made up of a Paleozoic basement of para- and orthogneisses intruded by the Permian Rofna Porphyry Complex, which consists of granitoids and effusive-type magmatites. Its Permian–Mesozoic cover, in Briançonnais facies, is largely of Triassic age. Locally the Triassic is overlain by Jurassic breccias. This cover crops out as thin layers; in one instance it follows a Suretta internal thrust fault, in other instances they are infolded into narrow synclines that were subsequently backfolded in the upper limb of the north facing Niemet-Beverin Backfold, whose axial trace runs across the Suretta Nappe.</skos:definition>
	<skos:inScheme rdf:resource="https://dev-lexic.swissgeol.ch/TectonicUnits"/>
	<skos:prefLabel xml:lang="en">Suretta Nappe</skos:prefLabel>
	<skos:prefLabel xml:lang="de">Suretta-Decke</skos:prefLabel>
	<skos:prefLabel xml:lang="fr">Nappe de Suretta</skos:prefLabel>
	<skos:prefLabel xml:lang="it">Falda di Suretta</skos:prefLabel>
	<skos:broader rdf:resource="https://dev-lexic.swissgeol.ch/TectonicUnits/MiddlePenninic"/>
	<status xmlns="http://www.w3.org/ns/adms#" rdf:resource="https://dev-lexic.swissgeol.ch/active"/>
</rdf:Description>

<rdf:Description rdf:about="https://dev-lexic.swissgeol.ch/TectonicUnits/SchamsNappeComplex">
	<rdf:type rdf:resource="http://www.w3.org/2004/02/skos/core#Concept"/>
	<rdfs:isDefinedBy xml:lang="en">Gouffon Yves (Editor) (2024): Tectonic Map of Switzerland 1:500000, Explanatory notes. Federal Office of Topography swisstopo, Wabern</rdfs:isDefinedBy>
	<skos:definition xml:lang="en">The Schams Nappe Complex is a Middle Penninic tectonic unit of eastern Switzerland encompassing a set of small nappes, which were folded after their emplacement around the Tambo-Suretta pair during the Niemet-Beverin post-nappe folding. The Schams Nappe Complex also contains different mélanges: to the west, in the lower limb of the Niemet-Beverin Backfold, the Knorren Mélange is in contact with the Tambo Nappe, while the Areua-Bruschghorn Mélange marks the boundary with the Tomül Nappe; to the east, in the upper (overturned) limb of the Niemet-Beverin Backfold, the Martegnas Mélange is in contact with the Arblatsch Flysch belonging to the Tomül Nappe.
The sedimentary sequences of the Schams Nappe Complex exhibit large facies variations and are rich in sedimentary syn-rift breccias of Middle Jurassic to Early Cretaceous age, indicating contemporaneous extension and sinistral strike-slip. The mid-Cretaceous to Cenozoic post-rift sediments are very similar to those found in the Falknis Nappe. Retrodeformation suggests that the Schams nappes formerly occupied an area north of the depositional area of the Tambo and Suretta Mesozoic. This is supported by facies arguments indicating that sediments in the originally northernmost paleogeographical position (now forming the Gelbhorn Nappe) suggest N-directed shedding of syn-rift breccias, and by the Subbriançonnais-type facies of the Triassic strata.</skos:definition>
	<skos:inScheme rdf:resource="https://dev-lexic.swissgeol.ch/TectonicUnits"/>
	<skos:prefLabel xml:lang="en">Schams Nappe Complex</skos:prefLabel>
	<skos:prefLabel xml:lang="de">Schams-Deckenkomplex</skos:prefLabel>
	<skos:prefLabel xml:lang="fr">Complexe de nappes du Schams</skos:prefLabel>
	<skos:prefLabel xml:lang="it">Complesso di falde dello Schams</skos:prefLabel>
	<skos:broader rdf:resource="https://dev-lexic.swissgeol.ch/TectonicUnits/MiddlePenninic"/>
	<skos:narrower rdf:resource="https://dev-lexic.swissgeol.ch/TectonicUnits/GelbhornNappe"/>
	<skos:narrower rdf:resource="https://dev-lexic.swissgeol.ch/TectonicUnits/Tschera-KalkbergNappe"/>
	<skos:narrower rdf:resource="https://dev-lexic.swissgeol.ch/TectonicUnits/KnorrenMelange"/>
	<skos:narrower rdf:resource="https://dev-lexic.swissgeol.ch/TectonicUnits/MartegnasMelange"/>
	<skos:narrower rdf:resource="https://dev-lexic.swissgeol.ch/TectonicUnits/Areua-BruschghornMelange"/>
	<status xmlns="http://www.w3.org/ns/adms#" rdf:resource="https://dev-lexic.swissgeol.ch/active"/>
</rdf:Description>

<rdf:Description rdf:about="https://dev-lexic.swissgeol.ch/TectonicUnits/FalknisNappe">
	<rdf:type rdf:resource="http://www.w3.org/2004/02/skos/core#Concept"/>
	<rdfs:isDefinedBy xml:lang="en">Gouffon Yves (Editor) (2024): Tectonic Map of Switzerland 1:500000, Explanatory notes. Federal Office of Topography swisstopo, Wabern</rdfs:isDefinedBy>
	<skos:definition xml:lang="en">The Middle Penninic Falknis Nappe (together with the tectonically higher Sulzfluh Nappe) discontinuously overlies thick Lower Penninic «Bündnerschiefer» and flysch of the Tomül Nappe in the Prättigau Half-Window. It is particularly well developed in the area of the eponymous summit where it is subdivided into several slices.
The Falknis Nappe is characterized by a more than 200 m thick Kimmeridgian–Tithonian Breccia overlain by Tithonian–Barremian marly limestones, Barremian–Aptian sandy limestones and fine grained breccias, as well as mid-Cretaceous to Cenozoic quartzbearing sandstone and Couches Rouges.</skos:definition>
	<skos:inScheme rdf:resource="https://dev-lexic.swissgeol.ch/TectonicUnits"/>
	<skos:prefLabel xml:lang="en">Falknis Nappe</skos:prefLabel>
	<skos:prefLabel xml:lang="de">Falknis-Decke</skos:prefLabel>
	<skos:prefLabel xml:lang="fr">Nappe du Falknis</skos:prefLabel>
	<skos:prefLabel xml:lang="it">Falda del Falknis</skos:prefLabel>
	<skos:broader rdf:resource="https://dev-lexic.swissgeol.ch/TectonicUnits/MiddlePenninic"/>
	<skos:narrower rdf:resource="https://dev-lexic.swissgeol.ch/TectonicUnits/TschingelSlice"/>
	<skos:narrower rdf:resource="https://dev-lexic.swissgeol.ch/TectonicUnits/GrauspitzSlice"/>
	<skos:narrower rdf:resource="https://dev-lexic.swissgeol.ch/TectonicUnits/GlegghornSlice"/>
	<status xmlns="http://www.w3.org/ns/adms#" rdf:resource="https://dev-lexic.swissgeol.ch/active"/>
</rdf:Description>

<rdf:Description rdf:about="https://dev-lexic.swissgeol.ch/TectonicUnits/SulzfluhNappe">
	<rdf:type rdf:resource="http://www.w3.org/2004/02/skos/core#Concept"/>
	<rdfs:isDefinedBy xml:lang="en">Gouffon Yves (Editor) (2024): Tectonic Map of Switzerland 1:500000, Explanatory notes. Federal Office of Topography swisstopo, Wabern</rdfs:isDefinedBy>
	<skos:definition xml:lang="en">The Middle Penninic Sulzfluh Nappe (together with the tectonically lower Falknis Nappe) discontinuously overlies thick Lower Penninic «Bündnerschiefer» and flysch of the Tomül Nappe in the Prättigau Half-Window. It consists of a series of Early Jurassic to Paleogene sediments of Briançonnais origin, with Late Jurassic sediments only represented by massive limestone (instead of breccia as in the Falknis Nappe). In a few places, crystalline basement lenses occur at the base of the Sulzfluh Nappe.</skos:definition>
	<skos:inScheme rdf:resource="https://dev-lexic.swissgeol.ch/TectonicUnits"/>
	<skos:prefLabel xml:lang="en">Sulzfluh Nappe</skos:prefLabel>
	<skos:prefLabel xml:lang="de">Sulzfluh-Decke</skos:prefLabel>
	<skos:prefLabel xml:lang="fr">Nappe de la Sulzfluh</skos:prefLabel>
	<skos:prefLabel xml:lang="it">Falda della Sulzfuh</skos:prefLabel>
	<skos:broader rdf:resource="https://dev-lexic.swissgeol.ch/TectonicUnits/MiddlePenninic"/>
	<status xmlns="http://www.w3.org/ns/adms#" rdf:resource="https://dev-lexic.swissgeol.ch/active"/>
</rdf:Description>

<rdf:Description rdf:about="https://dev-lexic.swissgeol.ch/TectonicUnits/FimberZone">
	<rdf:type rdf:resource="http://www.w3.org/2004/02/skos/core#Concept"/>
	<rdfs:isDefinedBy xml:lang="en">Gouffon Yves (Editor) (2024): Tectonic Map of Switzerland 1:500000, Explanatory notes. Federal Office of Topography swisstopo, Wabern</rdfs:isDefinedBy>
	<skos:definition xml:lang="en">In the northeastern (mostly Austrian) sector of the Lower Engadine Window, the Middle Penninic Fimber Zone replaces the Tasna Nappe. It consists of a mélange formation dominated by Late Cretaceous to Paleogene flysch-type sediments. These contain tectonic slices and olistoliths of highly variable size and lithological composition; many of them are lithologically identical with basement and Mesozoic cover typical for the Tasna Nappe. As this mélange contains quite a lot of ophiolitic bodies, the Fimber Zone – or at least a part of it – could also be correlated with the Arosa Zone.</skos:definition>
	<skos:inScheme rdf:resource="https://dev-lexic.swissgeol.ch/TectonicUnits"/>
	<skos:prefLabel xml:lang="en">Fimber Zone</skos:prefLabel>
	<skos:prefLabel xml:lang="de">Fimber-Zone</skos:prefLabel>
	<skos:prefLabel xml:lang="fr">Zone du Fimber</skos:prefLabel>
	<skos:prefLabel xml:lang="it">Zona del Fimber</skos:prefLabel>
	<skos:broader rdf:resource="https://dev-lexic.swissgeol.ch/TectonicUnits/MiddlePenninic"/>
	<status xmlns="http://www.w3.org/ns/adms#" rdf:resource="https://dev-lexic.swissgeol.ch/active"/>
</rdf:Description>

<rdf:Description rdf:about="https://dev-lexic.swissgeol.ch/TectonicUnits/TasnaNappe">
	<rdf:type rdf:resource="http://www.w3.org/2004/02/skos/core#Concept"/>
	<rdfs:isDefinedBy xml:lang="en">Gouffon Yves (Editor) (2024): Tectonic Map of Switzerland 1:500000, Explanatory notes. Federal Office of Topography swisstopo, Wabern</rdfs:isDefinedBy>
	<skos:definition xml:lang="en">The Tasna Nappe is a Middle Penninic tectonic unit of the Lower Engadine Window. In its western apart, its continental basement is stratigraphically overlain by Triassic to Jurassic sediments that have close similarities to those found in the Falknis Nappe. North of Ardez a Cretaceous–Paleogene sequence, again similar to that of the Briançonnais-derived Falknis Nappe, unconformably covers a former ocean-continent transition characterized by a detachment fault that exhumed subcontinental mantle.</skos:definition>
	<skos:inScheme rdf:resource="https://dev-lexic.swissgeol.ch/TectonicUnits"/>
	<skos:prefLabel xml:lang="en">Tasna Nappe</skos:prefLabel>
	<skos:prefLabel xml:lang="de">Tasna-Decke</skos:prefLabel>
	<skos:prefLabel xml:lang="fr">Nappe de Tasna</skos:prefLabel>
	<skos:prefLabel xml:lang="it">Falda di Tasna</skos:prefLabel>
	<skos:broader rdf:resource="https://dev-lexic.swissgeol.ch/TectonicUnits/MiddlePenninic"/>
	<status xmlns="http://www.w3.org/ns/adms#" rdf:resource="https://dev-lexic.swissgeol.ch/active"/>
</rdf:Description>

<rdf:Description rdf:about="https://dev-lexic.swissgeol.ch/TectonicUnits/GetsNappe">
	<rdf:type rdf:resource="http://www.w3.org/2004/02/skos/core#Concept"/>
	<rdfs:isDefinedBy xml:lang="en">Gouffon Yves (Editor) (2024): Tectonic Map of Switzerland 1:500000, Explanatory notes. Federal Office of Topography swisstopo, Wabern</rdfs:isDefinedBy>
	<skos:definition xml:lang="en">The Gets Nappe is the highest Upper Penninic tectonic units of the Prealps, featuring a very complicated structure and characteristically containing ophiolitic rocks.</skos:definition>
	<skos:inScheme rdf:resource="https://dev-lexic.swissgeol.ch/TectonicUnits"/>
	<skos:prefLabel xml:lang="en">Gets Nappe</skos:prefLabel>
	<skos:prefLabel xml:lang="de">Gets-Decke</skos:prefLabel>
	<skos:prefLabel xml:lang="fr">Nappe des Gets</skos:prefLabel>
	<skos:prefLabel xml:lang="it">Falda dei Gets</skos:prefLabel>
	<skos:broader rdf:resource="https://dev-lexic.swissgeol.ch/TectonicUnits/UpperPenninic"/>
	<status xmlns="http://www.w3.org/ns/adms#" rdf:resource="https://dev-lexic.swissgeol.ch/active"/>
</rdf:Description>

<rdf:Description rdf:about="https://dev-lexic.swissgeol.ch/TectonicUnits/SimmeNappe">
	<rdf:type rdf:resource="http://www.w3.org/2004/02/skos/core#Concept"/>
	<rdfs:isDefinedBy xml:lang="en">Gouffon Yves (Editor) (2024): Tectonic Map of Switzerland 1:500000, Explanatory notes. Federal Office of Topography swisstopo, Wabern</rdfs:isDefinedBy>
	<skos:definition xml:lang="en">The Simme Nappe is an Upper Penninic tectonic unit of the Prealps. It is constituted by pelagic Mesozoic sediments of Adriatic affinity (Middle Jurassic–Early Cretaceous) overlain by a Turonian–Santonian flysch. This succession is disrupted by internal thrusts that repeat part of the sequence and create an internal mélange. This internal structure of the Simme Nappe implies a north to south thrust of the northern part over the southern part during Late Cretaceous times.</skos:definition>
	<skos:inScheme rdf:resource="https://dev-lexic.swissgeol.ch/TectonicUnits"/>
	<skos:prefLabel xml:lang="en">Simme Nappe</skos:prefLabel>
	<skos:prefLabel xml:lang="de">Simmen-Decke</skos:prefLabel>
	<skos:prefLabel xml:lang="fr">Nappe de la Simme</skos:prefLabel>
	<skos:prefLabel xml:lang="it">Falda della Simme</skos:prefLabel>
	<skos:broader rdf:resource="https://dev-lexic.swissgeol.ch/TectonicUnits/UpperPenninic"/>
	<status xmlns="http://www.w3.org/ns/adms#" rdf:resource="https://dev-lexic.swissgeol.ch/active"/>
</rdf:Description>

<rdf:Description rdf:about="https://dev-lexic.swissgeol.ch/TectonicUnits/DransesNappe">
	<rdf:type rdf:resource="http://www.w3.org/2004/02/skos/core#Concept"/>
	<rdfs:isDefinedBy xml:lang="en">Gouffon Yves (Editor) (2024): Tectonic Map of Switzerland 1:500000, Explanatory notes. Federal Office of Topography swisstopo, Wabern</rdfs:isDefinedBy>
	<skos:definition xml:lang="en">The Dranses Nappe is an Upper Penninic tectonic unit of the Prealps. It is constituted by a basal shaly complex followed by a thick succession of calcareous flysch rich in trace fossils (Nereites isp. [formerly Helminthoidea isp.]) and occasional conglomerate beds. The age of this series is Late Cretaceous.</skos:definition>
	<skos:inScheme rdf:resource="https://dev-lexic.swissgeol.ch/TectonicUnits"/>
	<skos:prefLabel xml:lang="en">Dranses Nappe</skos:prefLabel>
	<skos:prefLabel xml:lang="de">Dranses-Decke</skos:prefLabel>
	<skos:prefLabel xml:lang="fr">Nappe des Dranses</skos:prefLabel>
	<skos:prefLabel xml:lang="it">Falda delle Dranses</skos:prefLabel>
	<skos:broader rdf:resource="https://dev-lexic.swissgeol.ch/TectonicUnits/UpperPenninic"/>
	<status xmlns="http://www.w3.org/ns/adms#" rdf:resource="https://dev-lexic.swissgeol.ch/active"/>
</rdf:Description>

<rdf:Description rdf:about="https://dev-lexic.swissgeol.ch/TectonicUnits/SarineNappe">
	<rdf:type rdf:resource="http://www.w3.org/2004/02/skos/core#Concept"/>
	<rdfs:isDefinedBy xml:lang="en">Gouffon Yves (Editor) (2024): Tectonic Map of Switzerland 1:500000, Explanatory notes. Federal Office of Topography swisstopo, Wabern</rdfs:isDefinedBy>
	<skos:definition xml:lang="en">The Sarine Nappe is an Upper Penninic tectonic unit of the Prealps. Although strongly resembling the Dranses Nappe lithologically, it is characterized by the presence of very fine-grained, lightcolored limestones with trace fossils (Chondrites isp.) and polymict micaceous conglomerates, often containing various crystalline rocks. The age of these rocks is latest Cretaceous to earliest Paleocene.</skos:definition>
	<skos:inScheme rdf:resource="https://dev-lexic.swissgeol.ch/TectonicUnits"/>
	<skos:prefLabel xml:lang="en">Sarine Nappe</skos:prefLabel>
	<skos:prefLabel xml:lang="de">Saane-Decke</skos:prefLabel>
	<skos:prefLabel xml:lang="fr">Nappe de la Sarine</skos:prefLabel>
	<skos:prefLabel xml:lang="it">Falda della Sarine</skos:prefLabel>
	<skos:broader rdf:resource="https://dev-lexic.swissgeol.ch/TectonicUnits/UpperPenninic"/>
	<status xmlns="http://www.w3.org/ns/adms#" rdf:resource="https://dev-lexic.swissgeol.ch/active"/>
</rdf:Description>

<rdf:Description rdf:about="https://dev-lexic.swissgeol.ch/TectonicUnits/AntronaNappe">
	<rdf:type rdf:resource="http://www.w3.org/2004/02/skos/core#Concept"/>
	<rdfs:isDefinedBy xml:lang="en">Gouffon Yves (Editor) (2024): Tectonic Map of Switzerland 1:500000, Explanatory notes. Federal Office of Topography swisstopo, Wabern</rdfs:isDefinedBy>
	<skos:definition xml:lang="en">The Antrona Nappe is an Upper Penninic tectonic unit made up of oceanic rocks with eclogitic relics (similar to the Zermatt-Saas Fee Nappe, except for the metacherts that are missing). Structurally, it is situated below the Monte Rosa Nappe, but above the Siviez-Mischabel Nappe and its probable extension in the Camughera Nappe. This peculiar position between two Middle Penninic units raises questions concerning its kinematic history and paleogeographic origin.</skos:definition>
	<skos:inScheme rdf:resource="https://dev-lexic.swissgeol.ch/TectonicUnits"/>
	<skos:prefLabel xml:lang="en">Antrona Nappe</skos:prefLabel>
	<skos:prefLabel xml:lang="de">Antrona-Decke</skos:prefLabel>
	<skos:prefLabel xml:lang="fr">Nappe d'Antrona</skos:prefLabel>
	<skos:prefLabel xml:lang="it">Falda di Antrona</skos:prefLabel>
	<skos:broader rdf:resource="https://dev-lexic.swissgeol.ch/TectonicUnits/UpperPenninic"/>
	<status xmlns="http://www.w3.org/ns/adms#" rdf:resource="https://dev-lexic.swissgeol.ch/active"/>
</rdf:Description>

<rdf:Description rdf:about="https://dev-lexic.swissgeol.ch/TectonicUnits/Zermatt-SaasFeeNappe">
	<rdf:type rdf:resource="http://www.w3.org/2004/02/skos/core#Concept"/>
	<rdfs:isDefinedBy xml:lang="en">Gouffon Yves (Editor) (2024): Tectonic Map of Switzerland 1:500000, Explanatory notes. Federal Office of Topography swisstopo, Wabern</rdfs:isDefinedBy>
	<skos:definition xml:lang="en">The Zermatt-Saas Fee Nappe is an Upper Penninic tectonic unit of the Western Alps consisting of rocks of Middle to Late Jurassic age derived from the Piemonte-Liguria Ocean. They are mostly large bodies of serpentinites, metagabbros and metabasalts in which pillow structures are locally well preserved. Oceanic sediments overlie these ophiolites, in particular metacherts (metaradiolarites). All of these rocks display relics of Early Eocene high-pressure metamorphism in eclogite facies.</skos:definition>
	<skos:inScheme rdf:resource="https://dev-lexic.swissgeol.ch/TectonicUnits"/>
	<skos:prefLabel xml:lang="en">Zermatt - Saas Fee Nappe</skos:prefLabel>
	<skos:prefLabel xml:lang="de">Zermatt-Saas-Fee-Decke</skos:prefLabel>
	<skos:prefLabel xml:lang="fr">Nappe de Zermatt - Sass Fee</skos:prefLabel>
	<skos:prefLabel xml:lang="it">Falda di Zermatt - Saas Fee</skos:prefLabel>
	<skos:broader rdf:resource="https://dev-lexic.swissgeol.ch/TectonicUnits/UpperPenninic"/>
	<status xmlns="http://www.w3.org/ns/adms#" rdf:resource="https://dev-lexic.swissgeol.ch/active"/>
</rdf:Description>

<rdf:Description rdf:about="https://dev-lexic.swissgeol.ch/TectonicUnits/TheodulgletscherSlice">
	<rdf:type rdf:resource="http://www.w3.org/2004/02/skos/core#Concept"/>
	<rdfs:isDefinedBy xml:lang="en">Gouffon Yves (Editor) (2024): Tectonic Map of Switzerland 1:500000, Explanatory notes. Federal Office of Topography swisstopo, Wabern</rdfs:isDefinedBy>
	<skos:definition xml:lang="en">The Theodulgletscher Slice is an Upper Penninic tectonic unit situated between the Zermatt-Saas Fee Nappe and the Tsaté Nappe. It comprises eclogitic continental basement rocks similar to that of the structurally higher Dent Blanche and Sesia nappes. It is likely derived from extensional allochthons, formed during the Jurassic opening of the Piemonte-Liguria Ocean in a more distal position than the Cervinia Terrane from which the Salassic nappes originate.</skos:definition>
	<skos:inScheme rdf:resource="https://dev-lexic.swissgeol.ch/TectonicUnits"/>
	<skos:prefLabel xml:lang="en">Theodulgletscher Slice</skos:prefLabel>
	<skos:prefLabel xml:lang="de">Theodulgletscher-Schuppe</skos:prefLabel>
	<skos:prefLabel xml:lang="fr">Écaille du Theodulgletscher</skos:prefLabel>
	<skos:prefLabel xml:lang="it">Scaglia del Theodulgletscher</skos:prefLabel>
	<skos:broader rdf:resource="https://dev-lexic.swissgeol.ch/TectonicUnits/UpperPenninic"/>
	<status xmlns="http://www.w3.org/ns/adms#" rdf:resource="https://dev-lexic.swissgeol.ch/active"/>
</rdf:Description>

<rdf:Description rdf:about="https://dev-lexic.swissgeol.ch/TectonicUnits/MontEmiliusNappe">
	<rdf:type rdf:resource="http://www.w3.org/2004/02/skos/core#Concept"/>
	<rdfs:isDefinedBy xml:lang="en">Gouffon Yves (Editor) (2024): Tectonic Map of Switzerland 1:500000, Explanatory notes. Federal Office of Topography swisstopo, Wabern</rdfs:isDefinedBy>
	<skos:definition xml:lang="en">The Mont Emilius Nappe is an Upper Penninic tectonic unit situated between the Zermatt-Saas Fee Nappe and the Tsaté Nappe. It comprises eclogitic continental basement rocks similar to that of the structurally higher Dent Blanche and Sesia nappes. It is likely derived from extensional allochthons, formed during the Jurassic opening of the Piemonte-Liguria Ocean in a more distal position than the Cervinia Terrane from which the Salassic nappes originate.</skos:definition>
	<skos:inScheme rdf:resource="https://dev-lexic.swissgeol.ch/TectonicUnits"/>
	<skos:prefLabel xml:lang="en">Mont Emilius Nappe</skos:prefLabel>
	<skos:prefLabel xml:lang="de">Mont-Emilius-Decke</skos:prefLabel>
	<skos:prefLabel xml:lang="fr">Nappe du Mont Emilius</skos:prefLabel>
	<skos:prefLabel xml:lang="it">Falda del Mont Emilius</skos:prefLabel>
	<skos:broader rdf:resource="https://dev-lexic.swissgeol.ch/TectonicUnits/UpperPenninic"/>
	<status xmlns="http://www.w3.org/ns/adms#" rdf:resource="https://dev-lexic.swissgeol.ch/active"/>
</rdf:Description>

<rdf:Description rdf:about="https://dev-lexic.swissgeol.ch/TectonicUnits/Etirol-LevazSlice">
	<rdf:type rdf:resource="http://www.w3.org/2004/02/skos/core#Concept"/>
	<rdfs:isDefinedBy xml:lang="en">Gouffon Yves (Editor) (2024): Tectonic Map of Switzerland 1:500000, Explanatory notes. Federal Office of Topography swisstopo, Wabern</rdfs:isDefinedBy>
	<skos:definition xml:lang="en">The Etirol-Levaz Slice is an Upper Penninic tectonic unit situated between the Zermatt-Saas Fee Nappe and the Tsaté Nappe. It comprises eclogitic micaschists similar to that of the structurally higher Dent Blanche and Sesia nappes. It is likely derived from extensional allochthons, formed during the Jurassic opening of the Piemonte-Liguria Ocean in a more distal position than the Cervinia Terrane from which the Salassic nappes originate.</skos:definition>
	<skos:inScheme rdf:resource="https://dev-lexic.swissgeol.ch/TectonicUnits"/>
	<skos:prefLabel xml:lang="en">Etirol-Levaz Slice</skos:prefLabel>
	<skos:prefLabel xml:lang="de">Etirol-Levaz-Schuppe</skos:prefLabel>
	<skos:prefLabel xml:lang="fr">Écaille d'Etirol-Levaz</skos:prefLabel>
	<skos:prefLabel xml:lang="it">Scaglia di Etirol-Levaz</skos:prefLabel>
	<skos:broader rdf:resource="https://dev-lexic.swissgeol.ch/TectonicUnits/UpperPenninic"/>
	<status xmlns="http://www.w3.org/ns/adms#" rdf:resource="https://dev-lexic.swissgeol.ch/active"/>
</rdf:Description>

<rdf:Description rdf:about="https://dev-lexic.swissgeol.ch/TectonicUnits/Chatillon-St-VincentSlices">
	<rdf:type rdf:resource="http://www.w3.org/2004/02/skos/core#Concept"/>
	<rdfs:isDefinedBy xml:lang="en">Gouffon Yves (Editor) (2024): Tectonic Map of Switzerland 1:500000, Explanatory notes. Federal Office of Topography swisstopo, Wabern</rdfs:isDefinedBy>
	<skos:definition xml:lang="en">The Châtillon-St-Vincent Slices are Upper Penninic tectonic units situated between the Zermatt-Saas Fee Nappe and the Tsaté Nappe. They comprise eclogitic continental basement rocks similar to that of the structurally higher Dent Blanche and Sesia nappes. They are likely derived from extensional allochthons, formed during the Jurassic opening of the Piemonte-Liguria Ocean in a more distal position than the Cervinia Terrane from which the Salassic nappes originate.</skos:definition>
	<skos:inScheme rdf:resource="https://dev-lexic.swissgeol.ch/TectonicUnits"/>
	<skos:prefLabel xml:lang="en">Châtillon-St-Vincent Slices</skos:prefLabel>
	<skos:prefLabel xml:lang="de">Châtillon-St-Vincent-Schuppen</skos:prefLabel>
	<skos:prefLabel xml:lang="fr">Écailles de Châtillon-St-Vincent</skos:prefLabel>
	<skos:prefLabel xml:lang="it">Scaglie di Châtillon-St-Vincent</skos:prefLabel>
	<skos:broader rdf:resource="https://dev-lexic.swissgeol.ch/TectonicUnits/UpperPenninic"/>
	<skos:narrower rdf:resource="https://dev-lexic.swissgeol.ch/TectonicUnits/ChatillonSlice"/>
	<skos:narrower rdf:resource="https://dev-lexic.swissgeol.ch/TectonicUnits/PonteySlice"/>
	<skos:narrower rdf:resource="https://dev-lexic.swissgeol.ch/TectonicUnits/GrunSlice"/>
	<skos:narrower rdf:resource="https://dev-lexic.swissgeol.ch/TectonicUnits/VollonSlice"/>
	<status xmlns="http://www.w3.org/ns/adms#" rdf:resource="https://dev-lexic.swissgeol.ch/active"/>
</rdf:Description>

<rdf:Description rdf:about="https://dev-lexic.swissgeol.ch/TectonicUnits/GornergratNappe">
	<rdf:type rdf:resource="http://www.w3.org/2004/02/skos/core#Concept"/>
	<rdfs:isDefinedBy xml:lang="en">Gouffon Yves (Editor) (2024): Tectonic Map of Switzerland 1:500000, Explanatory notes. Federal Office of Topography swisstopo, Wabern</rdfs:isDefinedBy>
	<skos:definition xml:lang="en">The Gornergrat Nappe is a thin tectonic unit located at the contact between the Middle and Upper Penninic in the Val d’Anniviers, Zermatt Valley and Valtournanche. It is composed of a series of Briançonnais-type Permian–Triassic sediments overlain by Jurassic breccias and limestone and calcschists probably of Cretaceous age (hence quite similar to that of the Mont Fort Nappe).</skos:definition>
	<skos:inScheme rdf:resource="https://dev-lexic.swissgeol.ch/TectonicUnits"/>
	<skos:prefLabel xml:lang="en">Gornergrat Nappe</skos:prefLabel>
	<skos:prefLabel xml:lang="de">Gornergrat-Decke</skos:prefLabel>
	<skos:prefLabel xml:lang="fr">Nappe du Gornergrat</skos:prefLabel>
	<skos:prefLabel xml:lang="it">Falda del Gornergrat</skos:prefLabel>
	<skos:broader rdf:resource="https://dev-lexic.swissgeol.ch/TectonicUnits/UpperPenninic"/>
	<status xmlns="http://www.w3.org/ns/adms#" rdf:resource="https://dev-lexic.swissgeol.ch/active"/>
</rdf:Description>

<rdf:Description rdf:about="https://dev-lexic.swissgeol.ch/TectonicUnits/CimesBlanchesNappe">
	<rdf:type rdf:resource="http://www.w3.org/2004/02/skos/core#Concept"/>
	<rdfs:isDefinedBy xml:lang="en">Gouffon Yves (Editor) (2024): Tectonic Map of Switzerland 1:500000, Explanatory notes. Federal Office of Topography swisstopo, Wabern</rdfs:isDefinedBy>
	<skos:definition xml:lang="en">The Cimes Blanches Nappe is a thin Upper Penninic tectonic unit intercalated within the Tsaté Nappe in the Val d’Anniviers, Zermatt Valley and Valtournanche. It is composed of a series of Briançonnais-type Permian–Triassic sediments overlain by Jurassic breccias and limestone and calcschists probably of Cretaceous age (hence quite similar to that of the Mont Fort Nappe).</skos:definition>
	<skos:inScheme rdf:resource="https://dev-lexic.swissgeol.ch/TectonicUnits"/>
	<skos:prefLabel xml:lang="en">Cimes Blanches Nappe</skos:prefLabel>
	<skos:prefLabel xml:lang="de">Cimes-Blanches-Decke</skos:prefLabel>
	<skos:prefLabel xml:lang="fr">Nappe des Cimes Blanches</skos:prefLabel>
	<skos:prefLabel xml:lang="it">Falda delle Cime Bianche</skos:prefLabel>
	<skos:broader rdf:resource="https://dev-lexic.swissgeol.ch/TectonicUnits/UpperPenninic"/>
	<status xmlns="http://www.w3.org/ns/adms#" rdf:resource="https://dev-lexic.swissgeol.ch/active"/>
</rdf:Description>

<rdf:Description rdf:about="https://dev-lexic.swissgeol.ch/TectonicUnits/FrilihornNappe">
	<rdf:type rdf:resource="http://www.w3.org/2004/02/skos/core#Concept"/>
	<rdfs:isDefinedBy xml:lang="en">Gouffon Yves (Editor) (2024): Tectonic Map of Switzerland 1:500000, Explanatory notes. Federal Office of Topography swisstopo, Wabern</rdfs:isDefinedBy>
	<skos:definition xml:lang="en">The Frilihorn Nappe is a thin Upper Penninic tectonic unit intercalated within the Tsaté Nappe in the Val d’Anniviers, Zermatt Valley and Valtournanche. It is composed of a series of Briançonnais-type Permian–Triassic sediments overlain by Jurassic breccias and limestone and calcschists probably of Cretaceous age (hence quite similar to that of the Mont Fort Nappe).</skos:definition>
	<skos:inScheme rdf:resource="https://dev-lexic.swissgeol.ch/TectonicUnits"/>
	<skos:prefLabel xml:lang="en">Frilihorn Nappe</skos:prefLabel>
	<skos:prefLabel xml:lang="de">Frilihorn-Decke</skos:prefLabel>
	<skos:prefLabel xml:lang="fr">Nappe du Frilihorn</skos:prefLabel>
	<skos:prefLabel xml:lang="it">Falda del Frilihorn</skos:prefLabel>
	<skos:broader rdf:resource="https://dev-lexic.swissgeol.ch/TectonicUnits/UpperPenninic"/>
	<status xmlns="http://www.w3.org/ns/adms#" rdf:resource="https://dev-lexic.swissgeol.ch/active"/>
</rdf:Description>

<rdf:Description rdf:about="https://dev-lexic.swissgeol.ch/TectonicUnits/TsateNappe">
	<rdf:type rdf:resource="http://www.w3.org/2004/02/skos/core#Concept"/>
	<rdfs:isDefinedBy xml:lang="en">Gouffon Yves (Editor) (2024): Tectonic Map of Switzerland 1:500000, Explanatory notes. Federal Office of Topography swisstopo, Wabern</rdfs:isDefinedBy>
	<skos:definition xml:lang="en">The Tsaté Nappe is an Upper Penninic tectonic unit of the Western Alps cropping out in southern Valais and in the Valle d’Aosta. It comprises oceanic metasediments (mainly calcschists and black shales of Cretaceous age) and ophiolitic rocks of Jurassic age originating from the Piemonte-Liguria Ocean. This nappe is characterized by a chaotic aspect and metamorphism under conditions of blueschist facies followed by greenschist facies. It is interpreted as the result of the formation of an accretionary wedge at the foot of the active Adriatic margin and the subsequent subduction below this continental plate.</skos:definition>
	<skos:inScheme rdf:resource="https://dev-lexic.swissgeol.ch/TectonicUnits"/>
	<skos:prefLabel xml:lang="en">Tsaté Nappe</skos:prefLabel>
	<skos:prefLabel xml:lang="de">Tsaté-Decke</skos:prefLabel>
	<skos:prefLabel xml:lang="fr">Nappe du Tsaté</skos:prefLabel>
	<skos:prefLabel xml:lang="it">Falda del Tsaté</skos:prefLabel>
	<skos:broader rdf:resource="https://dev-lexic.swissgeol.ch/TectonicUnits/UpperPenninic"/>
	<status xmlns="http://www.w3.org/ns/adms#" rdf:resource="https://dev-lexic.swissgeol.ch/active"/>
</rdf:Description>

<rdf:Description rdf:about="https://dev-lexic.swissgeol.ch/TectonicUnits/AversNappe">
	<rdf:type rdf:resource="http://www.w3.org/2004/02/skos/core#Concept"/>
	<rdfs:isDefinedBy xml:lang="en">Gouffon Yves (Editor) (2024): Tectonic Map of Switzerland 1:500000, Explanatory notes. Federal Office of Topography swisstopo, Wabern</rdfs:isDefinedBy>
	<skos:definition xml:lang="en">The Avers Nappe is an Upper Penninic tectonic unit of eastern Switzerland made up of shaly-calcareous-sandy marine sediments and ophiolitic rocks originating from the Piemonte-Liguria Ocean. This nappe represents an accretionary wedge at the base of an upper plate consisting of the other Upper Penninic and overlying Austroalpine nappes. This wedge directly overlies the Mesozoic cover of the Middle Penninic Suretta Nappe and probably formed in the Early Paleocene. The basal thrust of the Avers Nappe was deformed congruently with the Suretta Nappe, and both units were later back-folded together in the upper limb of the huge Niemet-Beverin Backfold. A backthrust that formed during this same phase brought part of the Middle Penninic Schams Nappe Complex back towards SE over the Avers Nappe. In its southernmost part, a large normal fault (Turba Mylonite Zone) separates the Avers Nappe and the backthrust Schams and Tomül nappes in the footwall from the Platta and Malenco-Forno-Lizun nappes in the hangingwall.</skos:definition>
	<skos:inScheme rdf:resource="https://dev-lexic.swissgeol.ch/TectonicUnits"/>
	<skos:prefLabel xml:lang="en">Avers Nappe</skos:prefLabel>
	<skos:prefLabel xml:lang="de">Avers-Decke</skos:prefLabel>
	<skos:prefLabel xml:lang="fr">Nappe de l'Avers</skos:prefLabel>
	<skos:prefLabel xml:lang="it">Falda dell'Avers</skos:prefLabel>
	<skos:broader rdf:resource="https://dev-lexic.swissgeol.ch/TectonicUnits/UpperPenninic"/>
	<status xmlns="http://www.w3.org/ns/adms#" rdf:resource="https://dev-lexic.swissgeol.ch/active"/>
</rdf:Description>

<rdf:Description rdf:about="https://dev-lexic.swissgeol.ch/TectonicUnits/Malenco-Forno-LizunNappe">
	<rdf:type rdf:resource="http://www.w3.org/2004/02/skos/core#Concept"/>
	<rdfs:isDefinedBy xml:lang="en">Gouffon Yves (Editor) (2024): Tectonic Map of Switzerland 1:500000, Explanatory notes. Federal Office of Topography swisstopo, Wabern</rdfs:isDefinedBy>
	<skos:definition xml:lang="en">The Malenco-Forno-Lizun Nappe is an Upper Penninic tectonic unit of eastern Switzerland encompassing three units situated in adjacent areas (in the hangingwall of the Turba Normal Fault) but with distinct lithological assemblages of oceanic origin.</skos:definition>
	<skos:inScheme rdf:resource="https://dev-lexic.swissgeol.ch/TectonicUnits"/>
	<skos:prefLabel xml:lang="en">Malenco-Forno-Lizun Nappe</skos:prefLabel>
	<skos:prefLabel xml:lang="de">Malenco-Forno-Lizun-Decke</skos:prefLabel>
	<skos:prefLabel xml:lang="fr">Nappe de Malenco-Forno-Lizun</skos:prefLabel>
	<skos:prefLabel xml:lang="it">Falda di Malenco-Forno-Lizun</skos:prefLabel>
	<skos:broader rdf:resource="https://dev-lexic.swissgeol.ch/TectonicUnits/UpperPenninic"/>
	<status xmlns="http://www.w3.org/ns/adms#" rdf:resource="https://dev-lexic.swissgeol.ch/active"/>
</rdf:Description>

<rdf:Description rdf:about="https://dev-lexic.swissgeol.ch/TectonicUnits/PlattaNappe">
	<rdf:type rdf:resource="http://www.w3.org/2004/02/skos/core#Concept"/>
	<rdfs:isDefinedBy xml:lang="en">Gouffon Yves (Editor) (2024): Tectonic Map of Switzerland 1:500000, Explanatory notes. Federal Office of Topography swisstopo, Wabern</rdfs:isDefinedBy>
	<skos:definition xml:lang="en">The Platta Nappe is an Upper Penninic tectonic unit of eastern Switzerland consisting mainly of an ophiolitic basement, including metabasalts, serpentinites and some metagabbros, covered by a thin Late Jurassic to Cretaceous oceanic sedimentary cover, beginning with radiolarian cherts. The mafic rocks have undergone an Alpine greenschist-facies metamorphism. The upper part of the nappe contains slivers of continental lithologies and shows characteristics of an ocean-continent transition (distal Adriatic margin).</skos:definition>
	<skos:inScheme rdf:resource="https://dev-lexic.swissgeol.ch/TectonicUnits"/>
	<skos:prefLabel xml:lang="en">Platta Nappe</skos:prefLabel>
	<skos:prefLabel xml:lang="de">Platta-Decke</skos:prefLabel>
	<skos:prefLabel xml:lang="fr">Nappe du Platta</skos:prefLabel>
	<skos:prefLabel xml:lang="it">Falda del Platta</skos:prefLabel>
	<skos:broader rdf:resource="https://dev-lexic.swissgeol.ch/TectonicUnits/UpperPenninic"/>
	<status xmlns="http://www.w3.org/ns/adms#" rdf:resource="https://dev-lexic.swissgeol.ch/active"/>
</rdf:Description>

<rdf:Description rdf:about="https://dev-lexic.swissgeol.ch/TectonicUnits/ArosaZone">
	<rdf:type rdf:resource="http://www.w3.org/2004/02/skos/core#Concept"/>
	<rdfs:isDefinedBy xml:lang="en">Gouffon Yves (Editor) (2024): Tectonic Map of Switzerland 1:500000, Explanatory notes. Federal Office of Topography swisstopo, Wabern</rdfs:isDefinedBy>
	<skos:definition xml:lang="en">The Upper Penninic Arosa Zone, always located at the base of the Austroalpine units to which it was accreted in Late Cretaceous times, is a mélange zone of heterogeneous composition. It consists of a shaly matrix with slivers of ophiolites (e.g. Totalp Ophiolite Complex), pelagic sediments and flysch sequences, as well as crystalline basement and Triassic sediments with Austroalpine affinity.</skos:definition>
	<skos:inScheme rdf:resource="https://dev-lexic.swissgeol.ch/TectonicUnits"/>
	<skos:prefLabel xml:lang="en">Arosa Zone</skos:prefLabel>
	<skos:prefLabel xml:lang="de">Arosa-Zone</skos:prefLabel>
	<skos:prefLabel xml:lang="fr">Zone d'Arosa</skos:prefLabel>
	<skos:prefLabel xml:lang="it">Zona di Arosa</skos:prefLabel>
	<skos:broader rdf:resource="https://dev-lexic.swissgeol.ch/TectonicUnits/UpperPenninic"/>
	<skos:narrower rdf:resource="https://dev-lexic.swissgeol.ch/TectonicUnits/HaupterhornSlice"/>
	<skos:narrower rdf:resource="https://dev-lexic.swissgeol.ch/TectonicUnits/WeissfluhSlice"/>
	<skos:narrower rdf:resource="https://dev-lexic.swissgeol.ch/TectonicUnits/GotschnawangSlice"/>
	<skos:narrower rdf:resource="https://dev-lexic.swissgeol.ch/TectonicUnits/DrosSlice"/>
	<skos:narrower rdf:resource="https://dev-lexic.swissgeol.ch/TectonicUnits/TotalpOphioliteComplex"/>
	<status xmlns="http://www.w3.org/ns/adms#" rdf:resource="https://dev-lexic.swissgeol.ch/active"/>
</rdf:Description>

<rdf:Description rdf:about="https://dev-lexic.swissgeol.ch/TectonicUnits/Infra-NiesenMelange">
	<rdf:type rdf:resource="http://www.w3.org/2004/02/skos/core#Concept"/>
	<rdfs:isDefinedBy xml:lang="en">Gouffon Yves (Editor) (2024): Tectonic Map of Switzerland 1:500000, Explanatory notes. Federal Office of Topography swisstopo, Wabern</rdfs:isDefinedBy>
	<skos:definition xml:lang="en">The Infra-Niesen Mélange, forming the base of the Niesen Nappe, is composed of slivers of pre-flysch series within a mainly gypsum-anhydrite and rarely “wildflysch” matrix. These slivers consist of rare gneiss, Triassic to Late Jurassic sedimentary rocks as well as Niesen Flysch.</skos:definition>
	<skos:inScheme rdf:resource="https://dev-lexic.swissgeol.ch/TectonicUnits"/>
	<skos:prefLabel xml:lang="en">Infra-Niesen Mélange</skos:prefLabel>
	<skos:prefLabel xml:lang="de">Infraniesen-Melange</skos:prefLabel>
	<skos:prefLabel xml:lang="fr">Mélange infra-Niesen</skos:prefLabel>
	<skos:prefLabel xml:lang="it">Mélange infra-Niesen</skos:prefLabel>
	<skos:broader rdf:resource="https://dev-lexic.swissgeol.ch/TectonicUnits/NiesenNappe"/>
	<status xmlns="http://www.w3.org/ns/adms#" rdf:resource="https://dev-lexic.swissgeol.ch/active"/>
</rdf:Description>

<rdf:Description rdf:about="https://dev-lexic.swissgeol.ch/TectonicUnits/RosswaldSlice">
	<rdf:type rdf:resource="http://www.w3.org/2004/02/skos/core#Concept"/>
	<rdfs:isDefinedBy xml:lang="en">Gouffon Yves (Editor) (2024): Tectonic Map of Switzerland 1:500000, Explanatory notes. Federal Office of Topography swisstopo, Wabern</rdfs:isDefinedBy>
	<skos:definition xml:lang="en">In the Brig area (upper Valais), the Rosswald Slice forms a large anticline together with the Roignais-Versoyen Slice. The Rosswald Slice is only present east of the Rhône-Simplon Fault and forms the normal, thrusting limb, extending further east at the border of the Lepontic units. It contains only the upper formation of the «Valaisan Flysch» (St-Christophe-Formation).</skos:definition>
	<skos:inScheme rdf:resource="https://dev-lexic.swissgeol.ch/TectonicUnits"/>
	<skos:prefLabel xml:lang="en">Rosswald Slice</skos:prefLabel>
	<skos:prefLabel xml:lang="de">Rosswald-Schuppe</skos:prefLabel>
	<skos:prefLabel xml:lang="fr">Écaille de Rosswald</skos:prefLabel>
	<skos:prefLabel xml:lang="it">Scaglia di Rosswald</skos:prefLabel>
	<skos:broader rdf:resource="https://dev-lexic.swissgeol.ch/TectonicUnits/Sion-CourmayeurNappe"/>
	<status xmlns="http://www.w3.org/ns/adms#" rdf:resource="https://dev-lexic.swissgeol.ch/active"/>
</rdf:Description>

<rdf:Description rdf:about="https://dev-lexic.swissgeol.ch/TectonicUnits/FerretSlice">
	<rdf:type rdf:resource="http://www.w3.org/2004/02/skos/core#Concept"/>
	<rdfs:isDefinedBy xml:lang="en">Gouffon Yves (Editor) (2024): Tectonic Map of Switzerland 1:500000, Explanatory notes. Federal Office of Topography swisstopo, Wabern</rdfs:isDefinedBy>
	<skos:definition xml:lang="en">The Ferret Slice occupies the external part of the Sion-Courmayeur Nappe in Valais. It consists mostly of Cretaceous metasediments.</skos:definition>
	<skos:inScheme rdf:resource="https://dev-lexic.swissgeol.ch/TectonicUnits"/>
	<skos:prefLabel xml:lang="en">Ferret Slice</skos:prefLabel>
	<skos:prefLabel xml:lang="de">Ferret-Schuppe</skos:prefLabel>
	<skos:prefLabel xml:lang="fr">Écaille de Ferret</skos:prefLabel>
	<skos:prefLabel xml:lang="it">Scaglia di Ferret</skos:prefLabel>
	<skos:broader rdf:resource="https://dev-lexic.swissgeol.ch/TectonicUnits/Sion-CourmayeurNappe"/>
	<status xmlns="http://www.w3.org/ns/adms#" rdf:resource="https://dev-lexic.swissgeol.ch/active"/>
</rdf:Description>

<rdf:Description rdf:about="https://dev-lexic.swissgeol.ch/TectonicUnits/MoutiersSlice">
	<rdf:type rdf:resource="http://www.w3.org/2004/02/skos/core#Concept"/>
	<rdfs:isDefinedBy xml:lang="en">Gouffon Yves (Editor) (2024): Tectonic Map of Switzerland 1:500000, Explanatory notes. Federal Office of Topography swisstopo, Wabern</rdfs:isDefinedBy>
	<skos:definition xml:lang="en">The Moûtiers Slice forms the external part of the Sion-Courmayeur Nappe in Savoy and in the Valle d’Aosta. It comprises Carboniferous, Triassic and Cretaceous metasediments.</skos:definition>
	<skos:inScheme rdf:resource="https://dev-lexic.swissgeol.ch/TectonicUnits"/>
	<skos:prefLabel xml:lang="en">Moûtiers Slice</skos:prefLabel>
	<skos:prefLabel xml:lang="de">Moûtiers-Schuppe</skos:prefLabel>
	<skos:prefLabel xml:lang="fr">Écaille de Moûtiers</skos:prefLabel>
	<skos:prefLabel xml:lang="it">Scaglia di Moûtiers</skos:prefLabel>
	<skos:broader rdf:resource="https://dev-lexic.swissgeol.ch/TectonicUnits/Sion-CourmayeurNappe"/>
	<status xmlns="http://www.w3.org/ns/adms#" rdf:resource="https://dev-lexic.swissgeol.ch/active"/>
</rdf:Description>

<rdf:Description rdf:about="https://dev-lexic.swissgeol.ch/TectonicUnits/Roignais-VersoyenSlice">
	<rdf:type rdf:resource="http://www.w3.org/2004/02/skos/core#Concept"/>
	<rdfs:isDefinedBy xml:lang="en">Gouffon Yves (Editor) (2024): Tectonic Map of Switzerland 1:500000, Explanatory notes. Federal Office of Topography swisstopo, Wabern</rdfs:isDefinedBy>
	<skos:definition xml:lang="en">The Roignais-Versoyen Slice forms the median part of the Sion-Courmayeur Nappe from Savoy to the upper Valais. Its very characteristic lithology includes the Cretaceous «Valaisan Flysch» and a pre-flysch series with ophiolites.</skos:definition>
	<skos:inScheme rdf:resource="https://dev-lexic.swissgeol.ch/TectonicUnits"/>
	<skos:prefLabel xml:lang="en">Roignais-Versoyen Slice</skos:prefLabel>
	<skos:prefLabel xml:lang="de">Roignais-Versoyen-Schuppe</skos:prefLabel>
	<skos:prefLabel xml:lang="fr">Écaille du Roignais-Versoyen</skos:prefLabel>
	<skos:prefLabel xml:lang="it">Scaglia del Roignais-Versoyen</skos:prefLabel>
	<skos:broader rdf:resource="https://dev-lexic.swissgeol.ch/TectonicUnits/Sion-CourmayeurNappe"/>
	<status xmlns="http://www.w3.org/ns/adms#" rdf:resource="https://dev-lexic.swissgeol.ch/active"/>
</rdf:Description>

<rdf:Description rdf:about="https://dev-lexic.swissgeol.ch/TectonicUnits/PierreAvoiSlice">
	<rdf:type rdf:resource="http://www.w3.org/2004/02/skos/core#Concept"/>
	<rdfs:isDefinedBy xml:lang="en">Gouffon Yves (Editor) (2024): Tectonic Map of Switzerland 1:500000, Explanatory notes. Federal Office of Topography swisstopo, Wabern</rdfs:isDefinedBy>
	<skos:definition xml:lang="en">The Pierre Avoi Slice forms the internal part of the Sion-Courmayeur Nappe, above the Roignais-Versoyen Slice. It consists of a Paleogene mélange zone, whose material mostly comes from the overlying Zone Houillère as a result of early erosion.</skos:definition>
	<skos:inScheme rdf:resource="https://dev-lexic.swissgeol.ch/TectonicUnits"/>
	<skos:prefLabel xml:lang="en">Pierre Avoi Slice</skos:prefLabel>
	<skos:prefLabel xml:lang="de">Pierre-Avoi-Schuppe</skos:prefLabel>
	<skos:prefLabel xml:lang="fr">Écaille de la Pierre Avoi</skos:prefLabel>
	<skos:prefLabel xml:lang="it">Scaglia della Pierre Avoi</skos:prefLabel>
	<skos:broader rdf:resource="https://dev-lexic.swissgeol.ch/TectonicUnits/Sion-CourmayeurNappe"/>
	<status xmlns="http://www.w3.org/ns/adms#" rdf:resource="https://dev-lexic.swissgeol.ch/active"/>
</rdf:Description>

<rdf:Description rdf:about="https://dev-lexic.swissgeol.ch/TectonicUnits/PetitSt-BernardSlice">
	<rdf:type rdf:resource="http://www.w3.org/2004/02/skos/core#Concept"/>
	<rdfs:isDefinedBy xml:lang="en">Gouffon Yves (Editor) (2024): Tectonic Map of Switzerland 1:500000, Explanatory notes. Federal Office of Topography swisstopo, Wabern</rdfs:isDefinedBy>
	<skos:definition xml:lang="en">The Petit Saint-Bernard Slice is restricted to the area of the eponymous pass on the French-Italian border. It consists of a series of Triassic–Jurassic sediments with Subbriançonnais facies and is often considered as an independent tectonic unit thrust over the Sion-Courmayeur Nappe and, together with it, thrust under the Middle Penninic Zone Houillère.</skos:definition>
	<skos:inScheme rdf:resource="https://dev-lexic.swissgeol.ch/TectonicUnits"/>
	<skos:prefLabel xml:lang="en">Petit St-Bernard Slice</skos:prefLabel>
	<skos:prefLabel xml:lang="de">Petit-St-Bernard-Schuppe</skos:prefLabel>
	<skos:prefLabel xml:lang="fr">Écaille du Petit St-Bernard</skos:prefLabel>
	<skos:prefLabel xml:lang="it">Scaglia del Piccolo San Bernardo</skos:prefLabel>
	<skos:broader rdf:resource="https://dev-lexic.swissgeol.ch/TectonicUnits/Sion-CourmayeurNappe"/>
	<status xmlns="http://www.w3.org/ns/adms#" rdf:resource="https://dev-lexic.swissgeol.ch/active"/>
</rdf:Description>

<rdf:Description rdf:about="https://dev-lexic.swissgeol.ch/TectonicUnits/ForbeschSlice">
	<rdf:type rdf:resource="http://www.w3.org/2004/02/skos/core#Concept"/>
	<rdfs:isDefinedBy xml:lang="en">Gouffon Yves (Editor) (2024): Tectonic Map of Switzerland 1:500000, Explanatory notes. Federal Office of Topography swisstopo, Wabern</rdfs:isDefinedBy>
	<skos:inScheme rdf:resource="https://dev-lexic.swissgeol.ch/TectonicUnits"/>
	<skos:prefLabel xml:lang="en">Forbesch Slice</skos:prefLabel>
	<skos:prefLabel xml:lang="de">Forbesch-Schuppe</skos:prefLabel>
	<skos:prefLabel xml:lang="fr">Écaille du Forbesch</skos:prefLabel>
	<skos:prefLabel xml:lang="it">Scaglia del Forbesch</skos:prefLabel>
	<skos:broader rdf:resource="https://dev-lexic.swissgeol.ch/TectonicUnits/TomuelNappe"/>
	<status xmlns="http://www.w3.org/ns/adms#" rdf:resource="https://dev-lexic.swissgeol.ch/active"/>
</rdf:Description>

<rdf:Description rdf:about="https://dev-lexic.swissgeol.ch/TectonicUnits/PrealpesMedianesPlastiques">
	<rdf:type rdf:resource="http://www.w3.org/2004/02/skos/core#Concept"/>
	<rdfs:isDefinedBy xml:lang="en">Gouffon Yves (Editor) (2024): Tectonic Map of Switzerland 1:500000, Explanatory notes. Federal Office of Topography swisstopo, Wabern</rdfs:isDefinedBy>
	<skos:definition xml:lang="en">The Préalpes Médianes Plastiques form the external part of the Préalpes Médianes Nappe (found both in the Romandes Prealps and the Chablais Prealps), which is characterized by a succession of large fault-related folds with axes oriented E–W to SSW–NNE.</skos:definition>
	<skos:inScheme rdf:resource="https://dev-lexic.swissgeol.ch/TectonicUnits"/>
	<skos:prefLabel xml:lang="en">Préalpes Médianes Plastiques</skos:prefLabel>
	<skos:prefLabel xml:lang="de">Préalpes Médianes Plastiques</skos:prefLabel>
	<skos:prefLabel xml:lang="fr">Préalpes Médianes Plastiques</skos:prefLabel>
	<skos:prefLabel xml:lang="it">Préalpes Médianes Plastiques</skos:prefLabel>
	<skos:broader rdf:resource="https://dev-lexic.swissgeol.ch/TectonicUnits/PrealpesMedianesNappe"/>
	<status xmlns="http://www.w3.org/ns/adms#" rdf:resource="https://dev-lexic.swissgeol.ch/active"/>
</rdf:Description>

<rdf:Description rdf:about="https://dev-lexic.swissgeol.ch/TectonicUnits/PrealpesMedianesRigides">
	<rdf:type rdf:resource="http://www.w3.org/2004/02/skos/core#Concept"/>
	<rdfs:isDefinedBy xml:lang="en">Gouffon Yves (Editor) (2024): Tectonic Map of Switzerland 1:500000, Explanatory notes. Federal Office of Topography swisstopo, Wabern</rdfs:isDefinedBy>
	<skos:definition xml:lang="en">The Préalpes Médianes Rigides form the internal part of the Préalpes Médianes Nappe (mainly located in the Romandes Prealps), which consists of large imbricates.</skos:definition>
	<skos:inScheme rdf:resource="https://dev-lexic.swissgeol.ch/TectonicUnits"/>
	<skos:prefLabel xml:lang="en">Préalpes Médianes Rigides</skos:prefLabel>
	<skos:prefLabel xml:lang="de">Préalpes Médianes Rigides</skos:prefLabel>
	<skos:prefLabel xml:lang="fr">Préalpes Médianes Rigides</skos:prefLabel>
	<skos:prefLabel xml:lang="it">Préalpes Médianes Rigides</skos:prefLabel>
	<skos:broader rdf:resource="https://dev-lexic.swissgeol.ch/TectonicUnits/PrealpesMedianesNappe"/>
	<status xmlns="http://www.w3.org/ns/adms#" rdf:resource="https://dev-lexic.swissgeol.ch/active"/>
</rdf:Description>

<rdf:Description rdf:about="https://dev-lexic.swissgeol.ch/TectonicUnits/Mythen-RoggeneggSlice">
	<rdf:type rdf:resource="http://www.w3.org/2004/02/skos/core#Concept"/>
	<rdfs:isDefinedBy xml:lang="en">Gouffon Yves (Editor) (2024): Tectonic Map of Switzerland 1:500000, Explanatory notes. Federal Office of Topography swisstopo, Wabern</rdfs:isDefinedBy>
	<skos:inScheme rdf:resource="https://dev-lexic.swissgeol.ch/TectonicUnits"/>
	<skos:prefLabel xml:lang="en">Mythen-Roggenegg Slice</skos:prefLabel>
	<skos:prefLabel xml:lang="de">Mythen-Roggenegg-Schuppe</skos:prefLabel>
	<skos:prefLabel xml:lang="fr">Écaille des Mythen-Roggenegg</skos:prefLabel>
	<skos:prefLabel xml:lang="it">Scaglia delle Mythen-Roggenegg</skos:prefLabel>
	<skos:broader rdf:resource="https://dev-lexic.swissgeol.ch/TectonicUnits/PrealpesMedianesNappe"/>
	<status xmlns="http://www.w3.org/ns/adms#" rdf:resource="https://dev-lexic.swissgeol.ch/active"/>
</rdf:Description>

<rdf:Description rdf:about="https://dev-lexic.swissgeol.ch/TectonicUnits/ObereRotenflueSlice">
	<rdf:type rdf:resource="http://www.w3.org/2004/02/skos/core#Concept"/>
	<rdfs:isDefinedBy xml:lang="en">Gouffon Yves (Editor) (2024): Tectonic Map of Switzerland 1:500000, Explanatory notes. Federal Office of Topography swisstopo, Wabern</rdfs:isDefinedBy>
	<skos:inScheme rdf:resource="https://dev-lexic.swissgeol.ch/TectonicUnits"/>
	<skos:prefLabel xml:lang="en">Obere Rotenflue Slice</skos:prefLabel>
	<skos:prefLabel xml:lang="de">Obere Rotenflue-Schuppe</skos:prefLabel>
	<skos:prefLabel xml:lang="fr">Écaille d'Obere Rotenflue</skos:prefLabel>
	<skos:prefLabel xml:lang="it">Scaglia di Obere Rotenflue</skos:prefLabel>
	<skos:broader rdf:resource="https://dev-lexic.swissgeol.ch/TectonicUnits/PrealpesMedianesNappe"/>
	<status xmlns="http://www.w3.org/ns/adms#" rdf:resource="https://dev-lexic.swissgeol.ch/active"/>
</rdf:Description>

<rdf:Description rdf:about="https://dev-lexic.swissgeol.ch/TectonicUnits/Staeglerenegg-BruennelistockSlices">
	<rdf:type rdf:resource="http://www.w3.org/2004/02/skos/core#Concept"/>
	<rdfs:isDefinedBy xml:lang="en">Gouffon Yves (Editor) (2024): Tectonic Map of Switzerland 1:500000, Explanatory notes. Federal Office of Topography swisstopo, Wabern</rdfs:isDefinedBy>
	<skos:inScheme rdf:resource="https://dev-lexic.swissgeol.ch/TectonicUnits"/>
	<skos:prefLabel xml:lang="en">Stäglerenegg-Brünnelistock Slices</skos:prefLabel>
	<skos:prefLabel xml:lang="de">Stäglerenegg-Brünnelistock-Schuppen</skos:prefLabel>
	<skos:prefLabel xml:lang="fr">Écailles de Stäglerenegg-Brünnelistock</skos:prefLabel>
	<skos:prefLabel xml:lang="it">Scaglie di Stäglerenegg-Brünnelistock</skos:prefLabel>
	<skos:broader rdf:resource="https://dev-lexic.swissgeol.ch/TectonicUnits/PrealpesMedianesNappe"/>
	<status xmlns="http://www.w3.org/ns/adms#" rdf:resource="https://dev-lexic.swissgeol.ch/active"/>
</rdf:Description>

<rdf:Description rdf:about="https://dev-lexic.swissgeol.ch/TectonicUnits/ExternalZoneHouillere">
	<rdf:type rdf:resource="http://www.w3.org/2004/02/skos/core#Concept"/>
	<rdfs:isDefinedBy xml:lang="en">Gouffon Yves (Editor) (2024): Tectonic Map of Switzerland 1:500000, Explanatory notes. Federal Office of Topography swisstopo, Wabern</rdfs:isDefinedBy>
	<skos:definition xml:lang="en">The external part of the Zone Houillère, displaying a complex imbricated structure, is situated in a lower structural position than its internal part. It essentially consists of black shales with rare lenses of anthracite and grey sandstone or quartzite, with some conglomeratic levels. Permian sediments appear to be largely absent, whereas Triassic deposits are well developed («Trias médian» intercalated between the External and Internal Zone Houillère).</skos:definition>
	<skos:inScheme rdf:resource="https://dev-lexic.swissgeol.ch/TectonicUnits"/>
	<skos:prefLabel xml:lang="en">External Zone Houillère</skos:prefLabel>
	<skos:prefLabel xml:lang="de">Zone Houillère externe</skos:prefLabel>
	<skos:prefLabel xml:lang="fr">Zone Houillère externe</skos:prefLabel>
	<skos:prefLabel xml:lang="it">Zona Houillère esterna</skos:prefLabel>
	<skos:broader rdf:resource="https://dev-lexic.swissgeol.ch/TectonicUnits/ZoneHouillere"/>
	<status xmlns="http://www.w3.org/ns/adms#" rdf:resource="https://dev-lexic.swissgeol.ch/active"/>
</rdf:Description>

<rdf:Description rdf:about="https://dev-lexic.swissgeol.ch/TectonicUnits/InternalZoneHouillere">
	<rdf:type rdf:resource="http://www.w3.org/2004/02/skos/core#Concept"/>
	<rdfs:isDefinedBy xml:lang="en">Gouffon Yves (Editor) (2024): Tectonic Map of Switzerland 1:500000, Explanatory notes. Federal Office of Topography swisstopo, Wabern</rdfs:isDefinedBy>
	<skos:definition xml:lang="en">The internal part of the Zone Houillère is situated in a higher structural position than its external part. It consists of a thin band of black shales topped by Permian conglomerates and sandstone, as well as a narrow band of gypsum and cornieule («Trias bordier»).</skos:definition>
	<skos:inScheme rdf:resource="https://dev-lexic.swissgeol.ch/TectonicUnits"/>
	<skos:prefLabel xml:lang="en">Internal Zone Houillère</skos:prefLabel>
	<skos:prefLabel xml:lang="de">Zone Houillère interne</skos:prefLabel>
	<skos:prefLabel xml:lang="fr">Zone Houillère interne</skos:prefLabel>
	<skos:prefLabel xml:lang="it">Zona Houillère interna</skos:prefLabel>
	<skos:broader rdf:resource="https://dev-lexic.swissgeol.ch/TectonicUnits/ZoneHouillere"/>
	<status xmlns="http://www.w3.org/ns/adms#" rdf:resource="https://dev-lexic.swissgeol.ch/active"/>
</rdf:Description>

<rdf:Description rdf:about="https://dev-lexic.swissgeol.ch/TectonicUnits/VisperterminenSlice">
	<rdf:type rdf:resource="http://www.w3.org/2004/02/skos/core#Concept"/>
	<rdfs:isDefinedBy xml:lang="en">Gouffon Yves (Editor) (2024): Tectonic Map of Switzerland 1:500000, Explanatory notes. Federal Office of Topography swisstopo, Wabern</rdfs:isDefinedBy>
	<skos:definition xml:lang="en">The Visperterminen Slice is a Middle Penninic tectonic unit occupying the core of a fold within the Sion-Courmayeur Nappe between Visp and the Simplonpass. It consists of graphitic schist and paragneiss. By lithological and structural analogy, it is attributed to the Zone Houillère occuring further west.</skos:definition>
	<skos:inScheme rdf:resource="https://dev-lexic.swissgeol.ch/TectonicUnits"/>
	<skos:prefLabel xml:lang="en">Visperterminen Slice</skos:prefLabel>
	<skos:prefLabel xml:lang="de">Visperterminen-Schuppe</skos:prefLabel>
	<skos:prefLabel xml:lang="fr">Écaille de Visperterminen</skos:prefLabel>
	<skos:prefLabel xml:lang="it">Scaglia di Visperterminen</skos:prefLabel>
	<skos:broader rdf:resource="https://dev-lexic.swissgeol.ch/TectonicUnits/ZoneHouillere"/>
	<status xmlns="http://www.w3.org/ns/adms#" rdf:resource="https://dev-lexic.swissgeol.ch/active"/>
</rdf:Description>

<rdf:Description rdf:about="https://dev-lexic.swissgeol.ch/TectonicUnits/LowerStaldenSlice">
	<rdf:type rdf:resource="http://www.w3.org/2004/02/skos/core#Concept"/>
	<rdfs:isDefinedBy xml:lang="en">Gouffon Yves (Editor) (2024): Tectonic Map of Switzerland 1:500000, Explanatory notes. Federal Office of Topography swisstopo, Wabern</rdfs:isDefinedBy>
	<skos:definition xml:lang="en">The Lower Stalden Slice is a Middle Penninic tectonic unit occuring between Visp and the Simplonpass and attributed to the Zone Houillère by lithological (graphitic schist and paragneiss) and structural analogy. It is overlain by the Upper Stalden Nappe and separated from the Sion-Courmayeur Nappe by the southern branch of the Rhône-Simplon Fault.</skos:definition>
	<skos:inScheme rdf:resource="https://dev-lexic.swissgeol.ch/TectonicUnits"/>
	<skos:prefLabel xml:lang="en">Lower Stalden Slice</skos:prefLabel>
	<skos:prefLabel xml:lang="de">Untere Stalden-Schuppe</skos:prefLabel>
	<skos:prefLabel xml:lang="fr">Écaille inférieure de Stalden</skos:prefLabel>
	<skos:prefLabel xml:lang="it">Scaglia inferiore di Stalden</skos:prefLabel>
	<skos:broader rdf:resource="https://dev-lexic.swissgeol.ch/TectonicUnits/ZoneHouillere"/>
	<status xmlns="http://www.w3.org/ns/adms#" rdf:resource="https://dev-lexic.swissgeol.ch/active"/>
</rdf:Description>

<rdf:Description rdf:about="https://dev-lexic.swissgeol.ch/TectonicUnits/GelbhornNappe">
	<rdf:type rdf:resource="http://www.w3.org/2004/02/skos/core#Concept"/>
	<rdfs:isDefinedBy xml:lang="en">Gouffon Yves (Editor) (2024): Tectonic Map of Switzerland 1:500000, Explanatory notes. Federal Office of Topography swisstopo, Wabern</rdfs:isDefinedBy>
	<skos:definition xml:lang="en">The Gelbhorn Nappe is part of the Schams Nappe Complex. In the hanging wall of the Suretta Nappe (eastern Shams), the outer, fine-grained, calcareous limb of the unit (1b) is normal, while the inner, coarse-grained limb (1a) is overturned on the Tschera-Kalkberg Nappe. In the Westschams, and thus in the footwall of the Suretta Nappe, the structural situation is the other way round, i.e. the outer limb is overturned and the inner limb is normal.</skos:definition>
	<skos:inScheme rdf:resource="https://dev-lexic.swissgeol.ch/TectonicUnits"/>
	<skos:prefLabel xml:lang="en">Gelbhorn Nappe</skos:prefLabel>
	<skos:prefLabel xml:lang="de">Gelbhorn-Decke</skos:prefLabel>
	<skos:prefLabel xml:lang="fr">Nappe du Gelbhorn</skos:prefLabel>
	<skos:prefLabel xml:lang="it">Falda del Gelbhorn</skos:prefLabel>
	<skos:broader rdf:resource="https://dev-lexic.swissgeol.ch/TectonicUnits/SchamsNappeComplex"/>
	<status xmlns="http://www.w3.org/ns/adms#" rdf:resource="https://dev-lexic.swissgeol.ch/active"/>
</rdf:Description>

<rdf:Description rdf:about="https://dev-lexic.swissgeol.ch/TectonicUnits/Tschera-KalkbergNappe">
	<rdf:type rdf:resource="http://www.w3.org/2004/02/skos/core#Concept"/>
	<rdfs:isDefinedBy xml:lang="en">Gouffon Yves (Editor) (2024): Tectonic Map of Switzerland 1:500000, Explanatory notes. Federal Office of Topography swisstopo, Wabern</rdfs:isDefinedBy>
	<skos:definition xml:lang="en">The Tschera-Kalkberg Nappe is a tectonically complex, mélange-like inner sheath of the Schams Nappe Complex. It is divided into three subunits based on lithological criteria.</skos:definition>
	<skos:inScheme rdf:resource="https://dev-lexic.swissgeol.ch/TectonicUnits"/>
	<skos:prefLabel xml:lang="en">Tschera-Kalkberg Nappe</skos:prefLabel>
	<skos:prefLabel xml:lang="de">Tschera-Kalkberg-Decke</skos:prefLabel>
	<skos:prefLabel xml:lang="fr">Nappe du Tschera-Kalkberg</skos:prefLabel>
	<skos:prefLabel xml:lang="it">Falda del Tschera-Kalkberg</skos:prefLabel>
	<skos:broader rdf:resource="https://dev-lexic.swissgeol.ch/TectonicUnits/SchamsNappeComplex"/>
	<status xmlns="http://www.w3.org/ns/adms#" rdf:resource="https://dev-lexic.swissgeol.ch/active"/>
</rdf:Description>

<rdf:Description rdf:about="https://dev-lexic.swissgeol.ch/TectonicUnits/KnorrenMelange">
	<rdf:type rdf:resource="http://www.w3.org/2004/02/skos/core#Concept"/>
	<rdfs:isDefinedBy xml:lang="en">Gouffon Yves (Editor) (2024): Tectonic Map of Switzerland 1:500000, Explanatory notes. Federal Office of Topography swisstopo, Wabern</rdfs:isDefinedBy>
	<skos:definition xml:lang="en">The Knorren Mélange is a tectonic mélange situated in the lower limb of the Niemet-Beverin Backfold, at the contact between the Schams Nappe Complex and the Tambo Nappe.</skos:definition>
	<skos:inScheme rdf:resource="https://dev-lexic.swissgeol.ch/TectonicUnits"/>
	<skos:prefLabel xml:lang="en">Knorren Mélange</skos:prefLabel>
	<skos:prefLabel xml:lang="de">Knorren-Melange</skos:prefLabel>
	<skos:prefLabel xml:lang="fr">Mélange de Knorren</skos:prefLabel>
	<skos:prefLabel xml:lang="it">Mélange di Knorren</skos:prefLabel>
	<skos:broader rdf:resource="https://dev-lexic.swissgeol.ch/TectonicUnits/SchamsNappeComplex"/>
	<status xmlns="http://www.w3.org/ns/adms#" rdf:resource="https://dev-lexic.swissgeol.ch/active"/>
</rdf:Description>

<rdf:Description rdf:about="https://dev-lexic.swissgeol.ch/TectonicUnits/MartegnasMelange">
	<rdf:type rdf:resource="http://www.w3.org/2004/02/skos/core#Concept"/>
	<rdfs:isDefinedBy xml:lang="en">Gouffon Yves (Editor) (2024): Tectonic Map of Switzerland 1:500000, Explanatory notes. Federal Office of Topography swisstopo, Wabern</rdfs:isDefinedBy>
	<skos:definition xml:lang="en">The Martegnas Mélange is a tectonic mélange situated in the upper (overturned) limb of the Niemet-Beverin Backfold, at the contact between the Schams Nappe Complex and the Arblatsch Flysch (Tomül Nappe).</skos:definition>
	<skos:inScheme rdf:resource="https://dev-lexic.swissgeol.ch/TectonicUnits"/>
	<skos:prefLabel xml:lang="en">Martegnas Mélange</skos:prefLabel>
	<skos:prefLabel xml:lang="de">Martegnas-Melange</skos:prefLabel>
	<skos:prefLabel xml:lang="fr">Mélange du Martegnas</skos:prefLabel>
	<skos:prefLabel xml:lang="it">Mélange del Martegnas</skos:prefLabel>
	<skos:broader rdf:resource="https://dev-lexic.swissgeol.ch/TectonicUnits/SchamsNappeComplex"/>
	<status xmlns="http://www.w3.org/ns/adms#" rdf:resource="https://dev-lexic.swissgeol.ch/active"/>
</rdf:Description>

<rdf:Description rdf:about="https://dev-lexic.swissgeol.ch/TectonicUnits/Areua-BruschghornMelange">
	<rdf:type rdf:resource="http://www.w3.org/2004/02/skos/core#Concept"/>
	<rdfs:isDefinedBy xml:lang="en">Gouffon Yves (Editor) (2024): Tectonic Map of Switzerland 1:500000, Explanatory notes. Federal Office of Topography swisstopo, Wabern</rdfs:isDefinedBy>
	<skos:definition xml:lang="en">The Areua-Bruschghorn Mélange is a tectonic mélange situated in the lower limb of the Niemet-Beverin Backfold, at the contact between the Schams Nappe Complex and the Tomül Nappe.</skos:definition>
	<skos:inScheme rdf:resource="https://dev-lexic.swissgeol.ch/TectonicUnits"/>
	<skos:prefLabel xml:lang="en">Areua-Bruschghorn Mélange</skos:prefLabel>
	<skos:prefLabel xml:lang="de">Areua-Bruschghorn-Melange</skos:prefLabel>
	<skos:prefLabel xml:lang="fr">Mélange d'Areua-Bruschghorn</skos:prefLabel>
	<skos:prefLabel xml:lang="it">Mélange di Areua-Bruschghorn</skos:prefLabel>
	<skos:broader rdf:resource="https://dev-lexic.swissgeol.ch/TectonicUnits/SchamsNappeComplex"/>
	<status xmlns="http://www.w3.org/ns/adms#" rdf:resource="https://dev-lexic.swissgeol.ch/active"/>
</rdf:Description>

<rdf:Description rdf:about="https://dev-lexic.swissgeol.ch/TectonicUnits/TschingelSlice">
	<rdf:type rdf:resource="http://www.w3.org/2004/02/skos/core#Concept"/>
	<rdfs:isDefinedBy xml:lang="en">Gouffon Yves (Editor) (2024): Tectonic Map of Switzerland 1:500000, Explanatory notes. Federal Office of Topography swisstopo, Wabern</rdfs:isDefinedBy>
	<skos:inScheme rdf:resource="https://dev-lexic.swissgeol.ch/TectonicUnits"/>
	<skos:prefLabel xml:lang="en">Tschingel Slice</skos:prefLabel>
	<skos:prefLabel xml:lang="de">Tschingel-Schuppe</skos:prefLabel>
	<skos:prefLabel xml:lang="fr">Écaille du Tschingel</skos:prefLabel>
	<skos:prefLabel xml:lang="it">Scaglia del Tschingel</skos:prefLabel>
	<skos:broader rdf:resource="https://dev-lexic.swissgeol.ch/TectonicUnits/FalknisNappe"/>
	<status xmlns="http://www.w3.org/ns/adms#" rdf:resource="https://dev-lexic.swissgeol.ch/active"/>
</rdf:Description>

<rdf:Description rdf:about="https://dev-lexic.swissgeol.ch/TectonicUnits/GrauspitzSlice">
	<rdf:type rdf:resource="http://www.w3.org/2004/02/skos/core#Concept"/>
	<rdfs:isDefinedBy xml:lang="en">Gouffon Yves (Editor) (2024): Tectonic Map of Switzerland 1:500000, Explanatory notes. Federal Office of Topography swisstopo, Wabern</rdfs:isDefinedBy>
	<skos:inScheme rdf:resource="https://dev-lexic.swissgeol.ch/TectonicUnits"/>
	<skos:prefLabel xml:lang="en">Grauspitz Slice</skos:prefLabel>
	<skos:prefLabel xml:lang="de">Grauspitz-Schuppe</skos:prefLabel>
	<skos:prefLabel xml:lang="fr">Écaille du Grauspitz</skos:prefLabel>
	<skos:prefLabel xml:lang="it">Scaglia del Grauspitz</skos:prefLabel>
	<skos:broader rdf:resource="https://dev-lexic.swissgeol.ch/TectonicUnits/FalknisNappe"/>
	<status xmlns="http://www.w3.org/ns/adms#" rdf:resource="https://dev-lexic.swissgeol.ch/active"/>
</rdf:Description>

<rdf:Description rdf:about="https://dev-lexic.swissgeol.ch/TectonicUnits/GlegghornSlice">
	<rdf:type rdf:resource="http://www.w3.org/2004/02/skos/core#Concept"/>
	<rdfs:isDefinedBy xml:lang="en">Gouffon Yves (Editor) (2024): Tectonic Map of Switzerland 1:500000, Explanatory notes. Federal Office of Topography swisstopo, Wabern</rdfs:isDefinedBy>
	<skos:inScheme rdf:resource="https://dev-lexic.swissgeol.ch/TectonicUnits"/>
	<skos:prefLabel xml:lang="en">Glegghorn Slice</skos:prefLabel>
	<skos:prefLabel xml:lang="de">Glegghorn-Schuppe</skos:prefLabel>
	<skos:prefLabel xml:lang="fr">Écaille du Glegghorn</skos:prefLabel>
	<skos:prefLabel xml:lang="it">Scaglia del Glegghorn</skos:prefLabel>
	<skos:broader rdf:resource="https://dev-lexic.swissgeol.ch/TectonicUnits/FalknisNappe"/>
	<status xmlns="http://www.w3.org/ns/adms#" rdf:resource="https://dev-lexic.swissgeol.ch/active"/>
</rdf:Description>

<rdf:Description rdf:about="https://dev-lexic.swissgeol.ch/TectonicUnits/ChatillonSlice">
	<rdf:type rdf:resource="http://www.w3.org/2004/02/skos/core#Concept"/>
	<rdfs:isDefinedBy xml:lang="en">Gouffon Yves (Editor) (2024): Tectonic Map of Switzerland 1:500000, Explanatory notes. Federal Office of Topography swisstopo, Wabern</rdfs:isDefinedBy>
	<skos:inScheme rdf:resource="https://dev-lexic.swissgeol.ch/TectonicUnits"/>
	<skos:prefLabel xml:lang="en">Châtillon Slice</skos:prefLabel>
	<skos:prefLabel xml:lang="de">Châtillon-Schuppe</skos:prefLabel>
	<skos:prefLabel xml:lang="fr">Écaille de Châtillon</skos:prefLabel>
	<skos:prefLabel xml:lang="it">Scaglia di Châtillon</skos:prefLabel>
	<skos:broader rdf:resource="https://dev-lexic.swissgeol.ch/TectonicUnits/Chatillon-St-VincentSlices"/>
	<status xmlns="http://www.w3.org/ns/adms#" rdf:resource="https://dev-lexic.swissgeol.ch/active"/>
</rdf:Description>

<rdf:Description rdf:about="https://dev-lexic.swissgeol.ch/TectonicUnits/PonteySlice">
	<rdf:type rdf:resource="http://www.w3.org/2004/02/skos/core#Concept"/>
	<rdfs:isDefinedBy xml:lang="en">Gouffon Yves (Editor) (2024): Tectonic Map of Switzerland 1:500000, Explanatory notes. Federal Office of Topography swisstopo, Wabern</rdfs:isDefinedBy>
	<skos:inScheme rdf:resource="https://dev-lexic.swissgeol.ch/TectonicUnits"/>
	<skos:prefLabel xml:lang="en">Pontey Slice</skos:prefLabel>
	<skos:prefLabel xml:lang="de">Pontey-Schuppe</skos:prefLabel>
	<skos:prefLabel xml:lang="fr">Écaille de Pontey</skos:prefLabel>
	<skos:prefLabel xml:lang="it">Scaglia di Pontey</skos:prefLabel>
	<skos:broader rdf:resource="https://dev-lexic.swissgeol.ch/TectonicUnits/Chatillon-St-VincentSlices"/>
	<status xmlns="http://www.w3.org/ns/adms#" rdf:resource="https://dev-lexic.swissgeol.ch/active"/>
</rdf:Description>

<rdf:Description rdf:about="https://dev-lexic.swissgeol.ch/TectonicUnits/GrunSlice">
	<rdf:type rdf:resource="http://www.w3.org/2004/02/skos/core#Concept"/>
	<rdfs:isDefinedBy xml:lang="en">Gouffon Yves (Editor) (2024): Tectonic Map of Switzerland 1:500000, Explanatory notes. Federal Office of Topography swisstopo, Wabern</rdfs:isDefinedBy>
	<skos:inScheme rdf:resource="https://dev-lexic.swissgeol.ch/TectonicUnits"/>
	<skos:prefLabel xml:lang="en">Grun Slice</skos:prefLabel>
	<skos:prefLabel xml:lang="de">Grun-Schuppe</skos:prefLabel>
	<skos:prefLabel xml:lang="fr">Écaille de Grun</skos:prefLabel>
	<skos:prefLabel xml:lang="it">Scaglia di Grun</skos:prefLabel>
	<skos:broader rdf:resource="https://dev-lexic.swissgeol.ch/TectonicUnits/Chatillon-St-VincentSlices"/>
	<status xmlns="http://www.w3.org/ns/adms#" rdf:resource="https://dev-lexic.swissgeol.ch/active"/>
</rdf:Description>

<rdf:Description rdf:about="https://dev-lexic.swissgeol.ch/TectonicUnits/VollonSlice">
	<rdf:type rdf:resource="http://www.w3.org/2004/02/skos/core#Concept"/>
	<rdfs:isDefinedBy xml:lang="en">Gouffon Yves (Editor) (2024): Tectonic Map of Switzerland 1:500000, Explanatory notes. Federal Office of Topography swisstopo, Wabern</rdfs:isDefinedBy>
	<skos:inScheme rdf:resource="https://dev-lexic.swissgeol.ch/TectonicUnits"/>
	<skos:prefLabel xml:lang="en">Vollon Slice</skos:prefLabel>
	<skos:prefLabel xml:lang="de">Vollon-Schuppe</skos:prefLabel>
	<skos:prefLabel xml:lang="fr">Écaille de Vollon</skos:prefLabel>
	<skos:prefLabel xml:lang="it">Scaglia di Vollon</skos:prefLabel>
	<skos:broader rdf:resource="https://dev-lexic.swissgeol.ch/TectonicUnits/Chatillon-St-VincentSlices"/>
	<status xmlns="http://www.w3.org/ns/adms#" rdf:resource="https://dev-lexic.swissgeol.ch/active"/>
</rdf:Description>

<rdf:Description rdf:about="https://dev-lexic.swissgeol.ch/TectonicUnits/HaupterhornSlice">
	<rdf:type rdf:resource="http://www.w3.org/2004/02/skos/core#Concept"/>
	<rdfs:isDefinedBy xml:lang="en">Gouffon Yves (Editor) (2024): Tectonic Map of Switzerland 1:500000, Explanatory notes. Federal Office of Topography swisstopo, Wabern</rdfs:isDefinedBy>
	<skos:inScheme rdf:resource="https://dev-lexic.swissgeol.ch/TectonicUnits"/>
	<skos:prefLabel xml:lang="en">Haupterhorn Slice</skos:prefLabel>
	<skos:prefLabel xml:lang="de">Haupterhorn-Scholle</skos:prefLabel>
	<skos:prefLabel xml:lang="fr">Écaille du Haupterhorn</skos:prefLabel>
	<skos:prefLabel xml:lang="it">Scaglia del Haupterhorn</skos:prefLabel>
	<skos:broader rdf:resource="https://dev-lexic.swissgeol.ch/TectonicUnits/ArosaZone"/>
	<skos:related rdf:resource="https://dev-lexic.swissgeol.ch/TectonicUnits/Austroalpine"/>
	<status xmlns="http://www.w3.org/ns/adms#" rdf:resource="https://dev-lexic.swissgeol.ch/active"/>
</rdf:Description>

<rdf:Description rdf:about="https://dev-lexic.swissgeol.ch/TectonicUnits/WeissfluhSlice">
	<rdf:type rdf:resource="http://www.w3.org/2004/02/skos/core#Concept"/>
	<rdfs:isDefinedBy xml:lang="en">Gouffon Yves (Editor) (2024): Tectonic Map of Switzerland 1:500000, Explanatory notes. Federal Office of Topography swisstopo, Wabern</rdfs:isDefinedBy>
	<skos:inScheme rdf:resource="https://dev-lexic.swissgeol.ch/TectonicUnits"/>
	<skos:prefLabel xml:lang="en">Weissfluh Slice</skos:prefLabel>
	<skos:prefLabel xml:lang="de">Weissfluh-Scholle</skos:prefLabel>
	<skos:prefLabel xml:lang="fr">Écaille de la Weissfluh</skos:prefLabel>
	<skos:prefLabel xml:lang="it">Scaglia della Weissfluh</skos:prefLabel>
	<skos:broader rdf:resource="https://dev-lexic.swissgeol.ch/TectonicUnits/ArosaZone"/>
	<skos:related rdf:resource="https://dev-lexic.swissgeol.ch/TectonicUnits/Austroalpine"/>
	<status xmlns="http://www.w3.org/ns/adms#" rdf:resource="https://dev-lexic.swissgeol.ch/active"/>
</rdf:Description>

<rdf:Description rdf:about="https://dev-lexic.swissgeol.ch/TectonicUnits/GotschnawangSlice">
	<rdf:type rdf:resource="http://www.w3.org/2004/02/skos/core#Concept"/>
	<rdfs:isDefinedBy xml:lang="en">Gouffon Yves (Editor) (2024): Tectonic Map of Switzerland 1:500000, Explanatory notes. Federal Office of Topography swisstopo, Wabern</rdfs:isDefinedBy>
	<skos:inScheme rdf:resource="https://dev-lexic.swissgeol.ch/TectonicUnits"/>
	<skos:prefLabel xml:lang="en">Gotschnawang Slice</skos:prefLabel>
	<skos:prefLabel xml:lang="de">Gotschnawang-Scholle</skos:prefLabel>
	<skos:prefLabel xml:lang="fr">Écaille de la Gotschnawang</skos:prefLabel>
	<skos:prefLabel xml:lang="it">Scaglia della Gotschnawang</skos:prefLabel>
	<skos:broader rdf:resource="https://dev-lexic.swissgeol.ch/TectonicUnits/ArosaZone"/>
	<skos:related rdf:resource="https://dev-lexic.swissgeol.ch/TectonicUnits/Austroalpine"/>
	<status xmlns="http://www.w3.org/ns/adms#" rdf:resource="https://dev-lexic.swissgeol.ch/active"/>
</rdf:Description>

<rdf:Description rdf:about="https://dev-lexic.swissgeol.ch/TectonicUnits/DrosSlice">
	<rdf:type rdf:resource="http://www.w3.org/2004/02/skos/core#Concept"/>
	<rdfs:isDefinedBy xml:lang="en">Gouffon Yves (Editor) (2024): Tectonic Map of Switzerland 1:500000, Explanatory notes. Federal Office of Topography swisstopo, Wabern</rdfs:isDefinedBy>
	<skos:inScheme rdf:resource="https://dev-lexic.swissgeol.ch/TectonicUnits"/>
	<skos:prefLabel xml:lang="en">Dros Slice</skos:prefLabel>
	<skos:prefLabel xml:lang="de">Dros-Scholle</skos:prefLabel>
	<skos:prefLabel xml:lang="fr">Écaille de Dros</skos:prefLabel>
	<skos:prefLabel xml:lang="it">Scaglia di Dros</skos:prefLabel>
	<skos:broader rdf:resource="https://dev-lexic.swissgeol.ch/TectonicUnits/ArosaZone"/>
	<skos:related rdf:resource="https://dev-lexic.swissgeol.ch/TectonicUnits/Austroalpine"/>
	<status xmlns="http://www.w3.org/ns/adms#" rdf:resource="https://dev-lexic.swissgeol.ch/active"/>
</rdf:Description>

<rdf:Description rdf:about="https://dev-lexic.swissgeol.ch/TectonicUnits/TotalpOphioliteComplex">
	<rdf:type rdf:resource="http://www.w3.org/2004/02/skos/core#Concept"/>
	<rdfs:isDefinedBy xml:lang="en">Gouffon Yves (Editor) (2024): Tectonic Map of Switzerland 1:500000, Explanatory notes. Federal Office of Topography swisstopo, Wabern</rdfs:isDefinedBy>
	<skos:definition xml:lang="en">The Totalp Ophiolite Complex is an ophiolitic sequence of the Arosa Zone. It consists mainly of spilite and N-MORB tholeiitic basalt.</skos:definition>
	<skos:inScheme rdf:resource="https://dev-lexic.swissgeol.ch/TectonicUnits"/>
	<skos:prefLabel xml:lang="en">Totalp Ophiolite Complex</skos:prefLabel>
	<skos:prefLabel xml:lang="de">Totalp-Ophiolithkomplex</skos:prefLabel>
	<skos:prefLabel xml:lang="fr">Complexe ophiolitique de la Totalp</skos:prefLabel>
	<skos:prefLabel xml:lang="it">Complesso ofiolitico della Totalp</skos:prefLabel>
	<skos:broader rdf:resource="https://dev-lexic.swissgeol.ch/TectonicUnits/ArosaZone"/>
	<status xmlns="http://www.w3.org/ns/adms#" rdf:resource="https://dev-lexic.swissgeol.ch/active"/>
</rdf:Description>

<rdf:Description rdf:about="https://dev-lexic.swissgeol.ch/TectonicUnits/Austroalpine">
	<rdf:type rdf:resource="http://www.w3.org/2004/02/skos/core#Concept"/>
	<rdfs:isDefinedBy xml:lang="en">Gouffon Yves (Editor) (2024): Tectonic Map of Switzerland 1:500000, Explanatory notes. Federal Office of Topography swisstopo, Wabern</rdfs:isDefinedBy>
	<rdfs:comment rdf:datatype="http://www.w3.org/1999/02/22-rdf-syntax-ns#HTML">https://data.geo.admin.ch/ch.swisstopo.geologie-tektonische_karte/pdf/Erl-TK500_2024.pdf</rdfs:comment>
	<rdfs:comment rdf:datatype="http://www.w3.org/1999/02/22-rdf-syntax-ns#HTML">https://www.strati.ch/en/tectonic/austroalpine</rdfs:comment>
	<skos:definition xml:lang="en">The Austroalpine tectonic domain is built up from allochthons derived from the Adriatic plate. The main episode of W- to NW- directed transport of nappe stacking is of Cretaceous age (“Eoalpine” orogeny reaching up to eclogitic conditions). Later, all these units became thrusted over the Penninic nappes towards the north during the Cenozoic, along a thrust that defines the outer limits of the Lower Engadine and the Tauern windows. The Austroalpine domain comprises two types of nappes. One type consists mainly of pre-Triassic crystalline basement rocks including their Permian – Mesozoic cover rocks (“basement-cover nappe”). The other type consists of detached allochthonous sedimentary cover rocks.
Because of the superposition of two orogenic cycles in the Austroalpine domain, its subdivision has always been difficult and controversial. In eastern Switzerland, the boundary between the Lower and Upper Austroalpine is largely based on paleogeographic considerations. The Upper Austroalpine units are derived from relatively more proximal parts of the Jurassic passive Adriatic continental margin in respect to the distal continental margin units preserved in the Lower Austroalpine, in particular in the Err Nappe characterized by the presence of rift-related polymict breccias of Early and Middle Jurassic age.</skos:definition>
	<skos:inScheme rdf:resource="https://dev-lexic.swissgeol.ch/TectonicUnits"/>
	<skos:topConceptOf rdf:resource="https://dev-lexic.swissgeol.ch/TectonicUnits"/>
	<skos:prefLabel xml:lang="en">Austroalpine</skos:prefLabel>
	<skos:prefLabel xml:lang="de">Ostalpin</skos:prefLabel>
	<skos:prefLabel xml:lang="fr">Austroalpin</skos:prefLabel>
	<skos:prefLabel xml:lang="it">Austroalpino</skos:prefLabel>
	<skos:narrower rdf:resource="https://dev-lexic.swissgeol.ch/TectonicUnits/LowerAustroalpine"/>
	<skos:narrower rdf:resource="https://dev-lexic.swissgeol.ch/TectonicUnits/UpperAustroalpine"/>
	<status xmlns="http://www.w3.org/ns/adms#" rdf:resource="https://dev-lexic.swissgeol.ch/active"/>
</rdf:Description>

<rdf:Description rdf:about="https://dev-lexic.swissgeol.ch/TectonicUnits/LowerAustroalpine">
	<rdf:type rdf:resource="http://www.w3.org/2004/02/skos/core#Concept"/>
	<rdfs:isDefinedBy xml:lang="en">Gouffon Yves (Editor) (2024): Tectonic Map of Switzerland 1:500000, Explanatory notes. Federal Office of Topography swisstopo, Wabern</rdfs:isDefinedBy>
	<skos:definition xml:lang="en">The Lower Austroalpine comprises tectonic units that are derived from the former distal continental margin of the Adriatic plate, which was affected by Jurassic extensional detachment faults. The strongly deformed pre- and syn-rift strata became intensely reshaped and reworked during the closure of the Piemonte-Liguria Ocean and subsequent Alpine continental collision.

The facies of syn- and post-rift sediments of the Lower Austroalpine has remarkable similarities with those found in the Canavese area around the town of Ivrea, which is a part of the South Alpine derived of the western part of the Adria.</skos:definition>
	<skos:inScheme rdf:resource="https://dev-lexic.swissgeol.ch/TectonicUnits"/>
	<skos:prefLabel xml:lang="en">Lower Austroalpine</skos:prefLabel>
	<skos:prefLabel xml:lang="de">Unterostalpin</skos:prefLabel>
	<skos:prefLabel xml:lang="fr">Austroalpin inférieur</skos:prefLabel>
	<skos:prefLabel xml:lang="it">Austroalpino inferiore</skos:prefLabel>
	<skos:broader rdf:resource="https://dev-lexic.swissgeol.ch/TectonicUnits/Austroalpine"/>
	<skos:narrower rdf:resource="https://dev-lexic.swissgeol.ch/TectonicUnits/Rothorn-SchwarzhornNappeComplex"/>
	<skos:narrower rdf:resource="https://dev-lexic.swissgeol.ch/TectonicUnits/Grueenhorn-CasannaSliceComplex"/>
	<skos:narrower rdf:resource="https://dev-lexic.swissgeol.ch/TectonicUnits/StammerspitzSlice"/>
	<skos:narrower rdf:resource="https://dev-lexic.swissgeol.ch/TectonicUnits/BerninaNappeComplex"/>
	<skos:narrower rdf:resource="https://dev-lexic.swissgeol.ch/TectonicUnits/ErrNappeComplex"/>
	<status xmlns="http://www.w3.org/ns/adms#" rdf:resource="https://dev-lexic.swissgeol.ch/active"/>
</rdf:Description>

<rdf:Description rdf:about="https://dev-lexic.swissgeol.ch/TectonicUnits/UpperAustroalpine">
	<rdf:type rdf:resource="http://www.w3.org/2004/02/skos/core#Concept"/>
	<rdfs:isDefinedBy xml:lang="en">Gouffon Yves (Editor) (2024): Tectonic Map of Switzerland 1:500000, Explanatory notes. Federal Office of Topography swisstopo, Wabern</rdfs:isDefinedBy>
	<skos:definition xml:lang="en">The Upper Austroalpine embraces those units originating from the Adriatic continental plate that are interpreted to originally have been relatively more proximal in respect to the distal continental margin units preserved in the Lower Austroalpine, which it overthrust. The Upper Austroalpine units underwent less deformation during the opening of the Piemonte-Liguria Ocean and generally appear less intensely deformed during the Alpine orogeny. Many of them are basement-cover nappes, except for the small Roggenstock-Mördergruebi Nappe, the nappes of the Northern Calcareous Alps and the Quattervals Nappe, which are made up entirely of sedimentary rocks.</skos:definition>
	<skos:inScheme rdf:resource="https://dev-lexic.swissgeol.ch/TectonicUnits"/>
	<skos:prefLabel xml:lang="en">Upper Austroalpine</skos:prefLabel>
	<skos:prefLabel xml:lang="de">Oberostalpin</skos:prefLabel>
	<skos:prefLabel xml:lang="fr">Austroalpin supérieur</skos:prefLabel>
	<skos:prefLabel xml:lang="it">Austroalpino superiore</skos:prefLabel>
	<skos:broader rdf:resource="https://dev-lexic.swissgeol.ch/TectonicUnits/Austroalpine"/>
	<skos:narrower rdf:resource="https://dev-lexic.swissgeol.ch/TectonicUnits/CampoNappeComplex"/>
	<skos:narrower rdf:resource="https://dev-lexic.swissgeol.ch/TectonicUnits/LanguardNappe"/>
	<skos:narrower rdf:resource="https://dev-lexic.swissgeol.ch/TectonicUnits/TonaleNappe"/>
	<skos:narrower rdf:resource="https://dev-lexic.swissgeol.ch/TectonicUnits/KrabachjochNappe"/>
	<skos:narrower rdf:resource="https://dev-lexic.swissgeol.ch/TectonicUnits/InntalNappe"/>
	<skos:narrower rdf:resource="https://dev-lexic.swissgeol.ch/TectonicUnits/Roggenstock-MoerdergruebiNappe"/>
	<skos:narrower rdf:resource="https://dev-lexic.swissgeol.ch/TectonicUnits/LechtalNappe"/>
	<skos:narrower rdf:resource="https://dev-lexic.swissgeol.ch/TectonicUnits/AllgaeuNappe"/>
	<skos:narrower rdf:resource="https://dev-lexic.swissgeol.ch/TectonicUnits/Cenoman-Randschuppe"/>
	<skos:narrower rdf:resource="https://dev-lexic.swissgeol.ch/TectonicUnits/SchiahornNappe"/>
	<skos:narrower rdf:resource="https://dev-lexic.swissgeol.ch/TectonicUnits/SilvrettaNappe"/>
	<skos:narrower rdf:resource="https://dev-lexic.swissgeol.ch/TectonicUnits/OetztalNappeComplex"/>
	<skos:narrower rdf:resource="https://dev-lexic.swissgeol.ch/TectonicUnits/Umbrail-TerzaSliceComplex"/>
	<skos:narrower rdf:resource="https://dev-lexic.swissgeol.ch/TectonicUnits/QuattervalsNappe"/>
	<skos:narrower rdf:resource="https://dev-lexic.swissgeol.ch/TectonicUnits/OrtlerNappe"/>
	<skos:narrower rdf:resource="https://dev-lexic.swissgeol.ch/TectonicUnits/S-Charl-SesvennaNappe"/>
	<status xmlns="http://www.w3.org/ns/adms#" rdf:resource="https://dev-lexic.swissgeol.ch/active"/>
</rdf:Description>

<rdf:Description rdf:about="https://dev-lexic.swissgeol.ch/TectonicUnits/Rothorn-SchwarzhornNappeComplex">
	<rdf:type rdf:resource="http://www.w3.org/2004/02/skos/core#Concept"/>
	<rdfs:isDefinedBy xml:lang="en">Gouffon Yves (Editor) (2024): Tectonic Map of Switzerland 1:500000, Explanatory notes. Federal Office of Topography swisstopo, Wabern</rdfs:isDefinedBy>
	<skos:definition xml:lang="en">The Rothorn-Schwarzhorn Nappe Complex encompasses relatively small tectonic units situated south and northeast of the Prättigau Half-Window and separating the Upper Penninic Arosa Zone from the Upper Austroalpine Schiahorn and Silvretta nappes. The lithofacies of the sediments preserved in these units have a Lower Austroalpine affinity, i.e., an Adriatic distal margin origin.</skos:definition>
	<skos:inScheme rdf:resource="https://dev-lexic.swissgeol.ch/TectonicUnits"/>
	<skos:prefLabel xml:lang="en">Rothorn-Schwarzhorn Nappe Complex</skos:prefLabel>
	<skos:prefLabel xml:lang="de">Rothorn-Schwarzhorn-Deckenkomplex</skos:prefLabel>
	<skos:prefLabel xml:lang="fr">Complexe de nappes du Rothorn-Schwarzhorn</skos:prefLabel>
	<skos:prefLabel xml:lang="it">Complesso di falde del Rothorn-Schwarzhorn</skos:prefLabel>
	<skos:broader rdf:resource="https://dev-lexic.swissgeol.ch/TectonicUnits/LowerAustroalpine"/>
	<skos:narrower rdf:resource="https://dev-lexic.swissgeol.ch/TectonicUnits/RothornNappe"/>
	<skos:narrower rdf:resource="https://dev-lexic.swissgeol.ch/TectonicUnits/TschirpenNappe"/>
	<skos:narrower rdf:resource="https://dev-lexic.swissgeol.ch/TectonicUnits/SchaflaegerNappe"/>
	<skos:narrower rdf:resource="https://dev-lexic.swissgeol.ch/TectonicUnits/DorfbergNappe"/>
	<status xmlns="http://www.w3.org/ns/adms#" rdf:resource="https://dev-lexic.swissgeol.ch/active"/>
</rdf:Description>

<rdf:Description rdf:about="https://dev-lexic.swissgeol.ch/TectonicUnits/Grueenhorn-CasannaSliceComplex">
	<rdf:type rdf:resource="http://www.w3.org/2004/02/skos/core#Concept"/>
	<rdfs:isDefinedBy xml:lang="en">Gouffon Yves (Editor) (2024): Tectonic Map of Switzerland 1:500000, Explanatory notes. Federal Office of Topography swisstopo, Wabern</rdfs:isDefinedBy>
	<skos:definition xml:lang="en">The Grüenhorn-Casanna Slice Complex is considered as an independant tectonic klippe correlated with the Err Nappe Complex and overlying the Arosa Zone. It is made of two small superimposed thrust sheets with a similar sedimentary series of Lower Austroalpine affinity. Near Davos, further comparable slices of Mesozoic strata of Lower Austroalpine affinity (such as the Weissfluh Slice) are also found within the Arosa Zone and considered a part of the mélange of the Arosa Zone.</skos:definition>
	<skos:inScheme rdf:resource="https://dev-lexic.swissgeol.ch/TectonicUnits"/>
	<skos:prefLabel xml:lang="en">Grüenhorn-Casanna Slice Complex</skos:prefLabel>
	<skos:prefLabel xml:lang="de">Grüenhorn-Casanna-Schuppenkomplex</skos:prefLabel>
	<skos:prefLabel xml:lang="fr">Complexe d'écailles du Grüenhorn-Casanna</skos:prefLabel>
	<skos:prefLabel xml:lang="it">Complesso di scaglie del Grüenhorn-Casanna</skos:prefLabel>
	<skos:broader rdf:resource="https://dev-lexic.swissgeol.ch/TectonicUnits/LowerAustroalpine"/>
	<skos:narrower rdf:resource="https://dev-lexic.swissgeol.ch/TectonicUnits/GrueenhornSlice"/>
	<skos:narrower rdf:resource="https://dev-lexic.swissgeol.ch/TectonicUnits/CasannaSlice"/>
	<status xmlns="http://www.w3.org/ns/adms#" rdf:resource="https://dev-lexic.swissgeol.ch/active"/>
</rdf:Description>

<rdf:Description rdf:about="https://dev-lexic.swissgeol.ch/TectonicUnits/StammerspitzSlice">
	<rdf:type rdf:resource="http://www.w3.org/2004/02/skos/core#Concept"/>
	<rdfs:isDefinedBy xml:lang="en">Gouffon Yves (Editor) (2024): Tectonic Map of Switzerland 1:500000, Explanatory notes. Federal Office of Topography swisstopo, Wabern</rdfs:isDefinedBy>
	<skos:definition xml:lang="en">At the rim of the Lower Engadine Window, the Stammerspitz Slice is made up of a sedimentary series with a Lower Austroalpine affinity. Due to its location as a klippe directly above the Roz-Champatsch Mélange, this slice can be interpreted either as the lowermost unit of the Lower Austroalpine or as a sliver within this mélange or even within the Fimber Zone.</skos:definition>
	<skos:inScheme rdf:resource="https://dev-lexic.swissgeol.ch/TectonicUnits"/>
	<skos:prefLabel xml:lang="en">Stammerspitz Slice</skos:prefLabel>
	<skos:prefLabel xml:lang="de">Stammerspitz-Schuppe</skos:prefLabel>
	<skos:prefLabel xml:lang="fr">Écaille du Stammerspitz</skos:prefLabel>
	<skos:prefLabel xml:lang="it">Scaglia dello Stammerspitz</skos:prefLabel>
	<skos:broader rdf:resource="https://dev-lexic.swissgeol.ch/TectonicUnits/LowerAustroalpine"/>
	<status xmlns="http://www.w3.org/ns/adms#" rdf:resource="https://dev-lexic.swissgeol.ch/active"/>
</rdf:Description>

<rdf:Description rdf:about="https://dev-lexic.swissgeol.ch/TectonicUnits/BerninaNappeComplex">
	<rdf:type rdf:resource="http://www.w3.org/2004/02/skos/core#Concept"/>
	<rdfs:isDefinedBy xml:lang="en">Gouffon Yves (Editor) (2024): Tectonic Map of Switzerland 1:500000, Explanatory notes. Federal Office of Topography swisstopo, Wabern</rdfs:isDefinedBy>
	<skos:definition xml:lang="en">The Lower Austroalpine Bernina Nappe Complex includes a series of subunits which occupied a somewhat more proximal paleogeographically position than those of the Err Nappe Complex. Structurally, the Bernina Nappe Complex occupies a higher tectonic position compared to the Err Nappe Complex. The Julier and Bernina Nappes are considered as a single tectonic unit, but carry different names only because of their different location in relation to the Engadine Fault. The Ela Nappe and underlying Madulain Slices are also considered to be part of the Bernina Nappe Complex. The Mezzaun Slice is a rather isolated piece of this nappe complex located southeast of the Engadine Fault directly underlying the Upper Austroalpine units, which justifies its attribution to the Bernina Nappe Complex on structural grounds.</skos:definition>
	<skos:inScheme rdf:resource="https://dev-lexic.swissgeol.ch/TectonicUnits"/>
	<skos:prefLabel xml:lang="en">Bernina Nappe Complex</skos:prefLabel>
	<skos:prefLabel xml:lang="de">Bernina-Deckenkomplex</skos:prefLabel>
	<skos:prefLabel xml:lang="fr">Complexe de nappes du Bernina</skos:prefLabel>
	<skos:prefLabel xml:lang="it">Complesso di falde del Bernina</skos:prefLabel>
	<skos:broader rdf:resource="https://dev-lexic.swissgeol.ch/TectonicUnits/LowerAustroalpine"/>
	<skos:narrower rdf:resource="https://dev-lexic.swissgeol.ch/TectonicUnits/ElaNappe"/>
	<skos:narrower rdf:resource="https://dev-lexic.swissgeol.ch/TectonicUnits/BerninaNappe"/>
	<skos:narrower rdf:resource="https://dev-lexic.swissgeol.ch/TectonicUnits/MuesellaSlice"/>
	<skos:narrower rdf:resource="https://dev-lexic.swissgeol.ch/TectonicUnits/MezzaunSlice"/>
	<skos:narrower rdf:resource="https://dev-lexic.swissgeol.ch/TectonicUnits/MadulainSlices"/>
	<skos:narrower rdf:resource="https://dev-lexic.swissgeol.ch/TectonicUnits/Schlattain-Clavadatsch-PadellaSlices"/>
	<skos:narrower rdf:resource="https://dev-lexic.swissgeol.ch/TectonicUnits/JulierNappe"/>
	<status xmlns="http://www.w3.org/ns/adms#" rdf:resource="https://dev-lexic.swissgeol.ch/active"/>
</rdf:Description>

<rdf:Description rdf:about="https://dev-lexic.swissgeol.ch/TectonicUnits/ErrNappeComplex">
	<rdf:type rdf:resource="http://www.w3.org/2004/02/skos/core#Concept"/>
	<rdfs:isDefinedBy xml:lang="en">Gouffon Yves (Editor) (2024): Tectonic Map of Switzerland 1:500000, Explanatory notes. Federal Office of Topography swisstopo, Wabern</rdfs:isDefinedBy>
	<skos:definition xml:lang="en">The Err Nappe Complex is a Lower Austroalpine tectonic unit encompassing a number of tectonic subunits that, from a paleogeographical point of view, are derived from the most distal part of the Adriatic passive margin which was linked to the adjacent oceanic realm of the Platta Nappe.</skos:definition>
	<skos:inScheme rdf:resource="https://dev-lexic.swissgeol.ch/TectonicUnits"/>
	<skos:prefLabel xml:lang="en">Err Nappe Complex</skos:prefLabel>
	<skos:prefLabel xml:lang="de">Err-Deckenkomplex</skos:prefLabel>
	<skos:prefLabel xml:lang="fr">Complexe de nappes d'Err</skos:prefLabel>
	<skos:prefLabel xml:lang="it">Complesso di falde di Err</skos:prefLabel>
	<skos:broader rdf:resource="https://dev-lexic.swissgeol.ch/TectonicUnits/LowerAustroalpine"/>
	<skos:narrower rdf:resource="https://dev-lexic.swissgeol.ch/TectonicUnits/MurtiroelSlice"/>
	<skos:narrower rdf:resource="https://dev-lexic.swissgeol.ch/TectonicUnits/ErrNappe"/>
	<skos:narrower rdf:resource="https://dev-lexic.swissgeol.ch/TectonicUnits/CarungasSlice"/>
	<skos:narrower rdf:resource="https://dev-lexic.swissgeol.ch/TectonicUnits/CorvatschSlice"/>
	<skos:narrower rdf:resource="https://dev-lexic.swissgeol.ch/TectonicUnits/ChasteletsSlice"/>
	<skos:narrower rdf:resource="https://dev-lexic.swissgeol.ch/TectonicUnits/Bardella-RoccabellaSlices"/>
	<status xmlns="http://www.w3.org/ns/adms#" rdf:resource="https://dev-lexic.swissgeol.ch/active"/>
</rdf:Description>

<rdf:Description rdf:about="https://dev-lexic.swissgeol.ch/TectonicUnits/CampoNappeComplex">
	<rdf:type rdf:resource="http://www.w3.org/2004/02/skos/core#Concept"/>
	<rdfs:isDefinedBy xml:lang="en">Gouffon Yves (Editor) (2024): Tectonic Map of Switzerland 1:500000, Explanatory notes. Federal Office of Topography swisstopo, Wabern</rdfs:isDefinedBy>
	<skos:definition xml:lang="en">The Upper Austroalpine Campo Nappe Complex (formerly Campo Nappe s.l.), dominated largely by Variscan basement, occupied the same tectonic position as the Silvretta and S-charl-Sesvenna nappes during the Cretaceous orogeny. This nappe complex is composed of different nappes which have substantial petrological and structural differences.</skos:definition>
	<skos:inScheme rdf:resource="https://dev-lexic.swissgeol.ch/TectonicUnits"/>
	<skos:prefLabel xml:lang="en">Campo Nappe Complex</skos:prefLabel>
	<skos:prefLabel xml:lang="de">Campo-Deckenkomplex</skos:prefLabel>
	<skos:prefLabel xml:lang="fr">Complexe de nappes de Campo</skos:prefLabel>
	<skos:prefLabel xml:lang="it">Complesso di falde di Campo</skos:prefLabel>
	<skos:broader rdf:resource="https://dev-lexic.swissgeol.ch/TectonicUnits/UpperAustroalpine"/>
	<skos:narrower rdf:resource="https://dev-lexic.swissgeol.ch/TectonicUnits/MasuccioNappe"/>
	<skos:narrower rdf:resource="https://dev-lexic.swissgeol.ch/TectonicUnits/CampoNappe"/>
	<skos:narrower rdf:resource="https://dev-lexic.swissgeol.ch/TectonicUnits/GrosinaNappe"/>
	<skos:narrower rdf:resource="https://dev-lexic.swissgeol.ch/TectonicUnits/LaasNappe"/>
	<skos:narrower rdf:resource="https://dev-lexic.swissgeol.ch/TectonicUnits/VinschgauShearZone"/>
	<status xmlns="http://www.w3.org/ns/adms#" rdf:resource="https://dev-lexic.swissgeol.ch/active"/>
</rdf:Description>

<rdf:Description rdf:about="https://dev-lexic.swissgeol.ch/TectonicUnits/LanguardNappe">
	<rdf:type rdf:resource="http://www.w3.org/2004/02/skos/core#Concept"/>
	<rdfs:isDefinedBy xml:lang="en">Gouffon Yves (Editor) (2024): Tectonic Map of Switzerland 1:500000, Explanatory notes. Federal Office of Topography swisstopo, Wabern</rdfs:isDefinedBy>
	<skos:definition xml:lang="en">The Languard Nappe covers is a basement-dominated Upper Austroalpine tectonic unit occupying a relatively small area. It is surrounded by the Engadine Fault in the northwest and lacks an equivalent on the northwestern side of this fault. It overthrusts the Bernina Nappe in the south, while in the north it overlies the Mezzaun Slice of the Bernina Nappe Complex and the Murtiröl Slice of the Err Nappe Complex; the thrust contacts being overprinted by normal faults (e. g., the Mezzaun Normal Fault) over large distances. To the east and northeast the Languard Nappe is overthrust by the basement of the Campo Nappe Complex and by the Ortler Nappe, which both occupy a higher tectonic position.</skos:definition>
	<skos:inScheme rdf:resource="https://dev-lexic.swissgeol.ch/TectonicUnits"/>
	<skos:prefLabel xml:lang="en">Languard Nappe</skos:prefLabel>
	<skos:prefLabel xml:lang="de">Languard-Decke</skos:prefLabel>
	<skos:prefLabel xml:lang="fr">Nappe du Languard</skos:prefLabel>
	<skos:prefLabel xml:lang="it">Falda del Languard</skos:prefLabel>
	<skos:broader rdf:resource="https://dev-lexic.swissgeol.ch/TectonicUnits/UpperAustroalpine"/>
	<status xmlns="http://www.w3.org/ns/adms#" rdf:resource="https://dev-lexic.swissgeol.ch/active"/>
</rdf:Description>

<rdf:Description rdf:about="https://dev-lexic.swissgeol.ch/TectonicUnits/TonaleNappe">
	<rdf:type rdf:resource="http://www.w3.org/2004/02/skos/core#Concept"/>
	<rdfs:isDefinedBy xml:lang="en">Gouffon Yves (Editor) (2024): Tectonic Map of Switzerland 1:500000, Explanatory notes. Federal Office of Topography swisstopo, Wabern</rdfs:isDefinedBy>
	<skos:definition xml:lang="en">The Tonale Nappe follows the E–W striking part of the Tonale Fault (Insubric Fault) and is is characterized by a very distinct and lithologically variable association of predominantly sillimanite-bearing paragneisses, marbles, quartzites and amphibolites metamorphosed during the Variscan cycle (Tonale Gneiss Complex).

In the west, between Giubasco and Sondrio, the Tonale Nappe forms a steeply N-dipping narrow strip of mylonitic series that are part of the Southern Steep Belt (or “root zone” north of the Tonale Fault), bounded by the tonalites of the Bregaglia Intrusion to the north and Alpine mylonites and cataclasites of the Tonale Fault in the south. Between Sondrio and Tirano, it then represents the hangingwall of the Late Cretaceous Mortirolo Normal Fault. Further east, a second Late Cretaceous normal fault, the SE-dipping Pejo Normal Fault, accommodates top-E extension combined with a sinistral strike-slip component in the present-day map view. Finally, east of the Passo del Tonale, the Tonale Nappe displays a rock association that is lithologically distinct from the Tonale Gneiss Complex and that is referred to as the Ulten (or Ultimo) Unit. It overlies the Tonale Gneiss Complex along a pre-Alpine tectonic contact.</skos:definition>
	<skos:inScheme rdf:resource="https://dev-lexic.swissgeol.ch/TectonicUnits"/>
	<skos:prefLabel xml:lang="en">Tonale Nappe</skos:prefLabel>
	<skos:prefLabel xml:lang="de">Tonale-Decke</skos:prefLabel>
	<skos:prefLabel xml:lang="fr">Nappe du Tonale</skos:prefLabel>
	<skos:prefLabel xml:lang="it">Falda del Tonale</skos:prefLabel>
	<skos:broader rdf:resource="https://dev-lexic.swissgeol.ch/TectonicUnits/UpperAustroalpine"/>
	<skos:narrower rdf:resource="https://dev-lexic.swissgeol.ch/TectonicUnits/UltenUnit"/>
	<status xmlns="http://www.w3.org/ns/adms#" rdf:resource="https://dev-lexic.swissgeol.ch/active"/>
</rdf:Description>

<rdf:Description rdf:about="https://dev-lexic.swissgeol.ch/TectonicUnits/KrabachjochNappe">
	<rdf:type rdf:resource="http://www.w3.org/2004/02/skos/core#Concept"/>
	<rdfs:isDefinedBy xml:lang="en">Gouffon Yves (Editor) (2024): Tectonic Map of Switzerland 1:500000, Explanatory notes. Federal Office of Topography swisstopo, Wabern</rdfs:isDefinedBy>
	<skos:definition xml:lang="en">The Krabachjoch Nappe is the upper tectonic unit of the Tirolic Nappe System (Upper Austroalpine) in the Northern Calcareous Alps. It has an exclusively Triassic stratigraphic sequence ranging from «Alpiner Buntsandstein» (Chazforà-/Fuorn-Fm.) up to «Hauptdolomit».</skos:definition>
	<skos:inScheme rdf:resource="https://dev-lexic.swissgeol.ch/TectonicUnits"/>
	<skos:prefLabel xml:lang="en">Krabachjoch Nappe</skos:prefLabel>
	<skos:prefLabel xml:lang="de">Krabachjoch-Decke</skos:prefLabel>
	<skos:prefLabel xml:lang="fr">Nappe du Krabachjoch</skos:prefLabel>
	<skos:prefLabel xml:lang="it">Falda del Krabachjoch</skos:prefLabel>
	<skos:broader rdf:resource="https://dev-lexic.swissgeol.ch/TectonicUnits/UpperAustroalpine"/>
	<status xmlns="http://www.w3.org/ns/adms#" rdf:resource="https://dev-lexic.swissgeol.ch/active"/>
</rdf:Description>

<rdf:Description rdf:about="https://dev-lexic.swissgeol.ch/TectonicUnits/InntalNappe">
	<rdf:type rdf:resource="http://www.w3.org/2004/02/skos/core#Concept"/>
	<rdfs:isDefinedBy xml:lang="en">Gouffon Yves (Editor) (2024): Tectonic Map of Switzerland 1:500000, Explanatory notes. Federal Office of Topography swisstopo, Wabern</rdfs:isDefinedBy>
	<skos:definition xml:lang="en">The Inntal Nappe is the lower tectonic unit of the Tirolic Nappe System (Upper Austroalpine) in the Northern Calcareous Alps. The stratigraphic sequence is characterised by thick Triassic deposits (up to 1700 m of Middle Triassic platform and basin sediments and over 2000 m of peritidal sediments of the Hauptdolomit Group).</skos:definition>
	<skos:inScheme rdf:resource="https://dev-lexic.swissgeol.ch/TectonicUnits"/>
	<skos:prefLabel xml:lang="en">Inntal Nappe</skos:prefLabel>
	<skos:prefLabel xml:lang="de">Inntal-Decke</skos:prefLabel>
	<skos:prefLabel xml:lang="fr">Nappe de l'Inntal</skos:prefLabel>
	<skos:prefLabel xml:lang="it">Falda dell'Inntal</skos:prefLabel>
	<skos:broader rdf:resource="https://dev-lexic.swissgeol.ch/TectonicUnits/UpperAustroalpine"/>
	<status xmlns="http://www.w3.org/ns/adms#" rdf:resource="https://dev-lexic.swissgeol.ch/active"/>
</rdf:Description>

<rdf:Description rdf:about="https://dev-lexic.swissgeol.ch/TectonicUnits/Roggenstock-MoerdergruebiNappe">
	<rdf:type rdf:resource="http://www.w3.org/2004/02/skos/core#Concept"/>
	<rdfs:isDefinedBy xml:lang="en">Gouffon Yves (Editor) (2024): Tectonic Map of Switzerland 1:500000, Explanatory notes. Federal Office of Topography swisstopo, Wabern</rdfs:isDefinedBy>
	<skos:definition xml:lang="en">The Roggenstock-Mördergruebi Nappe consists of a pair of isolated klippes forming the highest unit of the Iberg Klippen in central Switzerland. It is in direct tectonic contact with the underlying Arosa Zone that in turn overthrusts Middle Penninic units and is therefore a testimony that Austroalpine cover nappes must have formerly extended as continuous thrust sheets westwards to the meridian of the Vierwaldstättersee. These klippes only expose Late Triassic to Early Jurassic sediments, which are correlated with the nappes of the Northern Calcareous Alps.</skos:definition>
	<skos:inScheme rdf:resource="https://dev-lexic.swissgeol.ch/TectonicUnits"/>
	<skos:prefLabel xml:lang="en">Roggenstock-Mördergruebi Nappe</skos:prefLabel>
	<skos:prefLabel xml:lang="de">Roggenstock-Mördergruebi-Decke</skos:prefLabel>
	<skos:prefLabel xml:lang="fr">Nappe du Roggenstock-Mördergruebi</skos:prefLabel>
	<skos:prefLabel xml:lang="it">Falda del Roggenstock-Mördergruebi</skos:prefLabel>
	<skos:broader rdf:resource="https://dev-lexic.swissgeol.ch/TectonicUnits/UpperAustroalpine"/>
	<status xmlns="http://www.w3.org/ns/adms#" rdf:resource="https://dev-lexic.swissgeol.ch/active"/>
</rdf:Description>

<rdf:Description rdf:about="https://dev-lexic.swissgeol.ch/TectonicUnits/LechtalNappe">
	<rdf:type rdf:resource="http://www.w3.org/2004/02/skos/core#Concept"/>
	<rdfs:isDefinedBy xml:lang="en">Gouffon Yves (Editor) (2024): Tectonic Map of Switzerland 1:500000, Explanatory notes. Federal Office of Topography swisstopo, Wabern</rdfs:isDefinedBy>
	<skos:definition xml:lang="en">The Lechtal Nappe is the upper tectonic unit of the Bajuvaric Nappe System (Upper Austroalpine) in the Northern Calcareous Alps. Its stratigraphic sequence is characterised by thick and widespread Jurassic and Cretaceous basin sediments, as well as local shallow sediments («Zürser Schwelle»).

In the northern Rätikon mountain range, between Austria, Liechtenstein and Switzerland, it is intersected by out-of-sequence thrust faults, which divided it into several slices (Schesaplana, Gorfion, Augstenberg, Ochsenkopf, Heubühl and Drei Schwestern slices) and also lead to the exposure of isolated lenses of the Arosa Zone. The «Northern Mittagspitz Zone», in the eastern Rätikon, and the Madrisa Slice, which is isolated north of Klosters between the Silvretta Nappe above and the Upper Penninic Arosa Zone below, are considered to be inverted slivers derived from the Lechtal Nappe.</skos:definition>
	<skos:inScheme rdf:resource="https://dev-lexic.swissgeol.ch/TectonicUnits"/>
	<skos:prefLabel xml:lang="en">Lechtal Nappe</skos:prefLabel>
	<skos:prefLabel xml:lang="de">Lechtal-Decke</skos:prefLabel>
	<skos:prefLabel xml:lang="fr">Nappe du Lechtal</skos:prefLabel>
	<skos:prefLabel xml:lang="it">Falda del Lechtal</skos:prefLabel>
	<skos:broader rdf:resource="https://dev-lexic.swissgeol.ch/TectonicUnits/UpperAustroalpine"/>
	<skos:narrower rdf:resource="https://dev-lexic.swissgeol.ch/TectonicUnits/MadrisaSlice"/>
	<skos:narrower rdf:resource="https://dev-lexic.swissgeol.ch/TectonicUnits/SchesaplanaSlice"/>
	<skos:narrower rdf:resource="https://dev-lexic.swissgeol.ch/TectonicUnits/GorvionSlice"/>
	<skos:narrower rdf:resource="https://dev-lexic.swissgeol.ch/TectonicUnits/AugstenbergSlice"/>
	<skos:narrower rdf:resource="https://dev-lexic.swissgeol.ch/TectonicUnits/OchsenkopfSlice"/>
	<skos:narrower rdf:resource="https://dev-lexic.swissgeol.ch/TectonicUnits/HeubuehlSlice"/>
	<skos:narrower rdf:resource="https://dev-lexic.swissgeol.ch/TectonicUnits/DreiSchwesternSlice"/>
	<status xmlns="http://www.w3.org/ns/adms#" rdf:resource="https://dev-lexic.swissgeol.ch/active"/>
</rdf:Description>

<rdf:Description rdf:about="https://dev-lexic.swissgeol.ch/TectonicUnits/AllgaeuNappe">
	<rdf:type rdf:resource="http://www.w3.org/2004/02/skos/core#Concept"/>
	<rdfs:isDefinedBy xml:lang="en">Gouffon Yves (Editor) (2024): Tectonic Map of Switzerland 1:500000, Explanatory notes. Federal Office of Topography swisstopo, Wabern</rdfs:isDefinedBy>
	<skos:definition xml:lang="en">The Allgäu Nappe is the lower tectonic unit of the Bajuvaric Nappe System (Upper Austroalpine) in the Northern Calcareous Alps.</skos:definition>
	<skos:inScheme rdf:resource="https://dev-lexic.swissgeol.ch/TectonicUnits"/>
	<skos:prefLabel xml:lang="en">Allgäu Nappe</skos:prefLabel>
	<skos:prefLabel xml:lang="de">Allgäu-Decke</skos:prefLabel>
	<skos:prefLabel xml:lang="fr">Nappe de l'Allgäu</skos:prefLabel>
	<skos:prefLabel xml:lang="it">Falda dell'Allgäu</skos:prefLabel>
	<skos:broader rdf:resource="https://dev-lexic.swissgeol.ch/TectonicUnits/UpperAustroalpine"/>
	<status xmlns="http://www.w3.org/ns/adms#" rdf:resource="https://dev-lexic.swissgeol.ch/active"/>
</rdf:Description>

<rdf:Description rdf:about="https://dev-lexic.swissgeol.ch/TectonicUnits/Cenoman-Randschuppe">
	<rdf:type rdf:resource="http://www.w3.org/2004/02/skos/core#Concept"/>
	<rdfs:isDefinedBy xml:lang="en">Gouffon Yves (Editor) (2024): Tectonic Map of Switzerland 1:500000, Explanatory notes. Federal Office of Topography swisstopo, Wabern</rdfs:isDefinedBy>
	<skos:definition xml:lang="en">The Cenoman-Randschuppe consists of an imbricate zone of slivers formed at the active margin between the Adriatic continental plate and the Piemonte-Liguria Ocean. It lies at the northern rim of the Upper Austroalpine (Northern Calcareous Alps) and consists of flysch-like coarse-grained deposits.</skos:definition>
	<skos:inScheme rdf:resource="https://dev-lexic.swissgeol.ch/TectonicUnits"/>
	<skos:prefLabel xml:lang="en">Cenoman-Randschuppe</skos:prefLabel>
	<skos:prefLabel xml:lang="de">Cenoman-Randschuppe</skos:prefLabel>
	<skos:prefLabel xml:lang="fr">Cenoman-Randschuppe</skos:prefLabel>
	<skos:prefLabel xml:lang="it">Cenoman-Randschuppe</skos:prefLabel>
	<skos:broader rdf:resource="https://dev-lexic.swissgeol.ch/TectonicUnits/UpperAustroalpine"/>
	<status xmlns="http://www.w3.org/ns/adms#" rdf:resource="https://dev-lexic.swissgeol.ch/active"/>
</rdf:Description>

<rdf:Description rdf:about="https://dev-lexic.swissgeol.ch/TectonicUnits/SchiahornNappe">
	<rdf:type rdf:resource="http://www.w3.org/2004/02/skos/core#Concept"/>
	<rdfs:isDefinedBy xml:lang="en">Gouffon Yves (Editor) (2024): Tectonic Map of Switzerland 1:500000, Explanatory notes. Federal Office of Topography swisstopo, Wabern</rdfs:isDefinedBy>
	<skos:definition xml:lang="en">The Schiahorn Nappe (formerly “Arosa Dolomites”) is a small unit underlying the Silvretta Nappe between Tiefencastel and Davos. It consists of Triassic to Early Jurassic sediments with lithofacies similar to that of the Upper Austroalpine Ortler Nappe.</skos:definition>
	<skos:inScheme rdf:resource="https://dev-lexic.swissgeol.ch/TectonicUnits"/>
	<skos:prefLabel xml:lang="en">Schiahorn Nappe</skos:prefLabel>
	<skos:prefLabel xml:lang="de">Schiahorn-Decke</skos:prefLabel>
	<skos:prefLabel xml:lang="fr">Nappe du Schiahorn</skos:prefLabel>
	<skos:prefLabel xml:lang="it">Falda dello Schiahorn</skos:prefLabel>
	<skos:altLabel xml:lang="de">Aroser Dolomiten</skos:altLabel>
	<skos:altLabel xml:lang="en">Arosa Dolomites</skos:altLabel>
	<skos:broader rdf:resource="https://dev-lexic.swissgeol.ch/TectonicUnits/UpperAustroalpine"/>
	<status xmlns="http://www.w3.org/ns/adms#" rdf:resource="https://dev-lexic.swissgeol.ch/active"/>
</rdf:Description>

<rdf:Description rdf:about="https://dev-lexic.swissgeol.ch/TectonicUnits/SilvrettaNappe">
	<rdf:type rdf:resource="http://www.w3.org/2004/02/skos/core#Concept"/>
	<rdfs:isDefinedBy xml:lang="en">Gouffon Yves (Editor) (2024): Tectonic Map of Switzerland 1:500000, Explanatory notes. Federal Office of Topography swisstopo, Wabern</rdfs:isDefinedBy>
	<skos:definition xml:lang="en">The Silvretta Nappe is the northernmost Upper Austroalpine basement-cover nappe extending over a large area located between the southern rim of the Northern Calcareous Alps in the north and the Engadine Fault in the south. Most of its area is occupied by high-grade metamorphic basement that was multiply deformed since the Precambrian, ending with an amphibolite-facies Variscan tectono-metamorphic event in the Carboniferous. A top-N Alpine thrust of secondary importance separates this high-grade basement from a narrow belt of low-grade basement referred to as the “Phyllitgneiszone” (including the Landeck Quartzphyllites) that is nowadays also considered to be a part of the Silvretta Nappe.

The Triassic cover of the Silvretta Nappe is preserved in two SW–NE striking synclines located at the western edge of the Silvretta Nappe, known as the Landwasser and Ducan synclines. They formed during top-NW thrusting in the Cretaceous, and then were overprinted by normal faulting still in the latest Cretaceous. Only very small lenses of Permo-Carboniferous and Early Triassic slivers (“Puschlin Zone”) are preserved within the Landeck Quarzphyllites.</skos:definition>
	<skos:inScheme rdf:resource="https://dev-lexic.swissgeol.ch/TectonicUnits"/>
	<skos:prefLabel xml:lang="en">Silvretta Nappe</skos:prefLabel>
	<skos:prefLabel xml:lang="de">Silvretta-Decke</skos:prefLabel>
	<skos:prefLabel xml:lang="fr">Nappe de la Silvretta</skos:prefLabel>
	<skos:prefLabel xml:lang="it">Falda della Silvretta</skos:prefLabel>
	<skos:broader rdf:resource="https://dev-lexic.swissgeol.ch/TectonicUnits/UpperAustroalpine"/>
	<skos:narrower rdf:resource="https://dev-lexic.swissgeol.ch/TectonicUnits/Phyllitgneiszone"/>
	<skos:narrower rdf:resource="https://dev-lexic.swissgeol.ch/TectonicUnits/S-ChanfSlices"/>
	<status xmlns="http://www.w3.org/ns/adms#" rdf:resource="https://dev-lexic.swissgeol.ch/active"/>
</rdf:Description>

<rdf:Description rdf:about="https://dev-lexic.swissgeol.ch/TectonicUnits/OetztalNappeComplex">
	<rdf:type rdf:resource="http://www.w3.org/2004/02/skos/core#Concept"/>
	<rdfs:isDefinedBy xml:lang="en">Gouffon Yves (Editor) (2024): Tectonic Map of Switzerland 1:500000, Explanatory notes. Federal Office of Topography swisstopo, Wabern</rdfs:isDefinedBy>
	<skos:definition xml:lang="en">The Ötztal Nappe Complex is an Upper Austroalpine tectonic unit spanning the Austria-Italy border southwest of Innsbruck. In Switzerland, only two lithologically and tectonically distinct units occur: the main Ötztal Nappe (polymetamorphic paragneisses with minor orthogneisses and amphibolites) and the smaller, overlying Matsch Nappe (characteristic polymetamorphic association of interlayered metapelites, amphibolites and pegmatites).</skos:definition>
	<skos:inScheme rdf:resource="https://dev-lexic.swissgeol.ch/TectonicUnits"/>
	<skos:prefLabel xml:lang="en">Ötztal Nappe Complex</skos:prefLabel>
	<skos:prefLabel xml:lang="de">Ötztal-Deckenkomplex</skos:prefLabel>
	<skos:prefLabel xml:lang="fr">Complexe de nappes de l'Ötztal</skos:prefLabel>
	<skos:prefLabel xml:lang="it">Complesso di falde dell'Ötztal</skos:prefLabel>
	<skos:broader rdf:resource="https://dev-lexic.swissgeol.ch/TectonicUnits/UpperAustroalpine"/>
	<skos:narrower rdf:resource="https://dev-lexic.swissgeol.ch/TectonicUnits/MatschNappe"/>
	<status xmlns="http://www.w3.org/ns/adms#" rdf:resource="https://dev-lexic.swissgeol.ch/active"/>
</rdf:Description>

<rdf:Description rdf:about="https://dev-lexic.swissgeol.ch/TectonicUnits/Umbrail-TerzaSliceComplex">
	<rdf:type rdf:resource="http://www.w3.org/2004/02/skos/core#Concept"/>
	<rdfs:isDefinedBy xml:lang="en">Gouffon Yves (Editor) (2024): Tectonic Map of Switzerland 1:500000, Explanatory notes. Federal Office of Topography swisstopo, Wabern</rdfs:isDefinedBy>
	<skos:definition xml:lang="en">The Umbrail-Terza Slice Complex consists of two geographically separated parts: the smaller Terza Slice (a klippe overlying the westernmost part of the Quattervals Nappe) and the larger Umbrail-Chavalatsch Slices further to the east (a very complicated zone of imbrication underneath the Ötztal Nappe Complex).</skos:definition>
	<skos:inScheme rdf:resource="https://dev-lexic.swissgeol.ch/TectonicUnits"/>
	<skos:prefLabel xml:lang="en">Umbrail-Terza Slice Complex</skos:prefLabel>
	<skos:prefLabel xml:lang="de">Umbrail-Terza-Schuppenkomplex</skos:prefLabel>
	<skos:prefLabel xml:lang="fr">Complexe d'écailles de l'Umbrail-Terza</skos:prefLabel>
	<skos:prefLabel xml:lang="it">Complesso di scaglie dell'Umbrail-Terza</skos:prefLabel>
	<skos:broader rdf:resource="https://dev-lexic.swissgeol.ch/TectonicUnits/UpperAustroalpine"/>
	<skos:narrower rdf:resource="https://dev-lexic.swissgeol.ch/TectonicUnits/Umbrail-ChavalatschSlices"/>
	<skos:narrower rdf:resource="https://dev-lexic.swissgeol.ch/TectonicUnits/TerzaSlice"/>
	<status xmlns="http://www.w3.org/ns/adms#" rdf:resource="https://dev-lexic.swissgeol.ch/active"/>
</rdf:Description>

<rdf:Description rdf:about="https://dev-lexic.swissgeol.ch/TectonicUnits/QuattervalsNappe">
	<rdf:type rdf:resource="http://www.w3.org/2004/02/skos/core#Concept"/>
	<rdfs:isDefinedBy xml:lang="en">Gouffon Yves (Editor) (2024): Tectonic Map of Switzerland 1:500000, Explanatory notes. Federal Office of Topography swisstopo, Wabern</rdfs:isDefinedBy>
	<skos:definition xml:lang="en">The Quattervals Nappe consists of a series of NNE-dipping slices that overthrust the Ortler Nappe along the western part of the Trupchun-Braulio Thrust. It comprises almost exclusively Late Triassic sediments, mostly dolomitic and calcareous formations of the Norian Hauptdolomit Group of considerable thickness overlain by Rhaetian deposits, which became detached from their former substratum along the Carnian Raibl Group during the Cretaceous orogeny.</skos:definition>
	<skos:inScheme rdf:resource="https://dev-lexic.swissgeol.ch/TectonicUnits"/>
	<skos:prefLabel xml:lang="en">Quattervals Nappe</skos:prefLabel>
	<skos:prefLabel xml:lang="de">Quattervals-Decke</skos:prefLabel>
	<skos:prefLabel xml:lang="fr">Nappe du Quattervals</skos:prefLabel>
	<skos:prefLabel xml:lang="it">Falda del Quattervals</skos:prefLabel>
	<skos:broader rdf:resource="https://dev-lexic.swissgeol.ch/TectonicUnits/UpperAustroalpine"/>
	<status xmlns="http://www.w3.org/ns/adms#" rdf:resource="https://dev-lexic.swissgeol.ch/active"/>
</rdf:Description>

<rdf:Description rdf:about="https://dev-lexic.swissgeol.ch/TectonicUnits/OrtlerNappe">
	<rdf:type rdf:resource="http://www.w3.org/2004/02/skos/core#Concept"/>
	<rdfs:isDefinedBy xml:lang="en">Gouffon Yves (Editor) (2024): Tectonic Map of Switzerland 1:500000, Explanatory notes. Federal Office of Topography swisstopo, Wabern</rdfs:isDefinedBy>
	<skos:definition xml:lang="en">The Upper Austroalpine Ortler Nappe overthrusts the Campo Nappe along the WNW–ESE striking Zebrù Thrust, which follows the incompetent sediments of the Raibl Group over most of its strike as the dominant basal décollement horizon. Only small occurrences of basement and pre-Carnian sediments are preserved locally, the main Mesozoic sequence being dominated by massive Late Triassic sediments. The hangingwall of the Ortler Nappe is defined by the Trupchun-Braulio Thrust that formed during a later stage of the Cretaceous orogeny and juxtaposed the Quattervals Nappe (in the west) and the Umbrail-Terza Slice Complex (in the east) over the Ortler Nappe.</skos:definition>
	<skos:inScheme rdf:resource="https://dev-lexic.swissgeol.ch/TectonicUnits"/>
	<skos:prefLabel xml:lang="en">Ortler Nappe</skos:prefLabel>
	<skos:prefLabel xml:lang="de">Ortler-Decke</skos:prefLabel>
	<skos:prefLabel xml:lang="fr">Nappe de l'Ortler</skos:prefLabel>
	<skos:prefLabel xml:lang="it">Falda dell'Ortler</skos:prefLabel>
	<skos:broader rdf:resource="https://dev-lexic.swissgeol.ch/TectonicUnits/UpperAustroalpine"/>
	<status xmlns="http://www.w3.org/ns/adms#" rdf:resource="https://dev-lexic.swissgeol.ch/active"/>
</rdf:Description>

<rdf:Description rdf:about="https://dev-lexic.swissgeol.ch/TectonicUnits/S-Charl-SesvennaNappe">
	<rdf:type rdf:resource="http://www.w3.org/2004/02/skos/core#Concept"/>
	<rdfs:isDefinedBy xml:lang="en">Gouffon Yves (Editor) (2024): Tectonic Map of Switzerland 1:500000, Explanatory notes. Federal Office of Topography swisstopo, Wabern</rdfs:isDefinedBy>
	<skos:definition xml:lang="en">The S-charl-Sesvenna Nappe (including the Tavrü Slice) in the southeastern compartment of the Engadine Fault occupies the same tectonic position as the Silvretta Nappe in the northwestern compartment of this fault.

The basement of the S-charl-Sesvenna Nappe is commonly referred to as the Sesvenna basement and its cover as “S-charl-Unterbau” (a series of NE–SW trending series of synclines and anticlines that affect both basement and cover without major detachments within the sedimentary sequence) and “S-charl-Oberbau” (nowadays referred to as Tavrü Slice, consisting entirely of a Norian to Cretaceous succession, volumetrically dominated by an over 2 km thick Hauptdolomit and completely detached from the Carnian Raibl Group).</skos:definition>
	<skos:inScheme rdf:resource="https://dev-lexic.swissgeol.ch/TectonicUnits"/>
	<skos:prefLabel xml:lang="en">S-charl-Sesvenna Nappe</skos:prefLabel>
	<skos:prefLabel xml:lang="de">S-charl-Sesvenna-Decke</skos:prefLabel>
	<skos:prefLabel xml:lang="fr">Nappe de S-charl-Sesvenna</skos:prefLabel>
	<skos:prefLabel xml:lang="it">Falda di S-charl-Sesvenna</skos:prefLabel>
	<skos:broader rdf:resource="https://dev-lexic.swissgeol.ch/TectonicUnits/UpperAustroalpine"/>
	<skos:narrower rdf:resource="https://dev-lexic.swissgeol.ch/TectonicUnits/TavrueSlice"/>
	<status xmlns="http://www.w3.org/ns/adms#" rdf:resource="https://dev-lexic.swissgeol.ch/active"/>
</rdf:Description>

<rdf:Description rdf:about="https://dev-lexic.swissgeol.ch/TectonicUnits/Salassic">
	<rdf:type rdf:resource="http://www.w3.org/2004/02/skos/core#Concept"/>
	<rdfs:isDefinedBy xml:lang="en">Gouffon Yves (Editor) (2024): Tectonic Map of Switzerland 1:500000, Explanatory notes. Federal Office of Topography swisstopo, Wabern</rdfs:isDefinedBy>
	<rdfs:comment rdf:datatype="http://www.w3.org/1999/02/22-rdf-syntax-ns#HTML">https://data.geo.admin.ch/ch.swisstopo.geologie-tektonische_karte/pdf/Erl-TK500_2024.pdf</rdfs:comment>
	<rdfs:comment rdf:datatype="http://www.w3.org/1999/02/22-rdf-syntax-ns#HTML">https://www.strati.ch/en/tectonic/salassikum</rdfs:comment>
	<skos:definition xml:lang="en">The Salassic Domain groups the tectonic units derived from an extensional allochthon split off from the most distal part of the Adriatic margin during the Middle Jurassic opening of the Piemonte-Liguria Ocean and subducted below the Austroalpine and South Alpine units in Late Cretaceous times. These units – Dent Blanche, Mont Mary and Sesia nappes in western Switzerland and adjacent Italy, together with the Margna and Sella nappes in southeastern Switzerland and partly in Italy – are characterised by their high-pressure metamorphism.</skos:definition>
	<skos:inScheme rdf:resource="https://dev-lexic.swissgeol.ch/TectonicUnits"/>
	<skos:topConceptOf rdf:resource="https://dev-lexic.swissgeol.ch/TectonicUnits"/>
	<skos:prefLabel xml:lang="en">Salassic</skos:prefLabel>
	<skos:prefLabel xml:lang="de">Salassikum</skos:prefLabel>
	<skos:prefLabel xml:lang="fr">Salassique</skos:prefLabel>
	<skos:prefLabel xml:lang="it">Salassico</skos:prefLabel>
	<skos:altLabel xml:lang="fr">Austroalpin valaisan</skos:altLabel>
	<skos:narrower rdf:resource="https://dev-lexic.swissgeol.ch/TectonicUnits/MontMaryNappe"/>
	<skos:narrower rdf:resource="https://dev-lexic.swissgeol.ch/TectonicUnits/Roisan-CignanaShearZone"/>
	<skos:narrower rdf:resource="https://dev-lexic.swissgeol.ch/TectonicUnits/DentBlancheNappe"/>
	<skos:narrower rdf:resource="https://dev-lexic.swissgeol.ch/TectonicUnits/SesiaNappe"/>
	<skos:narrower rdf:resource="https://dev-lexic.swissgeol.ch/TectonicUnits/MargnaNappe"/>
	<skos:narrower rdf:resource="https://dev-lexic.swissgeol.ch/TectonicUnits/SellaNappe"/>
	<status xmlns="http://www.w3.org/ns/adms#" rdf:resource="https://dev-lexic.swissgeol.ch/active"/>
</rdf:Description>

<rdf:Description rdf:about="https://dev-lexic.swissgeol.ch/TectonicUnits/MontMaryNappe">
	<rdf:type rdf:resource="http://www.w3.org/2004/02/skos/core#Concept"/>
	<rdfs:isDefinedBy xml:lang="en">Gouffon Yves (Editor) (2024): Tectonic Map of Switzerland 1:500000, Explanatory notes. Federal Office of Topography swisstopo, Wabern</rdfs:isDefinedBy>
	<skos:definition xml:lang="en">The Mont Mary Nappe is a Salassic tectonic unit of the Italian and Western Swiss Alps. It is constituted by two crystalline basement units: a Lower Unit mainly comprising pre-Alpine amphibolite-facies paragneisses with minor amphibolites and orthogneisses and an Upper Unit comprising pre-Alpine amphibolite- to granulite-facies paragneisses with mafic and carbonate rocks.</skos:definition>
	<skos:inScheme rdf:resource="https://dev-lexic.swissgeol.ch/TectonicUnits"/>
	<skos:prefLabel xml:lang="en">Mont Mary Nappe</skos:prefLabel>
	<skos:prefLabel xml:lang="de">Mont-Mary-Decke</skos:prefLabel>
	<skos:prefLabel xml:lang="fr">Nappe du Mont Mary</skos:prefLabel>
	<skos:prefLabel xml:lang="it">Falda del Mont Mary</skos:prefLabel>
	<skos:broader rdf:resource="https://dev-lexic.swissgeol.ch/TectonicUnits/Salassic"/>
	<skos:narrower rdf:resource="https://dev-lexic.swissgeol.ch/TectonicUnits/LowerUnitOfTheMontMaryNappe"/>
	<skos:narrower rdf:resource="https://dev-lexic.swissgeol.ch/TectonicUnits/UpperUnitOfTheMontMaryNappe"/>
	<status xmlns="http://www.w3.org/ns/adms#" rdf:resource="https://dev-lexic.swissgeol.ch/active"/>
</rdf:Description>

<rdf:Description rdf:about="https://dev-lexic.swissgeol.ch/TectonicUnits/Roisan-CignanaShearZone">
	<rdf:type rdf:resource="http://www.w3.org/2004/02/skos/core#Concept"/>
	<rdfs:isDefinedBy xml:lang="en">Gouffon Yves (Editor) (2024): Tectonic Map of Switzerland 1:500000, Explanatory notes. Federal Office of Topography swisstopo, Wabern</rdfs:isDefinedBy>
	<skos:definition xml:lang="en">The Roisan-Cignana Shear Zone consists of slices of Mesozoic sediments and crystalline basement in a mylonitic matrix derived from the adjacent Dent Blanche Nappe (Arolla Unit) and of the Mont Mary Nappe (Lower and Upper units). The high-pressure mineral assemblages along the contact between these tectonic slices indicates that their emplacement occurred in an early deformation stage, before or during the subduction.</skos:definition>
	<skos:inScheme rdf:resource="https://dev-lexic.swissgeol.ch/TectonicUnits"/>
	<skos:prefLabel xml:lang="en">Roisan-Cignana Shear Zone</skos:prefLabel>
	<skos:prefLabel xml:lang="de">Roisan-Cignana-Scherzone</skos:prefLabel>
	<skos:prefLabel xml:lang="fr">Zone de cisaillement de Roisan-Cignana</skos:prefLabel>
	<skos:prefLabel xml:lang="it">Zona di taglio di Roisan-Cignana</skos:prefLabel>
	<skos:broader rdf:resource="https://dev-lexic.swissgeol.ch/TectonicUnits/Salassic"/>
	<status xmlns="http://www.w3.org/ns/adms#" rdf:resource="https://dev-lexic.swissgeol.ch/active"/>
</rdf:Description>

<rdf:Description rdf:about="https://dev-lexic.swissgeol.ch/TectonicUnits/DentBlancheNappe">
	<rdf:type rdf:resource="http://www.w3.org/2004/02/skos/core#Concept"/>
	<rdfs:isDefinedBy xml:lang="en">Gouffon Yves (Editor) (2024): Tectonic Map of Switzerland 1:500000, Explanatory notes. Federal Office of Topography swisstopo, Wabern</rdfs:isDefinedBy>
	<skos:definition xml:lang="en">The Dent Blanche Nappe is a Salassic tectonic unit comprising two crystalline basement units. The lower Arolla Unit is essentially composed of metagranitoids and some metagabbro bodies, all of Permian age and more or less deformed. The upper Valpelline Unit consists of paragneisses with mafic and carbonate rocks, characterized by a pre-Alpine amphibolite to granulite-facies metamorphism. A Triassic–Jurassic sedimentary cover (Mont Dolin series) overlies the Arolla Unit in a small area of the Val d’Hérens, west of Arolla.</skos:definition>
	<skos:inScheme rdf:resource="https://dev-lexic.swissgeol.ch/TectonicUnits"/>
	<skos:prefLabel xml:lang="en">Dent Blanche Nappe</skos:prefLabel>
	<skos:prefLabel xml:lang="de">Dent-Blanche-Decke</skos:prefLabel>
	<skos:prefLabel xml:lang="fr">Nappe de la Dent Blanche</skos:prefLabel>
	<skos:prefLabel xml:lang="it">Falda della Dent Blanche</skos:prefLabel>
	<skos:broader rdf:resource="https://dev-lexic.swissgeol.ch/TectonicUnits/Salassic"/>
	<skos:narrower rdf:resource="https://dev-lexic.swissgeol.ch/TectonicUnits/ArollaUnit"/>
	<skos:narrower rdf:resource="https://dev-lexic.swissgeol.ch/TectonicUnits/ValpellineUnit"/>
	<status xmlns="http://www.w3.org/ns/adms#" rdf:resource="https://dev-lexic.swissgeol.ch/active"/>
</rdf:Description>

<rdf:Description rdf:about="https://dev-lexic.swissgeol.ch/TectonicUnits/SesiaNappe">
	<rdf:type rdf:resource="http://www.w3.org/2004/02/skos/core#Concept"/>
	<rdfs:isDefinedBy xml:lang="en">Gouffon Yves (Editor) (2024): Tectonic Map of Switzerland 1:500000, Explanatory notes. Federal Office of Topography swisstopo, Wabern</rdfs:isDefinedBy>
	<skos:definition xml:lang="en">The Sesia Nappe is a Salassic tectonic unit located between the Canavese Fault to the east and the Upper Penninic units to the west. It is composed of three units of crystalline basement characterized by different lithological associations: the Second Dioritic-Kinzigitic Zone, The Gneiss Minuti Unit and the Eclogitic Micaschist Unit.</skos:definition>
	<skos:inScheme rdf:resource="https://dev-lexic.swissgeol.ch/TectonicUnits"/>
	<skos:prefLabel xml:lang="en">Sesia Nappe</skos:prefLabel>
	<skos:prefLabel xml:lang="de">Sesia-Decke</skos:prefLabel>
	<skos:prefLabel xml:lang="fr">Nappe de Sesia</skos:prefLabel>
	<skos:prefLabel xml:lang="it">Falda di Sesia</skos:prefLabel>
	<skos:broader rdf:resource="https://dev-lexic.swissgeol.ch/TectonicUnits/Salassic"/>
	<skos:narrower rdf:resource="https://dev-lexic.swissgeol.ch/TectonicUnits/SecondDioritic-KinzigiticZone"/>
	<skos:narrower rdf:resource="https://dev-lexic.swissgeol.ch/TectonicUnits/Gneiss-MinutiUnit"/>
	<skos:narrower rdf:resource="https://dev-lexic.swissgeol.ch/TectonicUnits/Micascisti-EclogiticiUnit"/>
	<status xmlns="http://www.w3.org/ns/adms#" rdf:resource="https://dev-lexic.swissgeol.ch/active"/>
</rdf:Description>

<rdf:Description rdf:about="https://dev-lexic.swissgeol.ch/TectonicUnits/MargnaNappe">
	<rdf:type rdf:resource="http://www.w3.org/2004/02/skos/core#Concept"/>
	<rdfs:isDefinedBy xml:lang="en">Gouffon Yves (Editor) (2024): Tectonic Map of Switzerland 1:500000, Explanatory notes. Federal Office of Topography swisstopo, Wabern</rdfs:isDefinedBy>
	<skos:definition xml:lang="en">The Margna Nappe is a Salassic tectonic unit thrust over the ophiolitic Malenco-Forno-Lizun Nappe divided into two W-facing flat-lying antiformal basement cores separated by a thrust fault highlighted by a thin Triassic sedimentary band. The basement cores include upper crustal granitoids and paragneisses, as well as lower crustal pelitic pre-Alpine granulites and Permian gabbros. The Mesozoic cover is mainly developed at the top of the nappe, where it forms a syncline that is believed to link the Margna Nappe to the overlying Sella Nappe.</skos:definition>
	<skos:inScheme rdf:resource="https://dev-lexic.swissgeol.ch/TectonicUnits"/>
	<skos:prefLabel xml:lang="en">Margna Nappe</skos:prefLabel>
	<skos:prefLabel xml:lang="de">Margna-Decke</skos:prefLabel>
	<skos:prefLabel xml:lang="fr">Nappe de la Margna</skos:prefLabel>
	<skos:prefLabel xml:lang="it">Falda della Margna</skos:prefLabel>
	<skos:broader rdf:resource="https://dev-lexic.swissgeol.ch/TectonicUnits/Salassic"/>
	<skos:narrower rdf:resource="https://dev-lexic.swissgeol.ch/TectonicUnits/ForcellinaSlice"/>
	<status xmlns="http://www.w3.org/ns/adms#" rdf:resource="https://dev-lexic.swissgeol.ch/active"/>
</rdf:Description>

<rdf:Description rdf:about="https://dev-lexic.swissgeol.ch/TectonicUnits/SellaNappe">
	<rdf:type rdf:resource="http://www.w3.org/2004/02/skos/core#Concept"/>
	<rdfs:isDefinedBy xml:lang="en">Gouffon Yves (Editor) (2024): Tectonic Map of Switzerland 1:500000, Explanatory notes. Federal Office of Topography swisstopo, Wabern</rdfs:isDefinedBy>
	<skos:definition xml:lang="en">The Sella Nappe is a Salassic tectonic unit of the Eastern Swiss Alps. It contains only upper crustal granitoids and paragneisses, very similar to that of the overlying Err and Bernina nappe complexes. A thin Mesozoic cover is present mainly at the front of the nappe in the northwest and from there over a few kilometers of its upper limb.</skos:definition>
	<skos:inScheme rdf:resource="https://dev-lexic.swissgeol.ch/TectonicUnits"/>
	<skos:prefLabel xml:lang="en">Sella Nappe</skos:prefLabel>
	<skos:prefLabel xml:lang="de">Sella-Decke</skos:prefLabel>
	<skos:prefLabel xml:lang="fr">Nappe de la Sella</skos:prefLabel>
	<skos:prefLabel xml:lang="it">Falda della Sella</skos:prefLabel>
	<skos:broader rdf:resource="https://dev-lexic.swissgeol.ch/TectonicUnits/Salassic"/>
	<status xmlns="http://www.w3.org/ns/adms#" rdf:resource="https://dev-lexic.swissgeol.ch/active"/>
</rdf:Description>

<rdf:Description rdf:about="https://dev-lexic.swissgeol.ch/TectonicUnits/LowerUnitOfTheMontMaryNappe">
	<rdf:type rdf:resource="http://www.w3.org/2004/02/skos/core#Concept"/>
	<rdfs:isDefinedBy xml:lang="en">Gouffon Yves (Editor) (2024): Tectonic Map of Switzerland 1:500000, Explanatory notes. Federal Office of Topography swisstopo, Wabern</rdfs:isDefinedBy>
	<skos:definition xml:lang="en">The Lower Unit of the Mont Mary Nappe mainly comprises pre-Alpine amphibolite-facies paragneisses and minor amphibolites and orthogneisses.</skos:definition>
	<skos:inScheme rdf:resource="https://dev-lexic.swissgeol.ch/TectonicUnits"/>
	<skos:prefLabel xml:lang="en">Lower Unit of the Mont Mary Nappe</skos:prefLabel>
	<skos:prefLabel xml:lang="de">Untere Einheit der Mont-Mary-Decke</skos:prefLabel>
	<skos:prefLabel xml:lang="fr">Unité Inférieure de la Nappe du Mont Mary</skos:prefLabel>
	<skos:prefLabel xml:lang="it">Unità Inferiore della Falda del Mont Mary</skos:prefLabel>
	<skos:broader rdf:resource="https://dev-lexic.swissgeol.ch/TectonicUnits/MontMaryNappe"/>
	<skos:related rdf:resource="https://dev-lexic.swissgeol.ch/TectonicUnits/ArollaUnit"/>
	<status xmlns="http://www.w3.org/ns/adms#" rdf:resource="https://dev-lexic.swissgeol.ch/active"/>
</rdf:Description>

<rdf:Description rdf:about="https://dev-lexic.swissgeol.ch/TectonicUnits/UpperUnitOfTheMontMaryNappe">
	<rdf:type rdf:resource="http://www.w3.org/2004/02/skos/core#Concept"/>
	<rdfs:isDefinedBy xml:lang="en">Gouffon Yves (Editor) (2024): Tectonic Map of Switzerland 1:500000, Explanatory notes. Federal Office of Topography swisstopo, Wabern</rdfs:isDefinedBy>
	<skos:definition xml:lang="en">The Upper Unit of the Mont Mary Nappe consists of high-grade pre-Alpine paragneisses (kinzigites auct.), amphibolites, marbles and minor spinel-amphibole harzburgites. It is similar to the Valpelline Unit of the Dent Blanche Nappe.</skos:definition>
	<skos:inScheme rdf:resource="https://dev-lexic.swissgeol.ch/TectonicUnits"/>
	<skos:prefLabel xml:lang="en">Upper Unit of the Mont Mary Nappe</skos:prefLabel>
	<skos:prefLabel xml:lang="de">Obere Einheit der Mont-Mary-Decke</skos:prefLabel>
	<skos:prefLabel xml:lang="fr">Unité Supérieure de la Nappe du Mont Mary</skos:prefLabel>
	<skos:prefLabel xml:lang="it">Unità Superiore della Falda del Mont Mary</skos:prefLabel>
	<skos:broader rdf:resource="https://dev-lexic.swissgeol.ch/TectonicUnits/MontMaryNappe"/>
	<skos:related rdf:resource="https://dev-lexic.swissgeol.ch/TectonicUnits/ValpellineUnit"/>
	<status xmlns="http://www.w3.org/ns/adms#" rdf:resource="https://dev-lexic.swissgeol.ch/active"/>
</rdf:Description>

<rdf:Description rdf:about="https://dev-lexic.swissgeol.ch/TectonicUnits/ArollaUnit">
	<rdf:type rdf:resource="http://www.w3.org/2004/02/skos/core#Concept"/>
	<rdfs:isDefinedBy xml:lang="en">Gouffon Yves (Editor) (2024): Tectonic Map of Switzerland 1:500000, Explanatory notes. Federal Office of Topography swisstopo, Wabern</rdfs:isDefinedBy>
	<skos:definition xml:lang="en">The Arolla Unit forms the structurally lower part of the Salassic Dent Blanche Nappe. It is essentially composed of metagranitoids and some metagabbro bodies, all of Permian age and more or less deformed.</skos:definition>
	<skos:inScheme rdf:resource="https://dev-lexic.swissgeol.ch/TectonicUnits"/>
	<skos:prefLabel xml:lang="en">Arolla Unit</skos:prefLabel>
	<skos:prefLabel xml:lang="de">Arolla-Einheit</skos:prefLabel>
	<skos:prefLabel xml:lang="fr">Unité d'Arolla</skos:prefLabel>
	<skos:prefLabel xml:lang="it">Unità di Arolla</skos:prefLabel>
	<skos:broader rdf:resource="https://dev-lexic.swissgeol.ch/TectonicUnits/DentBlancheNappe"/>
	<skos:related rdf:resource="https://dev-lexic.swissgeol.ch/TectonicUnits/LowerUnitOfTheMontMaryNappe"/>
	<status xmlns="http://www.w3.org/ns/adms#" rdf:resource="https://dev-lexic.swissgeol.ch/active"/>
</rdf:Description>

<rdf:Description rdf:about="https://dev-lexic.swissgeol.ch/TectonicUnits/ValpellineUnit">
	<rdf:type rdf:resource="http://www.w3.org/2004/02/skos/core#Concept"/>
	<rdfs:isDefinedBy xml:lang="en">Gouffon Yves (Editor) (2024): Tectonic Map of Switzerland 1:500000, Explanatory notes. Federal Office of Topography swisstopo, Wabern</rdfs:isDefinedBy>
	<skos:definition xml:lang="en">The Valpelline Unit forms the structurally upper part of the Salassic Dent Blanche Nappe. It consists of paragneisses with mafic and carbonate rocks, characterized by a pre-Alpine amphibolite to granulite-facies metamorphism.</skos:definition>
	<skos:inScheme rdf:resource="https://dev-lexic.swissgeol.ch/TectonicUnits"/>
	<skos:prefLabel xml:lang="en">Valpelline Unit</skos:prefLabel>
	<skos:prefLabel xml:lang="de">Valpelline-Einheit</skos:prefLabel>
	<skos:prefLabel xml:lang="fr">Unité de Valpelline</skos:prefLabel>
	<skos:prefLabel xml:lang="it">Unità di Valpelline</skos:prefLabel>
	<skos:broader rdf:resource="https://dev-lexic.swissgeol.ch/TectonicUnits/DentBlancheNappe"/>
	<skos:related rdf:resource="https://dev-lexic.swissgeol.ch/TectonicUnits/UpperUnitOfTheMontMaryNappe"/>
	<status xmlns="http://www.w3.org/ns/adms#" rdf:resource="https://dev-lexic.swissgeol.ch/active"/>
</rdf:Description>

<rdf:Description rdf:about="https://dev-lexic.swissgeol.ch/TectonicUnits/SecondDioritic-KinzigiticZone">
	<rdf:type rdf:resource="http://www.w3.org/2004/02/skos/core#Concept"/>
	<rdfs:isDefinedBy xml:lang="en">Gouffon Yves (Editor) (2024): Tectonic Map of Switzerland 1:500000, Explanatory notes. Federal Office of Topography swisstopo, Wabern</rdfs:isDefinedBy>
	<skos:definition xml:lang="en">The Second Dioritic-Kinzigitic Zone (2DK) of the Sesia Nappe consists of kilometer-scale slices of micaschists, characterized by well-preserved pre-Alpine amphibolite to granulite-facies mineral assemblages as well as minor amphibolites and marbles, locally overprinted by the early Alpine high-pressure metamorphism.</skos:definition>
	<skos:inScheme rdf:resource="https://dev-lexic.swissgeol.ch/TectonicUnits"/>
	<skos:prefLabel xml:lang="en">Second Dioritic-Kinzigitic Zone</skos:prefLabel>
	<skos:prefLabel xml:lang="de">Seconda Zona Dioritico-Kinzigitica</skos:prefLabel>
	<skos:prefLabel xml:lang="fr">Seconde Zone Dioritico-Kinzigitique</skos:prefLabel>
	<skos:prefLabel xml:lang="it">Seconda Zona Dioritico-Kinzigitica</skos:prefLabel>
	<skos:broader rdf:resource="https://dev-lexic.swissgeol.ch/TectonicUnits/SesiaNappe"/>
	<status xmlns="http://www.w3.org/ns/adms#" rdf:resource="https://dev-lexic.swissgeol.ch/active"/>
</rdf:Description>

<rdf:Description rdf:about="https://dev-lexic.swissgeol.ch/TectonicUnits/Gneiss-MinutiUnit">
	<rdf:type rdf:resource="http://www.w3.org/2004/02/skos/core#Concept"/>
	<rdfs:isDefinedBy xml:lang="en">Gouffon Yves (Editor) (2024): Tectonic Map of Switzerland 1:500000, Explanatory notes. Federal Office of Topography swisstopo, Wabern</rdfs:isDefinedBy>
	<skos:definition xml:lang="en">The Gneiss Minuti Unit of the Sesia Nappe consists mainly of orthogneisses, derived from granitoid of probable Permian age and interbedded with more mafic layers. High-pressure metamorphism of this unit was largely obliterated by the later greenschist-facies metamorphism.</skos:definition>
	<skos:inScheme rdf:resource="https://dev-lexic.swissgeol.ch/TectonicUnits"/>
	<skos:prefLabel xml:lang="en">Gneiss-minuti Unit</skos:prefLabel>
	<skos:prefLabel xml:lang="de">Gneiss-minuti-Einheit</skos:prefLabel>
	<skos:prefLabel xml:lang="fr">Unité des Gneiss minuti</skos:prefLabel>
	<skos:prefLabel xml:lang="it">Unità degli Gneiss minuti</skos:prefLabel>
	<skos:broader rdf:resource="https://dev-lexic.swissgeol.ch/TectonicUnits/SesiaNappe"/>
	<status xmlns="http://www.w3.org/ns/adms#" rdf:resource="https://dev-lexic.swissgeol.ch/active"/>
</rdf:Description>

<rdf:Description rdf:about="https://dev-lexic.swissgeol.ch/TectonicUnits/Micascisti-EclogiticiUnit">
	<rdf:type rdf:resource="http://www.w3.org/2004/02/skos/core#Concept"/>
	<rdfs:isDefinedBy xml:lang="en">Gouffon Yves (Editor) (2024): Tectonic Map of Switzerland 1:500000, Explanatory notes. Federal Office of Topography swisstopo, Wabern</rdfs:isDefinedBy>
	<skos:definition xml:lang="en">The Eclogitic Micaschist Unit of the Sesia Nappe comprises mostly paragneisses with minor mafic rocks, orthogneisses and calcitic marbles. Eclogitic mineral assemblages are well preserved, rarely overprinted by the subsequent greenschist-facies metamorphism.</skos:definition>
	<skos:inScheme rdf:resource="https://dev-lexic.swissgeol.ch/TectonicUnits"/>
	<skos:prefLabel xml:lang="en">Micascisti-eclogitici Unit</skos:prefLabel>
	<skos:prefLabel xml:lang="de">Micascisti-eclogitici-Einheit</skos:prefLabel>
	<skos:prefLabel xml:lang="fr">Unité des Micaschistes éclogitiques</skos:prefLabel>
	<skos:prefLabel xml:lang="it">Unità dei Micascisti eclogitici</skos:prefLabel>
	<skos:broader rdf:resource="https://dev-lexic.swissgeol.ch/TectonicUnits/SesiaNappe"/>
	<status xmlns="http://www.w3.org/ns/adms#" rdf:resource="https://dev-lexic.swissgeol.ch/active"/>
</rdf:Description>

<rdf:Description rdf:about="https://dev-lexic.swissgeol.ch/TectonicUnits/ForcellinaSlice">
	<rdf:type rdf:resource="http://www.w3.org/2004/02/skos/core#Concept"/>
	<rdfs:isDefinedBy xml:lang="en">Gouffon Yves (Editor) (2024): Tectonic Map of Switzerland 1:500000, Explanatory notes. Federal Office of Topography swisstopo, Wabern</rdfs:isDefinedBy>
	<skos:inScheme rdf:resource="https://dev-lexic.swissgeol.ch/TectonicUnits"/>
	<skos:prefLabel xml:lang="en">Forcellina Slice</skos:prefLabel>
	<skos:prefLabel xml:lang="de">Forcellina-Schuppe</skos:prefLabel>
	<skos:prefLabel xml:lang="fr">Écaille de la Forcellina</skos:prefLabel>
	<skos:prefLabel xml:lang="it">Scaglia della Forcellina</skos:prefLabel>
	<skos:broader rdf:resource="https://dev-lexic.swissgeol.ch/TectonicUnits/MargnaNappe"/>
	<status xmlns="http://www.w3.org/ns/adms#" rdf:resource="https://dev-lexic.swissgeol.ch/active"/>
</rdf:Description>

<rdf:Description rdf:about="https://dev-lexic.swissgeol.ch/TectonicUnits/RothornNappe">
	<rdf:type rdf:resource="http://www.w3.org/2004/02/skos/core#Concept"/>
	<rdfs:isDefinedBy xml:lang="en">Gouffon Yves (Editor) (2024): Tectonic Map of Switzerland 1:500000, Explanatory notes. Federal Office of Topography swisstopo, Wabern</rdfs:isDefinedBy>
	<skos:definition xml:lang="en">The small Rothorn Nappe, with a basement-cover sequence, directly underlies the Upper Austroalpine Schiahorn Nappe in the southwestern part of the Prättigau Half-Window, between Tiefencastel and Arosa.</skos:definition>
	<skos:inScheme rdf:resource="https://dev-lexic.swissgeol.ch/TectonicUnits"/>
	<skos:prefLabel xml:lang="en">Rothorn Nappe</skos:prefLabel>
	<skos:prefLabel xml:lang="de">Rothorn-Decke</skos:prefLabel>
	<skos:prefLabel xml:lang="fr">Nappe du Rothorn</skos:prefLabel>
	<skos:prefLabel xml:lang="it">Falda del Rothorn</skos:prefLabel>
	<skos:broader rdf:resource="https://dev-lexic.swissgeol.ch/TectonicUnits/Rothorn-SchwarzhornNappeComplex"/>
	<status xmlns="http://www.w3.org/ns/adms#" rdf:resource="https://dev-lexic.swissgeol.ch/active"/>
</rdf:Description>

<rdf:Description rdf:about="https://dev-lexic.swissgeol.ch/TectonicUnits/TschirpenNappe">
	<rdf:type rdf:resource="http://www.w3.org/2004/02/skos/core#Concept"/>
	<rdfs:isDefinedBy xml:lang="en">Gouffon Yves (Editor) (2024): Tectonic Map of Switzerland 1:500000, Explanatory notes. Federal Office of Topography swisstopo, Wabern</rdfs:isDefinedBy>
	<skos:definition xml:lang="en">The small Tschirpen Nappe is a Lower Austroalpine sedimentary sequence overlying the Arosa Zone in the southwestern part of the Prättigau Half-Window, between Tiefencastel and Arosa.</skos:definition>
	<skos:inScheme rdf:resource="https://dev-lexic.swissgeol.ch/TectonicUnits"/>
	<skos:prefLabel xml:lang="en">Tschirpen Nappe</skos:prefLabel>
	<skos:prefLabel xml:lang="de">Tschirpen-Decke</skos:prefLabel>
	<skos:prefLabel xml:lang="fr">Nappe du Tschirpen</skos:prefLabel>
	<skos:prefLabel xml:lang="it">Falda del Tschirpen</skos:prefLabel>
	<skos:broader rdf:resource="https://dev-lexic.swissgeol.ch/TectonicUnits/Rothorn-SchwarzhornNappeComplex"/>
	<status xmlns="http://www.w3.org/ns/adms#" rdf:resource="https://dev-lexic.swissgeol.ch/active"/>
</rdf:Description>

<rdf:Description rdf:about="https://dev-lexic.swissgeol.ch/TectonicUnits/SchaflaegerNappe">
	<rdf:type rdf:resource="http://www.w3.org/2004/02/skos/core#Concept"/>
	<rdfs:isDefinedBy xml:lang="en">Gouffon Yves (Editor) (2024): Tectonic Map of Switzerland 1:500000, Explanatory notes. Federal Office of Topography swisstopo, Wabern</rdfs:isDefinedBy>
	<skos:definition xml:lang="en">The thin, discontinuous sedimentary Schafläger Nappe, locally overlain by crystalline rocks of the Rothorn Nappe, separates the Dorfberg Nappe from the overlying Schiahorn Nappe and Silvretta Nappe respectively. The Schafläger Nappe can be correlated with the Tschirpen Nappe.</skos:definition>
	<skos:inScheme rdf:resource="https://dev-lexic.swissgeol.ch/TectonicUnits"/>
	<skos:prefLabel xml:lang="en">Schafläger Nappe</skos:prefLabel>
	<skos:prefLabel xml:lang="de">Schafläger-Decke</skos:prefLabel>
	<skos:prefLabel xml:lang="fr">Nappe du Schafläger</skos:prefLabel>
	<skos:prefLabel xml:lang="it">Falda dello Schafläger</skos:prefLabel>
	<skos:broader rdf:resource="https://dev-lexic.swissgeol.ch/TectonicUnits/Rothorn-SchwarzhornNappeComplex"/>
	<status xmlns="http://www.w3.org/ns/adms#" rdf:resource="https://dev-lexic.swissgeol.ch/active"/>
</rdf:Description>

<rdf:Description rdf:about="https://dev-lexic.swissgeol.ch/TectonicUnits/DorfbergNappe">
	<rdf:type rdf:resource="http://www.w3.org/2004/02/skos/core#Concept"/>
	<rdfs:isDefinedBy xml:lang="en">Gouffon Yves (Editor) (2024): Tectonic Map of Switzerland 1:500000, Explanatory notes. Federal Office of Topography swisstopo, Wabern</rdfs:isDefinedBy>
	<skos:definition xml:lang="en">To the northeast of the Prättigau Half-Window, the crystalline Dorfberg Nappe is intercalated between the Arosa Zone and the Schiahorn Nappe as far as the Davoser See, respectively by the Silvretta Nappe further to Klosters.</skos:definition>
	<skos:inScheme rdf:resource="https://dev-lexic.swissgeol.ch/TectonicUnits"/>
	<skos:prefLabel xml:lang="en">Dorfberg Nappe</skos:prefLabel>
	<skos:prefLabel xml:lang="de">Dorfberg-Decke</skos:prefLabel>
	<skos:prefLabel xml:lang="fr">Nappe du Dorfberg</skos:prefLabel>
	<skos:prefLabel xml:lang="it">Falda del Dorfberg</skos:prefLabel>
	<skos:broader rdf:resource="https://dev-lexic.swissgeol.ch/TectonicUnits/Rothorn-SchwarzhornNappeComplex"/>
	<status xmlns="http://www.w3.org/ns/adms#" rdf:resource="https://dev-lexic.swissgeol.ch/active"/>
</rdf:Description>

<rdf:Description rdf:about="https://dev-lexic.swissgeol.ch/TectonicUnits/GrueenhornSlice">
	<rdf:type rdf:resource="http://www.w3.org/2004/02/skos/core#Concept"/>
	<rdfs:isDefinedBy xml:lang="en">Gouffon Yves (Editor) (2024): Tectonic Map of Switzerland 1:500000, Explanatory notes. Federal Office of Topography swisstopo, Wabern</rdfs:isDefinedBy>
	<skos:definition xml:lang="en">The Grüenhorn Slice is considered as an independant tectonic klippe correlated with the Err Nappe Complex and overlying the Arosa Zone. It is made up of a sedimentary series of Lower Austroalpine affinity.</skos:definition>
	<skos:inScheme rdf:resource="https://dev-lexic.swissgeol.ch/TectonicUnits"/>
	<skos:prefLabel xml:lang="en">Grüenhorn Slice</skos:prefLabel>
	<skos:prefLabel xml:lang="de">Grüenhorn-Schuppe</skos:prefLabel>
	<skos:prefLabel xml:lang="fr">Écaille du Grüenhorn</skos:prefLabel>
	<skos:prefLabel xml:lang="it">Scaglia del Grüenhorn</skos:prefLabel>
	<skos:broader rdf:resource="https://dev-lexic.swissgeol.ch/TectonicUnits/Grueenhorn-CasannaSliceComplex"/>
	<status xmlns="http://www.w3.org/ns/adms#" rdf:resource="https://dev-lexic.swissgeol.ch/active"/>
</rdf:Description>

<rdf:Description rdf:about="https://dev-lexic.swissgeol.ch/TectonicUnits/CasannaSlice">
	<rdf:type rdf:resource="http://www.w3.org/2004/02/skos/core#Concept"/>
	<rdfs:isDefinedBy xml:lang="en">Gouffon Yves (Editor) (2024): Tectonic Map of Switzerland 1:500000, Explanatory notes. Federal Office of Topography swisstopo, Wabern</rdfs:isDefinedBy>
	<skos:definition xml:lang="en">The Casanna Slice is considered as an independant tectonic klippe correlated with the Err Nappe Complex and overlying the Arosa Zone. It is made up of a sedimentary series of Lower Austroalpine affinity.</skos:definition>
	<skos:inScheme rdf:resource="https://dev-lexic.swissgeol.ch/TectonicUnits"/>
	<skos:prefLabel xml:lang="en">Casanna Slice</skos:prefLabel>
	<skos:prefLabel xml:lang="de">Casanna-Schuppe</skos:prefLabel>
	<skos:prefLabel xml:lang="fr">Écaille de la Casanna</skos:prefLabel>
	<skos:prefLabel xml:lang="it">Scaglia della Casanna</skos:prefLabel>
	<skos:broader rdf:resource="https://dev-lexic.swissgeol.ch/TectonicUnits/Grueenhorn-CasannaSliceComplex"/>
	<status xmlns="http://www.w3.org/ns/adms#" rdf:resource="https://dev-lexic.swissgeol.ch/active"/>
</rdf:Description>

<rdf:Description rdf:about="https://dev-lexic.swissgeol.ch/TectonicUnits/ElaNappe">
	<rdf:type rdf:resource="http://www.w3.org/2004/02/skos/core#Concept"/>
	<rdfs:isDefinedBy xml:lang="en">Gouffon Yves (Editor) (2024): Tectonic Map of Switzerland 1:500000, Explanatory notes. Federal Office of Topography swisstopo, Wabern</rdfs:isDefinedBy>
	<skos:definition xml:lang="en">The Ela Nappe, which forms the hangingwall of the Madulain Slices and the footwall of the Upper Austroalpine Silvretta Nappe, consists of a sedimentary sequence that was completely detached from its former crystalline substrate during Cretaceous top-W thrusting along Carnian evaporites. Large parts of it were affected by sinistrally transpressive deformation during Cretaceous shortening, followed by an extensional overprint in the latest Cretaceous and the N-directed thrusting of the Silvretta Nappe during the Cenozoic orogeny. Hence, the internal structure of the Ela Nappe is highly complex due to its polyphase deformation.</skos:definition>
	<skos:inScheme rdf:resource="https://dev-lexic.swissgeol.ch/TectonicUnits"/>
	<skos:prefLabel xml:lang="en">Ela Nappe</skos:prefLabel>
	<skos:prefLabel xml:lang="de">Ela-Decke</skos:prefLabel>
	<skos:prefLabel xml:lang="fr">Nappe de l'Ela</skos:prefLabel>
	<skos:prefLabel xml:lang="it">Falda di Ela</skos:prefLabel>
	<skos:broader rdf:resource="https://dev-lexic.swissgeol.ch/TectonicUnits/BerninaNappeComplex"/>
	<status xmlns="http://www.w3.org/ns/adms#" rdf:resource="https://dev-lexic.swissgeol.ch/active"/>
</rdf:Description>

<rdf:Description rdf:about="https://dev-lexic.swissgeol.ch/TectonicUnits/BerninaNappe">
	<rdf:type rdf:resource="http://www.w3.org/2004/02/skos/core#Concept"/>
	<rdfs:isDefinedBy xml:lang="en">Gouffon Yves (Editor) (2024): Tectonic Map of Switzerland 1:500000, Explanatory notes. Federal Office of Topography swisstopo, Wabern</rdfs:isDefinedBy>
	<skos:definition xml:lang="en">The Lower Austroalpine Bernina Nappe is a basement-dominated nappe that occupies a very large area southeast of the Engadine Fault. The basement is dominated by Late to Post-Variscan magmatic rocks, which intrude an older basement of presumably Precambrian age with Variscan overprint that is mainly preserved in the northern part of the nappe. Its Mesozoic cover is rather sparsely preserved, except for two important and famous occurrences, one around Piz Alv, north of the Bernina Pass, in the footwall of the Languard Nappe, and the other at the Sassalb, east of Poschiavo, in the footwall of the Campo Nappe. The Bernina Nappe lacks a clear separation from the underlying Sella Nappe, which is attributed to the Salassic. South of Poschiavo, the Bernina Nappe is folded around the E-plunging Pass d’Ur Antiform and can be followed westward along the Southern Steep Belt north of the Tonale Fault, until being cut off by the Bregaglia Intrusion.</skos:definition>
	<skos:inScheme rdf:resource="https://dev-lexic.swissgeol.ch/TectonicUnits"/>
	<skos:prefLabel xml:lang="en">Bernina Nappe</skos:prefLabel>
	<skos:prefLabel xml:lang="de">Bernina-Decke</skos:prefLabel>
	<skos:prefLabel xml:lang="fr">Nappe du Bernina</skos:prefLabel>
	<skos:prefLabel xml:lang="it">Falda del Bernina</skos:prefLabel>
	<skos:broader rdf:resource="https://dev-lexic.swissgeol.ch/TectonicUnits/BerninaNappeComplex"/>
	<status xmlns="http://www.w3.org/ns/adms#" rdf:resource="https://dev-lexic.swissgeol.ch/active"/>
</rdf:Description>

<rdf:Description rdf:about="https://dev-lexic.swissgeol.ch/TectonicUnits/MuesellaSlice">
	<rdf:type rdf:resource="http://www.w3.org/2004/02/skos/core#Concept"/>
	<rdfs:isDefinedBy xml:lang="en">Gouffon Yves (Editor) (2024): Tectonic Map of Switzerland 1:500000, Explanatory notes. Federal Office of Topography swisstopo, Wabern</rdfs:isDefinedBy>
	<skos:definition xml:lang="en">The Müsella Slice is composed of the Müsella basement and an overlying band of strongly tectonized Mesozoic sediments (“Corn element”). This slice is considered part of the Bernina Nappe Complex mainly for structural reasons. Thereby the Müsella basement is correlated with the basement of the Julier Nappe while the Mesozoic sediments are correlated with the Ela Nappe on the north-western side of the Engadine Fault. The Mesozoic sediments of the Müsella Slice are overthrust by the Upper Austroalpine Languard Nappe. Alternatively, this slice could be considered as part of the Upper Austroalpine Languard Nappe.</skos:definition>
	<skos:inScheme rdf:resource="https://dev-lexic.swissgeol.ch/TectonicUnits"/>
	<skos:prefLabel xml:lang="en">Müsella Slice</skos:prefLabel>
	<skos:prefLabel xml:lang="de">Müsella-Schuppe</skos:prefLabel>
	<skos:prefLabel xml:lang="fr">Écaille du Müsella</skos:prefLabel>
	<skos:prefLabel xml:lang="it">Scaglia del Müsella</skos:prefLabel>
	<skos:broader rdf:resource="https://dev-lexic.swissgeol.ch/TectonicUnits/BerninaNappeComplex"/>
	<status xmlns="http://www.w3.org/ns/adms#" rdf:resource="https://dev-lexic.swissgeol.ch/active"/>
</rdf:Description>

<rdf:Description rdf:about="https://dev-lexic.swissgeol.ch/TectonicUnits/MezzaunSlice">
	<rdf:type rdf:resource="http://www.w3.org/2004/02/skos/core#Concept"/>
	<rdfs:isDefinedBy xml:lang="en">Gouffon Yves (Editor) (2024): Tectonic Map of Switzerland 1:500000, Explanatory notes. Federal Office of Topography swisstopo, Wabern</rdfs:isDefinedBy>
	<skos:definition xml:lang="en">The Mezzaun Slice crops out southeast of the Engadine Fault around the Piz Mezzaun. It is composed of a Mesozoic sequence considered as part of the Bernina Nappe Complex. This slice is downfaulted by the Late Cretaceous Mezzaun Normal Fault in respect to the domal structure of the Murtiröl Slice (Err Nappe Complex) forming the footwall of this fault. It is overthrust by the Müsella Slice.</skos:definition>
	<skos:inScheme rdf:resource="https://dev-lexic.swissgeol.ch/TectonicUnits"/>
	<skos:prefLabel xml:lang="en">Mezzaun Slice</skos:prefLabel>
	<skos:prefLabel xml:lang="de">Mezzaun-Schuppe</skos:prefLabel>
	<skos:prefLabel xml:lang="fr">Écaille du Mezzaun</skos:prefLabel>
	<skos:prefLabel xml:lang="it">Scaglia del Mezzaun</skos:prefLabel>
	<skos:broader rdf:resource="https://dev-lexic.swissgeol.ch/TectonicUnits/BerninaNappeComplex"/>
	<status xmlns="http://www.w3.org/ns/adms#" rdf:resource="https://dev-lexic.swissgeol.ch/active"/>
</rdf:Description>

<rdf:Description rdf:about="https://dev-lexic.swissgeol.ch/TectonicUnits/MadulainSlices">
	<rdf:type rdf:resource="http://www.w3.org/2004/02/skos/core#Concept"/>
	<rdfs:isDefinedBy xml:lang="en">Gouffon Yves (Editor) (2024): Tectonic Map of Switzerland 1:500000, Explanatory notes. Federal Office of Topography swisstopo, Wabern</rdfs:isDefinedBy>
	<skos:definition xml:lang="en">The Madulain Slices (“Albula Steilzone”) are located on the northwestern side of the Engadine Fault, where they lie to the north of the underlying Err Nappe and represent the base of the overlying Ela Nappe. This tectonic unit is made up of slices of sediments, attributed to the Bernina Nappe Complex by facies, in which thin and intensely folded slices of Err basement and sediments are inserted. This slice complex extends from west of the Pass d’Alvra (Albulapass) all the way to Madulain in the Engadine Valley.</skos:definition>
	<skos:inScheme rdf:resource="https://dev-lexic.swissgeol.ch/TectonicUnits"/>
	<skos:prefLabel xml:lang="en">Madulain Slices</skos:prefLabel>
	<skos:prefLabel xml:lang="de">Madulain-Schuppen</skos:prefLabel>
	<skos:prefLabel xml:lang="fr">Écailles de Madulain</skos:prefLabel>
	<skos:prefLabel xml:lang="it">Scaglie di Madulain</skos:prefLabel>
	<skos:altLabel xml:lang="de">Albula Steilzone</skos:altLabel>
	<skos:broader rdf:resource="https://dev-lexic.swissgeol.ch/TectonicUnits/BerninaNappeComplex"/>
	<status xmlns="http://www.w3.org/ns/adms#" rdf:resource="https://dev-lexic.swissgeol.ch/active"/>
</rdf:Description>

<rdf:Description rdf:about="https://dev-lexic.swissgeol.ch/TectonicUnits/Schlattain-Clavadatsch-PadellaSlices">
	<rdf:type rdf:resource="http://www.w3.org/2004/02/skos/core#Concept"/>
	<rdfs:isDefinedBy xml:lang="en">Gouffon Yves (Editor) (2024): Tectonic Map of Switzerland 1:500000, Explanatory notes. Federal Office of Topography swisstopo, Wabern</rdfs:isDefinedBy>
	<skos:definition xml:lang="en">The Schlattain-Clavadatsch-Padella Slices form small isolated klippes, located in the core of the synclinorium of the “Samedan Zone” and composed of Triassic to Late Cretaceous sediments. They were thrust onto the cover of the Err Nappe and therefore attributed to the Bernina Nappe Complex.</skos:definition>
	<skos:inScheme rdf:resource="https://dev-lexic.swissgeol.ch/TectonicUnits"/>
	<skos:prefLabel xml:lang="en">Schlattain-Clavadatsch-Padella Slices</skos:prefLabel>
	<skos:prefLabel xml:lang="de">Schlattain-Clavadatsch-Padella-Schuppen</skos:prefLabel>
	<skos:prefLabel xml:lang="fr">Écailles du Schlattain-Clavadatsch-Padella</skos:prefLabel>
	<skos:prefLabel xml:lang="it">Scaglie dello Schlattain-Clavadatsch-Padella</skos:prefLabel>
	<skos:broader rdf:resource="https://dev-lexic.swissgeol.ch/TectonicUnits/BerninaNappeComplex"/>
	<status xmlns="http://www.w3.org/ns/adms#" rdf:resource="https://dev-lexic.swissgeol.ch/active"/>
</rdf:Description>

<rdf:Description rdf:about="https://dev-lexic.swissgeol.ch/TectonicUnits/JulierNappe">
	<rdf:type rdf:resource="http://www.w3.org/2004/02/skos/core#Concept"/>
	<rdfs:isDefinedBy xml:lang="en">Gouffon Yves (Editor) (2024): Tectonic Map of Switzerland 1:500000, Explanatory notes. Federal Office of Topography swisstopo, Wabern</rdfs:isDefinedBy>
	<skos:definition xml:lang="en">The Julier Nappe represents the equivalent of the Bernina Nappe northwest of the Engadine Fault. This fault sinistrally offsets the two basement-dominated nappes, combined with relative uplift of the Bernina Nappe in respect to the Julier Nappe. The lithological characteristics of the basement are identical to those of the Bernina Nappe. An undisturbed contact between basement and cover of the Julier Nappe is not preserved. Parts of its former cover became detached and form klippes preserved in the core of the multiphase synclinorium of the “Samedan Zone” (Schlattain-Clavadatsch-Padella Slices). In the area of Piz Nair near St. Moritz, however, the base of the Julier Nappe appears to have overthrust its own cover.</skos:definition>
	<skos:inScheme rdf:resource="https://dev-lexic.swissgeol.ch/TectonicUnits"/>
	<skos:prefLabel xml:lang="en">Julier Nappe</skos:prefLabel>
	<skos:prefLabel xml:lang="de">Julier-Decke</skos:prefLabel>
	<skos:prefLabel xml:lang="fr">Nappe du Julier</skos:prefLabel>
	<skos:prefLabel xml:lang="it">Falda del Julier</skos:prefLabel>
	<skos:broader rdf:resource="https://dev-lexic.swissgeol.ch/TectonicUnits/BerninaNappeComplex"/>
	<status xmlns="http://www.w3.org/ns/adms#" rdf:resource="https://dev-lexic.swissgeol.ch/active"/>
</rdf:Description>

<rdf:Description rdf:about="https://dev-lexic.swissgeol.ch/TectonicUnits/MurtiroelSlice">
	<rdf:type rdf:resource="http://www.w3.org/2004/02/skos/core#Concept"/>
	<rdfs:isDefinedBy xml:lang="en">Gouffon Yves (Editor) (2024): Tectonic Map of Switzerland 1:500000, Explanatory notes. Federal Office of Topography swisstopo, Wabern</rdfs:isDefinedBy>
	<skos:definition xml:lang="en">The Murtiröl Slice, consisting of basement and cover, forms a dome-like feature in the footwall of an important extensional detachment. This detachment fault and the adjacent Engadine Fault separate the Murtiröl Slice from all the surrounding units belonging to either the Bernina Nappe Complex (in the northwest and southwest) or to the Upper Austroalpine Languard and Ortler nappes (in the east and northeast).</skos:definition>
	<skos:inScheme rdf:resource="https://dev-lexic.swissgeol.ch/TectonicUnits"/>
	<skos:prefLabel xml:lang="en">Murtiröl Slice</skos:prefLabel>
	<skos:prefLabel xml:lang="de">Murtiröl-Schuppe</skos:prefLabel>
	<skos:prefLabel xml:lang="fr">Écaille du Murtiröl</skos:prefLabel>
	<skos:prefLabel xml:lang="it">Scaglia del Murtiröl</skos:prefLabel>
	<skos:broader rdf:resource="https://dev-lexic.swissgeol.ch/TectonicUnits/ErrNappeComplex"/>
	<status xmlns="http://www.w3.org/ns/adms#" rdf:resource="https://dev-lexic.swissgeol.ch/active"/>
</rdf:Description>

<rdf:Description rdf:about="https://dev-lexic.swissgeol.ch/TectonicUnits/ErrNappe">
	<rdf:type rdf:resource="http://www.w3.org/2004/02/skos/core#Concept"/>
	<rdfs:isDefinedBy xml:lang="en">Gouffon Yves (Editor) (2024): Tectonic Map of Switzerland 1:500000, Explanatory notes. Federal Office of Topography swisstopo, Wabern</rdfs:isDefinedBy>
	<skos:definition xml:lang="en">The Err Nappe is a Lower Austroalpine tectonic unit confined to an area northwest of the Engadine Fault between Albulapass and Julierpass where it overlies the Carungas Slice. Towards the south it is separated from the Julier Nappe (Bernina Nappe Complex) by a multiply deformed synclinorium, the so-called “Samedan Zone”.</skos:definition>
	<skos:inScheme rdf:resource="https://dev-lexic.swissgeol.ch/TectonicUnits"/>
	<skos:prefLabel xml:lang="en">Err Nappe</skos:prefLabel>
	<skos:prefLabel xml:lang="de">Err-Decke</skos:prefLabel>
	<skos:prefLabel xml:lang="fr">Nappe d'Err</skos:prefLabel>
	<skos:prefLabel xml:lang="it">Falda di Err</skos:prefLabel>
	<skos:broader rdf:resource="https://dev-lexic.swissgeol.ch/TectonicUnits/ErrNappeComplex"/>
	<status xmlns="http://www.w3.org/ns/adms#" rdf:resource="https://dev-lexic.swissgeol.ch/active"/>
</rdf:Description>

<rdf:Description rdf:about="https://dev-lexic.swissgeol.ch/TectonicUnits/CarungasSlice">
	<rdf:type rdf:resource="http://www.w3.org/2004/02/skos/core#Concept"/>
	<rdfs:isDefinedBy xml:lang="en">Gouffon Yves (Editor) (2024): Tectonic Map of Switzerland 1:500000, Explanatory notes. Federal Office of Topography swisstopo, Wabern</rdfs:isDefinedBy>
	<skos:definition xml:lang="en">The Lower Austroalpine Carungas Slice, consisting of a band of predominantly overturned Mesozoic sediments and its associated crystalline basement, forms the hangingwall of the Platta Nappe and the footwall of the Err Nappe. This slice extends from east of Savognin all the way to the Julierpass road above Bivio, along the western margin of the Err Nappe (Manatschal &amp; Nievergelt 1997, their “lower Err Nappe”). The small portion of crystalline rock wedged between the two branches of the Engadine Fault near Sils Maria is also related to the Carungas Slice. This slice is derived from the most distal part of the former Adriatic continental margin.</skos:definition>
	<skos:inScheme rdf:resource="https://dev-lexic.swissgeol.ch/TectonicUnits"/>
	<skos:prefLabel xml:lang="en">Carungas Slice</skos:prefLabel>
	<skos:prefLabel xml:lang="de">Carungas-Schuppe</skos:prefLabel>
	<skos:prefLabel xml:lang="fr">Écaille du Carungas</skos:prefLabel>
	<skos:prefLabel xml:lang="it">Scaglia del Carungas</skos:prefLabel>
	<skos:broader rdf:resource="https://dev-lexic.swissgeol.ch/TectonicUnits/ErrNappeComplex"/>
	<status xmlns="http://www.w3.org/ns/adms#" rdf:resource="https://dev-lexic.swissgeol.ch/active"/>
</rdf:Description>

<rdf:Description rdf:about="https://dev-lexic.swissgeol.ch/TectonicUnits/CorvatschSlice">
	<rdf:type rdf:resource="http://www.w3.org/2004/02/skos/core#Concept"/>
	<rdfs:isDefinedBy xml:lang="en">Gouffon Yves (Editor) (2024): Tectonic Map of Switzerland 1:500000, Explanatory notes. Federal Office of Topography swisstopo, Wabern</rdfs:isDefinedBy>
	<skos:definition xml:lang="en">The Corvatsch Slice, located southeast of the Engadine Fault, can be seen as the equivalent of the Err Nappe. It is predominantly made up of intensely deformed pre-Mesozoic basement. Its Mesozoic cover is only rarely preserved just below the overlying Bernina Nappe (e.g., at Fuorcla Surlej).</skos:definition>
	<skos:inScheme rdf:resource="https://dev-lexic.swissgeol.ch/TectonicUnits"/>
	<skos:prefLabel xml:lang="en">Corvatsch Slice</skos:prefLabel>
	<skos:prefLabel xml:lang="de">Corvatsch-Schuppe</skos:prefLabel>
	<skos:prefLabel xml:lang="fr">Écaille du Corvatsch</skos:prefLabel>
	<skos:prefLabel xml:lang="it">Scaglia del Corvatsch</skos:prefLabel>
	<skos:broader rdf:resource="https://dev-lexic.swissgeol.ch/TectonicUnits/ErrNappeComplex"/>
	<status xmlns="http://www.w3.org/ns/adms#" rdf:resource="https://dev-lexic.swissgeol.ch/active"/>
</rdf:Description>

<rdf:Description rdf:about="https://dev-lexic.swissgeol.ch/TectonicUnits/ChasteletsSlice">
	<rdf:type rdf:resource="http://www.w3.org/2004/02/skos/core#Concept"/>
	<rdfs:isDefinedBy xml:lang="en">Gouffon Yves (Editor) (2024): Tectonic Map of Switzerland 1:500000, Explanatory notes. Federal Office of Topography swisstopo, Wabern</rdfs:isDefinedBy>
	<skos:definition xml:lang="en">The Chastelets Slice, located southeast of the Engadine Fault, is a small slice of basement and cover in the footwall of the Corvatsch Slice. It directly overlies the Platta Nappe and hence occupies a similar position to that of the Roccabella Slice northwest of the Engadine Fault.</skos:definition>
	<skos:inScheme rdf:resource="https://dev-lexic.swissgeol.ch/TectonicUnits"/>
	<skos:prefLabel xml:lang="en">Chastelets Slice</skos:prefLabel>
	<skos:prefLabel xml:lang="de">Chastelets-Schuppe</skos:prefLabel>
	<skos:prefLabel xml:lang="fr">Écaille du Chastelets</skos:prefLabel>
	<skos:prefLabel xml:lang="it">Scaglia del Chastelets</skos:prefLabel>
	<skos:broader rdf:resource="https://dev-lexic.swissgeol.ch/TectonicUnits/ErrNappeComplex"/>
	<status xmlns="http://www.w3.org/ns/adms#" rdf:resource="https://dev-lexic.swissgeol.ch/active"/>
</rdf:Description>

<rdf:Description rdf:about="https://dev-lexic.swissgeol.ch/TectonicUnits/Bardella-RoccabellaSlices">
	<rdf:type rdf:resource="http://www.w3.org/2004/02/skos/core#Concept"/>
	<rdfs:isDefinedBy xml:lang="en">Gouffon Yves (Editor) (2024): Tectonic Map of Switzerland 1:500000, Explanatory notes. Federal Office of Topography swisstopo, Wabern</rdfs:isDefinedBy>
	<skos:definition xml:lang="en">The Bardella-Roccabella Slices, located northwest of the Engadine Fault, are part of the Lower Austroalpine Err Nappe Complex. Their sedimentary series are detached from their former crystalline substrate.</skos:definition>
	<skos:inScheme rdf:resource="https://dev-lexic.swissgeol.ch/TectonicUnits"/>
	<skos:prefLabel xml:lang="en">Bardella-Roccabella Slices</skos:prefLabel>
	<skos:prefLabel xml:lang="de">Bardella-Roccabella-Schuppen</skos:prefLabel>
	<skos:prefLabel xml:lang="fr">Écailles de Bardella-Roccabella</skos:prefLabel>
	<skos:prefLabel xml:lang="it">Scaglie di Bardella-Roccabella</skos:prefLabel>
	<skos:broader rdf:resource="https://dev-lexic.swissgeol.ch/TectonicUnits/ErrNappeComplex"/>
	<status xmlns="http://www.w3.org/ns/adms#" rdf:resource="https://dev-lexic.swissgeol.ch/active"/>
</rdf:Description>

<rdf:Description rdf:about="https://dev-lexic.swissgeol.ch/TectonicUnits/MasuccioNappe">
	<rdf:type rdf:resource="http://www.w3.org/2004/02/skos/core#Concept"/>
	<rdfs:isDefinedBy xml:lang="en">Gouffon Yves (Editor) (2024): Tectonic Map of Switzerland 1:500000, Explanatory notes. Federal Office of Topography swisstopo, Wabern</rdfs:isDefinedBy>
	<skos:definition xml:lang="en">The Masuccio Nappe, consisting exclusively of amphibolite-facies Variscan basement, is the lowermost unit of the Campo Nappe Complex. It overthrusts the Bernina Nappe and is located in the footwall of the Late Cretaceous Mortirolo Normal Fault, a transtensional top-E directed extensional fault that became folded around the Pass d’Ur Antiform during Cenozoic folding. In the south, the Masuccio Nappe is in a subvertical orientation and part of the Southern Steep Belt (or root zone) located north of the Tonale Fault, where it is juxtaposed with the structurally much higher Tonale Nappe, located further south and directly adjacent to the Tonale Fault.</skos:definition>
	<skos:inScheme rdf:resource="https://dev-lexic.swissgeol.ch/TectonicUnits"/>
	<skos:prefLabel xml:lang="en">Masuccio Nappe</skos:prefLabel>
	<skos:prefLabel xml:lang="de">Masuccio-Decke</skos:prefLabel>
	<skos:prefLabel xml:lang="fr">Nappe du Masuccio</skos:prefLabel>
	<skos:prefLabel xml:lang="it">Falda del Masuccio</skos:prefLabel>
	<skos:broader rdf:resource="https://dev-lexic.swissgeol.ch/TectonicUnits/CampoNappeComplex"/>
	<status xmlns="http://www.w3.org/ns/adms#" rdf:resource="https://dev-lexic.swissgeol.ch/active"/>
</rdf:Description>

<rdf:Description rdf:about="https://dev-lexic.swissgeol.ch/TectonicUnits/CampoNappe">
	<rdf:type rdf:resource="http://www.w3.org/2004/02/skos/core#Concept"/>
	<rdfs:isDefinedBy xml:lang="en">Gouffon Yves (Editor) (2024): Tectonic Map of Switzerland 1:500000, Explanatory notes. Federal Office of Topography swisstopo, Wabern</rdfs:isDefinedBy>
	<skos:definition xml:lang="en">The Campo Nappe is the largest unit of the Upper Austroalpine Campo Nappe Complex and predominantly consists of Variscan basement, locally intruded by Permian magmatites (e.g., Sondalo Gabbro, Martell Granite). This nappe tectonically overlies the Masuccio Nappe in the southwest and the Languard Nappe in the northeast and extends all along the base of the tectonically higher Ortler Nappe. Its former Permian–Mesozoic cover has been almost completely detached very early during WNW-directed Late Cretaceous thrusting and is not present nowadays due to erosion, except as small occurrences more or less attached to the basement of the Campo Nappe.</skos:definition>
	<skos:inScheme rdf:resource="https://dev-lexic.swissgeol.ch/TectonicUnits"/>
	<skos:prefLabel xml:lang="en">Campo Nappe</skos:prefLabel>
	<skos:prefLabel xml:lang="de">Campo-Decke</skos:prefLabel>
	<skos:prefLabel xml:lang="fr">Nappe de Campo</skos:prefLabel>
	<skos:prefLabel xml:lang="it">Falda di Campo</skos:prefLabel>
	<skos:broader rdf:resource="https://dev-lexic.swissgeol.ch/TectonicUnits/CampoNappeComplex"/>
	<status xmlns="http://www.w3.org/ns/adms#" rdf:resource="https://dev-lexic.swissgeol.ch/active"/>
</rdf:Description>

<rdf:Description rdf:about="https://dev-lexic.swissgeol.ch/TectonicUnits/GrosinaNappe">
	<rdf:type rdf:resource="http://www.w3.org/2004/02/skos/core#Concept"/>
	<rdfs:isDefinedBy xml:lang="en">Gouffon Yves (Editor) (2024): Tectonic Map of Switzerland 1:500000, Explanatory notes. Federal Office of Topography swisstopo, Wabern</rdfs:isDefinedBy>
	<skos:definition xml:lang="en">The Grosina Nappe forms a series of tectonic klippes on the southwestern parts of the Campo Nappe along a distinct mylonitic zone associated with top-NW to top-N senses of shear of Cretaceous age that possibly reworked a Jurassic décollement zone. The amphibolite-facies Variscan basement of the Grosina Nappe is in parts similar to that of the underlying Campo Nappe. However, the basement of the Grosina Nappe differs in that orthogneisses are much more frequent, and, additionally, in that there is often a pervasive greenschist-facies metamorphic overprint of the older high-grade fabrics. The root zone of the Grosina Nappe most probably occurs at the southern margin of the Campo Nappe Complex and in the immediate footwall of the tectonically higher Tonale Nappe.</skos:definition>
	<skos:inScheme rdf:resource="https://dev-lexic.swissgeol.ch/TectonicUnits"/>
	<skos:prefLabel xml:lang="en">Grosina Nappe</skos:prefLabel>
	<skos:prefLabel xml:lang="de">Grosina-Decke</skos:prefLabel>
	<skos:prefLabel xml:lang="fr">Nappe de la Grosina</skos:prefLabel>
	<skos:prefLabel xml:lang="it">Falda della Grosina</skos:prefLabel>
	<skos:broader rdf:resource="https://dev-lexic.swissgeol.ch/TectonicUnits/CampoNappeComplex"/>
	<status xmlns="http://www.w3.org/ns/adms#" rdf:resource="https://dev-lexic.swissgeol.ch/active"/>
</rdf:Description>

<rdf:Description rdf:about="https://dev-lexic.swissgeol.ch/TectonicUnits/LaasNappe">
	<rdf:type rdf:resource="http://www.w3.org/2004/02/skos/core#Concept"/>
	<rdfs:isDefinedBy xml:lang="en">Gouffon Yves (Editor) (2024): Tectonic Map of Switzerland 1:500000, Explanatory notes. Federal Office of Topography swisstopo, Wabern</rdfs:isDefinedBy>
	<skos:definition xml:lang="en">The Laas Nappe exposes a series of often subvertically northward inclined garnet and staurolite bearing paragneisses, marbles and amphibolites metamorphosed under amphibolite-facies conditions during the Variscan orogeny. Cretaceous metamorphic overprint varies from greenschist facies in the west to lower amphibolite facies in the east. This nappe occupies a much-debated and still unclear position in the Upper Austroalpine nappe pile.</skos:definition>
	<skos:inScheme rdf:resource="https://dev-lexic.swissgeol.ch/TectonicUnits"/>
	<skos:prefLabel xml:lang="en">Laas Nappe</skos:prefLabel>
	<skos:prefLabel xml:lang="de">Laas-Decke</skos:prefLabel>
	<skos:prefLabel xml:lang="fr">Nappe de Laas</skos:prefLabel>
	<skos:prefLabel xml:lang="it">Falda di Laas</skos:prefLabel>
	<skos:broader rdf:resource="https://dev-lexic.swissgeol.ch/TectonicUnits/CampoNappeComplex"/>
	<status xmlns="http://www.w3.org/ns/adms#" rdf:resource="https://dev-lexic.swissgeol.ch/active"/>
</rdf:Description>

<rdf:Description rdf:about="https://dev-lexic.swissgeol.ch/TectonicUnits/VinschgauShearZone">
	<rdf:type rdf:resource="http://www.w3.org/2004/02/skos/core#Concept"/>
	<rdfs:isDefinedBy xml:lang="en">Gouffon Yves (Editor) (2024): Tectonic Map of Switzerland 1:500000, Explanatory notes. Federal Office of Topography swisstopo, Wabern</rdfs:isDefinedBy>
	<skos:definition xml:lang="en">The Vinschgau Shear Zone represents the structurally highest unit of the Campo Nappe Complex and constitutes a greenschist-facies Alpine mylonitic belt with a thickness of up to 2–3 km that accommodates W-directed thrusting of the Ötztal Nappe Complex in the area north of the Vinschgau Valley floor. South of the valley floor and in the lowermost Val Müstair, the same mylonitic belt accommodates WNW-directed thrusting of the easternmost part of the Umbrail-Terza Slice Complex over the S-charl-Sesvenna Nappe.</skos:definition>
	<skos:inScheme rdf:resource="https://dev-lexic.swissgeol.ch/TectonicUnits"/>
	<skos:prefLabel xml:lang="en">Vinschgau Shear Zone</skos:prefLabel>
	<skos:prefLabel xml:lang="de">Vinschgau-Scherzone</skos:prefLabel>
	<skos:prefLabel xml:lang="fr">Zone de cisaillement du Vinschgau</skos:prefLabel>
	<skos:prefLabel xml:lang="it">Zona di taglio del Vinschgau</skos:prefLabel>
	<skos:broader rdf:resource="https://dev-lexic.swissgeol.ch/TectonicUnits/CampoNappeComplex"/>
	<status xmlns="http://www.w3.org/ns/adms#" rdf:resource="https://dev-lexic.swissgeol.ch/active"/>
</rdf:Description>

<rdf:Description rdf:about="https://dev-lexic.swissgeol.ch/TectonicUnits/UltenUnit">
	<rdf:type rdf:resource="http://www.w3.org/2004/02/skos/core#Concept"/>
	<rdfs:isDefinedBy xml:lang="en">Gouffon Yves (Editor) (2024): Tectonic Map of Switzerland 1:500000, Explanatory notes. Federal Office of Topography swisstopo, Wabern</rdfs:isDefinedBy>
	<skos:definition xml:lang="en">East of Val di Peio (Mezzana region), the Ulten Unit overlies the Tonale Gneiss Complex along a pre-Alpine tectonic contact. It is characterized by kyanite-bearing paragneisses and migmatites, containing boudins of amphibolitized eclogites, metagabbros and peridotites. Its metamorphic history (high-pressure event of unknown age, exhumation to a lower crustal depth between Devonian and Carboniferous times, slow cooling during Permian to Jurassic times), as well as its original location in the lower crust within the Variscan orogen, are reminiscent of the Ivrea Zone located south of the Tonale Fault.</skos:definition>
	<skos:inScheme rdf:resource="https://dev-lexic.swissgeol.ch/TectonicUnits"/>
	<skos:prefLabel xml:lang="en">Ulten Unit</skos:prefLabel>
	<skos:prefLabel xml:lang="de">Ulten-Einheit</skos:prefLabel>
	<skos:prefLabel xml:lang="fr">Unité d'Ulten</skos:prefLabel>
	<skos:prefLabel xml:lang="it">Unità di Ulten</skos:prefLabel>
	<skos:broader rdf:resource="https://dev-lexic.swissgeol.ch/TectonicUnits/TonaleNappe"/>
	<status xmlns="http://www.w3.org/ns/adms#" rdf:resource="https://dev-lexic.swissgeol.ch/active"/>
</rdf:Description>

<rdf:Description rdf:about="https://dev-lexic.swissgeol.ch/TectonicUnits/MadrisaSlice">
	<rdf:type rdf:resource="http://www.w3.org/2004/02/skos/core#Concept"/>
	<rdfs:isDefinedBy xml:lang="en">Gouffon Yves (Editor) (2024): Tectonic Map of Switzerland 1:500000, Explanatory notes. Federal Office of Topography swisstopo, Wabern</rdfs:isDefinedBy>
	<skos:definition xml:lang="en">The Madrisa Slice, which is isolated north of Klosters between the Silvretta Nappe above and the Upper Penninic Arosa Zone below, is considered to be an inverted sliver derived from the Lechtal Nappe.</skos:definition>
	<skos:inScheme rdf:resource="https://dev-lexic.swissgeol.ch/TectonicUnits"/>
	<skos:prefLabel xml:lang="en">Madrisa Slice</skos:prefLabel>
	<skos:prefLabel xml:lang="de">Madrisa-Schuppe</skos:prefLabel>
	<skos:prefLabel xml:lang="fr">Écaille de Madrisa</skos:prefLabel>
	<skos:prefLabel xml:lang="it">Scaglia di Madrisa</skos:prefLabel>
	<skos:broader rdf:resource="https://dev-lexic.swissgeol.ch/TectonicUnits/LechtalNappe"/>
	<status xmlns="http://www.w3.org/ns/adms#" rdf:resource="https://dev-lexic.swissgeol.ch/active"/>
</rdf:Description>

<rdf:Description rdf:about="https://dev-lexic.swissgeol.ch/TectonicUnits/SchesaplanaSlice">
	<rdf:type rdf:resource="http://www.w3.org/2004/02/skos/core#Concept"/>
	<rdfs:isDefinedBy xml:lang="en">Gouffon Yves (Editor) (2024): Tectonic Map of Switzerland 1:500000, Explanatory notes. Federal Office of Topography swisstopo, Wabern</rdfs:isDefinedBy>
	<skos:definition xml:lang="en">The Schesaplana Slice is a tectonic subunit of the Lechtal Nappe at its southwestern border.</skos:definition>
	<skos:inScheme rdf:resource="https://dev-lexic.swissgeol.ch/TectonicUnits"/>
	<skos:prefLabel xml:lang="en">Schesaplana Slice</skos:prefLabel>
	<skos:prefLabel xml:lang="de">Schesaplana-Schuppe</skos:prefLabel>
	<skos:prefLabel xml:lang="fr">Écaille de Schesaplana</skos:prefLabel>
	<skos:prefLabel xml:lang="it">Scaglia di Schesaplana</skos:prefLabel>
	<skos:broader rdf:resource="https://dev-lexic.swissgeol.ch/TectonicUnits/LechtalNappe"/>
	<status xmlns="http://www.w3.org/ns/adms#" rdf:resource="https://dev-lexic.swissgeol.ch/active"/>
</rdf:Description>

<rdf:Description rdf:about="https://dev-lexic.swissgeol.ch/TectonicUnits/GorvionSlice">
	<rdf:type rdf:resource="http://www.w3.org/2004/02/skos/core#Concept"/>
	<rdfs:isDefinedBy xml:lang="en">Gouffon Yves (Editor) (2024): Tectonic Map of Switzerland 1:500000, Explanatory notes. Federal Office of Topography swisstopo, Wabern</rdfs:isDefinedBy>
	<skos:definition xml:lang="en">The Gorvion Slice is a tectonic subunit of the Lechtal Nappe at its southwestern border.</skos:definition>
	<skos:inScheme rdf:resource="https://dev-lexic.swissgeol.ch/TectonicUnits"/>
	<skos:prefLabel xml:lang="en">Gorvion Slice</skos:prefLabel>
	<skos:prefLabel xml:lang="de">Gorvion-Schuppe</skos:prefLabel>
	<skos:prefLabel xml:lang="fr">Écaille du Gorvion</skos:prefLabel>
	<skos:prefLabel xml:lang="it">Scaglia del Gorvion</skos:prefLabel>
	<skos:broader rdf:resource="https://dev-lexic.swissgeol.ch/TectonicUnits/LechtalNappe"/>
	<status xmlns="http://www.w3.org/ns/adms#" rdf:resource="https://dev-lexic.swissgeol.ch/active"/>
</rdf:Description>

<rdf:Description rdf:about="https://dev-lexic.swissgeol.ch/TectonicUnits/AugstenbergSlice">
	<rdf:type rdf:resource="http://www.w3.org/2004/02/skos/core#Concept"/>
	<rdfs:isDefinedBy xml:lang="en">Gouffon Yves (Editor) (2024): Tectonic Map of Switzerland 1:500000, Explanatory notes. Federal Office of Topography swisstopo, Wabern</rdfs:isDefinedBy>
	<skos:definition xml:lang="en">The Augstenberg Slice is a tectonic subunit of the Lechtal Nappe at its southwestern border.</skos:definition>
	<skos:inScheme rdf:resource="https://dev-lexic.swissgeol.ch/TectonicUnits"/>
	<skos:prefLabel xml:lang="en">Augstenberg Slice</skos:prefLabel>
	<skos:prefLabel xml:lang="de">Augstenberg-Schuppe</skos:prefLabel>
	<skos:prefLabel xml:lang="fr">Écaille de l'Augstenberg</skos:prefLabel>
	<skos:prefLabel xml:lang="it">Scaglia dell'Augstenberg</skos:prefLabel>
	<skos:broader rdf:resource="https://dev-lexic.swissgeol.ch/TectonicUnits/LechtalNappe"/>
	<status xmlns="http://www.w3.org/ns/adms#" rdf:resource="https://dev-lexic.swissgeol.ch/active"/>
</rdf:Description>

<rdf:Description rdf:about="https://dev-lexic.swissgeol.ch/TectonicUnits/OchsenkopfSlice">
	<rdf:type rdf:resource="http://www.w3.org/2004/02/skos/core#Concept"/>
	<rdfs:isDefinedBy xml:lang="en">Gouffon Yves (Editor) (2024): Tectonic Map of Switzerland 1:500000, Explanatory notes. Federal Office of Topography swisstopo, Wabern</rdfs:isDefinedBy>
	<skos:definition xml:lang="en">The Ochsenkopf Slice is a tectonic subunit of the western part of the Lechtal Nappe.</skos:definition>
	<skos:inScheme rdf:resource="https://dev-lexic.swissgeol.ch/TectonicUnits"/>
	<skos:prefLabel xml:lang="en">Ochsenkopf Slice</skos:prefLabel>
	<skos:prefLabel xml:lang="de">Ochsenkopf-Schuppe</skos:prefLabel>
	<skos:prefLabel xml:lang="fr">Écaille de l'Ochsenkopf</skos:prefLabel>
	<skos:prefLabel xml:lang="it">Scaglia dell'Ochsenkopf</skos:prefLabel>
	<skos:broader rdf:resource="https://dev-lexic.swissgeol.ch/TectonicUnits/LechtalNappe"/>
	<status xmlns="http://www.w3.org/ns/adms#" rdf:resource="https://dev-lexic.swissgeol.ch/active"/>
</rdf:Description>

<rdf:Description rdf:about="https://dev-lexic.swissgeol.ch/TectonicUnits/HeubuehlSlice">
	<rdf:type rdf:resource="http://www.w3.org/2004/02/skos/core#Concept"/>
	<rdfs:isDefinedBy xml:lang="en">Gouffon Yves (Editor) (2024): Tectonic Map of Switzerland 1:500000, Explanatory notes. Federal Office of Topography swisstopo, Wabern</rdfs:isDefinedBy>
	<skos:definition xml:lang="en">The Heubühl Slice is a tectonic subunit of the Lechtal Nappe at its southwestern border. It has an exclusively Triassic stratigraphic sequence ranging from «Alpiner Buntsandstein» (Chazforà-/Fuorn-Fm.) up to «Hauptdolomit».</skos:definition>
	<skos:inScheme rdf:resource="https://dev-lexic.swissgeol.ch/TectonicUnits"/>
	<skos:prefLabel xml:lang="en">Heubühl Slice</skos:prefLabel>
	<skos:prefLabel xml:lang="de">Heubühl-Schuppe</skos:prefLabel>
	<skos:prefLabel xml:lang="fr">Écaille du Heubühl</skos:prefLabel>
	<skos:prefLabel xml:lang="it">Scaglia del Heubühl</skos:prefLabel>
	<skos:broader rdf:resource="https://dev-lexic.swissgeol.ch/TectonicUnits/LechtalNappe"/>
	<status xmlns="http://www.w3.org/ns/adms#" rdf:resource="https://dev-lexic.swissgeol.ch/active"/>
</rdf:Description>

<rdf:Description rdf:about="https://dev-lexic.swissgeol.ch/TectonicUnits/DreiSchwesternSlice">
	<rdf:type rdf:resource="http://www.w3.org/2004/02/skos/core#Concept"/>
	<rdfs:isDefinedBy xml:lang="en">Gouffon Yves (Editor) (2024): Tectonic Map of Switzerland 1:500000, Explanatory notes. Federal Office of Topography swisstopo, Wabern</rdfs:isDefinedBy>
	<skos:definition xml:lang="en">The Drei Schwestern Slice is a tectonic subunit of the Lechtal Nappe at its northwestern border. It has an exclusively Triassic stratigraphic sequence ranging from «Alpiner Buntsandstein» (Chazforà-/Fuorn-Fm.) up to «Hauptdolomit».</skos:definition>
	<skos:inScheme rdf:resource="https://dev-lexic.swissgeol.ch/TectonicUnits"/>
	<skos:prefLabel xml:lang="en">Drei Schwestern Slice</skos:prefLabel>
	<skos:prefLabel xml:lang="de">Drei-Schwestern-Schuppe</skos:prefLabel>
	<skos:prefLabel xml:lang="fr">Écaille des Drei Schwestern</skos:prefLabel>
	<skos:prefLabel xml:lang="it">Scaglia delle Drei Schwestern</skos:prefLabel>
	<skos:broader rdf:resource="https://dev-lexic.swissgeol.ch/TectonicUnits/LechtalNappe"/>
	<status xmlns="http://www.w3.org/ns/adms#" rdf:resource="https://dev-lexic.swissgeol.ch/active"/>
</rdf:Description>

<rdf:Description rdf:about="https://dev-lexic.swissgeol.ch/TectonicUnits/Phyllitgneiszone">
	<rdf:type rdf:resource="http://www.w3.org/2004/02/skos/core#Concept"/>
	<rdfs:isDefinedBy xml:lang="en">Gouffon Yves (Editor) (2024): Tectonic Map of Switzerland 1:500000, Explanatory notes. Federal Office of Topography swisstopo, Wabern</rdfs:isDefinedBy>
	<skos:definition xml:lang="en">The “Phyllitgneiszone” is a narrow belt of low-grade basement representing the northern, strongly retrogressed and phyllonitic part of the Silvretta Nappe.</skos:definition>
	<skos:inScheme rdf:resource="https://dev-lexic.swissgeol.ch/TectonicUnits"/>
	<skos:prefLabel xml:lang="en">Phyllitgneiszone</skos:prefLabel>
	<skos:prefLabel xml:lang="de">Phyllitgneiszone</skos:prefLabel>
	<skos:prefLabel xml:lang="fr">Phyllitgneiszone</skos:prefLabel>
	<skos:prefLabel xml:lang="it">Phyllitgneiszone</skos:prefLabel>
	<skos:broader rdf:resource="https://dev-lexic.swissgeol.ch/TectonicUnits/SilvrettaNappe"/>
	<status xmlns="http://www.w3.org/ns/adms#" rdf:resource="https://dev-lexic.swissgeol.ch/active"/>
</rdf:Description>

<rdf:Description rdf:about="https://dev-lexic.swissgeol.ch/TectonicUnits/S-ChanfSlices">
	<rdf:type rdf:resource="http://www.w3.org/2004/02/skos/core#Concept"/>
	<rdfs:isDefinedBy xml:lang="en">Gouffon Yves (Editor) (2024): Tectonic Map of Switzerland 1:500000, Explanatory notes. Federal Office of Topography swisstopo, Wabern</rdfs:isDefinedBy>
	<skos:inScheme rdf:resource="https://dev-lexic.swissgeol.ch/TectonicUnits"/>
	<skos:prefLabel xml:lang="en">S-chanf Slices</skos:prefLabel>
	<skos:prefLabel xml:lang="de">S-chanf-Schuppen</skos:prefLabel>
	<skos:prefLabel xml:lang="fr">Écailles de S-chanf</skos:prefLabel>
	<skos:prefLabel xml:lang="it">Scaglie di S-chanf</skos:prefLabel>
	<skos:broader rdf:resource="https://dev-lexic.swissgeol.ch/TectonicUnits/SilvrettaNappe"/>
	<status xmlns="http://www.w3.org/ns/adms#" rdf:resource="https://dev-lexic.swissgeol.ch/active"/>
</rdf:Description>

<rdf:Description rdf:about="https://dev-lexic.swissgeol.ch/TectonicUnits/MatschNappe">
	<rdf:type rdf:resource="http://www.w3.org/2004/02/skos/core#Concept"/>
	<rdfs:isDefinedBy xml:lang="en">Gouffon Yves (Editor) (2024): Tectonic Map of Switzerland 1:500000, Explanatory notes. Federal Office of Topography swisstopo, Wabern</rdfs:isDefinedBy>
	<skos:definition xml:lang="en">The Matsch Nappe differs from the underlying Ötztal Nappe in that it is built up of a characteristic polymetamorphic (Variscan, Permian and Alpine) association of interlayered metapelites, amphibolites and pegmatites. Manifestations of Permian metamorphism, associated with the intrusion of pegmatites, are absent in the Ötztal Nappe, and hence thrusting of the Matsch Nappe over the Ötztal Nappe must be of early Alpine age, predating emplacement and metamorphism within the Ötztal Nappe Complex at around 90 Ma.</skos:definition>
	<skos:inScheme rdf:resource="https://dev-lexic.swissgeol.ch/TectonicUnits"/>
	<skos:prefLabel xml:lang="en">Matsch Nappe</skos:prefLabel>
	<skos:prefLabel xml:lang="de">Matsch-Decke</skos:prefLabel>
	<skos:prefLabel xml:lang="fr">Nappe de Matsch</skos:prefLabel>
	<skos:prefLabel xml:lang="it">Falda di Matsch</skos:prefLabel>
	<skos:broader rdf:resource="https://dev-lexic.swissgeol.ch/TectonicUnits/OetztalNappeComplex"/>
	<status xmlns="http://www.w3.org/ns/adms#" rdf:resource="https://dev-lexic.swissgeol.ch/active"/>
</rdf:Description>

<rdf:Description rdf:about="https://dev-lexic.swissgeol.ch/TectonicUnits/Umbrail-ChavalatschSlices">
	<rdf:type rdf:resource="http://www.w3.org/2004/02/skos/core#Concept"/>
	<rdfs:isDefinedBy xml:lang="en">Gouffon Yves (Editor) (2024): Tectonic Map of Switzerland 1:500000, Explanatory notes. Federal Office of Topography swisstopo, Wabern</rdfs:isDefinedBy>
	<skos:definition xml:lang="en">The WNW-facing Umbrail-Chavalatsch Slices consist of a very complicated zone of imbrication with two lithologically and tectonically separate units: firstly, slices of Late Triassic sediments of the Raibl and Hauptdolomit groups, which were sheared off their original stratigraphical underpinnings (S-charl-Sesvenna Nappe), and secondly, pre-Mesozoic basement slices that are correlated with the tectonically higher basement of the Ötztal Nappe Complex that tectonically overlies the S-charl-Sesvenna nappe.</skos:definition>
	<skos:inScheme rdf:resource="https://dev-lexic.swissgeol.ch/TectonicUnits"/>
	<skos:prefLabel xml:lang="en">Umbrail-Chavalatsch Slices</skos:prefLabel>
	<skos:prefLabel xml:lang="de">Umbrail-Chavalatsch-Schuppen</skos:prefLabel>
	<skos:prefLabel xml:lang="fr">Écailles de l'Umbrail-Chavalatsch</skos:prefLabel>
	<skos:prefLabel xml:lang="it">Scaglie dell'Umbrail-Chavalatsch</skos:prefLabel>
	<skos:broader rdf:resource="https://dev-lexic.swissgeol.ch/TectonicUnits/Umbrail-TerzaSliceComplex"/>
	<status xmlns="http://www.w3.org/ns/adms#" rdf:resource="https://dev-lexic.swissgeol.ch/active"/>
</rdf:Description>

<rdf:Description rdf:about="https://dev-lexic.swissgeol.ch/TectonicUnits/TerzaSlice">
	<rdf:type rdf:resource="http://www.w3.org/2004/02/skos/core#Concept"/>
	<rdfs:isDefinedBy xml:lang="en">Gouffon Yves (Editor) (2024): Tectonic Map of Switzerland 1:500000, Explanatory notes. Federal Office of Topography swisstopo, Wabern</rdfs:isDefinedBy>
	<skos:definition xml:lang="en">The Terza Slice is a klippe of the Umbrail-Terza Slice Complex overlying the westernmost part of the Quattervals Nappe. It comprises Norian to Rhaetian sediments detached from the incompetent Raibl Group. </skos:definition>
	<skos:inScheme rdf:resource="https://dev-lexic.swissgeol.ch/TectonicUnits"/>
	<skos:prefLabel xml:lang="en">Terza Slice</skos:prefLabel>
	<skos:prefLabel xml:lang="de">Terza-Schuppe</skos:prefLabel>
	<skos:prefLabel xml:lang="fr">Écaille de Terza</skos:prefLabel>
	<skos:prefLabel xml:lang="it">Scaglia di Terza</skos:prefLabel>
	<skos:broader rdf:resource="https://dev-lexic.swissgeol.ch/TectonicUnits/Umbrail-TerzaSliceComplex"/>
	<status xmlns="http://www.w3.org/ns/adms#" rdf:resource="https://dev-lexic.swissgeol.ch/active"/>
</rdf:Description>

<rdf:Description rdf:about="https://dev-lexic.swissgeol.ch/TectonicUnits/TavrueSlice">
	<rdf:type rdf:resource="http://www.w3.org/2004/02/skos/core#Concept"/>
	<rdfs:isDefinedBy xml:lang="en">Gouffon Yves (Editor) (2024): Tectonic Map of Switzerland 1:500000, Explanatory notes. Federal Office of Topography swisstopo, Wabern</rdfs:isDefinedBy>
	<skos:definition xml:lang="en">Within the S-charl-Sesvenna Nappe, the Tavrü Slice (formerly known as “S-charl-Oberbau”) consists entirely of a Norian to Cretaceous succession, volumetrically dominated by an over 2 km thick Hauptdolomit. It is completely detached from the Carnian Raibl Group. This slice, separated from the tectonically higher Ötztal Nappe by the Schlinig Thrust, suffered substantial internal extension in a domino-style.</skos:definition>
	<skos:inScheme rdf:resource="https://dev-lexic.swissgeol.ch/TectonicUnits"/>
	<skos:prefLabel xml:lang="en">Tavrü Slice</skos:prefLabel>
	<skos:prefLabel xml:lang="de">Tavrü-Schuppe</skos:prefLabel>
	<skos:prefLabel xml:lang="fr">Écaille du Tavrü</skos:prefLabel>
	<skos:prefLabel xml:lang="it">Scaglia del Tavrü</skos:prefLabel>
	<skos:broader rdf:resource="https://dev-lexic.swissgeol.ch/TectonicUnits/S-Charl-SesvennaNappe"/>
	<status xmlns="http://www.w3.org/ns/adms#" rdf:resource="https://dev-lexic.swissgeol.ch/active"/>
</rdf:Description>

<rdf:Description rdf:about="https://dev-lexic.swissgeol.ch/TectonicUnits/SouthAlpine">
	<rdf:type rdf:resource="http://www.w3.org/2004/02/skos/core#Concept"/>
	<rdfs:isDefinedBy xml:lang="en">Gouffon Yves (Editor) (2024): Tectonic Map of Switzerland 1:500000, Explanatory notes. Federal Office of Topography swisstopo, Wabern</rdfs:isDefinedBy>
	<rdfs:comment rdf:datatype="http://www.w3.org/1999/02/22-rdf-syntax-ns#HTML">https://data.geo.admin.ch/ch.swisstopo.geologie-tektonische_karte/pdf/Erl-TK500_2024.pdf</rdfs:comment>
	<rdfs:comment rdf:datatype="http://www.w3.org/1999/02/22-rdf-syntax-ns#HTML">https://www.strati.ch/en/tectonic/sudalpino</rdfs:comment>
	<skos:definition xml:lang="en">The South Alpine tectonic domain exposes a complete section of the Adriatic continental crust from ultramafic (slices of uppermost continental mantle lithosphere), mafic and felsic granulite-facies rocks (lower continental crust: Ivrea Zone) through medium- and low-grade basement rocks (middle–upper continental crust: Strona-Ceneri and Val Colla zones, basement of the Orobic units) to unconformably overlying non-metamorphic Late Carboniferous sediments that were involved in post-Variscan folding.
The detached Variscan continental crust and its overlying Permian to Miocene sedimentary cover form a fold-and-thrust belt, the southern S-vergent back-chain of the Alps, separated from the other domains of the Western and Central Alps to the west by the Canavese Fault and to the north by the Tonale Fault. Both faults are part of an Oligocene–Miocene post-collisional system of transpressive transfer faults along the northwestern boundary of the Adriatic indenter.</skos:definition>
	<skos:inScheme rdf:resource="https://dev-lexic.swissgeol.ch/TectonicUnits"/>
	<skos:topConceptOf rdf:resource="https://dev-lexic.swissgeol.ch/TectonicUnits"/>
	<skos:prefLabel xml:lang="en">South Alpine</skos:prefLabel>
	<skos:prefLabel xml:lang="de">Südalpin</skos:prefLabel>
	<skos:prefLabel xml:lang="fr">Sudalpin</skos:prefLabel>
	<skos:prefLabel xml:lang="it">Sudalpino</skos:prefLabel>
	<skos:narrower rdf:resource="https://dev-lexic.swissgeol.ch/TectonicUnits/CanaveseZone"/>
	<skos:narrower rdf:resource="https://dev-lexic.swissgeol.ch/TectonicUnits/Ivrea-CeneriComplex"/>
	<skos:narrower rdf:resource="https://dev-lexic.swissgeol.ch/TectonicUnits/MilanBelt"/>
	<skos:narrower rdf:resource="https://dev-lexic.swissgeol.ch/TectonicUnits/LowerOrobicImbricates"/>
	<skos:narrower rdf:resource="https://dev-lexic.swissgeol.ch/TectonicUnits/UpperOrobicNappe"/>
	<skos:narrower rdf:resource="https://dev-lexic.swissgeol.ch/TectonicUnits/VaresottoImbricates"/>
	<skos:narrower rdf:resource="https://dev-lexic.swissgeol.ch/TectonicUnits/Strona-Ceneri-Zone"/>
	<status xmlns="http://www.w3.org/ns/adms#" rdf:resource="https://dev-lexic.swissgeol.ch/active"/>
</rdf:Description>

<rdf:Description rdf:about="https://dev-lexic.swissgeol.ch/TectonicUnits/CanaveseZone">
	<rdf:type rdf:resource="http://www.w3.org/2004/02/skos/core#Concept"/>
	<rdfs:isDefinedBy xml:lang="en">Gouffon Yves (Editor) (2024): Tectonic Map of Switzerland 1:500000, Explanatory notes. Federal Office of Topography swisstopo, Wabern</rdfs:isDefinedBy>
	<skos:definition xml:lang="en">The intensely mylonitized Canavese Zone consists of individual slivers of basement and Mesozoic sedimentary cover rocks trapped along the Internal and the External Canavese faults between the Ivrea-Ceneri Complex in the southeast and the Sesia Nappe in the northwest, dismembered by Alpine shear zones and brittle faults. It extends from the area west of Ivrea to Locarno where it is truncated by a fault that links the Centovalli Fault to the Tonale Fault. It includes migmatitic and leucogranitic basement rocks with inclusions of mafic granulites similar to those of the Ivrea Zone, and amphibolite-facies basement rocks with granitic intrusions similar to those of the Strona-Ceneri Zone. The Mesozoic sedimentary cover can be compared to that of the Lower Austroalpine Err Nappe Complex in Graubünden and is interpreted as part of the distal Adriatic margin.</skos:definition>
	<skos:inScheme rdf:resource="https://dev-lexic.swissgeol.ch/TectonicUnits"/>
	<skos:prefLabel xml:lang="en">Canavese Zone</skos:prefLabel>
	<skos:prefLabel xml:lang="de">Canavese-Zone</skos:prefLabel>
	<skos:prefLabel xml:lang="fr">Zone du Canavese</skos:prefLabel>
	<skos:prefLabel xml:lang="it">Zona del Canavese</skos:prefLabel>
	<skos:broader rdf:resource="https://dev-lexic.swissgeol.ch/TectonicUnits/SouthAlpine"/>
	<status xmlns="http://www.w3.org/ns/adms#" rdf:resource="https://dev-lexic.swissgeol.ch/active"/>
</rdf:Description>

<rdf:Description rdf:about="https://dev-lexic.swissgeol.ch/TectonicUnits/Ivrea-CeneriComplex">
	<rdf:type rdf:resource="http://www.w3.org/2004/02/skos/core#Concept"/>
	<rdfs:isDefinedBy xml:lang="en">Gouffon Yves (Editor) (2024): Tectonic Map of Switzerland 1:500000, Explanatory notes. Federal Office of Topography swisstopo, Wabern</rdfs:isDefinedBy>
	<skos:definition xml:lang="en">The Ivrea-Ceneri Complex is a thick-skinned tectonic unit developped during the Alpine orogeny. It includes the lower crustal rocks of the Ivrea Zone and the WNW part of the middle to upper crustal Strona-Ceneri Zone. In the northwest, the Ivrea-Ceneri Complex is separated from the Canavese Zone by the Internal Canavese Fault, east of Locarno from the Central Alps by the Tonale Fault. In the east and southeast, the transition to the Upper Orobic Nappe is not clearly defined. The boundary can be traced along the Tamaro Thrust and the Lago Maggiore Fault. In the south, west of Lago Maggiore, the Ivrea-Ceneri Complex with its Mesozoic cover is overlain by the post-orogenic deposits of the Po Plain.</skos:definition>
	<skos:inScheme rdf:resource="https://dev-lexic.swissgeol.ch/TectonicUnits"/>
	<skos:prefLabel xml:lang="en">Ivrea-Ceneri Complex</skos:prefLabel>
	<skos:prefLabel xml:lang="de">Ivrea-Ceneri-Komplex</skos:prefLabel>
	<skos:prefLabel xml:lang="fr">Complexe d'Ivrea-Ceneri</skos:prefLabel>
	<skos:prefLabel xml:lang="it">Complesso di Ivrea-Ceneri</skos:prefLabel>
	<skos:broader rdf:resource="https://dev-lexic.swissgeol.ch/TectonicUnits/SouthAlpine"/>
	<skos:narrower rdf:resource="https://dev-lexic.swissgeol.ch/TectonicUnits/IvreaZone"/>
	<skos:narrower rdf:resource="https://dev-lexic.swissgeol.ch/TectonicUnits/Strona-Ceneri-Zone_PartIvrea-Ceneri"/>
	<status xmlns="http://www.w3.org/ns/adms#" rdf:resource="https://dev-lexic.swissgeol.ch/active"/>
</rdf:Description>

<rdf:Description rdf:about="https://dev-lexic.swissgeol.ch/TectonicUnits/MilanBelt">
	<rdf:type rdf:resource="http://www.w3.org/2004/02/skos/core#Concept"/>
	<rdfs:isDefinedBy xml:lang="en">Gouffon Yves (Editor) (2024): Tectonic Map of Switzerland 1:500000, Explanatory notes. Federal Office of Topography swisstopo, Wabern</rdfs:isDefinedBy>
	<skos:definition xml:lang="en">The Milan Belt represents the southernmost (i.e. most external) and lowest thin-skinned thrust sheets of the eastern South Alpine domain west of Lago di Garda. Its basement ramps are hidden below the Po Plain like most of the deformed sedimentary cover. The Milan Belt consists of thrust imbricates, locally inverting Mesozoic high-angle faults, developed as a frontal accretion of the western South Alpine domain during the Miocene. </skos:definition>
	<skos:inScheme rdf:resource="https://dev-lexic.swissgeol.ch/TectonicUnits"/>
	<skos:prefLabel xml:lang="en">Milan Belt</skos:prefLabel>
	<skos:prefLabel xml:lang="de">Milano-Belt</skos:prefLabel>
	<skos:prefLabel xml:lang="fr">Milan Belt</skos:prefLabel>
	<skos:prefLabel xml:lang="it">Milano Belt</skos:prefLabel>
	<skos:broader rdf:resource="https://dev-lexic.swissgeol.ch/TectonicUnits/SouthAlpine"/>
	<skos:narrower rdf:resource="https://dev-lexic.swissgeol.ch/TectonicUnits/ExternalGiudicarieZone"/>
	<status xmlns="http://www.w3.org/ns/adms#" rdf:resource="https://dev-lexic.swissgeol.ch/active"/>
</rdf:Description>

<rdf:Description rdf:about="https://dev-lexic.swissgeol.ch/TectonicUnits/LowerOrobicImbricates">
	<rdf:type rdf:resource="http://www.w3.org/2004/02/skos/core#Concept"/>
	<rdfs:isDefinedBy xml:lang="en">Gouffon Yves (Editor) (2024): Tectonic Map of Switzerland 1:500000, Explanatory notes. Federal Office of Topography swisstopo, Wabern</rdfs:isDefinedBy>
	<skos:definition xml:lang="en">The Lower Orobic Imbricates encompasses units of the median part of the thin-skinned thrust sheets of the eastern South Alpine domain. The en-échelon arrangement of its ramp anticlines is similar to that of the overlying Upper Orobic Nappe with a more diffuse deformation in the sedimentary cover. A large part of the Bergamasc Alps and of the Giudicarie region belongs to this unit.</skos:definition>
	<skos:inScheme rdf:resource="https://dev-lexic.swissgeol.ch/TectonicUnits"/>
	<skos:prefLabel xml:lang="en">Lower Orobic Imbricates</skos:prefLabel>
	<skos:prefLabel xml:lang="de">Untere Orobische Schuppen</skos:prefLabel>
	<skos:prefLabel xml:lang="fr">Écailles Orobiques inférieures</skos:prefLabel>
	<skos:prefLabel xml:lang="it">Scaglie Orobiche inferiore</skos:prefLabel>
	<skos:altLabel xml:lang="de">Untere Orobische Decke</skos:altLabel>
	<skos:altLabel xml:lang="fr">Nappe Orobique inférieure</skos:altLabel>
	<skos:broader rdf:resource="https://dev-lexic.swissgeol.ch/TectonicUnits/SouthAlpine"/>
	<skos:narrower rdf:resource="https://dev-lexic.swissgeol.ch/TectonicUnits/InternalGiudicarieZone"/>
	<status xmlns="http://www.w3.org/ns/adms#" rdf:resource="https://dev-lexic.swissgeol.ch/active"/>
</rdf:Description>

<rdf:Description rdf:about="https://dev-lexic.swissgeol.ch/TectonicUnits/UpperOrobicNappe">
	<rdf:type rdf:resource="http://www.w3.org/2004/02/skos/core#Concept"/>
	<rdfs:isDefinedBy xml:lang="en">Gouffon Yves (Editor) (2024): Tectonic Map of Switzerland 1:500000, Explanatory notes. Federal Office of Topography swisstopo, Wabern</rdfs:isDefinedBy>
	<skos:definition xml:lang="en">The Upper Orobic Nappe is the uppermost and oldest thin-skinned thrust sheets of the eastern South Alpine domain. It consists of an around 5 to 7 km thick basement sheet, arranged in a series of en-échelon anticlines. The thrusts associated with the Upper Orobic Nappe ramped into the sedimentary cover, creating several duplexes that occur in a belt of klippes. The distribution of these erosional remnants reflects the later deformation by the basement ramps of the underlying younger local thrust sheets and imbricates (Lower Orobic Imbricates).</skos:definition>
	<skos:inScheme rdf:resource="https://dev-lexic.swissgeol.ch/TectonicUnits"/>
	<skos:prefLabel xml:lang="en">Upper Orobic Nappe</skos:prefLabel>
	<skos:prefLabel xml:lang="de">Obere Orobische Decke</skos:prefLabel>
	<skos:prefLabel xml:lang="fr">Nappe Orobique supérieure</skos:prefLabel>
	<skos:prefLabel xml:lang="it">Falda Orobica superiore</skos:prefLabel>
	<skos:broader rdf:resource="https://dev-lexic.swissgeol.ch/TectonicUnits/SouthAlpine"/>
	<skos:narrower rdf:resource="https://dev-lexic.swissgeol.ch/TectonicUnits/ValCollaZone"/>
	<skos:narrower rdf:resource="https://dev-lexic.swissgeol.ch/TectonicUnits/Strona-Ceneri-Zone_UpperOrobicPart"/>
	<status xmlns="http://www.w3.org/ns/adms#" rdf:resource="https://dev-lexic.swissgeol.ch/active"/>
</rdf:Description>

<rdf:Description rdf:about="https://dev-lexic.swissgeol.ch/TectonicUnits/VaresottoImbricates">
	<rdf:type rdf:resource="http://www.w3.org/2004/02/skos/core#Concept"/>
	<rdfs:isDefinedBy xml:lang="en">Gouffon Yves (Editor) (2024): Tectonic Map of Switzerland 1:500000, Explanatory notes. Federal Office of Topography swisstopo, Wabern</rdfs:isDefinedBy>
	<skos:definition xml:lang="en">The Varesotto Imbricates encompass the tectonic units situated below and in front of the Upper Orobic Nappe, in analogy to the Lower Orobic Imbricates. Between the Lago Maggiore and the Lugano Fault, the Variscan basement of the Varesotto Imbricates is unconformably overlain by Permian volcanics and Mesozoic sediments with rapid lateral changes in thickness and facies.</skos:definition>
	<skos:inScheme rdf:resource="https://dev-lexic.swissgeol.ch/TectonicUnits"/>
	<skos:prefLabel xml:lang="en">Varesotto Imbricates</skos:prefLabel>
	<skos:prefLabel xml:lang="de">Varesotto-Schuppen</skos:prefLabel>
	<skos:prefLabel xml:lang="fr">Écailles du Varesotto</skos:prefLabel>
	<skos:prefLabel xml:lang="it">Scaglie del Varesotto</skos:prefLabel>
	<skos:broader rdf:resource="https://dev-lexic.swissgeol.ch/TectonicUnits/SouthAlpine"/>
	<status xmlns="http://www.w3.org/ns/adms#" rdf:resource="https://dev-lexic.swissgeol.ch/active"/>
</rdf:Description>

<rdf:Description rdf:about="https://dev-lexic.swissgeol.ch/TectonicUnits/Strona-Ceneri-Zone">
	<rdf:type rdf:resource="http://www.w3.org/2004/02/skos/core#Concept"/>
	<rdfs:isDefinedBy xml:lang="en">Gouffon Yves (Editor) (2024): Tectonic Map of Switzerland 1:500000, Explanatory notes. Federal Office of Topography swisstopo, Wabern</rdfs:isDefinedBy>
	<skos:definition xml:lang="en">The Strona-Ceneri-Zone is an ante-alpine, thick-skinned tectonic unit of the western South Alpine domain. It is made up of polymetamorphic (para)gneisses and amphibolites, as well as late to post-Variscan plutonic and volcanic rocks.</skos:definition>
	<skos:inScheme rdf:resource="https://dev-lexic.swissgeol.ch/TectonicUnits"/>
	<skos:prefLabel xml:lang="en">Strona-Ceneri-Zone</skos:prefLabel>
	<skos:prefLabel xml:lang="de">Strona-Ceneri-Zone</skos:prefLabel>
	<skos:prefLabel xml:lang="fr">Zone de Strona-Ceneri</skos:prefLabel>
	<skos:prefLabel xml:lang="it">Zona Strona-Ceneri</skos:prefLabel>
	<skos:broader rdf:resource="https://dev-lexic.swissgeol.ch/TectonicUnits/SouthAlpine"/>
	<skos:narrower rdf:resource="https://dev-lexic.swissgeol.ch/TectonicUnits/Strona-Ceneri-Zone_PartIvrea-Ceneri"/>
	<skos:narrower rdf:resource="https://dev-lexic.swissgeol.ch/TectonicUnits/Strona-Ceneri-Zone_UpperOrobicPart"/>
	<status xmlns="http://www.w3.org/ns/adms#" rdf:resource="https://dev-lexic.swissgeol.ch/active"/>
</rdf:Description>

<rdf:Description rdf:about="https://dev-lexic.swissgeol.ch/TectonicUnits/IvreaZone">
	<rdf:type rdf:resource="http://www.w3.org/2004/02/skos/core#Concept"/>
	<rdfs:isDefinedBy xml:lang="en">Gouffon Yves (Editor) (2024): Tectonic Map of Switzerland 1:500000, Explanatory notes. Federal Office of Topography swisstopo, Wabern</rdfs:isDefinedBy>
	<skos:definition xml:lang="en">The Ivrea Zone is an ante-alpine, thick-skinned tectonic unit of the western South Alpine domain, made up of high-grade polymetamorphic gneisses ("kinzigite"), a mafic to ultramafic complex, as well as subordinated pegmatites and marbles.</skos:definition>
	<skos:inScheme rdf:resource="https://dev-lexic.swissgeol.ch/TectonicUnits"/>
	<skos:prefLabel xml:lang="en">Ivrea Zone</skos:prefLabel>
	<skos:prefLabel xml:lang="de">Ivrea-Zone</skos:prefLabel>
	<skos:prefLabel xml:lang="fr">Zone d'Ivrea</skos:prefLabel>
	<skos:prefLabel xml:lang="it">Zona di Ivrea</skos:prefLabel>
	<skos:broader rdf:resource="https://dev-lexic.swissgeol.ch/TectonicUnits/Ivrea-CeneriComplex"/>
	<status xmlns="http://www.w3.org/ns/adms#" rdf:resource="https://dev-lexic.swissgeol.ch/active"/>
</rdf:Description>

<rdf:Description rdf:about="https://dev-lexic.swissgeol.ch/TectonicUnits/Strona-Ceneri-Zone_PartIvrea-Ceneri">
	<rdf:type rdf:resource="http://www.w3.org/2004/02/skos/core#Concept"/>
	<rdfs:isDefinedBy xml:lang="en">Gouffon Yves (Editor) (2024): Tectonic Map of Switzerland 1:500000, Explanatory notes. Federal Office of Topography swisstopo, Wabern</rdfs:isDefinedBy>
	<skos:inScheme rdf:resource="https://dev-lexic.swissgeol.ch/TectonicUnits"/>
	<skos:prefLabel xml:lang="en">Strona-Ceneri-Zone (Ivrea-Ceneri-Anteil)</skos:prefLabel>
	<skos:prefLabel xml:lang="de">Strona-Ceneri-Zone (Ivrea-Ceneri-Anteil)</skos:prefLabel>
	<skos:prefLabel xml:lang="fr">Zone de Strona-Ceneri (partie Ivrea-Ceneri)</skos:prefLabel>
	<skos:prefLabel xml:lang="it">Zona Strona-Ceneri (parte Ivrea-Ceneri)</skos:prefLabel>
	<skos:broader rdf:resource="https://dev-lexic.swissgeol.ch/TectonicUnits/Ivrea-CeneriComplex"/>
	<skos:broader rdf:resource="https://dev-lexic.swissgeol.ch/TectonicUnits/Strona-Ceneri-Zone"/>
	<skos:related rdf:resource="https://dev-lexic.swissgeol.ch/TectonicUnits/Strona-Ceneri-Zone_PartUpperOrobic"/>
	<status xmlns="http://www.w3.org/ns/adms#" rdf:resource="https://dev-lexic.swissgeol.ch/active"/>
</rdf:Description>

<rdf:Description rdf:about="https://dev-lexic.swissgeol.ch/TectonicUnits/ExternalGiudicarieZone">
	<rdf:type rdf:resource="http://www.w3.org/2004/02/skos/core#Concept"/>
	<rdfs:isDefinedBy xml:lang="en">Gouffon Yves (Editor) (2024): Tectonic Map of Switzerland 1:500000, Explanatory notes. Federal Office of Topography swisstopo, Wabern</rdfs:isDefinedBy>
	<skos:definition xml:lang="en">The External Giudicarie Zone represents the southernmost (i.e. most external) and lowest thin-skinned thrust sheets of the eastern South Alpine domain east of Lago di Garda. It is linked kinematically to the Milan Belt.</skos:definition>
	<skos:inScheme rdf:resource="https://dev-lexic.swissgeol.ch/TectonicUnits"/>
	<skos:prefLabel xml:lang="en">External Giudicarie Zone</skos:prefLabel>
	<skos:prefLabel xml:lang="de">Externe Judicarien-Zone</skos:prefLabel>
	<skos:prefLabel xml:lang="fr">Zone des Giudicarie externe</skos:prefLabel>
	<skos:prefLabel xml:lang="it">Zona delle Giudicarie esterna</skos:prefLabel>
	<skos:broader rdf:resource="https://dev-lexic.swissgeol.ch/TectonicUnits/MilanBelt"/>
	<status xmlns="http://www.w3.org/ns/adms#" rdf:resource="https://dev-lexic.swissgeol.ch/active"/>
</rdf:Description>

<rdf:Description rdf:about="https://dev-lexic.swissgeol.ch/TectonicUnits/InternalGiudicarieZone">
	<rdf:type rdf:resource="http://www.w3.org/2004/02/skos/core#Concept"/>
	<rdfs:isDefinedBy xml:lang="en">Gouffon Yves (Editor) (2024): Tectonic Map of Switzerland 1:500000, Explanatory notes. Federal Office of Topography swisstopo, Wabern</rdfs:isDefinedBy>
	<skos:definition xml:lang="en">The Internal Giudicarie Zone is linked kinematically to the Lower Orobic Imbricates.</skos:definition>
	<skos:inScheme rdf:resource="https://dev-lexic.swissgeol.ch/TectonicUnits"/>
	<skos:prefLabel xml:lang="en">Internal Giudicarie Zone</skos:prefLabel>
	<skos:prefLabel xml:lang="de">Interne Judicarien-Zone</skos:prefLabel>
	<skos:prefLabel xml:lang="fr">Zone des Giudicarie interne</skos:prefLabel>
	<skos:prefLabel xml:lang="it">Zona delle Giudicarie interna</skos:prefLabel>
	<skos:broader rdf:resource="https://dev-lexic.swissgeol.ch/TectonicUnits/LowerOrobicImbricates"/>
	<status xmlns="http://www.w3.org/ns/adms#" rdf:resource="https://dev-lexic.swissgeol.ch/active"/>
</rdf:Description>

<rdf:Description rdf:about="https://dev-lexic.swissgeol.ch/TectonicUnits/ValCollaZone">
	<rdf:type rdf:resource="http://www.w3.org/2004/02/skos/core#Concept"/>
	<rdfs:isDefinedBy xml:lang="en">Gouffon Yves (Editor) (2024): Tectonic Map of Switzerland 1:500000, Explanatory notes. Federal Office of Topography swisstopo, Wabern</rdfs:isDefinedBy>
	<skos:definition xml:lang="en">The Val Colla Zone is a Variscan tectonic unit representing, together with part of the Strona-Ceneri Zone, the basement of the Upper Orobic Nappe. It consists mainly of paragneisses, hornblende-epidote schists and metagranites. These Variscan, originally amphibolite-facies metamorphic rocks, were retrogressed to the greenschist facies, possibly during Mesozoic rifting and associated exhumation of the basement rocks.</skos:definition>
	<skos:inScheme rdf:resource="https://dev-lexic.swissgeol.ch/TectonicUnits"/>
	<skos:prefLabel xml:lang="en">Val Colla Zone</skos:prefLabel>
	<skos:prefLabel xml:lang="de">Val-Colla-Zone</skos:prefLabel>
	<skos:prefLabel xml:lang="fr">Zone du Val Colla</skos:prefLabel>
	<skos:prefLabel xml:lang="it">Zona della Val Colla</skos:prefLabel>
	<skos:broader rdf:resource="https://dev-lexic.swissgeol.ch/TectonicUnits/UpperOrobicNappe"/>
	<status xmlns="http://www.w3.org/ns/adms#" rdf:resource="https://dev-lexic.swissgeol.ch/active"/>
</rdf:Description>

<rdf:Description rdf:about="https://dev-lexic.swissgeol.ch/TectonicUnits/Strona-Ceneri-Zone_UpperOrobicPart">
	<rdf:type rdf:resource="http://www.w3.org/2004/02/skos/core#Concept"/>
	<rdfs:isDefinedBy xml:lang="en">Gouffon Yves (Editor) (2024): Tectonic Map of Switzerland 1:500000, Explanatory notes. Federal Office of Topography swisstopo, Wabern</rdfs:isDefinedBy>
	<skos:inScheme rdf:resource="https://dev-lexic.swissgeol.ch/TectonicUnits"/>
	<skos:prefLabel xml:lang="en">Strona-Ceneri-Zone (Upper Orobic part)</skos:prefLabel>
	<skos:prefLabel xml:lang="de">Strona-Ceneri-Zone (Obere Orobische-Anteil)</skos:prefLabel>
	<skos:prefLabel xml:lang="fr">Zone de Strona-Ceneri (partie Orobique supérieure)</skos:prefLabel>
	<skos:prefLabel xml:lang="it">Zona Strona-Ceneri (parte Orobica superiore)</skos:prefLabel>
	<skos:broader rdf:resource="https://dev-lexic.swissgeol.ch/TectonicUnits/UpperOrobicNappe"/>
	<skos:broader rdf:resource="https://dev-lexic.swissgeol.ch/TectonicUnits/Strona-Ceneri-Zone"/>
	<skos:related rdf:resource="https://dev-lexic.swissgeol.ch/TectonicUnits/Strona-Ceneri-Zone_PartIvrea-Ceneri"/>
	<status xmlns="http://www.w3.org/ns/adms#" rdf:resource="https://dev-lexic.swissgeol.ch/active"/>
</rdf:Description>

<rdf:Description rdf:about="https://dev-lexic.swissgeol.ch/TectonicUnits/PeriadriaticMagmaticProvince">
	<rdf:type rdf:resource="http://www.w3.org/2004/02/skos/core#Concept"/>
	<rdfs:isDefinedBy xml:lang="en">Gouffon Yves (Editor) (2024): Tectonic Map of Switzerland 1:500000, Explanatory notes. Federal Office of Topography swisstopo, Wabern</rdfs:isDefinedBy>
	<skos:definition xml:lang="en">The Periadriatic Magmatic Province gave rise to plutons and many dykes of Eocene–Oligocene age straddling the Periadriatic Fault System. The final emplacement of the plutons often coincides temporally with activity along this fault system.</skos:definition>
	<skos:inScheme rdf:resource="https://dev-lexic.swissgeol.ch/TectonicUnits"/>
	<skos:prefLabel xml:lang="en">Periadriatic Magmatic Province</skos:prefLabel>
	<skos:prefLabel xml:lang="de">Periadriatische magmatische Provinz</skos:prefLabel>
	<skos:prefLabel xml:lang="fr">Province magmatique périadriatique</skos:prefLabel>
	<skos:prefLabel xml:lang="it">Provincia magmatica periadriatica</skos:prefLabel>
	<skos:altLabel xml:lang="de">Periadriatische Provinz</skos:altLabel>
	<skos:broader rdf:resource="https://dev-lexic.swissgeol.ch/TectonicUnits/CenozoicMagmaticRocks"/>
	<skos:narrower rdf:resource="https://dev-lexic.swissgeol.ch/TectonicUnits/BiellaVolcanicSeries"/>
	<skos:narrower rdf:resource="https://dev-lexic.swissgeol.ch/TectonicUnits/ColleGalloSubvolcanicBody"/>
	<skos:narrower rdf:resource="https://dev-lexic.swissgeol.ch/TectonicUnits/GandinoSubvolcanicBody"/>
	<skos:narrower rdf:resource="https://dev-lexic.swissgeol.ch/TectonicUnits/BregagliaIntrusion"/>
	<skos:narrower rdf:resource="https://dev-lexic.swissgeol.ch/TectonicUnits/NovateIntrusion"/>
	<skos:narrower rdf:resource="https://dev-lexic.swissgeol.ch/TectonicUnits/AdamelloBatholith"/>
	<status xmlns="http://www.w3.org/ns/adms#" rdf:resource="https://dev-lexic.swissgeol.ch/active"/>
</rdf:Description>

<rdf:Description rdf:about="https://dev-lexic.swissgeol.ch/TectonicUnits/BiellaVolcanicSeries">
	<rdf:type rdf:resource="http://www.w3.org/2004/02/skos/core#Concept"/>
	<rdfs:isDefinedBy xml:lang="en">Gouffon Yves (Editor) (2024): Tectonic Map of Switzerland 1:500000, Explanatory notes. Federal Office of Topography swisstopo, Wabern</rdfs:isDefinedBy>
	<skos:definition xml:lang="en">The Biella Volcanic Suite is an Oligocene volcano-sedimentary series covering the most internal portion of the Sesia Nappe along the Canavese Fault in the Biella region. These mostly calc-alkaline andesitic rocks were deposited onto an erosional surface of the Eclogitic Micaschist Unit of the Sesia Nappe 33–32 Ma ago.</skos:definition>
	<skos:inScheme rdf:resource="https://dev-lexic.swissgeol.ch/TectonicUnits"/>
	<skos:prefLabel xml:lang="en">Biella Volcanic Series</skos:prefLabel>
	<skos:prefLabel xml:lang="de">Vulkanische Serie von Biella</skos:prefLabel>
	<skos:prefLabel xml:lang="fr">Série volcanique de Biella</skos:prefLabel>
	<skos:prefLabel xml:lang="it">Serie vulcanica di Biella</skos:prefLabel>
	<skos:broader rdf:resource="https://dev-lexic.swissgeol.ch/TectonicUnits/PeriadriaticMagmaticProvince"/>
	<status xmlns="http://www.w3.org/ns/adms#" rdf:resource="https://dev-lexic.swissgeol.ch/active"/>
</rdf:Description>

<rdf:Description rdf:about="https://dev-lexic.swissgeol.ch/TectonicUnits/ColleGalloSubvolcanicBody">
	<rdf:type rdf:resource="http://www.w3.org/2004/02/skos/core#Concept"/>
	<rdfs:isDefinedBy xml:lang="en">Gouffon Yves (Editor) (2024): Tectonic Map of Switzerland 1:500000, Explanatory notes. Federal Office of Topography swisstopo, Wabern</rdfs:isDefinedBy>
	<skos:definition xml:lang="en">The Colle Gallo Subvolcanic Body, situated near Albino (northeast of Bergamo), encompasses many sills and small magma bodies of andesitic composition intruded the Lower Orobic Imbricates and the Upper Orobic Nappe. The unit is associated with normal faults and cut earlier thrusts. Intrusion ages around 40 Ma and geochemical analyses suggest a close relationship with the earliest Adamello intrusion stages.</skos:definition>
	<skos:inScheme rdf:resource="https://dev-lexic.swissgeol.ch/TectonicUnits"/>
	<skos:prefLabel xml:lang="en">Colle Gallo Subvolcanic Body</skos:prefLabel>
	<skos:prefLabel xml:lang="de">Subvulkanischer Körper vom Colle Gallo</skos:prefLabel>
	<skos:prefLabel xml:lang="fr">Corps subvolcanique du Colle Gallo</skos:prefLabel>
	<skos:prefLabel xml:lang="it">Corpo subvulcanico del Colle Gallo</skos:prefLabel>
	<skos:broader rdf:resource="https://dev-lexic.swissgeol.ch/TectonicUnits/PeriadriaticMagmaticProvince"/>
	<status xmlns="http://www.w3.org/ns/adms#" rdf:resource="https://dev-lexic.swissgeol.ch/active"/>
</rdf:Description>

<rdf:Description rdf:about="https://dev-lexic.swissgeol.ch/TectonicUnits/GandinoSubvolcanicBody">
	<rdf:type rdf:resource="http://www.w3.org/2004/02/skos/core#Concept"/>
	<rdfs:isDefinedBy xml:lang="en">Gouffon Yves (Editor) (2024): Tectonic Map of Switzerland 1:500000, Explanatory notes. Federal Office of Topography swisstopo, Wabern</rdfs:isDefinedBy>
	<skos:definition xml:lang="en">The Gandino Subvolcanic Body, situated northeast of Bergamo, encompasses many sills and small magma bodies of andesitic composition intruded the Lower Orobic Imbricates and the Upper Orobic Nappe. The unit is associated with normal faults and cut earlier thrusts. Intrusion ages around 40 Ma and geochemical analyses suggest a close relationship with the earliest Adamello intrusion stages.</skos:definition>
	<skos:inScheme rdf:resource="https://dev-lexic.swissgeol.ch/TectonicUnits"/>
	<skos:prefLabel xml:lang="en">Gandino Subvolcanic Body</skos:prefLabel>
	<skos:prefLabel xml:lang="de">Subvulkanischer Körper von Gandino</skos:prefLabel>
	<skos:prefLabel xml:lang="fr">Corps subvolcanique de Gandino</skos:prefLabel>
	<skos:prefLabel xml:lang="it">Corpo subvulcanico di Gandino</skos:prefLabel>
	<skos:broader rdf:resource="https://dev-lexic.swissgeol.ch/TectonicUnits/PeriadriaticMagmaticProvince"/>
	<status xmlns="http://www.w3.org/ns/adms#" rdf:resource="https://dev-lexic.swissgeol.ch/active"/>
</rdf:Description>

<rdf:Description rdf:about="https://dev-lexic.swissgeol.ch/TectonicUnits/BregagliaIntrusion">
	<rdf:type rdf:resource="http://www.w3.org/2004/02/skos/core#Concept"/>
	<rdfs:isDefinedBy xml:lang="en">Gouffon Yves (Editor) (2024): Tectonic Map of Switzerland 1:500000, Explanatory notes. Federal Office of Topography swisstopo, Wabern</rdfs:isDefinedBy>
	<skos:definition xml:lang="en">The Bregaglia Intrusion forms a large plutonic body between the Val Bregaglia in the north and the Tonale Fault in the south; it extends with a narrow tail of about 40 km westward along the Tonale Fault (Insubric Fault). It comprises mainly calc-alkaline tonalite and granodiorite, derived from a primitive mantle melt and channeled from the base of the continental crust into the Periadriatic Fault System. The base of the pluton overlying the Gruf Complex shows evidence of synmagmatic folding and thrusting indicating contemporaneous late stage N–S shortening. Crystallization and emplacement of the Bregaglia Intrusion took place between 32 and 28 Ma. A smaller body related to the Bregaglia Intrusion crops out northwest of Sondrio (Triangia Pluton), where it intrudes the subvertical Tonale Nappe and its contact with the adjacent root zone of the Campo Nappe Complex.</skos:definition>
	<skos:inScheme rdf:resource="https://dev-lexic.swissgeol.ch/TectonicUnits"/>
	<skos:prefLabel xml:lang="en">Bregaglia Intrusion</skos:prefLabel>
	<skos:prefLabel xml:lang="de">Bregaglia-Intrusionskörper</skos:prefLabel>
	<skos:prefLabel xml:lang="fr">Intrusion de la Bregaglia</skos:prefLabel>
	<skos:prefLabel xml:lang="it">Intrusione della Bregaglia</skos:prefLabel>
	<skos:altLabel xml:lang="de">Bergell-Intrusionskörper</skos:altLabel>
	<skos:altLabel xml:lang="fr">Intrusion du Bergell</skos:altLabel>
	<skos:broader rdf:resource="https://dev-lexic.swissgeol.ch/TectonicUnits/PeriadriaticMagmaticProvince"/>
	<status xmlns="http://www.w3.org/ns/adms#" rdf:resource="https://dev-lexic.swissgeol.ch/active"/>
</rdf:Description>

<rdf:Description rdf:about="https://dev-lexic.swissgeol.ch/TectonicUnits/NovateIntrusion">
	<rdf:type rdf:resource="http://www.w3.org/2004/02/skos/core#Concept"/>
	<rdfs:isDefinedBy xml:lang="en">Gouffon Yves (Editor) (2024): Tectonic Map of Switzerland 1:500000, Explanatory notes. Federal Office of Topography swisstopo, Wabern</rdfs:isDefinedBy>
	<skos:definition xml:lang="en">The main stock of the Novate Intrusion partially cuts the Bregaglia Intrusion while smaller parts lie just west of it. The Novate Intrusion is younger in age (24 Ma, Liati et al. 2000) and consists of a leucogranite. Its peraluminous chemical composition suggests that this granite is not related to the calc-alkaline Bregaglia suite, but was derived from the partial melting of crustal rocks that are widespread in the Southern Steep Belt – or root zone – north of the Tonale Fault.</skos:definition>
	<skos:inScheme rdf:resource="https://dev-lexic.swissgeol.ch/TectonicUnits"/>
	<skos:prefLabel xml:lang="en">Novate Intrusion</skos:prefLabel>
	<skos:prefLabel xml:lang="de">Novate-Intrusionskörper</skos:prefLabel>
	<skos:prefLabel xml:lang="fr">Intrusion de Novate</skos:prefLabel>
	<skos:prefLabel xml:lang="it">Intrusione di Novate</skos:prefLabel>
	<skos:broader rdf:resource="https://dev-lexic.swissgeol.ch/TectonicUnits/PeriadriaticMagmaticProvince"/>
	<status xmlns="http://www.w3.org/ns/adms#" rdf:resource="https://dev-lexic.swissgeol.ch/active"/>
</rdf:Description>

<rdf:Description rdf:about="https://dev-lexic.swissgeol.ch/TectonicUnits/AdamelloBatholith">
	<rdf:type rdf:resource="http://www.w3.org/2004/02/skos/core#Concept"/>
	<rdfs:isDefinedBy xml:lang="en">Gouffon Yves (Editor) (2024): Tectonic Map of Switzerland 1:500000, Explanatory notes. Federal Office of Topography swisstopo, Wabern</rdfs:isDefinedBy>
	<skos:definition xml:lang="en">The Adamello Batholith is the largest Paleogene pluton of the Alps. It is located in the South Alpine domain, adjacent to the Tonale Fault in the north and the Giudicarie Fault in the east. It comprises several intrusions that succeeded each other between 42 and 28 Ma, generally becoming younger in age from south to north. The rocks of this batholith are mainly tonalites accompanied by granodiorites.
In contrast to the Bregaglia Intrusion and most other Periadriatic plutons, ascent and main emplacement of the different batches of the Adamello Batholith were unrelated to the activity of the neighboring Periadriatic Fault System and occurred by forceful intrusion. The youngest intrusions however, located in the north of the batholith and adjacent to the Tonale Fault (the foliated Avio and Presanella intrusions with ages of 34.6 Ma and 32.0 Ma, respectively), produced a contact metamorphism during which the adjacent mylonites of the Tonale Fault (Southern Mylonite Zone) became deformed under temperatures of up to more than 620 °C. This indicates that dextral strike-slip faulting along the Tonale Fault, recorded in these mylonites within the contact metamorphic aureole, must have started as early as around 34 Ma ago.</skos:definition>
	<skos:inScheme rdf:resource="https://dev-lexic.swissgeol.ch/TectonicUnits"/>
	<skos:prefLabel xml:lang="en">Adamello Batholith</skos:prefLabel>
	<skos:prefLabel xml:lang="de">Adamello-Batholith</skos:prefLabel>
	<skos:prefLabel xml:lang="fr">Batholite de l'Adamello</skos:prefLabel>
	<skos:prefLabel xml:lang="it">Batolite dell'Adamello</skos:prefLabel>
	<skos:broader rdf:resource="https://dev-lexic.swissgeol.ch/TectonicUnits/PeriadriaticMagmaticProvince"/>
	<status xmlns="http://www.w3.org/ns/adms#" rdf:resource="https://dev-lexic.swissgeol.ch/active"/>
</rdf:Description>

<rdf:Description rdf:about="https://dev-lexic.swissgeol.ch/TectonicUnits/PlaineMorteMelange">
	<rdf:type rdf:resource="http://www.w3.org/2004/02/skos/core#Concept"/>
	<skos:definition xml:lang="en">The Plaine Morte Mélange is a chaotic deposit dominated by block-in-matrix fabrics, directly overlying many Lower and Upper Helvetic units in the Western Swiss Alps (Aiguilles Rouges Massif, Morcles and Jägerchrüz nappes, Wildhorn Nappe Complex). In many cases, this mélange lies directly above the Helvetic flysch and has therefore occasionally been considered as the top of the Helvetic sedimentary series.</skos:definition>
	<skos:inScheme rdf:resource="https://dev-lexic.swissgeol.ch/TectonicUnits"/>
	<skos:prefLabel xml:lang="en">Plaine Morte Mélange</skos:prefLabel>
	<skos:prefLabel xml:lang="de">Plaine-Morte Melange</skos:prefLabel>
	<skos:prefLabel xml:lang="fr">Mélange de la Plaine Morte</skos:prefLabel>
	<skos:prefLabel xml:lang="it">Mélange della Plaine Morte</skos:prefLabel>
	<skos:broader rdf:resource="https://dev-lexic.swissgeol.ch/TectonicUnits/PillonMelangeZone"/>
</rdf:Description>

<rdf:Description rdf:about="https://dev-lexic.swissgeol.ch/TectonicUnits/MaliensSlice">
	<rdf:type rdf:resource="http://www.w3.org/2004/02/skos/core#Concept"/>
	<skos:definition xml:lang="en">The Maliens Slice is a sheared-off branch of the uppermost fold of the Tschep Slice situated north of Trin (southwest of Kunkelpass). It forms a small klippe made up of Dogger and Malm.</skos:definition>
	<skos:inScheme rdf:resource="https://dev-lexic.swissgeol.ch/TectonicUnits"/>
	<skos:prefLabel xml:lang="en">Maliens Slice</skos:prefLabel>
	<skos:prefLabel xml:lang="de">Maliens-Schuppe</skos:prefLabel>
	<skos:prefLabel xml:lang="fr">Écaille de Maliens</skos:prefLabel>
	<skos:prefLabel xml:lang="it">Scaglia di Maliens</skos:prefLabel>
	<skos:broader rdf:resource="https://dev-lexic.swissgeol.ch/TectonicUnits/AarMassif"/>
</rdf:Description>

<rdf:Description rdf:about="https://dev-lexic.swissgeol.ch/TectonicUnits/AnzeindeSlivers">
	<rdf:type rdf:resource="http://www.w3.org/2004/02/skos/core#Concept"/>
	<skos:definition xml:lang="en">Within the Upper Helvetic Pillon Mélange Zone, the Anzeinde-type slivers (composed of a Malm-Cretaceous series) often overly the Plaine Morte Mélange.</skos:definition>
	<skos:inScheme rdf:resource="https://dev-lexic.swissgeol.ch/TectonicUnits"/>
	<skos:prefLabel xml:lang="en">Anzeinde-type slivers</skos:prefLabel>
	<skos:broader rdf:resource="https://dev-lexic.swissgeol.ch/TectonicUnits/PillonMelangeZone"/>
</rdf:Description>

<rdf:Description rdf:about="https://dev-lexic.swissgeol.ch/TectonicUnits/SexMortSlivers">
	<rdf:type rdf:resource="http://www.w3.org/2004/02/skos/core#Concept"/>
	<skos:definition xml:lang="en">Within the Upper Helvetic Pillon Mélange Zone, the Sex Mort-type slivers (composed of a Malm and Eocene series) occur exclusively on top and in front of the Sublage Nappe (Wildhorn Nappe Complex).</skos:definition>
	<skos:inScheme rdf:resource="https://dev-lexic.swissgeol.ch/TectonicUnits"/>
	<skos:prefLabel xml:lang="en">Sex Mort-type slivers</skos:prefLabel>
	<skos:broader rdf:resource="https://dev-lexic.swissgeol.ch/TectonicUnits/PillonMelangeZone"/>
</rdf:Description>

<rdf:Description rdf:about="https://dev-lexic.swissgeol.ch/TectonicUnits/ArveyesSlivers">
	<rdf:type rdf:resource="http://www.w3.org/2004/02/skos/core#Concept"/>
	<skos:definition xml:lang="en">Within the Upper Helvetic Pillon Mélange Zone, the Arveyes-type slivers (composed of a Dogger and Eocene series) occur between the Prealps nappes and the frontal folds of the Lower and Upper Helvetic nappes.</skos:definition>
	<skos:inScheme rdf:resource="https://dev-lexic.swissgeol.ch/TectonicUnits"/>
	<skos:prefLabel xml:lang="en">Arveyes-type slivers</skos:prefLabel>
	<skos:broader rdf:resource="https://dev-lexic.swissgeol.ch/TectonicUnits/PillonMelangeZone"/>
</rdf:Description>

<rdf:Description rdf:about="https://dev-lexic.swissgeol.ch/TectonicUnits/BexLaubhornSlivers">
	<rdf:type rdf:resource="http://www.w3.org/2004/02/skos/core#Concept"/>
	<skos:definition xml:lang="en">Within the Upper Helvetic Pillon Mélange Zone, the Bex-Laubhorn-type slivers (composed of a Triassic to Early Jurassic series) occur between the Prealps nappes and the frontal folds of the Lower and Upper Helvetic nappes.</skos:definition>
	<skos:inScheme rdf:resource="https://dev-lexic.swissgeol.ch/TectonicUnits"/>
	<skos:prefLabel xml:lang="en">Bex-Laubhorn-type slivers</skos:prefLabel>
	<skos:broader rdf:resource="https://dev-lexic.swissgeol.ch/TectonicUnits/PillonMelangeZone"/>
</rdf:Description>

<rdf:Description rdf:about="https://dev-lexic.swissgeol.ch/TectonicUnits/MeilleretSlivers">
	<rdf:type rdf:resource="http://www.w3.org/2004/02/skos/core#Concept"/>
	<skos:definition xml:lang="en">Within the Upper Helvetic Pillon Mélange Zone, the Meilleret-type slivers (composed of Eocene flysch) occur between the Prealps nappes and the frontal folds of the Lower and Upper Helvetic nappes.</skos:definition>
	<skos:inScheme rdf:resource="https://dev-lexic.swissgeol.ch/TectonicUnits"/>
	<skos:prefLabel xml:lang="en">Meilleret-type slivers</skos:prefLabel>
	<skos:broader rdf:resource="https://dev-lexic.swissgeol.ch/TectonicUnits/PillonMelangeZone"/>
</rdf:Description>

<rdf:Description rdf:about="https://dev-lexic.swissgeol.ch/TectonicUnits/OetztalNappe">
	<rdf:type rdf:resource="http://www.w3.org/2004/02/skos/core#Concept"/>
	<skos:definition xml:lang="en">The Ötztal Nappe forms the main part of the Ötztal Nappe Complex. It consists mainly of polymetamorphic paragneisses with minor orthogneisses and amphibolites.</skos:definition>
	<skos:inScheme rdf:resource="https://dev-lexic.swissgeol.ch/TectonicUnits"/>
	<skos:prefLabel xml:lang="en">Ötztal Nappe</skos:prefLabel>
	<skos:prefLabel xml:lang="de">Ötztal-Decke</skos:prefLabel>
	<skos:prefLabel xml:lang="fr">Nappe de l'Ötztal</skos:prefLabel>
	<skos:prefLabel xml:lang="it">Falda dell'Ötztal</skos:prefLabel>
	<skos:broader rdf:resource="https://dev-lexic.swissgeol.ch/TectonicUnits/OetztalNappeComplex"/>
</rdf:Description>

<rdf:Description rdf:about="https://dev-lexic.swissgeol.ch/TectonicUnits/ForelandPlateau">
	<rdf:type rdf:resource="http://www.w3.org/2004/02/skos/core#Concept"/>
	<skos:definition xml:lang="en">The Foreland Plateau covers the detached part of the Molasse Basin and its Mesozoic basement. It is characterized by NE–SW trending low amplitude folds.</skos:definition>
	<skos:inScheme rdf:resource="https://dev-lexic.swissgeol.ch/TectonicUnits"/>
	<skos:prefLabel xml:lang="en">Foreland Plateau</skos:prefLabel>
	<skos:prefLabel xml:lang="de">Vorlandplateau</skos:prefLabel>
	<skos:prefLabel xml:lang="fr">Plateau de l'Avant-pays</skos:prefLabel>
	<skos:prefLabel xml:lang="it">Altopiano dell'Avampaese</skos:prefLabel>
	<skos:broader rdf:resource="https://dev-lexic.swissgeol.ch/TectonicUnits/InternalFoldedJuraAndForelandPlateau"/>
</rdf:Description>

<rdf:Description rdf:about="https://dev-lexic.swissgeol.ch/TectonicUnits/InternalFoldedJura">
	<rdf:type rdf:resource="http://www.w3.org/2004/02/skos/core#Concept"/>
	<skos:definition xml:lang="en">The Internal Folded Jura represents the most intensely deformed part of the Detached North Alpine Foreland. In a similar manner to the whole Jura Mountains, it forms a prominent arcuate chain («Haute Chaîne») in eastern France and northwestern Switzerland.</skos:definition>
	<skos:inScheme rdf:resource="https://dev-lexic.swissgeol.ch/TectonicUnits"/>
	<skos:prefLabel xml:lang="en">Internal Folded Jura</skos:prefLabel>
	<skos:prefLabel xml:lang="de">Interner Faltenjura</skos:prefLabel>
	<skos:prefLabel xml:lang="fr">Jura Plissé Interne</skos:prefLabel>
	<skos:prefLabel xml:lang="it">Giura Piegato Interno</skos:prefLabel>
	<skos:broader rdf:resource="https://dev-lexic.swissgeol.ch/TectonicUnits/InternalFoldedJuraAndForelandPlateau"/>
</rdf:Description>

</rdf:RDF>